# baseURI: http://w3id.org/ogeochem/def/instrument/ontology
# imports: http://purl.org/dc/elements/1.1/
# imports: http://www.w3.org/2000/01/rdf-schema
# imports: http://www.w3.org/2004/02/skos/core

@prefix dcterm: <http://purl.org/dc/terms/> .
@prefix dspl: <http://vocab.nerc.ac.uk/collection/P08/current/> .
@prefix grg: <http://www.isotc211.org/schemas/grg/> .
@prefix inst: <http://vocab.nerc.ac.uk/collection/L22/current/> .
@prefix owl: <http://www.w3.org/2002/07/owl#> .
@prefix pav: <http://purl.org/pav/> .
@prefix prov: <https://www.w3.org/ns/prov#> .
@prefix rdf: <http://www.w3.org/1999/02/22-rdf-syntax-ns#> .
@prefix rdfs: <http://www.w3.org/2000/01/rdf-schema#> .
@prefix sdev: <http://vocab.nerc.ac.uk/collection/L05/current/> .
@prefix sdnc: <http://vocab.nerc.ac.uk/collection/L21/current/> .
@prefix sdnd: <http://vocab.nerc.ac.uk/collection/C77/current/> .
@prefix sdnk: <http://vocab.nerc.ac.uk/collection/L19/current/> .
@prefix skos: <http://www.w3.org/2004/02/skos/core#> .
@prefix xml: <http://www.w3.org/XML/1998/namespace> .
@prefix xsd: <http://www.w3.org/2001/XMLSchema#> .

pav:authoredOn
  rdf:type owl:AnnotationProperty ;
.
pav:hasCurrentVersion
  rdf:type owl:AnnotationProperty ;
.
pav:hasVersion
  rdf:type owl:AnnotationProperty ;
.
pav:version
  rdf:type owl:AnnotationProperty ;
.
<http://vocab.nerc.ac.uk/collection/L05/current/101>
  rdf:type skos:Concept ;
  dcterm:date "2013-02-26 17:11:07.0" ;
  dcterm:identifier "SDN:L05::101" ;
  dcterm:source <http://vocab.nerc.ac.uk/scheme/EDMED_DCAT_THEMES/current> ;
  dcterm:source <http://vocab.nerc.ac.uk/scheme/SDNDEV/current> ;
  pav:authoredOn "2013-02-26 17:11:07.0" ;
  pav:hasCurrentVersion <http://vocab.nerc.ac.uk/collection/L05/current/101/2> ;
  pav:hasVersion <http://vocab.nerc.ac.uk/collection/L05/current/101/1> ;
  owl:versionInfo "2" ;
  skos:broader sdnc:ICAT04 ;
  skos:definition "Instrument that measures wind speed and direction at a single elevation."@en ;
  skos:inScheme <http://vocab.nerc.ac.uk/scheme/EDMED_DCAT_THEMES/current> ;
  skos:inScheme <http://vocab.nerc.ac.uk/scheme/SDNDEV/current> ;
  skos:narrower <http://vocab.nerc.ac.uk/collection/W01/current/003> ;
  skos:notation "SDN:L05::101" ;
  skos:note "accepted"@en ;
  skos:prefLabel "anemometers"@en ;
.
<http://vocab.nerc.ac.uk/collection/L05/current/102>
  rdf:type skos:Concept ;
  dcterm:date "2013-02-26 17:11:07.0" ;
  dcterm:identifier "SDN:L05::102" ;
  dcterm:source <http://vocab.nerc.ac.uk/scheme/EDMED_DCAT_THEMES/current> ;
  dcterm:source <http://vocab.nerc.ac.uk/scheme/NETMAR_OCEAN/current> ;
  dcterm:source <http://vocab.nerc.ac.uk/scheme/NETOC_INSTRUMENT/current> ;
  dcterm:source <http://vocab.nerc.ac.uk/scheme/SDNDEV/current> ;
  pav:authoredOn "2013-02-26 17:11:07.0" ;
  pav:hasCurrentVersion <http://vocab.nerc.ac.uk/collection/L05/current/102/2> ;
  pav:hasVersion <http://vocab.nerc.ac.uk/collection/L05/current/102/1> ;
  owl:versionInfo "2" ;
  skos:broader sdnc:ICAT04 ;
  skos:definition "Instrument that makes routine meteorological measurements on the atmosphere, typically air pressure, temperature and humidity."@en ;
  skos:inScheme <http://vocab.nerc.ac.uk/scheme/EDMED_DCAT_THEMES/current> ;
  skos:inScheme <http://vocab.nerc.ac.uk/scheme/NETMAR_OCEAN/current> ;
  skos:inScheme <http://vocab.nerc.ac.uk/scheme/NETOC_INSTRUMENT/current> ;
  skos:inScheme <http://vocab.nerc.ac.uk/scheme/SDNDEV/current> ;
  skos:narrower inst:TOOL0281 ;
  skos:narrower inst:TOOL0282 ;
  skos:narrower inst:TOOL0283 ;
  skos:narrower <http://vocab.nerc.ac.uk/collection/W01/current/003> ;
  skos:notation "SDN:L05::102" ;
  skos:note "accepted"@en ;
  skos:prefLabel "meteorological packages"@en ;
  skos:related <http://vocab.nerc.ac.uk/collection/P25/current/ATEMP> ;
.
<http://vocab.nerc.ac.uk/collection/L05/current/103>
  rdf:type skos:Concept ;
  dcterm:date "2007-11-20 09:34:40.0" ;
  dcterm:identifier "SDN:L05::103" ;
  dcterm:source <http://vocab.nerc.ac.uk/scheme/EDMED_DCAT_THEMES/current> ;
  dcterm:source <http://vocab.nerc.ac.uk/scheme/SDNDEV/current> ;
  pav:authoredOn "2007-11-20 09:34:40.0" ;
  pav:hasCurrentVersion <http://vocab.nerc.ac.uk/collection/L05/current/103/1> ;
  owl:versionInfo "1" ;
  skos:broader sdnc:ICAT04 ;
  skos:definition "A balloon-borne package equipped with a radio transmitter and meteorological sensors typically measuring temperature, pressure, and humidity."@en ;
  skos:inScheme <http://vocab.nerc.ac.uk/scheme/EDMED_DCAT_THEMES/current> ;
  skos:inScheme <http://vocab.nerc.ac.uk/scheme/SDNDEV/current> ;
  skos:narrower <http://vocab.nerc.ac.uk/collection/W01/current/003> ;
  skos:notation "SDN:L05::103" ;
  skos:note "accepted"@en ;
  skos:prefLabel "radiosondes"@en ;
.
<http://vocab.nerc.ac.uk/collection/L05/current/110>
  rdf:type skos:Concept ;
  dcterm:date "2007-11-20 09:34:40.0" ;
  dcterm:identifier "SDN:L05::110" ;
  dcterm:source <http://vocab.nerc.ac.uk/scheme/EDMED_DCAT_THEMES/current> ;
  dcterm:source <http://vocab.nerc.ac.uk/scheme/SDNDEV/current> ;
  pav:authoredOn "2007-11-20 09:34:40.0" ;
  pav:hasCurrentVersion <http://vocab.nerc.ac.uk/collection/L05/current/110/1> ;
  owl:versionInfo "1" ;
  skos:broader sdnc:ICAT04 ;
  skos:definition "Instrument that measures water column surface wave parameters including height, period, direction and energy spectra."@en ;
  skos:inScheme <http://vocab.nerc.ac.uk/scheme/EDMED_DCAT_THEMES/current> ;
  skos:inScheme <http://vocab.nerc.ac.uk/scheme/SDNDEV/current> ;
  skos:narrower <http://vocab.nerc.ac.uk/collection/W01/current/003> ;
  skos:notation "SDN:L05::110" ;
  skos:note "accepted"@en ;
  skos:prefLabel "wave recorders"@en ;
  skos:scopeNote "subclasses: radasr wave monitors, waverider buoys, wave sensors" ;
.
<http://vocab.nerc.ac.uk/collection/L05/current/113>
  rdf:type skos:Concept ;
  dcterm:date "2013-02-26 17:11:07.0" ;
  dcterm:identifier "SDN:L05::113" ;
  dcterm:source <http://vocab.nerc.ac.uk/scheme/EDMED_DCAT_THEMES/current> ;
  dcterm:source <http://vocab.nerc.ac.uk/scheme/NETMAR_OCEAN/current> ;
  dcterm:source <http://vocab.nerc.ac.uk/scheme/NETOC_INSTRUMENT/current> ;
  dcterm:source <http://vocab.nerc.ac.uk/scheme/SDNDEV/current> ;
  pav:authoredOn "2013-02-26 17:11:07.0" ;
  pav:hasCurrentVersion <http://vocab.nerc.ac.uk/collection/L05/current/113/2> ;
  pav:hasVersion <http://vocab.nerc.ac.uk/collection/L05/current/113/1> ;
  owl:versionInfo "2" ;
  skos:broader sdnc:ICAT04 ;
  skos:definition "Instrument that measures the amount of stimulated electromagnetic radiation produced by pulses of electromagnetic radiation emitted into the water column."@en ;
  skos:inScheme <http://vocab.nerc.ac.uk/scheme/EDMED_DCAT_THEMES/current> ;
  skos:inScheme <http://vocab.nerc.ac.uk/scheme/NETMAR_OCEAN/current> ;
  skos:inScheme <http://vocab.nerc.ac.uk/scheme/NETOC_INSTRUMENT/current> ;
  skos:inScheme <http://vocab.nerc.ac.uk/scheme/SDNDEV/current> ;
  skos:narrower <http://vocab.nerc.ac.uk/collection/W01/current/003> ;
  skos:notation "SDN:L05::113" ;
  skos:note "accepted"@en ;
  skos:prefLabel "fluorometers"@en ;
  skos:related <http://vocab.nerc.ac.uk/collection/P25/current/CHLA> ;
  skos:related <http://vocab.nerc.ac.uk/collection/P25/current/PHAEO> ;
.
<http://vocab.nerc.ac.uk/collection/L05/current/114>
  rdf:type skos:Concept ;
  dcterm:date "2013-02-26 17:11:07.0" ;
  dcterm:identifier "SDN:L05::114" ;
  dcterm:source <http://vocab.nerc.ac.uk/scheme/EDMED_DCAT_THEMES/current> ;
  dcterm:source <http://vocab.nerc.ac.uk/scheme/SDNDEV/current> ;
  pav:authoredOn "2013-02-26 17:11:07.0" ;
  pav:hasCurrentVersion <http://vocab.nerc.ac.uk/collection/L05/current/114/2> ;
  pav:hasVersion <http://vocab.nerc.ac.uk/collection/L05/current/114/1> ;
  owl:versionInfo "2" ;
  skos:broader sdnc:ICAT04 ;
  skos:definition "Instrument that measures current speed and direction at a single depth."@en ;
  skos:inScheme <http://vocab.nerc.ac.uk/scheme/EDMED_DCAT_THEMES/current> ;
  skos:inScheme <http://vocab.nerc.ac.uk/scheme/SDNDEV/current> ;
  skos:narrower <http://vocab.nerc.ac.uk/collection/W01/current/003> ;
  skos:notation "SDN:L05::114" ;
  skos:note "accepted"@en ;
  skos:prefLabel "current meters"@en ;
.
<http://vocab.nerc.ac.uk/collection/L05/current/115>
  rdf:type skos:Concept ;
  dcterm:date "2013-02-26 17:11:07.0" ;
  dcterm:identifier "SDN:L05::115" ;
  dcterm:source <http://vocab.nerc.ac.uk/scheme/EDMED_DCAT_THEMES/current> ;
  dcterm:source <http://vocab.nerc.ac.uk/scheme/SDNDEV/current> ;
  pav:authoredOn "2013-02-26 17:11:07.0" ;
  pav:hasCurrentVersion <http://vocab.nerc.ac.uk/collection/L05/current/115/2> ;
  pav:hasVersion <http://vocab.nerc.ac.uk/collection/L05/current/115/1> ;
  owl:versionInfo "2" ;
  skos:broader sdnc:ICAT04 ;
  skos:definition "Instrument that measures current speed and direction at multiple predetermined depths simultaneously."@en ;
  skos:inScheme <http://vocab.nerc.ac.uk/scheme/EDMED_DCAT_THEMES/current> ;
  skos:inScheme <http://vocab.nerc.ac.uk/scheme/SDNDEV/current> ;
  skos:narrower <http://mmisw.org/ont/trdi/glossary/acousticDopplerCurrentProfiler> ;
  skos:narrower <http://vocab.nerc.ac.uk/collection/W01/current/003> ;
  skos:notation "SDN:L05::115" ;
  skos:note "accepted"@en ;
  skos:prefLabel "current profilers"@en ;
.
<http://vocab.nerc.ac.uk/collection/L05/current/121>
  rdf:type skos:Concept ;
  dcterm:date "2016-03-10 06:50:01.0" ;
  dcterm:identifier "SDN:L05::121" ;
  dcterm:source <http://vocab.nerc.ac.uk/scheme/EDMED_DCAT_THEMES/current> ;
  dcterm:source <http://vocab.nerc.ac.uk/scheme/SDNDEV/current> ;
  pav:authoredOn "2016-03-10 06:50:01.0" ;
  pav:hasCurrentVersion <http://vocab.nerc.ac.uk/collection/L05/current/121/2> ;
  pav:hasVersion <http://vocab.nerc.ac.uk/collection/L05/current/121/1> ;
  owl:versionInfo "2" ;
  skos:broader sdnc:ICAT05 ;
  skos:definition "A network of satellites that determines the position of a transponder by triangulation such as Argos. Generally used to track surface buoys for the determination of Lagrangian currents."@en ;
  skos:inScheme <http://vocab.nerc.ac.uk/scheme/EDMED_DCAT_THEMES/current> ;
  skos:inScheme <http://vocab.nerc.ac.uk/scheme/SDNDEV/current> ;
  skos:narrower inst:TOOL0697 ;
  skos:narrower <http://vocab.nerc.ac.uk/collection/W01/current/003> ;
  skos:notation "SDN:L05::121" ;
  skos:note "accepted"@en ;
  skos:prefLabel "satellite tracking system"@en ;
.
<http://vocab.nerc.ac.uk/collection/L05/current/122>
  rdf:type skos:Concept ;
  dcterm:date "2013-02-26 17:11:07.0" ;
  dcterm:identifier "SDN:L05::122" ;
  dcterm:source <http://vocab.nerc.ac.uk/scheme/EDMED_DCAT_THEMES/current> ;
  dcterm:source <http://vocab.nerc.ac.uk/scheme/SDNDEV/current> ;
  pav:authoredOn "2013-02-26 17:11:07.0" ;
  pav:hasCurrentVersion <http://vocab.nerc.ac.uk/collection/L05/current/122/2> ;
  pav:hasVersion <http://vocab.nerc.ac.uk/collection/L05/current/122/1> ;
  owl:versionInfo "2" ;
  skos:broader sdnc:ICAT04 ;
  skos:definition "Instrument that measures the intensity of electromagnetic radiation in either the atmosphere or the water column."@en ;
  skos:inScheme <http://vocab.nerc.ac.uk/scheme/EDMED_DCAT_THEMES/current> ;
  skos:inScheme <http://vocab.nerc.ac.uk/scheme/SDNDEV/current> ;
  skos:narrower <http://vocab.nerc.ac.uk/collection/W01/current/003> ;
  skos:notation "SDN:L05::122" ;
  skos:note "accepted"@en ;
  skos:prefLabel "radiometers"@en ;
  skos:scopeNote "subclass: solar radiation sensor, light intensity recorder, pyranometer, color sensor, photosynthetically activie radiation sensor (surface or underwater), pyrgeometer, spectroradiometer, UV sensor/radiometer" ;
.
<http://vocab.nerc.ac.uk/collection/L05/current/123>
  rdf:type skos:Concept ;
  dcterm:date "2007-11-20 09:34:40.0" ;
  dcterm:identifier "SDN:L05::123" ;
  dcterm:source <http://vocab.nerc.ac.uk/scheme/EDMED_DCAT_THEMES/current> ;
  dcterm:source <http://vocab.nerc.ac.uk/scheme/NETMAR_OCEAN/current> ;
  dcterm:source <http://vocab.nerc.ac.uk/scheme/NETOC_INSTRUMENT/current> ;
  dcterm:source <http://vocab.nerc.ac.uk/scheme/NETOC_ORTHO/current> ;
  dcterm:source <http://vocab.nerc.ac.uk/scheme/SDNDEV/current> ;
  pav:authoredOn "2007-11-20 09:34:40.0" ;
  pav:hasCurrentVersion <http://vocab.nerc.ac.uk/collection/L05/current/123/1> ;
  owl:versionInfo "1" ;
  skos:broader sdnc:ICAT04 ;
  skos:definition "Instrument that measures the amount of electromagnetic radiation emitted into the water column returned to the instrument."@en ;
  skos:inScheme <http://vocab.nerc.ac.uk/scheme/EDMED_DCAT_THEMES/current> ;
  skos:inScheme <http://vocab.nerc.ac.uk/scheme/NETMAR_OCEAN/current> ;
  skos:inScheme <http://vocab.nerc.ac.uk/scheme/NETOC_INSTRUMENT/current> ;
  skos:inScheme <http://vocab.nerc.ac.uk/scheme/NETOC_ORTHO/current> ;
  skos:inScheme <http://vocab.nerc.ac.uk/scheme/SDNDEV/current> ;
  skos:narrower <http://vocab.nerc.ac.uk/collection/W01/current/003> ;
  skos:notation "SDN:L05::123" ;
  skos:note "accepted"@en ;
  skos:prefLabel "optical backscatter sensors"@en ;
  skos:related <http://vocab.nerc.ac.uk/collection/P25/current/TURB> ;
.
<http://vocab.nerc.ac.uk/collection/L05/current/124>
  rdf:type skos:Concept ;
  dcterm:date "2007-11-20 09:34:40.0" ;
  dcterm:identifier "SDN:L05::124" ;
  dcterm:source <http://vocab.nerc.ac.uk/scheme/EDMED_DCAT_THEMES/current> ;
  dcterm:source <http://vocab.nerc.ac.uk/scheme/NETMAR_OCEAN/current> ;
  dcterm:source <http://vocab.nerc.ac.uk/scheme/NETOC_INSTRUMENT/current> ;
  dcterm:source <http://vocab.nerc.ac.uk/scheme/NETOC_ORTHO/current> ;
  dcterm:source <http://vocab.nerc.ac.uk/scheme/SDNDEV/current> ;
  pav:authoredOn "2007-11-20 09:34:40.0" ;
  pav:hasCurrentVersion <http://vocab.nerc.ac.uk/collection/L05/current/124/1> ;
  owl:versionInfo "1" ;
  skos:broader sdnc:ICAT04 ;
  skos:definition "Systems that measure the attenuation of electromagnetic radiation by the water column. Includes human observer plus Secchi Disk."@en ;
  skos:inScheme <http://vocab.nerc.ac.uk/scheme/EDMED_DCAT_THEMES/current> ;
  skos:inScheme <http://vocab.nerc.ac.uk/scheme/NETMAR_OCEAN/current> ;
  skos:inScheme <http://vocab.nerc.ac.uk/scheme/NETOC_INSTRUMENT/current> ;
  skos:inScheme <http://vocab.nerc.ac.uk/scheme/NETOC_ORTHO/current> ;
  skos:inScheme <http://vocab.nerc.ac.uk/scheme/SDNDEV/current> ;
  skos:narrower inst:TOOL0148 ;
  skos:narrower inst:TOOL0430 ;
  skos:narrower <http://vocab.nerc.ac.uk/collection/W01/current/003> ;
  skos:notation "SDN:L05::124" ;
  skos:note "accepted"@en ;
  skos:prefLabel "transmissometers"@en ;
  skos:related <http://vocab.nerc.ac.uk/collection/P25/current/TURB> ;
.
<http://vocab.nerc.ac.uk/collection/L05/current/130>
  rdf:type skos:Concept ;
  dcterm:date "2018-04-06 17:31:36.0" ;
  dcterm:identifier "SDN:L05::130" ;
  dcterm:source <http://vocab.nerc.ac.uk/scheme/EDMED_DCAT_THEMES/current> ;
  dcterm:source <http://vocab.nerc.ac.uk/scheme/NETMAR_OCEAN/current> ;
  dcterm:source <http://vocab.nerc.ac.uk/scheme/NETOC_INSTRUMENT/current> ;
  dcterm:source <http://vocab.nerc.ac.uk/scheme/SDNDEV/current> ;
  pav:authoredOn "2018-04-06 17:31:36.0" ;
  pav:hasCurrentVersion <http://vocab.nerc.ac.uk/collection/L05/current/130/3> ;
  pav:hasVersion <http://vocab.nerc.ac.uk/collection/L05/current/130/1> ;
  pav:hasVersion <http://vocab.nerc.ac.uk/collection/L05/current/130/2> ;
  owl:versionInfo "3" ;
  skos:broader sdnc:ICAT04 ;
  skos:definition "A reusable instrument that always simultaneously measures conductivity and temperature (for salinity) and pressure (for depth)."@en ;
  skos:inScheme <http://vocab.nerc.ac.uk/scheme/EDMED_DCAT_THEMES/current> ;
  skos:inScheme <http://vocab.nerc.ac.uk/scheme/NETMAR_OCEAN/current> ;
  skos:inScheme <http://vocab.nerc.ac.uk/scheme/NETOC_INSTRUMENT/current> ;
  skos:inScheme <http://vocab.nerc.ac.uk/scheme/SDNDEV/current> ;
  skos:narrower <http://vocab.nerc.ac.uk/collection/W01/current/003> ;
  skos:notation "SDN:L05::130" ;
  skos:note "accepted"@en ;
  skos:prefLabel "CTD"@en ;
  skos:related inst:TOOL0001 ;
  skos:related <http://vocab.nerc.ac.uk/collection/P25/current/SALIN> ;
  skos:related <http://vocab.nerc.ac.uk/collection/P25/current/WTEMP> ;
.
<http://vocab.nerc.ac.uk/collection/L05/current/131>
  rdf:type skos:Concept ;
  dcterm:date "2018-04-06 17:31:36.0" ;
  dcterm:identifier "SDN:L05::131" ;
  dcterm:source <http://vocab.nerc.ac.uk/scheme/EDMED_DCAT_THEMES/current> ;
  dcterm:source <http://vocab.nerc.ac.uk/scheme/NETMAR_OCEAN/current> ;
  dcterm:source <http://vocab.nerc.ac.uk/scheme/NETOC_INSTRUMENT/current> ;
  dcterm:source <http://vocab.nerc.ac.uk/scheme/SDNDEV/current> ;
  pav:authoredOn "2018-04-06 17:31:36.0" ;
  pav:hasCurrentVersion <http://vocab.nerc.ac.uk/collection/L05/current/131/2> ;
  pav:hasVersion <http://vocab.nerc.ac.uk/collection/L05/current/131/1> ;
  owl:versionInfo "2" ;
  skos:broader sdnc:ICAT04 ;
  skos:definition "An undulating platform towed behind a ship carrying an instrument that measures temperature, conductivity and pressure (for depth) and possibly other instruments such as fluorometers. Current thinking is that this is a platform category and not an instrument category and so its inclusion in this vocabulary was an error. Its usage is not recommended."@en ;
  skos:inScheme <http://vocab.nerc.ac.uk/scheme/EDMED_DCAT_THEMES/current> ;
  skos:inScheme <http://vocab.nerc.ac.uk/scheme/NETMAR_OCEAN/current> ;
  skos:inScheme <http://vocab.nerc.ac.uk/scheme/NETOC_INSTRUMENT/current> ;
  skos:inScheme <http://vocab.nerc.ac.uk/scheme/SDNDEV/current> ;
  skos:narrower <http://vocab.nerc.ac.uk/collection/W01/current/003> ;
  skos:notation "SDN:L05::131" ;
  skos:note "accepted"@en ;
  skos:prefLabel "CTD undulators"@en ;
  skos:related <http://vocab.nerc.ac.uk/collection/P25/current/SALIN> ;
  skos:related <http://vocab.nerc.ac.uk/collection/P25/current/WTEMP> ;
.
<http://vocab.nerc.ac.uk/collection/L05/current/132>
  rdf:type skos:Concept ;
  dcterm:date "2007-11-20 09:34:40.0" ;
  dcterm:identifier "SDN:L05::132" ;
  dcterm:source <http://vocab.nerc.ac.uk/scheme/EDMED_DCAT_THEMES/current> ;
  dcterm:source <http://vocab.nerc.ac.uk/scheme/NETMAR_OCEAN/current> ;
  dcterm:source <http://vocab.nerc.ac.uk/scheme/NETOC_INSTRUMENT/current> ;
  dcterm:source <http://vocab.nerc.ac.uk/scheme/SDNDEV/current> ;
  pav:authoredOn "2007-11-20 09:34:40.0" ;
  pav:hasCurrentVersion <http://vocab.nerc.ac.uk/collection/L05/current/132/1> ;
  owl:versionInfo "1" ;
  skos:broader sdnc:ICAT04 ;
  skos:definition "Instruments that measure vertical profiles of sea temperature by either lowering a pressure plus temperature senor package (MBT) or dropping a free falling disposable sensor (XBT)."@en ;
  skos:inScheme <http://vocab.nerc.ac.uk/scheme/EDMED_DCAT_THEMES/current> ;
  skos:inScheme <http://vocab.nerc.ac.uk/scheme/NETMAR_OCEAN/current> ;
  skos:inScheme <http://vocab.nerc.ac.uk/scheme/NETOC_INSTRUMENT/current> ;
  skos:inScheme <http://vocab.nerc.ac.uk/scheme/SDNDEV/current> ;
  skos:narrower <http://vocab.nerc.ac.uk/collection/L05/current/389> ;
  skos:narrower <http://vocab.nerc.ac.uk/collection/L05/current/390> ;
  skos:narrower <http://vocab.nerc.ac.uk/collection/W01/current/003> ;
  skos:notation "SDN:L05::132" ;
  skos:note "accepted"@en ;
  skos:prefLabel "bathythermographs"@en ;
  skos:related <http://vocab.nerc.ac.uk/collection/P25/current/WTEMP> ;
.
<http://vocab.nerc.ac.uk/collection/L05/current/133>
  rdf:type skos:Concept ;
  dcterm:date "2007-11-20 09:34:40.0" ;
  dcterm:identifier "SDN:L05::133" ;
  dcterm:source <http://vocab.nerc.ac.uk/scheme/EDMED_DCAT_THEMES/current> ;
  dcterm:source <http://vocab.nerc.ac.uk/scheme/NETMAR_OCEAN/current> ;
  dcterm:source <http://vocab.nerc.ac.uk/scheme/NETOC_INSTRUMENT/current> ;
  dcterm:source <http://vocab.nerc.ac.uk/scheme/SDNDEV/current> ;
  pav:authoredOn "2007-11-20 09:34:40.0" ;
  pav:hasCurrentVersion <http://vocab.nerc.ac.uk/collection/L05/current/133/1> ;
  owl:versionInfo "1" ;
  skos:broader sdnc:ICAT04 ;
  skos:definition "Temperature and conductivity sensors mounted on a sea-surface platform continuously measuring a surface water supply."@en ;
  skos:inScheme <http://vocab.nerc.ac.uk/scheme/EDMED_DCAT_THEMES/current> ;
  skos:inScheme <http://vocab.nerc.ac.uk/scheme/NETMAR_OCEAN/current> ;
  skos:inScheme <http://vocab.nerc.ac.uk/scheme/NETOC_INSTRUMENT/current> ;
  skos:inScheme <http://vocab.nerc.ac.uk/scheme/SDNDEV/current> ;
  skos:narrower <http://vocab.nerc.ac.uk/collection/W01/current/003> ;
  skos:notation "SDN:L05::133" ;
  skos:note "accepted"@en ;
  skos:prefLabel "thermosalinographs"@en ;
  skos:related <http://vocab.nerc.ac.uk/collection/P25/current/SALIN> ;
  skos:related <http://vocab.nerc.ac.uk/collection/P25/current/WTEMP> ;
.
<http://vocab.nerc.ac.uk/collection/L05/current/134>
  rdf:type skos:Concept ;
  dcterm:date "2013-02-26 17:11:07.0" ;
  dcterm:identifier "SDN:L05::134" ;
  dcterm:source <http://vocab.nerc.ac.uk/scheme/EDMED_DCAT_THEMES/current> ;
  dcterm:source <http://vocab.nerc.ac.uk/scheme/NETMAR_OCEAN/current> ;
  dcterm:source <http://vocab.nerc.ac.uk/scheme/NETOC_INSTRUMENT/current> ;
  dcterm:source <http://vocab.nerc.ac.uk/scheme/SDNDEV/current> ;
  pav:authoredOn "2013-02-26 17:11:07.0" ;
  pav:hasCurrentVersion <http://vocab.nerc.ac.uk/collection/L05/current/134/3> ;
  pav:hasVersion <http://vocab.nerc.ac.uk/collection/L05/current/134/1> ;
  pav:hasVersion <http://vocab.nerc.ac.uk/collection/L05/current/134/2> ;
  owl:versionInfo "3" ;
  skos:broader sdnc:ICAT04 ;
  skos:definition "An instrument that measures the temperature of the water with which it is in contact."@en ;
  skos:inScheme <http://vocab.nerc.ac.uk/scheme/EDMED_DCAT_THEMES/current> ;
  skos:inScheme <http://vocab.nerc.ac.uk/scheme/NETMAR_OCEAN/current> ;
  skos:inScheme <http://vocab.nerc.ac.uk/scheme/NETOC_INSTRUMENT/current> ;
  skos:inScheme <http://vocab.nerc.ac.uk/scheme/SDNDEV/current> ;
  skos:narrower inst:TOOL0001 ;
  skos:narrower inst:TOOL0237 ;
  skos:narrower inst:TOOL0238 ;
  skos:narrower inst:TOOL1638 ;
  skos:narrower <http://vocab.nerc.ac.uk/collection/W01/current/003> ;
  skos:notation "SDN:L05::134" ;
  skos:note "accepted"@en ;
  skos:prefLabel "water temperature sensor"@en ;
  skos:related <http://vocab.nerc.ac.uk/collection/P25/current/WTEMP> ;
.
<http://vocab.nerc.ac.uk/collection/L05/current/135>
  rdf:type skos:Concept ;
  dcterm:date "2007-11-20 09:34:40.0" ;
  dcterm:identifier "SDN:L05::135" ;
  dcterm:source <http://vocab.nerc.ac.uk/scheme/EDMED_DCAT_THEMES/current> ;
  dcterm:source <http://vocab.nerc.ac.uk/scheme/NETMAR_OCEAN/current> ;
  dcterm:source <http://vocab.nerc.ac.uk/scheme/NETOC_INSTRUMENT/current> ;
  dcterm:source <http://vocab.nerc.ac.uk/scheme/SDNDEV/current> ;
  pav:authoredOn "2007-11-20 09:34:40.0" ;
  pav:hasCurrentVersion <http://vocab.nerc.ac.uk/collection/L05/current/135/1> ;
  owl:versionInfo "1" ;
  skos:broader sdnc:ICAT04 ;
  skos:definition "A group of rigidly-mounted temperature sensors sampled by a common data logger held at various depths in the water column."@en ;
  skos:inScheme <http://vocab.nerc.ac.uk/scheme/EDMED_DCAT_THEMES/current> ;
  skos:inScheme <http://vocab.nerc.ac.uk/scheme/NETMAR_OCEAN/current> ;
  skos:inScheme <http://vocab.nerc.ac.uk/scheme/NETOC_INSTRUMENT/current> ;
  skos:inScheme <http://vocab.nerc.ac.uk/scheme/SDNDEV/current> ;
  skos:narrower <http://vocab.nerc.ac.uk/collection/W01/current/003> ;
  skos:notation "SDN:L05::135" ;
  skos:note "accepted"@en ;
  skos:prefLabel "thermistor chains"@en ;
  skos:related <http://vocab.nerc.ac.uk/collection/P25/current/WTEMP> ;
.
<http://vocab.nerc.ac.uk/collection/L05/current/150>
  rdf:type skos:Concept ;
  dcterm:date "2017-08-08 14:48:18.0" ;
  dcterm:identifier "SDN:L05::150" ;
  dcterm:source <http://vocab.nerc.ac.uk/scheme/EDMED_DCAT_THEMES/current> ;
  dcterm:source <http://vocab.nerc.ac.uk/scheme/SDNDEV/current> ;
  pav:authoredOn "2017-08-08 14:48:18.0" ;
  pav:hasCurrentVersion <http://vocab.nerc.ac.uk/collection/L05/current/150/3> ;
  pav:hasVersion <http://vocab.nerc.ac.uk/collection/L05/current/150/1> ;
  pav:hasVersion <http://vocab.nerc.ac.uk/collection/L05/current/150/2> ;
  owl:versionInfo "3" ;
  skos:broader sdnc:ICAT04 ;
  skos:definition "Sensors or instruments physically located in any body of water that measure the size spectrum of particles suspended in it."@en ;
  skos:inScheme <http://vocab.nerc.ac.uk/scheme/EDMED_DCAT_THEMES/current> ;
  skos:inScheme <http://vocab.nerc.ac.uk/scheme/SDNDEV/current> ;
  skos:narrower <http://vocab.nerc.ac.uk/collection/W01/current/003> ;
  skos:notation "SDN:L05::150" ;
  skos:note "accepted"@en ;
  skos:prefLabel "in-situ particle sizers"@en ;
.
<http://vocab.nerc.ac.uk/collection/L05/current/152>
  rdf:type skos:Concept ;
  dcterm:date "2022-11-17 09:42:34.0" ;
  dcterm:identifier "SDN:L05::152" ;
  dcterm:source <http://vocab.nerc.ac.uk/scheme/EDMED_DCAT_THEMES/current> ;
  dcterm:source <http://vocab.nerc.ac.uk/scheme/SDNDEV/current> ;
  pav:authoredOn "2022-11-17 09:42:34.0" ;
  pav:hasCurrentVersion <http://vocab.nerc.ac.uk/collection/L05/current/152/2> ;
  pav:hasVersion <http://vocab.nerc.ac.uk/collection/L05/current/152/1> ;
  owl:versionInfo "2" ;
  skos:broader sdnc:ICAT04 ;
  skos:definition "Instruments with directional acoustic transmitters and receivers fitted to an underwater platform that emit fan-shaped pulses down toward the seafloor across a wide angle perpendicular to the path of the platform through the water. Used for the classification of seafloor substrates and structures according to the intensity of signal return. Higher signal return intensities indicate harder substrates or structures, and vice versa."@en ;
  skos:inScheme <http://vocab.nerc.ac.uk/scheme/EDMED_DCAT_THEMES/current> ;
  skos:inScheme <http://vocab.nerc.ac.uk/scheme/SDNDEV/current> ;
  skos:narrower <http://vocab.nerc.ac.uk/collection/W01/current/003> ;
  skos:notation "SDN:L05::152" ;
  skos:note "accepted"@en ;
  skos:prefLabel "sidescan sonars"@en ;
.
<http://vocab.nerc.ac.uk/collection/L05/current/153>
  rdf:type skos:Concept ;
  dcterm:date "2010-02-19 11:58:13.0" ;
  dcterm:identifier "SDN:L05::153" ;
  dcterm:source <http://vocab.nerc.ac.uk/scheme/EDMED_DCAT_THEMES/current> ;
  dcterm:source <http://vocab.nerc.ac.uk/scheme/SDNDEV/current> ;
  pav:authoredOn "2010-02-19 11:58:13.0" ;
  pav:hasCurrentVersion <http://vocab.nerc.ac.uk/collection/L05/current/153/2> ;
  pav:hasVersion <http://vocab.nerc.ac.uk/collection/L05/current/153/1> ;
  owl:versionInfo "2" ;
  skos:broader sdnc:ICAT04 ;
  skos:definition "An energy source of unspecified frequency plus a single string of towed hydrophones (streamer) that determine geologic structure by detecting waves reflected by subsurface layers."@en ;
  skos:inScheme <http://vocab.nerc.ac.uk/scheme/EDMED_DCAT_THEMES/current> ;
  skos:inScheme <http://vocab.nerc.ac.uk/scheme/SDNDEV/current> ;
  skos:narrower <http://vocab.nerc.ac.uk/collection/L05/current/362> ;
  skos:narrower <http://vocab.nerc.ac.uk/collection/L05/current/363> ;
  skos:narrower <http://vocab.nerc.ac.uk/collection/L05/current/371> ;
  skos:narrower <http://vocab.nerc.ac.uk/collection/L05/current/372> ;
  skos:narrower <http://vocab.nerc.ac.uk/collection/L05/current/373> ;
  skos:narrower <http://vocab.nerc.ac.uk/collection/W01/current/003> ;
  skos:notation "SDN:L05::153" ;
  skos:note "accepted"@en ;
  skos:prefLabel "single-channel seismic reflection systems"@en ;
  skos:related inst:TOOL0353 ;
  skos:related inst:TOOL0354 ;
  skos:related inst:TOOL0355 ;
  skos:related inst:TOOL0356 ;
  skos:related inst:TOOL0357 ;
  skos:related inst:TOOL0358 ;
.
<http://vocab.nerc.ac.uk/collection/L05/current/154>
  rdf:type skos:Concept ;
  dcterm:date "2010-02-19 11:59:29.0" ;
  dcterm:identifier "SDN:L05::154" ;
  dcterm:source <http://vocab.nerc.ac.uk/scheme/EDMED_DCAT_THEMES/current> ;
  dcterm:source <http://vocab.nerc.ac.uk/scheme/SDNDEV/current> ;
  pav:authoredOn "2010-02-19 11:59:29.0" ;
  pav:hasCurrentVersion <http://vocab.nerc.ac.uk/collection/L05/current/154/2> ;
  pav:hasVersion <http://vocab.nerc.ac.uk/collection/L05/current/154/1> ;
  owl:versionInfo "2" ;
  skos:broader sdnc:ICAT04 ;
  skos:definition "An energy source of unspecified frequency plus a multiple strings of towed hydrophones (streamers) that determine geologic structure by detecting waves reflected by subsurface layers."@en ;
  skos:inScheme <http://vocab.nerc.ac.uk/scheme/EDMED_DCAT_THEMES/current> ;
  skos:inScheme <http://vocab.nerc.ac.uk/scheme/SDNDEV/current> ;
  skos:narrower <http://vocab.nerc.ac.uk/collection/L05/current/364> ;
  skos:narrower <http://vocab.nerc.ac.uk/collection/L05/current/365> ;
  skos:narrower <http://vocab.nerc.ac.uk/collection/L05/current/366> ;
  skos:narrower <http://vocab.nerc.ac.uk/collection/L05/current/374> ;
  skos:narrower <http://vocab.nerc.ac.uk/collection/L05/current/375> ;
  skos:narrower <http://vocab.nerc.ac.uk/collection/W01/current/003> ;
  skos:notation "SDN:L05::154" ;
  skos:note "accepted"@en ;
  skos:prefLabel "multi-channel seismic reflection systems"@en ;
  skos:related inst:TOOL0353 ;
  skos:related inst:TOOL0354 ;
  skos:related inst:TOOL0355 ;
  skos:related inst:TOOL0356 ;
  skos:related inst:TOOL0357 ;
  skos:related inst:TOOL0358 ;
.
<http://vocab.nerc.ac.uk/collection/L05/current/155>
  rdf:type skos:Concept ;
  dcterm:date "2007-11-20 09:34:40.0" ;
  dcterm:identifier "SDN:L05::155" ;
  dcterm:source <http://vocab.nerc.ac.uk/scheme/EDMED_DCAT_THEMES/current> ;
  dcterm:source <http://vocab.nerc.ac.uk/scheme/SDNDEV/current> ;
  pav:authoredOn "2007-11-20 09:34:40.0" ;
  pav:hasCurrentVersion <http://vocab.nerc.ac.uk/collection/L05/current/155/1> ;
  owl:versionInfo "1" ;
  skos:broader sdnc:ICAT04 ;
  skos:definition "A network of seismometers or geophones plus an energy source that determine geologic structure by detecting waves refracted by subsurface layers."@en ;
  skos:inScheme <http://vocab.nerc.ac.uk/scheme/EDMED_DCAT_THEMES/current> ;
  skos:inScheme <http://vocab.nerc.ac.uk/scheme/SDNDEV/current> ;
  skos:narrower <http://vocab.nerc.ac.uk/collection/W01/current/003> ;
  skos:notation "SDN:L05::155" ;
  skos:note "accepted"@en ;
  skos:prefLabel "seismic refraction systems"@en ;
.
<http://vocab.nerc.ac.uk/collection/L05/current/156>
  rdf:type skos:Concept ;
  dcterm:date "2013-02-26 17:11:07.0" ;
  dcterm:identifier "SDN:L05::156" ;
  dcterm:source <http://vocab.nerc.ac.uk/scheme/EDMED_DCAT_THEMES/current> ;
  dcterm:source <http://vocab.nerc.ac.uk/scheme/NETMAR_OCEAN/current> ;
  dcterm:source <http://vocab.nerc.ac.uk/scheme/NETOC_INSTRUMENT/current> ;
  dcterm:source <http://vocab.nerc.ac.uk/scheme/SDNDEV/current> ;
  pav:authoredOn "2013-02-26 17:11:07.0" ;
  pav:hasCurrentVersion <http://vocab.nerc.ac.uk/collection/L05/current/156/2> ;
  pav:hasVersion <http://vocab.nerc.ac.uk/collection/L05/current/156/1> ;
  owl:versionInfo "2" ;
  skos:broader sdnc:ICAT04 ;
  skos:definition "Instruments that measure water depth at a single point below the platform by timing pulses of sound reflected on the seafloor."@en ;
  skos:inScheme <http://vocab.nerc.ac.uk/scheme/EDMED_DCAT_THEMES/current> ;
  skos:inScheme <http://vocab.nerc.ac.uk/scheme/NETMAR_OCEAN/current> ;
  skos:inScheme <http://vocab.nerc.ac.uk/scheme/NETOC_INSTRUMENT/current> ;
  skos:inScheme <http://vocab.nerc.ac.uk/scheme/SDNDEV/current> ;
  skos:narrower <http://vocab.nerc.ac.uk/collection/W01/current/003> ;
  skos:notation "SDN:L05::156" ;
  skos:note "accepted"@en ;
  skos:prefLabel "single-beam echosounders"@en ;
  skos:related <http://vocab.nerc.ac.uk/collection/P25/current/ELEV> ;
.
<http://vocab.nerc.ac.uk/collection/L05/current/157>
  rdf:type skos:Concept ;
  dcterm:date "2013-02-26 17:11:07.0" ;
  dcterm:identifier "SDN:L05::157" ;
  dcterm:source <http://vocab.nerc.ac.uk/scheme/EDMED_DCAT_THEMES/current> ;
  dcterm:source <http://vocab.nerc.ac.uk/scheme/NETMAR_OCEAN/current> ;
  dcterm:source <http://vocab.nerc.ac.uk/scheme/NETOC_INSTRUMENT/current> ;
  dcterm:source <http://vocab.nerc.ac.uk/scheme/SDNDEV/current> ;
  pav:authoredOn "2013-02-26 17:11:07.0" ;
  pav:hasCurrentVersion <http://vocab.nerc.ac.uk/collection/L05/current/157/2> ;
  pav:hasVersion <http://vocab.nerc.ac.uk/collection/L05/current/157/1> ;
  owl:versionInfo "2" ;
  skos:broader sdnc:ICAT04 ;
  skos:definition "Instruments that measure water depth along several tracks parallel to the platform track by timing pulses of sound reflected on the seafloor."@en ;
  skos:inScheme <http://vocab.nerc.ac.uk/scheme/EDMED_DCAT_THEMES/current> ;
  skos:inScheme <http://vocab.nerc.ac.uk/scheme/NETMAR_OCEAN/current> ;
  skos:inScheme <http://vocab.nerc.ac.uk/scheme/NETOC_INSTRUMENT/current> ;
  skos:inScheme <http://vocab.nerc.ac.uk/scheme/SDNDEV/current> ;
  skos:narrower <http://vocab.nerc.ac.uk/collection/W01/current/003> ;
  skos:notation "SDN:L05::157" ;
  skos:note "accepted"@en ;
  skos:prefLabel "multi-beam echosounders"@en ;
  skos:related <http://vocab.nerc.ac.uk/collection/P25/current/ELEV> ;
.
<http://vocab.nerc.ac.uk/collection/L05/current/158>
  rdf:type skos:Concept ;
  dcterm:date "2013-02-26 17:11:07.0" ;
  dcterm:identifier "SDN:L05::158" ;
  dcterm:source <http://vocab.nerc.ac.uk/scheme/EDMED_DCAT_THEMES/current> ;
  dcterm:source <http://vocab.nerc.ac.uk/scheme/SDNDEV/current> ;
  pav:authoredOn "2013-02-26 17:11:07.0" ;
  pav:hasCurrentVersion <http://vocab.nerc.ac.uk/collection/L05/current/158/2> ;
  pav:hasVersion <http://vocab.nerc.ac.uk/collection/L05/current/158/1> ;
  owl:versionInfo "2" ;
  skos:broader sdnc:ICAT04 ;
  skos:definition "Instrument that makes measurements of the Earth's gravity field."@en ;
  skos:inScheme <http://vocab.nerc.ac.uk/scheme/EDMED_DCAT_THEMES/current> ;
  skos:inScheme <http://vocab.nerc.ac.uk/scheme/SDNDEV/current> ;
  skos:narrower <http://vocab.nerc.ac.uk/collection/W01/current/003> ;
  skos:notation "SDN:L05::158" ;
  skos:note "accepted"@en ;
  skos:prefLabel "gravimeters"@en ;
.
<http://vocab.nerc.ac.uk/collection/L05/current/159>
  rdf:type skos:Concept ;
  dcterm:date "2013-02-26 17:11:07.0" ;
  dcterm:identifier "SDN:L05::159" ;
  dcterm:source <http://vocab.nerc.ac.uk/scheme/EDMED_DCAT_THEMES/current> ;
  dcterm:source <http://vocab.nerc.ac.uk/scheme/SDNDEV/current> ;
  pav:authoredOn "2013-02-26 17:11:07.0" ;
  pav:hasCurrentVersion <http://vocab.nerc.ac.uk/collection/L05/current/159/2> ;
  pav:hasVersion <http://vocab.nerc.ac.uk/collection/L05/current/159/1> ;
  owl:versionInfo "2" ;
  skos:broader sdnc:ICAT04 ;
  skos:definition "Instrument that makes measurements of the Earth's magnetic field."@en ;
  skos:inScheme <http://vocab.nerc.ac.uk/scheme/EDMED_DCAT_THEMES/current> ;
  skos:inScheme <http://vocab.nerc.ac.uk/scheme/SDNDEV/current> ;
  skos:narrower <http://vocab.nerc.ac.uk/collection/W01/current/003> ;
  skos:notation "SDN:L05::159" ;
  skos:note "accepted"@en ;
  skos:prefLabel "magnetometers"@en ;
.
<http://vocab.nerc.ac.uk/collection/L05/current/180>
  rdf:type skos:Concept ;
  <http://purl.org/dc/terms/:isReplacedBy> <http://vocab.nerc.ac.uk/collection/L05/current/311> ;
  dcterm:date "2020-09-18 10:24:38.0" ;
  dcterm:identifier "SDN:L05::180" ;
  dcterm:source <http://vocab.nerc.ac.uk/scheme/EDMED_DCAT_THEMES/current> ;
  dcterm:source <http://vocab.nerc.ac.uk/scheme/SDNDEV/current> ;
  pav:authoredOn "2020-09-18 10:24:38.0" ;
  pav:hasCurrentVersion <http://vocab.nerc.ac.uk/collection/L05/current/180/5> ;
  pav:hasVersion <http://vocab.nerc.ac.uk/collection/L05/current/180/1> ;
  pav:hasVersion <http://vocab.nerc.ac.uk/collection/L05/current/180/2> ;
  pav:hasVersion <http://vocab.nerc.ac.uk/collection/L05/current/180/3> ;
  pav:hasVersion <http://vocab.nerc.ac.uk/collection/L05/current/180/4> ;
  owl:deprecated "true" ;
  owl:versionInfo "5" ;
  skos:broader <http://vocab.nerc.ac.uk/collection/L05/current/311> ;
  skos:definition "Code deprecated on 18Sep2020: created in error. Description was: All types of photographic equipment that may be deployed underwater including stills, video, film and digital systems."@en ;
  skos:inScheme <http://vocab.nerc.ac.uk/scheme/EDMED_DCAT_THEMES/current> ;
  skos:inScheme <http://vocab.nerc.ac.uk/scheme/SDNDEV/current> ;
  skos:narrower <http://vocab.nerc.ac.uk/collection/L05/current/378> ;
  skos:narrower <http://vocab.nerc.ac.uk/collection/W01/current/003> ;
  skos:notation "SDN:L05::180" ;
  skos:note "deprecated"@en ;
  skos:prefLabel "underwater cameras"@en ;
.
<http://vocab.nerc.ac.uk/collection/L05/current/181>
  rdf:type skos:Concept ;
  dcterm:date "2013-02-26 17:11:07.0" ;
  dcterm:identifier "SDN:L05::181" ;
  dcterm:source <http://vocab.nerc.ac.uk/scheme/EDMED_DCAT_THEMES/current> ;
  dcterm:source <http://vocab.nerc.ac.uk/scheme/NETMAR_OCEAN/current> ;
  dcterm:source <http://vocab.nerc.ac.uk/scheme/NETOC_INSTRUMENT/current> ;
  dcterm:source <http://vocab.nerc.ac.uk/scheme/SDNDEV/current> ;
  pav:authoredOn "2013-02-26 17:11:07.0" ;
  pav:hasCurrentVersion <http://vocab.nerc.ac.uk/collection/L05/current/181/2> ;
  pav:hasVersion <http://vocab.nerc.ac.uk/collection/L05/current/181/1> ;
  owl:versionInfo "2" ;
  skos:broader sdnc:ICAT04 ;
  skos:definition "Instrument that makes in-situ measurements of one or more of nitrate, nitrite, ammonium, urea, phosphate or silicate dissolved in the water column."@en ;
  skos:inScheme <http://vocab.nerc.ac.uk/scheme/EDMED_DCAT_THEMES/current> ;
  skos:inScheme <http://vocab.nerc.ac.uk/scheme/NETMAR_OCEAN/current> ;
  skos:inScheme <http://vocab.nerc.ac.uk/scheme/NETOC_INSTRUMENT/current> ;
  skos:inScheme <http://vocab.nerc.ac.uk/scheme/SDNDEV/current> ;
  skos:narrower <http://vocab.nerc.ac.uk/collection/W01/current/003> ;
  skos:notation "SDN:L05::181" ;
  skos:note "accepted"@en ;
  skos:prefLabel "nutrient analysers"@en ;
  skos:related <http://vocab.nerc.ac.uk/collection/P25/current/NO2> ;
  skos:related <http://vocab.nerc.ac.uk/collection/P25/current/NO3> ;
  skos:related <http://vocab.nerc.ac.uk/collection/P25/current/NO3NO2> ;
  skos:related <http://vocab.nerc.ac.uk/collection/P25/current/PO4> ;
  skos:related <http://vocab.nerc.ac.uk/collection/P25/current/SLCA> ;
.
<http://vocab.nerc.ac.uk/collection/L05/current/183>
  rdf:type skos:Concept ;
  dcterm:date "2007-11-20 09:34:40.0" ;
  dcterm:identifier "SDN:L05::183" ;
  dcterm:source <http://vocab.nerc.ac.uk/scheme/EDMED_DCAT_THEMES/current> ;
  dcterm:source <http://vocab.nerc.ac.uk/scheme/SDNDEV/current> ;
  pav:authoredOn "2007-11-20 09:34:40.0" ;
  pav:hasCurrentVersion <http://vocab.nerc.ac.uk/collection/L05/current/183/1> ;
  owl:versionInfo "1" ;
  skos:broader sdnc:ICAT04 ;
  skos:definition "Instrument that measures the amount of sound energy transmitted into the water column returned to the instrument."@en ;
  skos:inScheme <http://vocab.nerc.ac.uk/scheme/EDMED_DCAT_THEMES/current> ;
  skos:inScheme <http://vocab.nerc.ac.uk/scheme/SDNDEV/current> ;
  skos:narrower <http://vocab.nerc.ac.uk/collection/W01/current/003> ;
  skos:notation "SDN:L05::183" ;
  skos:note "accepted"@en ;
  skos:prefLabel "acoustic backscatter sensors"@en ;
.
<http://vocab.nerc.ac.uk/collection/L05/current/184>
  rdf:type skos:Concept ;
  dcterm:date "2012-02-23 10:11:31.0" ;
  dcterm:identifier "SDN:L05::184" ;
  dcterm:source <http://vocab.nerc.ac.uk/scheme/EDMED_DCAT_THEMES/current> ;
  dcterm:source <http://vocab.nerc.ac.uk/scheme/SDNDEV/current> ;
  pav:authoredOn "2012-02-23 10:11:31.0" ;
  pav:hasCurrentVersion <http://vocab.nerc.ac.uk/collection/L05/current/184/2> ;
  pav:hasVersion <http://vocab.nerc.ac.uk/collection/L05/current/184/1> ;
  owl:versionInfo "2" ;
  skos:broader sdnc:ICAT04 ;
  skos:definition "Fast response sensors sampled at high frequency to determine the distribution of water body properties on a millimetric scale."@en ;
  skos:inScheme <http://vocab.nerc.ac.uk/scheme/EDMED_DCAT_THEMES/current> ;
  skos:inScheme <http://vocab.nerc.ac.uk/scheme/SDNDEV/current> ;
  skos:narrower <http://vocab.nerc.ac.uk/collection/W01/current/003> ;
  skos:notation "SDN:L05::184" ;
  skos:note "accepted"@en ;
  skos:prefLabel "microstructure sensors"@en ;
.
<http://vocab.nerc.ac.uk/collection/L05/current/185>
  rdf:type skos:Concept ;
  dcterm:date "2013-02-26 17:11:07.0" ;
  dcterm:identifier "SDN:L05::185" ;
  dcterm:source <http://vocab.nerc.ac.uk/scheme/EDMED_DCAT_THEMES/current> ;
  dcterm:source <http://vocab.nerc.ac.uk/scheme/SDNDEV/current> ;
  pav:authoredOn "2013-02-26 17:11:07.0" ;
  pav:hasCurrentVersion <http://vocab.nerc.ac.uk/collection/L05/current/185/2> ;
  pav:hasVersion <http://vocab.nerc.ac.uk/collection/L05/current/185/1> ;
  owl:versionInfo "2" ;
  skos:broader sdnc:ICAT04 ;
  skos:definition "Instrument that measures the velocity of sound in seawater."@en ;
  skos:inScheme <http://vocab.nerc.ac.uk/scheme/EDMED_DCAT_THEMES/current> ;
  skos:inScheme <http://vocab.nerc.ac.uk/scheme/SDNDEV/current> ;
  skos:narrower <http://vocab.nerc.ac.uk/collection/W01/current/003> ;
  skos:notation "SDN:L05::185" ;
  skos:note "accepted"@en ;
  skos:prefLabel "sound velocity sensors"@en ;
.
<http://vocab.nerc.ac.uk/collection/L05/current/186>
  rdf:type skos:Concept ;
  dcterm:date "2011-04-15 14:18:31.0" ;
  dcterm:identifier "SDN:L05::186" ;
  dcterm:source <http://vocab.nerc.ac.uk/scheme/EDMED_DCAT_THEMES/current> ;
  dcterm:source <http://vocab.nerc.ac.uk/scheme/NETMAR_OCEAN/current> ;
  dcterm:source <http://vocab.nerc.ac.uk/scheme/NETOC_INSTRUMENT/current> ;
  dcterm:source <http://vocab.nerc.ac.uk/scheme/SDNDEV/current> ;
  pav:authoredOn "2011-04-15 14:18:31.0" ;
  pav:hasCurrentVersion <http://vocab.nerc.ac.uk/collection/L05/current/186/2> ;
  pav:hasVersion <http://vocab.nerc.ac.uk/collection/L05/current/186/1> ;
  owl:versionInfo "2" ;
  skos:broader sdnc:ICAT05 ;
  skos:definition "Instruments that determine the distance between the platform and the Earth's surface by timing reflected electromagnetic radiation, usually microwaves."@en ;
  skos:inScheme <http://vocab.nerc.ac.uk/scheme/EDMED_DCAT_THEMES/current> ;
  skos:inScheme <http://vocab.nerc.ac.uk/scheme/NETMAR_OCEAN/current> ;
  skos:inScheme <http://vocab.nerc.ac.uk/scheme/NETOC_INSTRUMENT/current> ;
  skos:inScheme <http://vocab.nerc.ac.uk/scheme/SDNDEV/current> ;
  skos:narrower inst:TOOL1043 ;
  skos:narrower inst:TOOL1044 ;
  skos:narrower inst:TOOL1045 ;
  skos:narrower inst:TOOL1046 ;
  skos:narrower inst:TOOL1047 ;
  skos:narrower inst:TOOL1078 ;
  skos:narrower <http://vocab.nerc.ac.uk/collection/W01/current/003> ;
  skos:notation "SDN:L05::186" ;
  skos:note "accepted"@en ;
  skos:prefLabel "radar altimeters"@en ;
  skos:related <http://vocab.nerc.ac.uk/collection/P25/current/ICEBERG> ;
  skos:related <http://vocab.nerc.ac.uk/collection/P25/current/ICETHICK> ;
.
<http://vocab.nerc.ac.uk/collection/L05/current/301>
  rdf:type skos:Concept ;
  dcterm:date "2007-11-20 09:03:34.0" ;
  dcterm:identifier "SDN:L05::301" ;
  dcterm:source <http://vocab.nerc.ac.uk/scheme/EDMED_DCAT_THEMES/current> ;
  dcterm:source <http://vocab.nerc.ac.uk/scheme/SDNDEV/current> ;
  pav:authoredOn "2007-11-20 09:03:34.0" ;
  pav:hasCurrentVersion <http://vocab.nerc.ac.uk/collection/L05/current/301/1> ;
  owl:versionInfo "1" ;
  skos:broader sdnc:ICAT05 ;
  skos:definition "A network of statellites that generate signals that allow a receiver to determine its position such as GPS."@en ;
  skos:inScheme <http://vocab.nerc.ac.uk/scheme/EDMED_DCAT_THEMES/current> ;
  skos:inScheme <http://vocab.nerc.ac.uk/scheme/SDNDEV/current> ;
  skos:narrower inst:TOOL1624 ;
  skos:narrower inst:TOOL1625 ;
  skos:narrower inst:TOOL1626 ;
  skos:narrower inst:TOOL1627 ;
  skos:narrower inst:TOOL1633 ;
  skos:narrower <http://vocab.nerc.ac.uk/collection/W01/current/003> ;
  skos:notation "SDN:L05::301" ;
  skos:note "accepted"@en ;
  skos:prefLabel "satellite positioning systems"@en ;
.
<http://vocab.nerc.ac.uk/collection/L05/current/302>
  rdf:type skos:Concept ;
  dcterm:date "2010-11-19 14:27:24.0" ;
  dcterm:identifier "SDN:L05::302" ;
  dcterm:source <http://vocab.nerc.ac.uk/scheme/EDMED_DCAT_THEMES/current> ;
  dcterm:source <http://vocab.nerc.ac.uk/scheme/NETMAR_OCEAN/current> ;
  dcterm:source <http://vocab.nerc.ac.uk/scheme/NETOC_INSTRUMENT/current> ;
  dcterm:source <http://vocab.nerc.ac.uk/scheme/SDNDEV/current> ;
  pav:authoredOn "2010-11-19 14:27:24.0" ;
  pav:hasCurrentVersion <http://vocab.nerc.ac.uk/collection/L05/current/302/3> ;
  pav:hasVersion <http://vocab.nerc.ac.uk/collection/L05/current/302/1> ;
  pav:hasVersion <http://vocab.nerc.ac.uk/collection/L05/current/302/2> ;
  owl:versionInfo "3" ;
  skos:broader sdnc:ICAT05 ;
  skos:definition "Sensors that measure the intensity and nature of electromagnetic radiation emitted from the Earth in a manner optimised for the determination of water body surface temperature."@en ;
  skos:inScheme <http://vocab.nerc.ac.uk/scheme/EDMED_DCAT_THEMES/current> ;
  skos:inScheme <http://vocab.nerc.ac.uk/scheme/NETMAR_OCEAN/current> ;
  skos:inScheme <http://vocab.nerc.ac.uk/scheme/NETOC_INSTRUMENT/current> ;
  skos:inScheme <http://vocab.nerc.ac.uk/scheme/SDNDEV/current> ;
  skos:narrower inst:TOOL0844 ;
  skos:narrower inst:TOOL0930 ;
  skos:narrower inst:TOOL1016 ;
  skos:narrower inst:TOOL1050 ;
  skos:narrower inst:TOOL1060 ;
  skos:narrower inst:TOOL1061 ;
  skos:narrower inst:TOOL1065 ;
  skos:narrower inst:TOOL1066 ;
  skos:narrower inst:TOOL1072 ;
  skos:narrower inst:TOOL1073 ;
  skos:narrower inst:TOOL1074 ;
  skos:narrower inst:TOOL1075 ;
  skos:narrower inst:TOOL1076 ;
  skos:narrower <http://vocab.nerc.ac.uk/collection/W01/current/003> ;
  skos:notation "SDN:L05::302" ;
  skos:note "accepted"@en ;
  skos:prefLabel "water body temperature sensor"@en ;
  skos:related <http://vocab.nerc.ac.uk/collection/P25/current/WTEMP> ;
.
<http://vocab.nerc.ac.uk/collection/L05/current/303>
  rdf:type skos:Concept ;
  dcterm:date "2013-02-26 17:11:07.0" ;
  dcterm:identifier "SDN:L05::303" ;
  dcterm:source <http://vocab.nerc.ac.uk/scheme/EDMED_DCAT_THEMES/current> ;
  dcterm:source <http://vocab.nerc.ac.uk/scheme/SDNDEV/current> ;
  pav:authoredOn "2013-02-26 17:11:07.0" ;
  pav:hasCurrentVersion <http://vocab.nerc.ac.uk/collection/L05/current/303/2> ;
  pav:hasVersion <http://vocab.nerc.ac.uk/collection/L05/current/303/1> ;
  owl:versionInfo "2" ;
  skos:broader sdnc:ICAT05 ;
  skos:definition "Instruments that measure the speed and direction of sea surface travel by timing reflected radio waves."@en ;
  skos:inScheme <http://vocab.nerc.ac.uk/scheme/EDMED_DCAT_THEMES/current> ;
  skos:inScheme <http://vocab.nerc.ac.uk/scheme/SDNDEV/current> ;
  skos:narrower <http://vocab.nerc.ac.uk/collection/W01/current/003> ;
  skos:notation "SDN:L05::303" ;
  skos:note "accepted"@en ;
  skos:prefLabel "surface current radars"@en ;
.
<http://vocab.nerc.ac.uk/collection/L05/current/304>
  rdf:type skos:Concept ;
  dcterm:date "2008-01-10 16:19:34.0" ;
  dcterm:identifier "SDN:L05::304" ;
  dcterm:source <http://vocab.nerc.ac.uk/scheme/EDMED_DCAT_THEMES/current> ;
  dcterm:source <http://vocab.nerc.ac.uk/scheme/NETMAR_OCEAN/current> ;
  dcterm:source <http://vocab.nerc.ac.uk/scheme/NETOC_INSTRUMENT/current> ;
  dcterm:source <http://vocab.nerc.ac.uk/scheme/SDNDEV/current> ;
  pav:authoredOn "2008-01-10 16:19:34.0" ;
  pav:hasCurrentVersion <http://vocab.nerc.ac.uk/collection/L05/current/304/2> ;
  pav:hasVersion <http://vocab.nerc.ac.uk/collection/L05/current/304/1> ;
  owl:versionInfo "2" ;
  skos:broader sdnc:ICAT05 ;
  skos:definition "Sensors that measure the intensity and nature of electromagnetic radiation in a manner optimised for the determination of ocean chlorophyll concentration."@en ;
  skos:inScheme <http://vocab.nerc.ac.uk/scheme/EDMED_DCAT_THEMES/current> ;
  skos:inScheme <http://vocab.nerc.ac.uk/scheme/NETMAR_OCEAN/current> ;
  skos:inScheme <http://vocab.nerc.ac.uk/scheme/NETOC_INSTRUMENT/current> ;
  skos:inScheme <http://vocab.nerc.ac.uk/scheme/SDNDEV/current> ;
  skos:narrower inst:TOOL0867 ;
  skos:narrower inst:TOOL1035 ;
  skos:narrower inst:TOOL1086 ;
  skos:narrower inst:TOOL1120 ;
  skos:narrower inst:TOOL1334 ;
  skos:narrower <http://vocab.nerc.ac.uk/collection/W01/current/003> ;
  skos:notation "SDN:L05::304" ;
  skos:note "accepted"@en ;
  skos:prefLabel "ocean colour radiometers"@en ;
  skos:related <http://vocab.nerc.ac.uk/collection/P25/current/CHLA> ;
  skos:related <http://vocab.nerc.ac.uk/collection/P25/current/SNWLR> ;
  skos:related <http://vocab.nerc.ac.uk/collection/P25/current/TURB> ;
.
<http://vocab.nerc.ac.uk/collection/L05/current/305>
  rdf:type skos:Concept ;
  dcterm:date "2007-11-20 09:03:34.0" ;
  dcterm:identifier "SDN:L05::305" ;
  dcterm:source <http://vocab.nerc.ac.uk/scheme/EDMED_DCAT_THEMES/current> ;
  dcterm:source <http://vocab.nerc.ac.uk/scheme/SDNDEV/current> ;
  pav:authoredOn "2007-11-20 09:03:34.0" ;
  pav:hasCurrentVersion <http://vocab.nerc.ac.uk/collection/L05/current/305/1> ;
  owl:versionInfo "1" ;
  skos:broader sdnc:ICAT05 ;
  skos:definition "Sensors that measure the reflection or scattering effect produced while scanning the surface of the earth. Primarily used to measure near surface winds over the oceans."@en ;
  skos:inScheme <http://vocab.nerc.ac.uk/scheme/EDMED_DCAT_THEMES/current> ;
  skos:inScheme <http://vocab.nerc.ac.uk/scheme/SDNDEV/current> ;
  skos:narrower inst:TOOL1064 ;
  skos:narrower inst:TOOL1070 ;
  skos:narrower inst:TOOL1675 ;
  skos:narrower <http://vocab.nerc.ac.uk/collection/W01/current/003> ;
  skos:notation "SDN:L05::305" ;
  skos:note "accepted"@en ;
  skos:prefLabel "scatterometers"@en ;
.
<http://vocab.nerc.ac.uk/collection/L05/current/306>
  rdf:type skos:Concept ;
  dcterm:date "2008-01-10 16:21:12.0" ;
  dcterm:identifier "SDN:L05::306" ;
  dcterm:source <http://vocab.nerc.ac.uk/scheme/EDMED_DCAT_THEMES/current> ;
  dcterm:source <http://vocab.nerc.ac.uk/scheme/NETMAR_OCEAN/current> ;
  dcterm:source <http://vocab.nerc.ac.uk/scheme/NETOC_INSTRUMENT/current> ;
  dcterm:source <http://vocab.nerc.ac.uk/scheme/SDNDEV/current> ;
  pav:authoredOn "2008-01-10 16:21:12.0" ;
  pav:hasCurrentVersion <http://vocab.nerc.ac.uk/collection/L05/current/306/1> ;
  owl:versionInfo "1" ;
  skos:broader sdnc:ICAT05 ;
  skos:definition "Instruments that generate maps of radar reflectivity through the synthesis of multiple pulses from a moving platform."@en ;
  skos:inScheme <http://vocab.nerc.ac.uk/scheme/EDMED_DCAT_THEMES/current> ;
  skos:inScheme <http://vocab.nerc.ac.uk/scheme/NETMAR_OCEAN/current> ;
  skos:inScheme <http://vocab.nerc.ac.uk/scheme/NETOC_INSTRUMENT/current> ;
  skos:inScheme <http://vocab.nerc.ac.uk/scheme/SDNDEV/current> ;
  skos:narrower inst:TOOL1064 ;
  skos:narrower inst:TOOL1069 ;
  skos:narrower inst:TOOL1088 ;
  skos:narrower <http://vocab.nerc.ac.uk/collection/W01/current/003> ;
  skos:notation "SDN:L05::306" ;
  skos:note "accepted"@en ;
  skos:prefLabel "synthetic aperture radars"@en ;
  skos:related <http://vocab.nerc.ac.uk/collection/P25/current/WINDF> ;
  skos:related <http://vocab.nerc.ac.uk/collection/P25/current/WINDS> ;
  skos:related <http://vocab.nerc.ac.uk/collection/P25/current/WINDT> ;
  skos:related <http://vocab.nerc.ac.uk/collection/P25/current/WINDX> ;
  skos:related <http://vocab.nerc.ac.uk/collection/P25/current/WINDY> ;
.
<http://vocab.nerc.ac.uk/collection/L05/current/307>
  rdf:type skos:Concept ;
  dcterm:date "2008-01-10 16:21:52.0" ;
  dcterm:identifier "SDN:L05::307" ;
  dcterm:source <http://vocab.nerc.ac.uk/scheme/EDMED_DCAT_THEMES/current> ;
  dcterm:source <http://vocab.nerc.ac.uk/scheme/SDNDEV/current> ;
  pav:authoredOn "2008-01-10 16:21:52.0" ;
  pav:hasCurrentVersion <http://vocab.nerc.ac.uk/collection/L05/current/307/1> ;
  owl:versionInfo "1" ;
  skos:broader sdnc:ICAT05 ;
  skos:definition "Instruments that measure non-gravitational accelerations acting upon a spacecraft."@en ;
  skos:inScheme <http://vocab.nerc.ac.uk/scheme/EDMED_DCAT_THEMES/current> ;
  skos:inScheme <http://vocab.nerc.ac.uk/scheme/SDNDEV/current> ;
  skos:narrower inst:TOOL1349 ;
  skos:narrower inst:TOOL1351 ;
  skos:narrower inst:TOOL1352 ;
  skos:narrower inst:TOOL1591 ;
  skos:narrower <http://vocab.nerc.ac.uk/collection/W01/current/003> ;
  skos:notation "SDN:L05::307" ;
  skos:note "accepted"@en ;
  skos:prefLabel "accelerometers"@en ;
.
<http://vocab.nerc.ac.uk/collection/L05/current/308>
  rdf:type skos:Concept ;
  dcterm:date "2008-01-10 16:22:48.0" ;
  dcterm:identifier "SDN:L05::308" ;
  dcterm:source <http://vocab.nerc.ac.uk/scheme/EDMED_DCAT_THEMES/current> ;
  dcterm:source <http://vocab.nerc.ac.uk/scheme/NETMAR_OCEAN/current> ;
  dcterm:source <http://vocab.nerc.ac.uk/scheme/NETOC_INSTRUMENT/current> ;
  dcterm:source <http://vocab.nerc.ac.uk/scheme/SDNDEV/current> ;
  pav:authoredOn "2008-01-10 16:22:48.0" ;
  pav:hasCurrentVersion <http://vocab.nerc.ac.uk/collection/L05/current/308/1> ;
  owl:versionInfo "1" ;
  skos:broader sdnc:ICAT05 ;
  skos:definition "Sensors that measure the intensity an nature of electromagnetic radiation in a manner optimised for the quantification of atmospheric phenomena."@en ;
  skos:inScheme <http://vocab.nerc.ac.uk/scheme/EDMED_DCAT_THEMES/current> ;
  skos:inScheme <http://vocab.nerc.ac.uk/scheme/NETMAR_OCEAN/current> ;
  skos:inScheme <http://vocab.nerc.ac.uk/scheme/NETOC_INSTRUMENT/current> ;
  skos:inScheme <http://vocab.nerc.ac.uk/scheme/SDNDEV/current> ;
  skos:narrower inst:TOOL0695 ;
  skos:narrower inst:TOOL0702 ;
  skos:narrower inst:TOOL0703 ;
  skos:narrower inst:TOOL0722 ;
  skos:narrower inst:TOOL0723 ;
  skos:narrower inst:TOOL0912 ;
  skos:narrower inst:TOOL1035 ;
  skos:narrower inst:TOOL1037 ;
  skos:narrower inst:TOOL1042 ;
  skos:narrower inst:TOOL1049 ;
  skos:narrower inst:TOOL1050 ;
  skos:narrower inst:TOOL1052 ;
  skos:narrower inst:TOOL1053 ;
  skos:narrower inst:TOOL1054 ;
  skos:narrower inst:TOOL1058 ;
  skos:narrower inst:TOOL1060 ;
  skos:narrower inst:TOOL1061 ;
  skos:narrower inst:TOOL1063 ;
  skos:narrower inst:TOOL1065 ;
  skos:narrower inst:TOOL1066 ;
  skos:narrower inst:TOOL1067 ;
  skos:narrower inst:TOOL1068 ;
  skos:narrower inst:TOOL1072 ;
  skos:narrower inst:TOOL1073 ;
  skos:narrower inst:TOOL1074 ;
  skos:narrower inst:TOOL1075 ;
  skos:narrower inst:TOOL1076 ;
  skos:narrower inst:TOOL1084 ;
  skos:narrower inst:TOOL1085 ;
  skos:narrower inst:TOOL1090 ;
  skos:narrower inst:TOOL1091 ;
  skos:narrower inst:TOOL1120 ;
  skos:narrower inst:TOOL1734 ;
  skos:narrower inst:TOOL1873 ;
  skos:narrower <http://vocab.nerc.ac.uk/collection/W01/current/003> ;
  skos:notation "SDN:L05::308" ;
  skos:note "accepted"@en ;
  skos:prefLabel "atmospheric radiometers"@en ;
  skos:related <http://vocab.nerc.ac.uk/collection/P25/current/ICEBERG> ;
  skos:related <http://vocab.nerc.ac.uk/collection/P25/current/ICECOV> ;
  skos:related <http://vocab.nerc.ac.uk/collection/P25/current/ICEDIR> ;
  skos:related <http://vocab.nerc.ac.uk/collection/P25/current/ICEDISP> ;
  skos:related <http://vocab.nerc.ac.uk/collection/P25/current/ICEEDGE> ;
  skos:related <http://vocab.nerc.ac.uk/collection/P25/current/ICESPD> ;
  skos:related <http://vocab.nerc.ac.uk/collection/P25/current/ICETEMP> ;
  skos:related <http://vocab.nerc.ac.uk/collection/P25/current/ICETYPE> ;
  skos:related <http://vocab.nerc.ac.uk/collection/P25/current/WTEMP> ;
.
<http://vocab.nerc.ac.uk/collection/L05/current/309>
  rdf:type skos:Concept ;
  <http://purl.org/dc/terms/:replaces> <http://vocab.nerc.ac.uk/collection/L05/current/314> ;
  <http://purl.org/dc/terms/:replaces> <http://vocab.nerc.ac.uk/collection/L05/current/315> ;
  dcterm:date "2008-01-10 16:23:53.0" ;
  dcterm:identifier "SDN:L05::309" ;
  dcterm:source <http://vocab.nerc.ac.uk/scheme/SDNDEV/current> ;
  pav:authoredOn "2008-01-10 16:23:53.0" ;
  pav:hasCurrentVersion <http://vocab.nerc.ac.uk/collection/L05/current/309/1> ;
  owl:versionInfo "1" ;
  skos:broader sdnc:ICAT05 ;
  skos:definition "Sensors that measure the intensity and nature of electromagnetic radiation in a manner optimised for the quantification of terrestrial phenomena."@en ;
  skos:inScheme <http://vocab.nerc.ac.uk/scheme/SDNDEV/current> ;
  skos:narrower inst:TOOL1036 ;
  skos:narrower inst:TOOL1037 ;
  skos:narrower inst:TOOL1038 ;
  skos:narrower inst:TOOL1041 ;
  skos:narrower inst:TOOL1056 ;
  skos:narrower inst:TOOL1057 ;
  skos:narrower inst:TOOL1059 ;
  skos:narrower inst:TOOL1061 ;
  skos:narrower inst:TOOL1065 ;
  skos:narrower inst:TOOL1066 ;
  skos:narrower inst:TOOL1071 ;
  skos:narrower inst:TOOL1073 ;
  skos:narrower inst:TOOL1074 ;
  skos:narrower inst:TOOL1075 ;
  skos:narrower inst:TOOL1076 ;
  skos:narrower inst:TOOL1077 ;
  skos:narrower <http://vocab.nerc.ac.uk/collection/W01/current/003> ;
  skos:notation "SDN:L05::309" ;
  skos:note "accepted"@en ;
  skos:prefLabel "terrestrial radiometers"@en ;
.
<http://vocab.nerc.ac.uk/collection/L05/current/310>
  rdf:type skos:Concept ;
  dcterm:date "2012-12-18 15:18:17.0" ;
  dcterm:identifier "SDN:L05::310" ;
  dcterm:source <http://vocab.nerc.ac.uk/scheme/EDMED_DCAT_THEMES/current> ;
  dcterm:source <http://vocab.nerc.ac.uk/scheme/SDNDEV/current> ;
  pav:authoredOn "2012-12-18 15:18:17.0" ;
  pav:hasCurrentVersion <http://vocab.nerc.ac.uk/collection/L05/current/310/2> ;
  pav:hasVersion <http://vocab.nerc.ac.uk/collection/L05/current/310/1> ;
  owl:versionInfo "2" ;
  skos:broader sdnc:ICAT05 ;
  skos:definition "Instruments that determine the distance between the platform and the Earth's surface by timing reflected pulses of laser light."@en ;
  skos:inScheme <http://vocab.nerc.ac.uk/scheme/EDMED_DCAT_THEMES/current> ;
  skos:inScheme <http://vocab.nerc.ac.uk/scheme/SDNDEV/current> ;
  skos:narrower inst:TOOL1079 ;
  skos:narrower <http://vocab.nerc.ac.uk/collection/W01/current/003> ;
  skos:notation "SDN:L05::310" ;
  skos:note "accepted"@en ;
  skos:prefLabel "laser altimeters"@en ;
.
<http://vocab.nerc.ac.uk/collection/L05/current/311>
  rdf:type skos:Concept ;
  <http://purl.org/dc/terms/:replaces> <http://vocab.nerc.ac.uk/collection/L05/current/180> ;
  dcterm:date "2020-09-18 10:36:01.0" ;
  dcterm:identifier "SDN:L05::311" ;
  dcterm:source <http://vocab.nerc.ac.uk/scheme/EDMED_DCAT_THEMES/current> ;
  dcterm:source <http://vocab.nerc.ac.uk/scheme/NETMAR_OCEAN/current> ;
  dcterm:source <http://vocab.nerc.ac.uk/scheme/NETOC_INSTRUMENT/current> ;
  dcterm:source <http://vocab.nerc.ac.uk/scheme/SDNDEV/current> ;
  pav:authoredOn "2020-09-18 10:36:01.0" ;
  pav:hasCurrentVersion <http://vocab.nerc.ac.uk/collection/L05/current/311/2> ;
  pav:hasVersion <http://vocab.nerc.ac.uk/collection/L05/current/311/1> ;
  owl:versionInfo "2" ;
  skos:broader sdnc:ICAT03 ;
  skos:broader sdnc:ICAT04 ;
  skos:broader sdnc:ICAT05 ;
  skos:definition "All types of photographic equipment used to record visual images. Includes stills, video, film and digital systems."@en ;
  skos:inScheme <http://vocab.nerc.ac.uk/scheme/EDMED_DCAT_THEMES/current> ;
  skos:inScheme <http://vocab.nerc.ac.uk/scheme/NETMAR_OCEAN/current> ;
  skos:inScheme <http://vocab.nerc.ac.uk/scheme/NETOC_INSTRUMENT/current> ;
  skos:inScheme <http://vocab.nerc.ac.uk/scheme/SDNDEV/current> ;
  skos:narrower inst:TOOL1038 ;
  skos:narrower inst:TOOL1083 ;
  skos:narrower <http://vocab.nerc.ac.uk/collection/W01/current/003> ;
  skos:notation "SDN:L05::311" ;
  skos:note "accepted"@en ;
  skos:prefLabel "cameras"@en ;
  skos:related <http://vocab.nerc.ac.uk/collection/P25/current/ICEBERG> ;
  skos:related <http://vocab.nerc.ac.uk/collection/P25/current/ICECOV> ;
.
<http://vocab.nerc.ac.uk/collection/L05/current/312>
  rdf:type skos:Concept ;
  dcterm:date "2009-10-16 11:58:26.0" ;
  dcterm:identifier "SDN:L05::312" ;
  dcterm:source <http://vocab.nerc.ac.uk/scheme/NETMAR_OCEAN/current> ;
  dcterm:source <http://vocab.nerc.ac.uk/scheme/NETOC_INSTRUMENT/current> ;
  dcterm:source <http://vocab.nerc.ac.uk/scheme/SDNDEV/current> ;
  pav:authoredOn "2009-10-16 11:58:26.0" ;
  pav:hasCurrentVersion <http://vocab.nerc.ac.uk/collection/L05/current/312/1> ;
  owl:versionInfo "1" ;
  skos:broader sdnc:ICAT05 ;
  skos:definition "Instruments that measure the depth of a water body by determining the distances from the platform to the surface and the bed by timing reflected pulses of laser light."@en ;
  skos:inScheme <http://vocab.nerc.ac.uk/scheme/NETMAR_OCEAN/current> ;
  skos:inScheme <http://vocab.nerc.ac.uk/scheme/NETOC_INSTRUMENT/current> ;
  skos:inScheme <http://vocab.nerc.ac.uk/scheme/SDNDEV/current> ;
  skos:narrower <http://vocab.nerc.ac.uk/collection/W01/current/003> ;
  skos:notation "SDN:L05::312" ;
  skos:note "accepted"@en ;
  skos:prefLabel "bathymetric LiDARs"@en ;
  skos:related <http://vocab.nerc.ac.uk/collection/P25/current/ELEV> ;
.
<http://vocab.nerc.ac.uk/collection/L05/current/313>
  rdf:type skos:Concept ;
  dcterm:date "2013-02-26 17:11:07.0" ;
  dcterm:identifier "SDN:L05::313" ;
  dcterm:source <http://vocab.nerc.ac.uk/scheme/SDNDEV/current> ;
  pav:authoredOn "2013-02-26 17:11:07.0" ;
  pav:hasCurrentVersion <http://vocab.nerc.ac.uk/collection/L05/current/313/2> ;
  pav:hasVersion <http://vocab.nerc.ac.uk/collection/L05/current/313/1> ;
  owl:versionInfo "2" ;
  skos:broader sdnc:ICAT05 ;
  skos:definition "X-band and S-band radar systems developed for the detection, tracking and counting of birds in flight."@en ;
  skos:inScheme <http://vocab.nerc.ac.uk/scheme/SDNDEV/current> ;
  skos:narrower <http://vocab.nerc.ac.uk/collection/W01/current/003> ;
  skos:notation "SDN:L05::313" ;
  skos:note "accepted"@en ;
  skos:prefLabel "bird detection radars"@en ;
.
<http://vocab.nerc.ac.uk/collection/L05/current/314>
  rdf:type skos:Concept ;
  <http://purl.org/dc/terms/:isReplacedBy> <http://vocab.nerc.ac.uk/collection/L05/current/309> ;
  dcterm:date "2017-03-09 16:15:08.0" ;
  dcterm:identifier "SDN:L05::314" ;
  dcterm:source <http://vocab.nerc.ac.uk/scheme/SDNDEV/current> ;
  pav:authoredOn "2017-03-09 16:15:08.0" ;
  pav:hasCurrentVersion <http://vocab.nerc.ac.uk/collection/L05/current/314/1> ;
  owl:versionInfo "1" ;
  skos:broader sdnc:ICAT05 ;
  skos:definition "Instruments that measure the intensity and nature of electromagnetic radiation in a manner optimised for the quantification of chemical compounds in the atmosphere."@en ;
  skos:inScheme <http://vocab.nerc.ac.uk/scheme/SDNDEV/current> ;
  skos:narrower inst:TOOL1039 ;
  skos:narrower inst:TOOL1040 ;
  skos:narrower inst:TOOL1048 ;
  skos:narrower inst:TOOL1051 ;
  skos:narrower inst:TOOL1055 ;
  skos:narrower inst:TOOL1062 ;
  skos:narrower inst:TOOL1080 ;
  skos:narrower inst:TOOL1081 ;
  skos:narrower inst:TOOL1082 ;
  skos:narrower inst:TOOL1087 ;
  skos:notation "SDN:L05::314" ;
  skos:note "accepted"@en ;
  skos:prefLabel "Atmospheric chemistry remote sensors"@en ;
.
<http://vocab.nerc.ac.uk/collection/L05/current/315>
  rdf:type skos:Concept ;
  <http://purl.org/dc/terms/:isReplacedBy> <http://vocab.nerc.ac.uk/collection/L05/current/309> ;
  dcterm:date "2017-03-09 16:39:05.0" ;
  dcterm:identifier "SDN:L05::315" ;
  dcterm:source <http://vocab.nerc.ac.uk/scheme/SDNDEV/current> ;
  pav:authoredOn "2017-03-09 16:39:05.0" ;
  pav:hasCurrentVersion <http://vocab.nerc.ac.uk/collection/L05/current/315/2> ;
  pav:hasVersion <http://vocab.nerc.ac.uk/collection/L05/current/315/1> ;
  owl:deprecated "true" ;
  owl:versionInfo "2" ;
  skos:broader sdnc:ICAT05 ;
  skos:definition "Instruments that measure the intensity and nature of electromagnetic radiation in a manner optimised for sea ice detection and quantification."@en ;
  skos:inScheme <http://vocab.nerc.ac.uk/scheme/SDNDEV/current> ;
  skos:notation "SDN:L05::315" ;
  skos:note "deprecated"@en ;
  skos:prefLabel "Sea ice remote sensors"@en ;
.
<http://vocab.nerc.ac.uk/collection/L05/current/350>
  rdf:type skos:Concept ;
  dcterm:date "2013-02-26 17:11:07.0" ;
  dcterm:identifier "SDN:L05::350" ;
  dcterm:source <http://vocab.nerc.ac.uk/scheme/EDMED_DCAT_THEMES/current> ;
  dcterm:source <http://vocab.nerc.ac.uk/scheme/NETMAR_OCEAN/current> ;
  dcterm:source <http://vocab.nerc.ac.uk/scheme/NETOC_INSTRUMENT/current> ;
  dcterm:source <http://vocab.nerc.ac.uk/scheme/SDNDEV/current> ;
  pav:authoredOn "2013-02-26 17:11:07.0" ;
  pav:hasCurrentVersion <http://vocab.nerc.ac.uk/collection/L05/current/350/3> ;
  pav:hasVersion <http://vocab.nerc.ac.uk/collection/L05/current/350/1> ;
  pav:hasVersion <http://vocab.nerc.ac.uk/collection/L05/current/350/2> ;
  owl:versionInfo "3" ;
  skos:broader sdnc:ICAT04 ;
  skos:definition "Instrument that simultaneously measures electrical conductivity and temperature in the water column to provide temperature and salinity data."@en ;
  skos:inScheme <http://vocab.nerc.ac.uk/scheme/EDMED_DCAT_THEMES/current> ;
  skos:inScheme <http://vocab.nerc.ac.uk/scheme/NETMAR_OCEAN/current> ;
  skos:inScheme <http://vocab.nerc.ac.uk/scheme/NETOC_INSTRUMENT/current> ;
  skos:inScheme <http://vocab.nerc.ac.uk/scheme/SDNDEV/current> ;
  skos:narrower inst:TOOL0001 ;
  skos:narrower inst:TOOL1272 ;
  skos:narrower <http://vocab.nerc.ac.uk/collection/W01/current/003> ;
  skos:notation "SDN:L05::350" ;
  skos:note "accepted"@en ;
  skos:prefLabel "salinity sensor"@en ;
  skos:related <http://vocab.nerc.ac.uk/collection/P25/current/SALIN> ;
.
<http://vocab.nerc.ac.uk/collection/L05/current/351>
  rdf:type skos:Concept ;
  dcterm:date "2013-02-26 17:11:07.0" ;
  dcterm:identifier "SDN:L05::351" ;
  dcterm:source <http://vocab.nerc.ac.uk/scheme/EDMED_DCAT_THEMES/current> ;
  dcterm:source <http://vocab.nerc.ac.uk/scheme/NETMAR_OCEAN/current> ;
  dcterm:source <http://vocab.nerc.ac.uk/scheme/NETOC_INSTRUMENT/current> ;
  dcterm:source <http://vocab.nerc.ac.uk/scheme/NETOC_ORTHO/current> ;
  dcterm:source <http://vocab.nerc.ac.uk/scheme/SDNDEV/current> ;
  pav:authoredOn "2013-02-26 17:11:07.0" ;
  pav:hasCurrentVersion <http://vocab.nerc.ac.uk/collection/L05/current/351/2> ;
  pav:hasVersion <http://vocab.nerc.ac.uk/collection/L05/current/351/1> ;
  owl:versionInfo "2" ;
  skos:broader sdnc:ICAT04 ;
  skos:definition "Instrument that measures the concentration of gases, generally oxygen, dissolved in the water column."@en ;
  skos:inScheme <http://vocab.nerc.ac.uk/scheme/EDMED_DCAT_THEMES/current> ;
  skos:inScheme <http://vocab.nerc.ac.uk/scheme/NETMAR_OCEAN/current> ;
  skos:inScheme <http://vocab.nerc.ac.uk/scheme/NETOC_INSTRUMENT/current> ;
  skos:inScheme <http://vocab.nerc.ac.uk/scheme/NETOC_ORTHO/current> ;
  skos:inScheme <http://vocab.nerc.ac.uk/scheme/SDNDEV/current> ;
  skos:narrower <http://vocab.nerc.ac.uk/collection/W01/current/003> ;
  skos:notation "SDN:L05::351" ;
  skos:note "accepted"@en ;
  skos:prefLabel "dissolved gas sensors"@en ;
  skos:related <http://vocab.nerc.ac.uk/collection/P25/current/DOXY> ;
  skos:related <http://vocab.nerc.ac.uk/collection/P25/current/OXYS> ;
.
<http://vocab.nerc.ac.uk/collection/L05/current/352>
  rdf:type skos:Concept ;
  dcterm:date "2020-07-30 12:20:21.0" ;
  dcterm:identifier "SDN:L05::352" ;
  dcterm:source <http://vocab.nerc.ac.uk/scheme/EDMED_DCAT_THEMES/current> ;
  dcterm:source <http://vocab.nerc.ac.uk/scheme/NETMAR_OCEAN/current> ;
  dcterm:source <http://vocab.nerc.ac.uk/scheme/NETOC_INSTRUMENT/current> ;
  dcterm:source <http://vocab.nerc.ac.uk/scheme/SDNDEV/current> ;
  pav:authoredOn "2020-07-30 12:20:21.0" ;
  pav:hasCurrentVersion <http://vocab.nerc.ac.uk/collection/L05/current/352/3> ;
  pav:hasVersion <http://vocab.nerc.ac.uk/collection/L05/current/352/1> ;
  pav:hasVersion <http://vocab.nerc.ac.uk/collection/L05/current/352/2> ;
  owl:versionInfo "3" ;
  skos:broader sdnc:ICAT04 ;
  skos:definition "Instruments that categorise and/or count plankton, and/or enable 2D/3D spatial reconstruction of plankton in the water column."@en ;
  skos:inScheme <http://vocab.nerc.ac.uk/scheme/EDMED_DCAT_THEMES/current> ;
  skos:inScheme <http://vocab.nerc.ac.uk/scheme/NETMAR_OCEAN/current> ;
  skos:inScheme <http://vocab.nerc.ac.uk/scheme/NETOC_INSTRUMENT/current> ;
  skos:inScheme <http://vocab.nerc.ac.uk/scheme/SDNDEV/current> ;
  skos:narrower <http://vocab.nerc.ac.uk/collection/W01/current/003> ;
  skos:notation "SDN:L05::352" ;
  skos:note "accepted"@en ;
  skos:prefLabel "plankton categorisers and counters"@en ;
  skos:related <http://vocab.nerc.ac.uk/collection/P25/current/PHYTABUND> ;
.
<http://vocab.nerc.ac.uk/collection/L05/current/353>
  rdf:type skos:Concept ;
  dcterm:date "2013-02-26 17:11:07.0" ;
  dcterm:identifier "SDN:L05::353" ;
  dcterm:source <http://vocab.nerc.ac.uk/scheme/EDMED_DCAT_THEMES/current> ;
  dcterm:source <http://vocab.nerc.ac.uk/scheme/NETMAR_OCEAN/current> ;
  dcterm:source <http://vocab.nerc.ac.uk/scheme/NETOC_INSTRUMENT/current> ;
  dcterm:source <http://vocab.nerc.ac.uk/scheme/SDNDEV/current> ;
  pav:authoredOn "2013-02-26 17:11:07.0" ;
  pav:hasCurrentVersion <http://vocab.nerc.ac.uk/collection/L05/current/353/2> ;
  pav:hasVersion <http://vocab.nerc.ac.uk/collection/L05/current/353/1> ;
  owl:versionInfo "2" ;
  skos:broader sdnc:ICAT04 ;
  skos:definition "Fluorometers that measure photosynthetic parameters by taking measurements whilst manipulating the phytoplankton with controlled high-intensity illumination such as pump and probe and FRRF."@en ;
  skos:inScheme <http://vocab.nerc.ac.uk/scheme/EDMED_DCAT_THEMES/current> ;
  skos:inScheme <http://vocab.nerc.ac.uk/scheme/NETMAR_OCEAN/current> ;
  skos:inScheme <http://vocab.nerc.ac.uk/scheme/NETOC_INSTRUMENT/current> ;
  skos:inScheme <http://vocab.nerc.ac.uk/scheme/SDNDEV/current> ;
  skos:narrower <http://vocab.nerc.ac.uk/collection/W01/current/003> ;
  skos:notation "SDN:L05::353" ;
  skos:note "accepted"@en ;
  skos:prefLabel "active fluorometers"@en ;
.
<http://vocab.nerc.ac.uk/collection/L05/current/355>
  rdf:type skos:Concept ;
  dcterm:date "2013-02-26 17:11:07.0" ;
  dcterm:identifier "SDN:L05::355" ;
  dcterm:source <http://vocab.nerc.ac.uk/scheme/EDMED_DCAT_THEMES/current> ;
  dcterm:source <http://vocab.nerc.ac.uk/scheme/SDNDEV/current> ;
  pav:authoredOn "2013-02-26 17:11:07.0" ;
  pav:hasCurrentVersion <http://vocab.nerc.ac.uk/collection/L05/current/355/2> ;
  pav:hasVersion <http://vocab.nerc.ac.uk/collection/L05/current/355/1> ;
  owl:sameAs <http://onto.nerc.ac.uk/CAST/146> ;
  owl:versionInfo "2" ;
  skos:broader sdnc:ICAT04 ;
  skos:definition "Instruments that measure the hydrogen ion concentration in the water column."@en ;
  skos:inScheme <http://vocab.nerc.ac.uk/scheme/EDMED_DCAT_THEMES/current> ;
  skos:inScheme <http://vocab.nerc.ac.uk/scheme/SDNDEV/current> ;
  skos:narrower <http://vocab.nerc.ac.uk/collection/W01/current/003> ;
  skos:notation "SDN:L05::355" ;
  skos:note "accepted"@en ;
  skos:prefLabel "pH sensors"@en ;
.
<http://vocab.nerc.ac.uk/collection/L05/current/356>
  rdf:type skos:Concept ;
  dcterm:date "2013-02-26 17:11:07.0" ;
  dcterm:identifier "SDN:L05::356" ;
  dcterm:source <http://vocab.nerc.ac.uk/scheme/EDMED_DCAT_THEMES/current> ;
  dcterm:source <http://vocab.nerc.ac.uk/scheme/SDNDEV/current> ;
  pav:authoredOn "2013-02-26 17:11:07.0" ;
  pav:hasCurrentVersion <http://vocab.nerc.ac.uk/collection/L05/current/356/2> ;
  pav:hasVersion <http://vocab.nerc.ac.uk/collection/L05/current/356/1> ;
  owl:versionInfo "2" ;
  skos:broader sdnc:ICAT04 ;
  skos:definition "Instruments that measure the tendency of the water column to either gain or lose electrons when it is subject to change by introduction of a new species."@en ;
  skos:inScheme <http://vocab.nerc.ac.uk/scheme/EDMED_DCAT_THEMES/current> ;
  skos:inScheme <http://vocab.nerc.ac.uk/scheme/SDNDEV/current> ;
  skos:narrower <http://vocab.nerc.ac.uk/collection/W01/current/003> ;
  skos:notation "SDN:L05::356" ;
  skos:note "accepted"@en ;
  skos:prefLabel "redox potential sensors"@en ;
.
<http://vocab.nerc.ac.uk/collection/L05/current/358>
  rdf:type skos:Concept ;
  dcterm:date "2008-01-10 16:15:11.0" ;
  dcterm:identifier "SDN:L05::358" ;
  dcterm:source <http://vocab.nerc.ac.uk/scheme/EDMED_DCAT_THEMES/current> ;
  dcterm:source <http://vocab.nerc.ac.uk/scheme/SDNDEV/current> ;
  pav:authoredOn "2008-01-10 16:15:11.0" ;
  pav:hasCurrentVersion <http://vocab.nerc.ac.uk/collection/L05/current/358/1> ;
  owl:versionInfo "1" ;
  skos:broader sdnc:ICAT04 ;
  skos:definition "Instruments that measure the concentration and size of air bubbles in the water column."@en ;
  skos:inScheme <http://vocab.nerc.ac.uk/scheme/EDMED_DCAT_THEMES/current> ;
  skos:inScheme <http://vocab.nerc.ac.uk/scheme/SDNDEV/current> ;
  skos:narrower <http://vocab.nerc.ac.uk/collection/W01/current/003> ;
  skos:notation "SDN:L05::358" ;
  skos:note "accepted"@en ;
  skos:prefLabel "bubble detectors"@en ;
.
<http://vocab.nerc.ac.uk/collection/L05/current/359>
  rdf:type skos:Concept ;
  dcterm:date "2010-02-19 12:00:55.0" ;
  dcterm:identifier "SDN:L05::359" ;
  dcterm:source <http://vocab.nerc.ac.uk/scheme/SDNDEV/current> ;
  pav:authoredOn "2010-02-19 12:00:55.0" ;
  pav:hasCurrentVersion <http://vocab.nerc.ac.uk/collection/L05/current/359/2> ;
  pav:hasVersion <http://vocab.nerc.ac.uk/collection/L05/current/359/1> ;
  owl:versionInfo "2" ;
  skos:broader sdnc:ICAT04 ;
  skos:definition "Devices comprising a weight attached to the end of a graduated rope used to measure point water depths."@en ;
  skos:inScheme <http://vocab.nerc.ac.uk/scheme/SDNDEV/current> ;
  skos:narrower <http://vocab.nerc.ac.uk/collection/W01/current/003> ;
  skos:notation "SDN:L05::359" ;
  skos:note "accepted"@en ;
  skos:prefLabel "plummets"@en ;
.
<http://vocab.nerc.ac.uk/collection/L05/current/360>
  rdf:type skos:Concept ;
  dcterm:date "2010-02-19 11:52:56.0" ;
  dcterm:identifier "SDN:L05::360" ;
  dcterm:source <http://vocab.nerc.ac.uk/scheme/SDNDEV/current> ;
  pav:authoredOn "2010-02-19 11:52:56.0" ;
  pav:hasCurrentVersion <http://vocab.nerc.ac.uk/collection/L05/current/360/1> ;
  owl:versionInfo "1" ;
  skos:broader sdnc:ICAT04 ;
  skos:definition "Devices that measure fluid  (air, gas, water, or oil) pressure within soil, sediment, rock or concrete providing information such as water table level in an aquifer system."@en ;
  skos:inScheme <http://vocab.nerc.ac.uk/scheme/SDNDEV/current> ;
  skos:narrower <http://vocab.nerc.ac.uk/collection/W01/current/003> ;
  skos:notation "SDN:L05::360" ;
  skos:note "accepted"@en ;
  skos:prefLabel "piezometers"@en ;
.
<http://vocab.nerc.ac.uk/collection/L05/current/361>
  rdf:type skos:Concept ;
  dcterm:date "2010-02-19 11:52:56.0" ;
  dcterm:identifier "SDN:L05::361" ;
  dcterm:source <http://vocab.nerc.ac.uk/scheme/EDMED_DCAT_THEMES/current> ;
  dcterm:source <http://vocab.nerc.ac.uk/scheme/SDNDEV/current> ;
  pav:authoredOn "2010-02-19 11:52:56.0" ;
  pav:hasCurrentVersion <http://vocab.nerc.ac.uk/collection/L05/current/361/1> ;
  owl:versionInfo "1" ;
  skos:broader sdnc:ICAT04 ;
  skos:definition "Dynamic or passive devices that determine the consistency or hardness of soil or sediment by measuring the depth or rate of penetration of a needle or cone rig into it when a known force is applied."@en ;
  skos:inScheme <http://vocab.nerc.ac.uk/scheme/EDMED_DCAT_THEMES/current> ;
  skos:inScheme <http://vocab.nerc.ac.uk/scheme/SDNDEV/current> ;
  skos:narrower <http://vocab.nerc.ac.uk/collection/W01/current/003> ;
  skos:notation "SDN:L05::361" ;
  skos:note "accepted"@en ;
  skos:prefLabel "penetrometers"@en ;
.
<http://vocab.nerc.ac.uk/collection/L05/current/362>
  rdf:type skos:Concept ;
  dcterm:date "2010-02-19 11:52:56.0" ;
  dcterm:identifier "SDN:L05::362" ;
  dcterm:source <http://vocab.nerc.ac.uk/scheme/EDMED_DCAT_THEMES/current> ;
  dcterm:source <http://vocab.nerc.ac.uk/scheme/SDNDEV/current> ;
  pav:authoredOn "2010-02-19 11:52:56.0" ;
  pav:hasCurrentVersion <http://vocab.nerc.ac.uk/collection/L05/current/362/1> ;
  owl:versionInfo "1" ;
  skos:broader <http://vocab.nerc.ac.uk/collection/L05/current/153> ;
  skos:definition "An energy source with a frequency up to 250 Hz (sampling interval ranging from 2-8 msec) plus a single string of towed hydrophones (streamer) that determine geologic structure by detecting waves reflected by subsurface layers."@en ;
  skos:inScheme <http://vocab.nerc.ac.uk/scheme/EDMED_DCAT_THEMES/current> ;
  skos:inScheme <http://vocab.nerc.ac.uk/scheme/SDNDEV/current> ;
  skos:narrower <http://vocab.nerc.ac.uk/collection/W01/current/003> ;
  skos:notation "SDN:L05::362" ;
  skos:note "accepted"@en ;
  skos:prefLabel "250 Hz top-bandwidth single-channel seismic reflection systems"@en ;
  skos:related inst:TOOL0353 ;
  skos:related inst:TOOL0354 ;
  skos:related inst:TOOL0355 ;
  skos:related inst:TOOL0356 ;
  skos:related inst:TOOL0357 ;
  skos:related inst:TOOL0358 ;
.
<http://vocab.nerc.ac.uk/collection/L05/current/363>
  rdf:type skos:Concept ;
  dcterm:date "2010-02-19 11:52:56.0" ;
  dcterm:identifier "SDN:L05::363" ;
  dcterm:source <http://vocab.nerc.ac.uk/scheme/EDMED_DCAT_THEMES/current> ;
  dcterm:source <http://vocab.nerc.ac.uk/scheme/SDNDEV/current> ;
  pav:authoredOn "2010-02-19 11:52:56.0" ;
  pav:hasCurrentVersion <http://vocab.nerc.ac.uk/collection/L05/current/363/1> ;
  owl:versionInfo "1" ;
  skos:broader <http://vocab.nerc.ac.uk/collection/L05/current/153> ;
  skos:definition "An energy source with a frequency up to 1000 Hz (sampling interval ranging from 2-0.5 msec) plus a single string of towed hydrophones (streamer) that determine geologic structure by detecting waves reflected by subsurface layers."@en ;
  skos:inScheme <http://vocab.nerc.ac.uk/scheme/EDMED_DCAT_THEMES/current> ;
  skos:inScheme <http://vocab.nerc.ac.uk/scheme/SDNDEV/current> ;
  skos:narrower <http://vocab.nerc.ac.uk/collection/W01/current/003> ;
  skos:notation "SDN:L05::363" ;
  skos:note "accepted"@en ;
  skos:prefLabel "1000 Hz top-bandwidth single-channel seismic reflection systems"@en ;
  skos:related inst:TOOL0354 ;
.
<http://vocab.nerc.ac.uk/collection/L05/current/364>
  rdf:type skos:Concept ;
  dcterm:date "2010-02-19 11:52:56.0" ;
  dcterm:identifier "SDN:L05::364" ;
  dcterm:source <http://vocab.nerc.ac.uk/scheme/EDMED_DCAT_THEMES/current> ;
  dcterm:source <http://vocab.nerc.ac.uk/scheme/SDNDEV/current> ;
  pav:authoredOn "2010-02-19 11:52:56.0" ;
  pav:hasCurrentVersion <http://vocab.nerc.ac.uk/collection/L05/current/364/1> ;
  owl:versionInfo "1" ;
  skos:broader <http://vocab.nerc.ac.uk/collection/L05/current/154> ;
  skos:definition "An energy source with a frequency up to 1000 Hz (sampling interval ranging from 2-0.5 msec) plus a multiple strings of towed hydrophones (streamers) that determine geologic structure by detecting waves reflected by subsurface layers."@en ;
  skos:inScheme <http://vocab.nerc.ac.uk/scheme/EDMED_DCAT_THEMES/current> ;
  skos:inScheme <http://vocab.nerc.ac.uk/scheme/SDNDEV/current> ;
  skos:narrower <http://vocab.nerc.ac.uk/collection/W01/current/003> ;
  skos:notation "SDN:L05::364" ;
  skos:note "accepted"@en ;
  skos:prefLabel "1000 Hz top-bandwidth multi-channel seismic reflection systems"@en ;
  skos:related inst:TOOL0354 ;
.
<http://vocab.nerc.ac.uk/collection/L05/current/365>
  rdf:type skos:Concept ;
  dcterm:date "2010-02-19 11:52:56.0" ;
  dcterm:identifier "SDN:L05::365" ;
  dcterm:source <http://vocab.nerc.ac.uk/scheme/SDNDEV/current> ;
  pav:authoredOn "2010-02-19 11:52:56.0" ;
  pav:hasCurrentVersion <http://vocab.nerc.ac.uk/collection/L05/current/365/1> ;
  owl:versionInfo "1" ;
  skos:broader <http://vocab.nerc.ac.uk/collection/L05/current/154> ;
  skos:definition "An energy source with a frequency up to 2000 Hz (sampling interval ranging from 0.5-0.25 msec) plus a multiple strings of towed hydrophones (streamers) that determine geologic structure by detecting waves reflected by subsurface layers."@en ;
  skos:inScheme <http://vocab.nerc.ac.uk/scheme/SDNDEV/current> ;
  skos:narrower <http://vocab.nerc.ac.uk/collection/W01/current/003> ;
  skos:notation "SDN:L05::365" ;
  skos:note "accepted"@en ;
  skos:prefLabel "2000 Hz top-bandwidth multi-channel seismic reflection systems"@en ;
  skos:related inst:TOOL0354 ;
.
<http://vocab.nerc.ac.uk/collection/L05/current/366>
  rdf:type skos:Concept ;
  dcterm:date "2010-02-19 11:52:56.0" ;
  dcterm:identifier "SDN:L05::366" ;
  dcterm:source <http://vocab.nerc.ac.uk/scheme/SDNDEV/current> ;
  pav:authoredOn "2010-02-19 11:52:56.0" ;
  pav:hasCurrentVersion <http://vocab.nerc.ac.uk/collection/L05/current/366/1> ;
  owl:versionInfo "1" ;
  skos:broader <http://vocab.nerc.ac.uk/collection/L05/current/154> ;
  skos:definition "An energy source with a frequency up to >2000 Hz (sampling interval lower than 0.25 msec) plus a multiple strings of towed hydrophones (streamers) that determine geologic structure by detecting waves reflected by subsurface layers."@en ;
  skos:inScheme <http://vocab.nerc.ac.uk/scheme/SDNDEV/current> ;
  skos:narrower <http://vocab.nerc.ac.uk/collection/W01/current/003> ;
  skos:notation "SDN:L05::366" ;
  skos:note "accepted"@en ;
  skos:prefLabel ">2000 Hz top-bandwidth multi-channel seismic reflection systems"@en ;
  skos:related inst:TOOL0354 ;
.
<http://vocab.nerc.ac.uk/collection/L05/current/367>
  rdf:type skos:Concept ;
  dcterm:date "2010-11-18 11:16:45.0" ;
  dcterm:identifier "SDN:L05::367" ;
  dcterm:source <http://vocab.nerc.ac.uk/scheme/EDMED_DCAT_THEMES/current> ;
  dcterm:source <http://vocab.nerc.ac.uk/scheme/SDNDEV/current> ;
  pav:authoredOn "2010-11-18 11:16:45.0" ;
  pav:hasCurrentVersion <http://vocab.nerc.ac.uk/collection/L05/current/367/2> ;
  pav:hasVersion <http://vocab.nerc.ac.uk/collection/L05/current/367/1> ;
  owl:versionInfo "2" ;
  skos:broader sdnc:ICAT04 ;
  skos:definition "Devices that provide information on unconsolidated sediment structure through transmission and reception of an energy source with a frequency corresponding to a sampling interval lower than 0.25 msec."@en ;
  skos:inScheme <http://vocab.nerc.ac.uk/scheme/EDMED_DCAT_THEMES/current> ;
  skos:inScheme <http://vocab.nerc.ac.uk/scheme/SDNDEV/current> ;
  skos:narrower <http://vocab.nerc.ac.uk/collection/W01/current/003> ;
  skos:notation "SDN:L05::367" ;
  skos:note "accepted"@en ;
  skos:prefLabel ">2000 Hz top-bandwidth sub-bottom penetrator and mud profiler systems"@en ;
.
<http://vocab.nerc.ac.uk/collection/L05/current/368>
  rdf:type skos:Concept ;
  dcterm:date "2010-02-19 11:52:56.0" ;
  dcterm:identifier "SDN:L05::368" ;
  dcterm:source <http://vocab.nerc.ac.uk/scheme/EDMED_DCAT_THEMES/current> ;
  dcterm:source <http://vocab.nerc.ac.uk/scheme/SDNDEV/current> ;
  pav:authoredOn "2010-02-19 11:52:56.0" ;
  pav:hasCurrentVersion <http://vocab.nerc.ac.uk/collection/L05/current/368/1> ;
  owl:versionInfo "1" ;
  skos:broader sdnc:ICAT04 ;
  skos:definition "Devices placed on the ground or seabed to measure physical movement of that substrate."@en ;
  skos:inScheme <http://vocab.nerc.ac.uk/scheme/EDMED_DCAT_THEMES/current> ;
  skos:inScheme <http://vocab.nerc.ac.uk/scheme/SDNDEV/current> ;
  skos:narrower <http://vocab.nerc.ac.uk/collection/W01/current/003> ;
  skos:notation "SDN:L05::368" ;
  skos:note "accepted"@en ;
  skos:prefLabel "seismometers"@en ;
  skos:scopeNote "subclasses: corehole seismometer, ocean bottom seismometer, posthole seismometer, optical seismometer" ;
.
<http://vocab.nerc.ac.uk/collection/L05/current/369>
  rdf:type skos:Concept ;
  dcterm:date "2010-02-19 11:52:56.0" ;
  dcterm:identifier "SDN:L05::369" ;
  dcterm:source <http://vocab.nerc.ac.uk/scheme/EDMED_DCAT_THEMES/current> ;
  dcterm:source <http://vocab.nerc.ac.uk/scheme/SDNDEV/current> ;
  pav:authoredOn "2010-02-19 11:52:56.0" ;
  pav:hasCurrentVersion <http://vocab.nerc.ac.uk/collection/L05/current/369/1> ;
  owl:versionInfo "1" ;
  skos:broader sdnc:ICAT04 ;
  skos:definition "Devices containing transducers that convert underwater sound waves into electrical signals."@en ;
  skos:inScheme <http://vocab.nerc.ac.uk/scheme/EDMED_DCAT_THEMES/current> ;
  skos:inScheme <http://vocab.nerc.ac.uk/scheme/SDNDEV/current> ;
  skos:narrower inst:TOOL0354 ;
  skos:narrower inst:TOOL1261 ;
  skos:narrower <http://vocab.nerc.ac.uk/collection/W01/current/003> ;
  skos:notation "SDN:L05::369" ;
  skos:note "accepted"@en ;
  skos:prefLabel "hydrophones"@en ;
.
<http://vocab.nerc.ac.uk/collection/L05/current/370>
  rdf:type skos:Concept ;
  dcterm:date "2010-11-18 11:35:46.0" ;
  dcterm:identifier "SDN:L05::370" ;
  dcterm:source <http://vocab.nerc.ac.uk/scheme/EDMED_DCAT_THEMES/current> ;
  dcterm:source <http://vocab.nerc.ac.uk/scheme/SDNDEV/current> ;
  pav:authoredOn "2010-11-18 11:35:46.0" ;
  pav:hasCurrentVersion <http://vocab.nerc.ac.uk/collection/L05/current/370/3> ;
  pav:hasVersion <http://vocab.nerc.ac.uk/collection/L05/current/370/1> ;
  pav:hasVersion <http://vocab.nerc.ac.uk/collection/L05/current/370/2> ;
  owl:versionInfo "3" ;
  skos:broader sdnc:ICAT04 ;
  skos:definition "Instruments carrying a sensor that determines the temperature (degree of hotness) within geological units."@en ;
  skos:inScheme <http://vocab.nerc.ac.uk/scheme/EDMED_DCAT_THEMES/current> ;
  skos:inScheme <http://vocab.nerc.ac.uk/scheme/SDNDEV/current> ;
  skos:narrower <http://vocab.nerc.ac.uk/collection/W01/current/003> ;
  skos:notation "SDN:L05::370" ;
  skos:note "accepted"@en ;
  skos:prefLabel "geothermometers"@en ;
.
<http://vocab.nerc.ac.uk/collection/L05/current/371>
  rdf:type skos:Concept ;
  dcterm:date "2010-02-19 11:52:56.0" ;
  dcterm:identifier "SDN:L05::371" ;
  dcterm:source <http://vocab.nerc.ac.uk/scheme/EDMED_DCAT_THEMES/current> ;
  dcterm:source <http://vocab.nerc.ac.uk/scheme/SDNDEV/current> ;
  pav:authoredOn "2010-02-19 11:52:56.0" ;
  pav:hasCurrentVersion <http://vocab.nerc.ac.uk/collection/L05/current/371/1> ;
  owl:versionInfo "1" ;
  skos:broader <http://vocab.nerc.ac.uk/collection/L05/current/153> ;
  skos:definition "An energy source with a frequency up to 60 Hz (sampling interval higher than 8 msec) plus a single string of towed hydrophones (streamer) that determine geologic structure by detecting waves reflected by subsurface layers."@en ;
  skos:inScheme <http://vocab.nerc.ac.uk/scheme/EDMED_DCAT_THEMES/current> ;
  skos:inScheme <http://vocab.nerc.ac.uk/scheme/SDNDEV/current> ;
  skos:narrower <http://vocab.nerc.ac.uk/collection/W01/current/003> ;
  skos:notation "SDN:L05::371" ;
  skos:note "accepted"@en ;
  skos:prefLabel "60 Hz top-bandwidth single-channel seismic reflection systems"@en ;
  skos:related inst:TOOL0354 ;
.
<http://vocab.nerc.ac.uk/collection/L05/current/372>
  rdf:type skos:Concept ;
  dcterm:date "2010-02-19 11:52:56.0" ;
  dcterm:identifier "SDN:L05::372" ;
  dcterm:source <http://vocab.nerc.ac.uk/scheme/SDNDEV/current> ;
  pav:authoredOn "2010-02-19 11:52:56.0" ;
  pav:hasCurrentVersion <http://vocab.nerc.ac.uk/collection/L05/current/372/1> ;
  owl:versionInfo "1" ;
  skos:broader <http://vocab.nerc.ac.uk/collection/L05/current/153> ;
  skos:definition "An energy source with a frequency up to 2000 Hz (sampling interval ranging from 0.5-0.25 msec) plus a single string of towed hydrophones (streamer) that determine geologic structure by detecting waves reflected by subsurface layers."@en ;
  skos:inScheme <http://vocab.nerc.ac.uk/scheme/SDNDEV/current> ;
  skos:narrower <http://vocab.nerc.ac.uk/collection/W01/current/003> ;
  skos:notation "SDN:L05::372" ;
  skos:note "accepted"@en ;
  skos:prefLabel "2000 Hz top-bandwidth single-channel seismic reflection systems"@en ;
  skos:related inst:TOOL0354 ;
.
<http://vocab.nerc.ac.uk/collection/L05/current/373>
  rdf:type skos:Concept ;
  dcterm:date "2010-02-19 11:52:56.0" ;
  dcterm:identifier "SDN:L05::373" ;
  dcterm:source <http://vocab.nerc.ac.uk/scheme/EDMED_DCAT_THEMES/current> ;
  dcterm:source <http://vocab.nerc.ac.uk/scheme/SDNDEV/current> ;
  pav:authoredOn "2010-02-19 11:52:56.0" ;
  pav:hasCurrentVersion <http://vocab.nerc.ac.uk/collection/L05/current/373/1> ;
  owl:versionInfo "1" ;
  skos:broader <http://vocab.nerc.ac.uk/collection/L05/current/153> ;
  skos:definition "An energy source with a frequency up to >2000 Hz (sampling interval lower than 0.25 msec) plus a single string of towed hydrophones (streamer) that determine geologic structure by detecting waves reflected by subsurface layers."@en ;
  skos:inScheme <http://vocab.nerc.ac.uk/scheme/EDMED_DCAT_THEMES/current> ;
  skos:inScheme <http://vocab.nerc.ac.uk/scheme/SDNDEV/current> ;
  skos:narrower <http://vocab.nerc.ac.uk/collection/W01/current/003> ;
  skos:notation "SDN:L05::373" ;
  skos:note "accepted"@en ;
  skos:prefLabel ">2000 Hz top-bandwidth single-channel seismic reflection systems"@en ;
  skos:related inst:TOOL0354 ;
.
<http://vocab.nerc.ac.uk/collection/L05/current/374>
  rdf:type skos:Concept ;
  dcterm:date "2010-02-19 11:52:56.0" ;
  dcterm:identifier "SDN:L05::374" ;
  dcterm:source <http://vocab.nerc.ac.uk/scheme/EDMED_DCAT_THEMES/current> ;
  dcterm:source <http://vocab.nerc.ac.uk/scheme/SDNDEV/current> ;
  pav:authoredOn "2010-02-19 11:52:56.0" ;
  pav:hasCurrentVersion <http://vocab.nerc.ac.uk/collection/L05/current/374/1> ;
  owl:versionInfo "1" ;
  skos:broader <http://vocab.nerc.ac.uk/collection/L05/current/154> ;
  skos:definition "An energy source with a frequency up to 60 Hz (sampling interval higher than 8 msec) plus a multiple strings of towed hydrophones (streamers) that determine geologic structure by detecting waves reflected by subsurface layers."@en ;
  skos:inScheme <http://vocab.nerc.ac.uk/scheme/EDMED_DCAT_THEMES/current> ;
  skos:inScheme <http://vocab.nerc.ac.uk/scheme/SDNDEV/current> ;
  skos:narrower <http://vocab.nerc.ac.uk/collection/W01/current/003> ;
  skos:notation "SDN:L05::374" ;
  skos:note "accepted"@en ;
  skos:prefLabel "60 Hz top-bandwidth multi-channel seismic reflection systems"@en ;
  skos:related inst:TOOL0354 ;
.
<http://vocab.nerc.ac.uk/collection/L05/current/375>
  rdf:type skos:Concept ;
  dcterm:date "2010-02-19 11:52:56.0" ;
  dcterm:identifier "SDN:L05::375" ;
  dcterm:source <http://vocab.nerc.ac.uk/scheme/SDNDEV/current> ;
  pav:authoredOn "2010-02-19 11:52:56.0" ;
  pav:hasCurrentVersion <http://vocab.nerc.ac.uk/collection/L05/current/375/1> ;
  owl:versionInfo "1" ;
  skos:broader <http://vocab.nerc.ac.uk/collection/L05/current/154> ;
  skos:definition "An energy source with a frequency up to 250 Hz (sampling interval ranging from 2-8 msec) plus a multiple strings of towed hydrophones (streamers) that determine geologic structure by detecting waves reflected by subsurface layers."@en ;
  skos:inScheme <http://vocab.nerc.ac.uk/scheme/SDNDEV/current> ;
  skos:narrower <http://vocab.nerc.ac.uk/collection/W01/current/003> ;
  skos:notation "SDN:L05::375" ;
  skos:note "accepted"@en ;
  skos:prefLabel "250 Hz top-bandwidth multi-channel seismic reflection systems"@en ;
  skos:related inst:TOOL0353 ;
  skos:related inst:TOOL0354 ;
  skos:related inst:TOOL0355 ;
  skos:related inst:TOOL0356 ;
  skos:related inst:TOOL0357 ;
  skos:related inst:TOOL0358 ;
.
<http://vocab.nerc.ac.uk/collection/L05/current/376>
  rdf:type skos:Concept ;
  dcterm:date "2010-04-22 15:13:51.0" ;
  dcterm:identifier "SDN:L05::376" ;
  dcterm:source <http://vocab.nerc.ac.uk/scheme/EDMED_DCAT_THEMES/current> ;
  dcterm:source <http://vocab.nerc.ac.uk/scheme/SDNDEV/current> ;
  pav:authoredOn "2010-04-22 15:13:51.0" ;
  pav:hasCurrentVersion <http://vocab.nerc.ac.uk/collection/L05/current/376/1> ;
  owl:versionInfo "1" ;
  skos:broader sdnc:ICAT04 ;
  skos:definition "Physical markers that allow changes in the position of the boundary between sediment and air or water by visible comparison against marked graduations in units of measurement of dimension length."@en ;
  skos:inScheme <http://vocab.nerc.ac.uk/scheme/EDMED_DCAT_THEMES/current> ;
  skos:inScheme <http://vocab.nerc.ac.uk/scheme/SDNDEV/current> ;
  skos:narrower <http://vocab.nerc.ac.uk/collection/W01/current/003> ;
  skos:notation "SDN:L05::376" ;
  skos:note "accepted"@en ;
  skos:prefLabel "sediment surface markers"@en ;
.
<http://vocab.nerc.ac.uk/collection/L05/current/377>
  rdf:type skos:Concept ;
  dcterm:date "2010-04-22 15:16:00.0" ;
  dcterm:identifier "SDN:L05::377" ;
  dcterm:source <http://vocab.nerc.ac.uk/scheme/EDMED_DCAT_THEMES/current> ;
  dcterm:source <http://vocab.nerc.ac.uk/scheme/SDNDEV/current> ;
  pav:authoredOn "2010-04-22 15:16:00.0" ;
  pav:hasCurrentVersion <http://vocab.nerc.ac.uk/collection/L05/current/377/1> ;
  owl:versionInfo "1" ;
  skos:broader sdnc:ICAT04 ;
  skos:definition "Fixed physical markers that allow changes in the position of the boundary between a water body and the atmosphere by visible comparison against marked graduations in units of measurement of dimension length."@en ;
  skos:inScheme <http://vocab.nerc.ac.uk/scheme/EDMED_DCAT_THEMES/current> ;
  skos:inScheme <http://vocab.nerc.ac.uk/scheme/SDNDEV/current> ;
  skos:narrower <http://vocab.nerc.ac.uk/collection/W01/current/003> ;
  skos:notation "SDN:L05::377" ;
  skos:note "accepted"@en ;
  skos:prefLabel "water level markers"@en ;
.
<http://vocab.nerc.ac.uk/collection/L05/current/378>
  rdf:type skos:Concept ;
  dcterm:date "2010-04-22 15:18:44.0" ;
  dcterm:identifier "SDN:L05::378" ;
  dcterm:source <http://vocab.nerc.ac.uk/scheme/EDMED_DCAT_THEMES/current> ;
  dcterm:source <http://vocab.nerc.ac.uk/scheme/SDNDEV/current> ;
  pav:authoredOn "2010-04-22 15:18:44.0" ;
  pav:hasCurrentVersion <http://vocab.nerc.ac.uk/collection/L05/current/378/1> ;
  owl:versionInfo "1" ;
  skos:broader <http://vocab.nerc.ac.uk/collection/L05/current/180> ;
  skos:broader <http://vocab.nerc.ac.uk/collection/L05/current/311> ;
  skos:broader sdnc:ICAT04 ;
  skos:definition "Devices that provide in-situ still or video images of a section including bottom water, the undisturbed sediment-water interface and the upper sediment layers."@en ;
  skos:inScheme <http://vocab.nerc.ac.uk/scheme/EDMED_DCAT_THEMES/current> ;
  skos:inScheme <http://vocab.nerc.ac.uk/scheme/SDNDEV/current> ;
  skos:narrower <http://vocab.nerc.ac.uk/collection/W01/current/003> ;
  skos:notation "SDN:L05::378" ;
  skos:note "accepted"@en ;
  skos:prefLabel "sediment profile imagers"@en ;
.
<http://vocab.nerc.ac.uk/collection/L05/current/379>
  rdf:type skos:Concept ;
  dcterm:date "2012-12-18 15:18:17.0" ;
  dcterm:identifier "SDN:L05::379" ;
  dcterm:source <http://vocab.nerc.ac.uk/scheme/EDMED_DCAT_THEMES/current> ;
  dcterm:source <http://vocab.nerc.ac.uk/scheme/SDNDEV/current> ;
  pav:authoredOn "2012-12-18 15:18:17.0" ;
  pav:hasCurrentVersion <http://vocab.nerc.ac.uk/collection/L05/current/379/2> ;
  pav:hasVersion <http://vocab.nerc.ac.uk/collection/L05/current/379/1> ;
  owl:versionInfo "2" ;
  skos:broader sdnc:ICAT04 ;
  skos:definition "Instruments that measure their distance above a specified elevation such as the sea surface or the seabed. Classification includes acoustic and pressure-based instruments that are designed to provide platform z co-ordinate spatial coverage in the atmosphere or a water body. It excludes remote sensing instruments such as LIDAR and satellite radar altimeters designed to map surface elevation."@en ;
  skos:inScheme <http://vocab.nerc.ac.uk/scheme/EDMED_DCAT_THEMES/current> ;
  skos:inScheme <http://vocab.nerc.ac.uk/scheme/SDNDEV/current> ;
  skos:narrower <http://vocab.nerc.ac.uk/collection/W01/current/003> ;
  skos:notation "SDN:L05::379" ;
  skos:note "accepted"@en ;
  skos:prefLabel "altimeters"@en ;
.
<http://vocab.nerc.ac.uk/collection/L05/current/380>
  rdf:type skos:Concept ;
  dcterm:date "2010-09-15 10:32:05.0" ;
  dcterm:identifier "SDN:L05::380" ;
  dcterm:source <http://vocab.nerc.ac.uk/scheme/EDMED_DCAT_THEMES/current> ;
  dcterm:source <http://vocab.nerc.ac.uk/scheme/SDNDEV/current> ;
  pav:authoredOn "2010-09-15 10:32:05.0" ;
  pav:hasCurrentVersion <http://vocab.nerc.ac.uk/collection/L05/current/380/1> ;
  owl:versionInfo "1" ;
  skos:broader sdnc:ICAT04 ;
  skos:definition "Electrical conductors routed beneath the sea and connecting land stations.  Oceanographic interest focuses on changes in electrical resistance that may be related to the magnitude of Lagrangian currents."@en ;
  skos:inScheme <http://vocab.nerc.ac.uk/scheme/EDMED_DCAT_THEMES/current> ;
  skos:inScheme <http://vocab.nerc.ac.uk/scheme/SDNDEV/current> ;
  skos:narrower <http://vocab.nerc.ac.uk/collection/W01/current/003> ;
  skos:notation "SDN:L05::380" ;
  skos:note "accepted"@en ;
  skos:prefLabel "submarine cables"@en ;
.
<http://vocab.nerc.ac.uk/collection/L05/current/381>
  rdf:type skos:Concept ;
  dcterm:date "2010-09-15 10:35:20.0" ;
  dcterm:identifier "SDN:L05::381" ;
  dcterm:source <http://vocab.nerc.ac.uk/scheme/EDMED_DCAT_THEMES/current> ;
  dcterm:source <http://vocab.nerc.ac.uk/scheme/SDNDEV/current> ;
  pav:authoredOn "2010-09-15 10:35:20.0" ;
  pav:hasCurrentVersion <http://vocab.nerc.ac.uk/collection/L05/current/381/1> ;
  owl:versionInfo "1" ;
  skos:broader sdnc:ICAT04 ;
  skos:definition "Instruments that measure either the rate of fall or integrated amount of rain, snow, sleet, hail or graupel."@en ;
  skos:inScheme <http://vocab.nerc.ac.uk/scheme/EDMED_DCAT_THEMES/current> ;
  skos:inScheme <http://vocab.nerc.ac.uk/scheme/SDNDEV/current> ;
  skos:narrower <http://onto.nerc.ac.uk/CAST/149> ;
  skos:narrower <http://vocab.nerc.ac.uk/collection/W01/current/003> ;
  skos:notation "SDN:L05::381" ;
  skos:note "accepted"@en ;
  skos:prefLabel "precipitation gauges"@en ;
  skos:scopeNote "subclasses: rain gauge, freezing rain sensor, snow gauge" ;
.
<http://vocab.nerc.ac.uk/collection/L05/current/382>
  rdf:type skos:Concept ;
  dcterm:date "2010-09-15 10:38:47.0" ;
  dcterm:identifier "SDN:L05::382" ;
  dcterm:source <http://vocab.nerc.ac.uk/scheme/SDNDEV/current> ;
  pav:authoredOn "2010-09-15 10:38:47.0" ;
  pav:hasCurrentVersion <http://vocab.nerc.ac.uk/collection/L05/current/382/1> ;
  owl:versionInfo "1" ;
  skos:broader sdnc:ICAT04 ;
  skos:definition "In-situ instruments that can determine the proportion of one or more gaseous components of the atmosphere."@en ;
  skos:inScheme <http://vocab.nerc.ac.uk/scheme/SDNDEV/current> ;
  skos:narrower <http://vocab.nerc.ac.uk/collection/W01/current/003> ;
  skos:notation "SDN:L05::382" ;
  skos:note "accepted"@en ;
  skos:prefLabel "atmospheric gas analysers"@en ;
.
<http://vocab.nerc.ac.uk/collection/L05/current/383>
  rdf:type skos:Concept ;
  dcterm:date "2010-09-15 10:41:46.0" ;
  dcterm:identifier "SDN:L05::383" ;
  dcterm:source <http://vocab.nerc.ac.uk/scheme/EDMED_DCAT_THEMES/current> ;
  dcterm:source <http://vocab.nerc.ac.uk/scheme/SDNDEV/current> ;
  pav:authoredOn "2010-09-15 10:41:46.0" ;
  pav:hasCurrentVersion <http://vocab.nerc.ac.uk/collection/L05/current/383/1> ;
  owl:versionInfo "1" ;
  skos:broader sdnc:ICAT04 ;
  skos:definition "In-situ instruments that can determine the total, dissolved or particulate concentration of one or more metallic elements (including trace metalloids like arsenic) in a water body."@en ;
  skos:inScheme <http://vocab.nerc.ac.uk/scheme/EDMED_DCAT_THEMES/current> ;
  skos:inScheme <http://vocab.nerc.ac.uk/scheme/SDNDEV/current> ;
  skos:narrower <http://vocab.nerc.ac.uk/collection/W01/current/003> ;
  skos:notation "SDN:L05::383" ;
  skos:note "accepted"@en ;
  skos:prefLabel "metal analysers"@en ;
.
<http://vocab.nerc.ac.uk/collection/L05/current/384>
  rdf:type skos:Concept ;
  dcterm:date "2010-09-15 10:51:26.0" ;
  dcterm:identifier "SDN:L05::384" ;
  dcterm:source <http://vocab.nerc.ac.uk/scheme/EDMED_DCAT_THEMES/current> ;
  dcterm:source <http://vocab.nerc.ac.uk/scheme/SDNDEV/current> ;
  pav:authoredOn "2010-09-15 10:51:26.0" ;
  pav:hasCurrentVersion <http://vocab.nerc.ac.uk/collection/L05/current/384/1> ;
  owl:versionInfo "1" ;
  skos:broader sdnc:ICAT04 ;
  skos:definition "ADV is the acronym for acoustic doppler velocimeter. The group includes all in-situ instruments that make high frequency measurements of three-dimensional current velocity in order to determine the extent of turbulence within a water body."@en ;
  skos:inScheme <http://vocab.nerc.ac.uk/scheme/EDMED_DCAT_THEMES/current> ;
  skos:inScheme <http://vocab.nerc.ac.uk/scheme/SDNDEV/current> ;
  skos:narrower <http://vocab.nerc.ac.uk/collection/W01/current/003> ;
  skos:notation "SDN:L05::384" ;
  skos:note "accepted"@en ;
  skos:prefLabel "ADVs and turbulence probes"@en ;
.
<http://vocab.nerc.ac.uk/collection/L05/current/385>
  rdf:type skos:Concept ;
  dcterm:date "2010-09-15 11:00:32.0" ;
  dcterm:identifier "SDN:L05::385" ;
  dcterm:source <http://vocab.nerc.ac.uk/scheme/EDMED_DCAT_THEMES/current> ;
  dcterm:source <http://vocab.nerc.ac.uk/scheme/SDNDEV/current> ;
  pav:authoredOn "2010-09-15 11:00:32.0" ;
  pav:hasCurrentVersion <http://vocab.nerc.ac.uk/collection/L05/current/385/1> ;
  owl:versionInfo "1" ;
  skos:broader sdnc:ICAT04 ;
  skos:definition "Instruments that measure platform orientation or rates of platform motion or acceleration in any direction or along any axis. Excludes inertial navigation systems that are designed to determine platform location with respect to an external co-ordinate reference system."@en ;
  skos:inScheme <http://vocab.nerc.ac.uk/scheme/EDMED_DCAT_THEMES/current> ;
  skos:inScheme <http://vocab.nerc.ac.uk/scheme/SDNDEV/current> ;
  skos:narrower <http://vocab.nerc.ac.uk/collection/W01/current/003> ;
  skos:notation "SDN:L05::385" ;
  skos:note "accepted"@en ;
  skos:prefLabel "platform attitude sensors"@en ;
  skos:scopeNote "subclasses: gyrocompass, spectroradiometer, wind speed sensor, fluxgate compass, motion sensor, GPS system, doppler speed log, magnetic compass, accelerometer." ;
.
<http://vocab.nerc.ac.uk/collection/L05/current/386>
  rdf:type skos:Concept ;
  dcterm:date "2010-10-01 10:36:44.0" ;
  dcterm:identifier "SDN:L05::386" ;
  dcterm:source <http://vocab.nerc.ac.uk/scheme/SDNDEV/current> ;
  pav:authoredOn "2010-10-01 10:36:44.0" ;
  pav:hasCurrentVersion <http://vocab.nerc.ac.uk/collection/L05/current/386/2> ;
  pav:hasVersion <http://vocab.nerc.ac.uk/collection/L05/current/386/1> ;
  owl:versionInfo "2" ;
  skos:broader sdnc:ICAT04 ;
  skos:definition "Instruments that determine physical attributes such as size and abundance of atmospheric aerosols."@en ;
  skos:inScheme <http://vocab.nerc.ac.uk/scheme/SDNDEV/current> ;
  skos:narrower <http://vocab.nerc.ac.uk/collection/W01/current/003> ;
  skos:notation "SDN:L05::386" ;
  skos:note "accepted"@en ;
  skos:prefLabel "Aerosol physical characterisers"@en ;
.
<http://vocab.nerc.ac.uk/collection/L05/current/387>
  rdf:type skos:Concept ;
  dcterm:date "2010-10-01 10:29:09.0" ;
  dcterm:identifier "SDN:L05::387" ;
  dcterm:source <http://vocab.nerc.ac.uk/scheme/SDNDEV/current> ;
  pav:authoredOn "2010-10-01 10:29:09.0" ;
  pav:hasCurrentVersion <http://vocab.nerc.ac.uk/collection/L05/current/387/1> ;
  owl:versionInfo "1" ;
  skos:broader sdnc:ICAT04 ;
  skos:definition "Instruments that quantify atmospheric particulate carbon ('black carbon') concentrations."@en ;
  skos:inScheme <http://vocab.nerc.ac.uk/scheme/SDNDEV/current> ;
  skos:narrower <http://vocab.nerc.ac.uk/collection/W01/current/003> ;
  skos:notation "SDN:L05::387" ;
  skos:note "accepted"@en ;
  skos:prefLabel "Aethalometers"@en ;
.
<http://vocab.nerc.ac.uk/collection/L05/current/388>
  rdf:type skos:Concept ;
  dcterm:date "2011-05-20 09:35:53.0" ;
  dcterm:identifier "SDN:L05::388" ;
  dcterm:source <http://vocab.nerc.ac.uk/scheme/EDMED_DCAT_THEMES/current> ;
  dcterm:source <http://vocab.nerc.ac.uk/scheme/SDNDEV/current> ;
  pav:authoredOn "2011-05-20 09:35:53.0" ;
  pav:hasCurrentVersion <http://vocab.nerc.ac.uk/collection/L05/current/388/1> ;
  owl:versionInfo "1" ;
  skos:broader sdnc:ICAT04 ;
  skos:definition "Sensors that quantify the rate at which fluids (e.g. water or air) pass through sensor packages, instruments or sampling devices."@en ;
  skos:inScheme <http://vocab.nerc.ac.uk/scheme/EDMED_DCAT_THEMES/current> ;
  skos:inScheme <http://vocab.nerc.ac.uk/scheme/SDNDEV/current> ;
  skos:narrower <http://vocab.nerc.ac.uk/collection/W01/current/003> ;
  skos:notation "SDN:L05::388" ;
  skos:note "accepted"@en ;
  skos:prefLabel "flow meters"@en ;
.
<http://vocab.nerc.ac.uk/collection/L05/current/389>
  rdf:type skos:Concept ;
  dcterm:date "2018-10-24 08:19:59.0" ;
  dcterm:identifier "SDN:L05::389" ;
  dcterm:source <http://vocab.nerc.ac.uk/scheme/SDNDEV/current> ;
  pav:authoredOn "2018-10-24 08:19:59.0" ;
  pav:hasCurrentVersion <http://vocab.nerc.ac.uk/collection/L05/current/389/1> ;
  owl:versionInfo "1" ;
  skos:broader <http://vocab.nerc.ac.uk/collection/L05/current/132> ;
  skos:definition "Disposable, free-falling probes that measure temperature in relation to depth using a thermistor and electronic data acquisition system. Probes are dropped into the water and a temperature signal is transferred to the platform by a wire that breaks when the wire is out. Depth is calculated as a function of time to descend and a known constant rate of descent."@en ;
  skos:inScheme <http://vocab.nerc.ac.uk/scheme/SDNDEV/current> ;
  skos:notation "SDN:L05::389" ;
  skos:note "accepted"@en ;
  skos:prefLabel "Expendable bathythermographs"@en ;
.
<http://vocab.nerc.ac.uk/collection/L05/current/390>
  rdf:type skos:Concept ;
  dcterm:date "2018-10-24 09:48:30.0" ;
  dcterm:identifier "SDN:L05::390" ;
  dcterm:source <http://vocab.nerc.ac.uk/scheme/SDNDEV/current> ;
  pav:authoredOn "2018-10-24 09:48:30.0" ;
  pav:hasCurrentVersion <http://vocab.nerc.ac.uk/collection/L05/current/390/1> ;
  owl:versionInfo "1" ;
  skos:broader <http://vocab.nerc.ac.uk/collection/L05/current/132> ;
  skos:definition "Tethered probes that measure temperature in relation to depth using a temperature and pressure package that is lowered into the water and subsequently retrieved using a winch. The profile of temperature is recorded mechanically by etchings on a glass slide. Depth is calculated as a function of pressure."@en ;
  skos:inScheme <http://vocab.nerc.ac.uk/scheme/SDNDEV/current> ;
  skos:notation "SDN:L05::390" ;
  skos:note "accepted"@en ;
  skos:prefLabel "Mechanical bathythermographs"@en ;
.
<http://vocab.nerc.ac.uk/collection/L05/current/393>
  rdf:type skos:Concept ;
  dcterm:date "2020-06-04 14:46:07.0" ;
  dcterm:identifier "SDN:L05::393" ;
  dcterm:source <http://vocab.nerc.ac.uk/scheme/SDNDEV/current> ;
  pav:authoredOn "2020-06-04 14:46:07.0" ;
  pav:hasCurrentVersion <http://vocab.nerc.ac.uk/collection/L05/current/393/1> ;
  owl:versionInfo "1" ;
  skos:broader sdnc:ICAT04 ;
  skos:definition "Optical tools used to magnify and observe terrestrial objects that are distant from the observer. This includes tools such as binoculars, monoculars, terrestrial telescopes and spotting scopes. It excludes astronomical telescopes, camera devices, and tools which enlarge objects close to the observer such as hand lenses."@en ;
  skos:inScheme <http://vocab.nerc.ac.uk/scheme/SDNDEV/current> ;
  skos:narrower inst:TOOL1477 ;
  skos:narrower inst:TOOL1478 ;
  skos:notation "SDN:L05::393" ;
  skos:note "accepted"@en ;
  skos:prefLabel "binoculars and terrestrial scopes"@en ;
.
<http://vocab.nerc.ac.uk/collection/L05/current/395>
  rdf:type skos:Concept ;
  dcterm:date "2021-04-20 18:54:05.0" ;
  dcterm:identifier "SDN:L05::395" ;
  dcterm:source <http://vocab.nerc.ac.uk/scheme/SDNDEV/current> ;
  pav:authoredOn "2021-04-20 18:54:05.0" ;
  pav:hasCurrentVersion <http://vocab.nerc.ac.uk/collection/L05/current/395/1> ;
  owl:versionInfo "1" ;
  skos:broader sdnc:ICAT04 ;
  skos:definition "Instruments that coordinate the time or frequency of independent time devices usually across networks."@en ;
  skos:inScheme <http://vocab.nerc.ac.uk/scheme/SDNDEV/current> ;
  skos:notation "SDN:L05::395" ;
  skos:note "accepted"@en ;
  skos:prefLabel "clock synchronisers"@en ;
.
<http://vocab.nerc.ac.uk/collection/L05/current/86>
  rdf:type skos:Concept ;
  dcterm:date "2016-10-03 14:55:30.0" ;
  dcterm:identifier "SDN:L05::86" ;
  dcterm:source <http://vocab.nerc.ac.uk/scheme/EDMED_DCAT_THEMES/current> ;
  dcterm:source <http://vocab.nerc.ac.uk/scheme/SDNDEV/current> ;
  pav:authoredOn "2016-10-03 14:55:30.0" ;
  pav:hasCurrentVersion <http://vocab.nerc.ac.uk/collection/L05/current/86/1> ;
  owl:versionInfo "1" ;
  skos:broader sdnc:ICAT03 ;
  skos:definition "Instruments measuring carbonate in sediments and inorganic carbon in the water column."@en ;
  skos:inScheme <http://vocab.nerc.ac.uk/scheme/EDMED_DCAT_THEMES/current> ;
  skos:inScheme <http://vocab.nerc.ac.uk/scheme/SDNDEV/current> ;
  skos:notation "SDN:L05::86" ;
  skos:note "accepted"@en ;
  skos:prefLabel "inorganic carbon analysers"@en ;
.
<http://vocab.nerc.ac.uk/collection/L05/current/91>
  rdf:type skos:Concept ;
  dcterm:date "2014-11-18 12:21:30.0" ;
  dcterm:identifier "SDN:L05::91" ;
  dcterm:source <http://vocab.nerc.ac.uk/scheme/EDMED_DCAT_THEMES/current> ;
  dcterm:source <http://vocab.nerc.ac.uk/scheme/NETMAR_OCEAN/current> ;
  dcterm:source <http://vocab.nerc.ac.uk/scheme/NETOC_INSTRUMENT/current> ;
  dcterm:source <http://vocab.nerc.ac.uk/scheme/SDNDEV/current> ;
  pav:authoredOn "2014-11-18 12:21:30.0" ;
  pav:hasCurrentVersion <http://vocab.nerc.ac.uk/collection/L05/current/91/3> ;
  pav:hasVersion <http://vocab.nerc.ac.uk/collection/L05/current/91/1> ;
  pav:hasVersion <http://vocab.nerc.ac.uk/collection/L05/current/91/2> ;
  owl:versionInfo "3" ;
  skos:broader sdnc:ICAT05 ;
  skos:definition "Humans who estimate a parameter through observation of a phenomenon such as bird counts, bird song mappings and visual wave observations."@en ;
  skos:inScheme <http://vocab.nerc.ac.uk/scheme/EDMED_DCAT_THEMES/current> ;
  skos:inScheme <http://vocab.nerc.ac.uk/scheme/NETMAR_OCEAN/current> ;
  skos:inScheme <http://vocab.nerc.ac.uk/scheme/NETOC_INSTRUMENT/current> ;
  skos:inScheme <http://vocab.nerc.ac.uk/scheme/SDNDEV/current> ;
  skos:narrower <http://vocab.nerc.ac.uk/collection/W01/current/003> ;
  skos:notation "SDN:L05::91" ;
  skos:note "accepted"@en ;
  skos:prefLabel "observers"@en ;
  skos:related <http://vocab.nerc.ac.uk/collection/P25/current/ARCOV> ;
  skos:related <http://vocab.nerc.ac.uk/collection/P25/current/VOL> ;
.
<http://vocab.nerc.ac.uk/collection/L05/current/92>
  rdf:type skos:Concept ;
  dcterm:date "2016-06-06 15:34:38.0" ;
  dcterm:identifier "SDN:L05::92" ;
  dcterm:source <http://vocab.nerc.ac.uk/scheme/SDNDEV/current> ;
  pav:authoredOn "2016-06-06 15:34:38.0" ;
  pav:hasCurrentVersion <http://vocab.nerc.ac.uk/collection/L05/current/92/1> ;
  owl:versionInfo "1" ;
  skos:broader sdnc:ICAT05 ;
  skos:definition "Instruments that measure meteorological phenomena such as wind speed, wind direction and air quality remotely by determining the distances from a platform to a reflective surface in the atmosphere or at ground level, calculated from timed return rates of continuous or pulsed emissions of laser light."@en ;
  skos:inScheme <http://vocab.nerc.ac.uk/scheme/SDNDEV/current> ;
  skos:narrower inst:TOOL1079 ;
  skos:notation "SDN:L05::92" ;
  skos:note "accepted"@en ;
  skos:prefLabel "meteorological LiDARs"@en ;
.
sdev:ATRANS
  rdf:type skos:Concept ;
  dcterm:date "2013-04-23 12:49:23.0" ;
  dcterm:identifier "SDN:L05::ATRANS" ;
  dcterm:source <http://vocab.nerc.ac.uk/scheme/SDNDEV/current> ;
  pav:authoredOn "2013-04-23 12:49:23.0" ;
  pav:hasCurrentVersion <http://vocab.nerc.ac.uk/collection/L05/current/ATRANS/1> ;
  owl:versionInfo "1" ;
  skos:broader sdnc:ICAT04 ;
  skos:definition "Instruments that quantify the degree of scattering and absorption of light passing through the atmosphere, including instruments that quantify aerosol and particulate concentrations (e.g. black carbon) and instruments measure meteorological visibility."@en ;
  skos:inScheme <http://vocab.nerc.ac.uk/scheme/SDNDEV/current> ;
  skos:narrower <http://vocab.nerc.ac.uk/collection/W01/current/003> ;
  skos:notation "SDN:L05::ATRANS" ;
  skos:note "accepted"@en ;
  skos:prefLabel "atmospheric transparency quantifiers"@en ;
.
sdev:BLUMS
  rdf:type skos:Concept ;
  dcterm:date "2014-02-04 12:34:21.0" ;
  dcterm:identifier "SDN:L05::BLUMS" ;
  dcterm:source <http://vocab.nerc.ac.uk/scheme/SDNDEV/current> ;
  pav:authoredOn "2014-02-04 12:34:21.0" ;
  pav:hasCurrentVersion <http://vocab.nerc.ac.uk/collection/L05/current/BLUMS/1> ;
  owl:versionInfo "1" ;
  skos:broader sdnc:ICAT04 ;
  skos:definition "Submersible instruments which measure visible emissions from bioluminescent organisms by stimulating intracellular chemiluminescence through mechanical-stressors, such as turbulent water-flow, and sensing by photodetectors, such as photodiodes or photomultiplier tubes. Excludes bioluminescence biosensors which detect the presence of target chemicals or compounds using engineered-bioluminescent bacteria."@en ;
  skos:inScheme <http://vocab.nerc.ac.uk/scheme/SDNDEV/current> ;
  skos:narrower <http://vocab.nerc.ac.uk/collection/W01/current/003> ;
  skos:notation "SDN:L05::BLUMS" ;
  skos:note "accepted"@en ;
  skos:prefLabel "bioluminescence sensors"@en ;
.
sdev:CCOV
  rdf:type skos:Concept ;
  dcterm:date "2013-04-23 13:40:00.0" ;
  dcterm:identifier "SDN:L05::CCOV" ;
  dcterm:source <http://vocab.nerc.ac.uk/scheme/SDNDEV/current> ;
  pav:authoredOn "2013-04-23 13:40:00.0" ;
  pav:hasCurrentVersion <http://vocab.nerc.ac.uk/collection/L05/current/CCOV/1> ;
  owl:versionInfo "1" ;
  skos:broader sdnc:ICAT04 ;
  skos:definition "Instruments that measure the proportion of the sky covered by cloud (cloud amount) and/or the height of the cloud above the ground (cloud base)."@en ;
  skos:inScheme <http://vocab.nerc.ac.uk/scheme/SDNDEV/current> ;
  skos:narrower <http://vocab.nerc.ac.uk/collection/W01/current/003> ;
  skos:notation "SDN:L05::CCOV" ;
  skos:note "accepted"@en ;
  skos:prefLabel "cloud cover quantifiers"@en ;
.
sdev:COLCMP
  rdf:type skos:Concept ;
  dcterm:date "2014-09-01 08:01:41.0" ;
  dcterm:identifier "SDN:L05::COLCMP" ;
  dcterm:source <http://vocab.nerc.ac.uk/scheme/SDNDEV/current> ;
  pav:authoredOn "2014-09-01 08:01:41.0" ;
  pav:hasCurrentVersion <http://vocab.nerc.ac.uk/collection/L05/current/COLCMP/1> ;
  owl:versionInfo "1" ;
  skos:broader sdnc:ICAT04 ;
  skos:definition "Sets of standard materials that provide reference colour charts for the quantification of the colour of an object by visual comparison."@en ;
  skos:inScheme <http://vocab.nerc.ac.uk/scheme/SDNDEV/current> ;
  skos:narrower <http://vocab.nerc.ac.uk/collection/W01/current/003> ;
  skos:notation "SDN:L05::COLCMP" ;
  skos:note "accepted"@en ;
  skos:prefLabel "Colour comparators"@en ;
.
sdev:CSEM
  rdf:type skos:Concept ;
  dcterm:date "2016-03-10 06:45:48.0" ;
  dcterm:identifier "SDN:L05::CSEM" ;
  dcterm:source <http://vocab.nerc.ac.uk/scheme/SDNDEV/current> ;
  pav:authoredOn "2016-03-10 06:45:48.0" ;
  pav:hasCurrentVersion <http://vocab.nerc.ac.uk/collection/L05/current/CSEM/2> ;
  pav:hasVersion <http://vocab.nerc.ac.uk/collection/L05/current/CSEM/1> ;
  owl:versionInfo "2" ;
  skos:altLabel "CSEM"@en ;
  skos:broader sdnc:ICAT05 ;
  skos:definition "Systems that measure sub-surface resistivity structure through the measurement of the electromegnetic fields resulting from stimulation by a towed source.  Includes systems incorporating both transmitter and receiver and systems where the transmitter and receiver are separate."@en ;
  skos:inScheme <http://vocab.nerc.ac.uk/scheme/SDNDEV/current> ;
  skos:narrower <http://vocab.nerc.ac.uk/collection/W01/current/003> ;
  skos:notation "SDN:L05::CSEM" ;
  skos:note "accepted"@en ;
  skos:prefLabel "controlled-source electromagnetic systems"@en ;
.
sdev:DLOG
  rdf:type skos:Concept ;
  dcterm:date "2017-12-05 11:14:23.0" ;
  dcterm:identifier "SDN:L05::DLOG" ;
  dcterm:source <http://vocab.nerc.ac.uk/scheme/SDNDEV/current> ;
  pav:authoredOn "2017-12-05 11:14:23.0" ;
  pav:hasCurrentVersion <http://vocab.nerc.ac.uk/collection/L05/current/DLOG/1> ;
  owl:versionInfo "1" ;
  skos:broader sdnc:ICAT04 ;
  skos:definition "Electronic devices that record data over time or in relation to location either with a built-in instrument or sensor or via external instruments and sensors."@en ;
  skos:inScheme <http://vocab.nerc.ac.uk/scheme/SDNDEV/current> ;
  skos:notation "SDN:L05::DLOG" ;
  skos:note "accepted"@en ;
  skos:prefLabel "data loggers"@en ;
.
sdev:EMSR
  rdf:type skos:Concept ;
  dcterm:date "2019-12-11 18:23:45.0" ;
  dcterm:identifier "SDN:L05::EMSR" ;
  dcterm:source <http://vocab.nerc.ac.uk/scheme/EDMED_DCAT_THEMES/current> ;
  dcterm:source <http://vocab.nerc.ac.uk/scheme/SDNDEV/current> ;
  pav:authoredOn "2019-12-11 18:23:45.0" ;
  pav:hasCurrentVersion <http://vocab.nerc.ac.uk/collection/L05/current/EMSR/2> ;
  pav:hasVersion <http://vocab.nerc.ac.uk/collection/L05/current/EMSR/1> ;
  owl:versionInfo "2" ;
  skos:broader sdnc:ICAT04 ;
  skos:definition "In-situ sensors that simultaneuously measure electrical and magnetic fields.  They are usually moored on the seabed for long periods of time for determination of deep structure through monitoring magnetotelluric currents.  However, some may also be configured to be receivers for active electromagnetic surveys such as CSEM."@en ;
  skos:inScheme <http://vocab.nerc.ac.uk/scheme/EDMED_DCAT_THEMES/current> ;
  skos:inScheme <http://vocab.nerc.ac.uk/scheme/SDNDEV/current> ;
  skos:narrower <http://vocab.nerc.ac.uk/collection/W01/current/003> ;
  skos:notation "SDN:L05::EMSR" ;
  skos:note "accepted"@en ;
  skos:prefLabel "electromagnetic sensors"@en ;
.
sdev:FFES
  rdf:type skos:Concept ;
  dcterm:date "2023-01-03 09:50:33.0" ;
  dcterm:identifier "SDN:L05::FFES" ;
  dcterm:source <http://vocab.nerc.ac.uk/scheme/EDMED_DCAT_THEMES/current> ;
  dcterm:source <http://vocab.nerc.ac.uk/scheme/SDNDEV/current> ;
  pav:authoredOn "2023-01-03 09:50:33.0" ;
  pav:hasCurrentVersion <http://vocab.nerc.ac.uk/collection/L05/current/FFES/2> ;
  pav:hasVersion <http://vocab.nerc.ac.uk/collection/L05/current/FFES/1> ;
  owl:versionInfo "2" ;
  skos:broader sdnc:ICAT04 ;
  skos:definition "Sonar instruments primarily designed to detect aquatic organisms through directed transmission and reception of acoustic signals. They often utilise multiple frequencies."@en ;
  skos:inScheme <http://vocab.nerc.ac.uk/scheme/EDMED_DCAT_THEMES/current> ;
  skos:inScheme <http://vocab.nerc.ac.uk/scheme/SDNDEV/current> ;
  skos:narrower <http://vocab.nerc.ac.uk/collection/W01/current/003> ;
  skos:notation "SDN:L05::FFES" ;
  skos:note "accepted"@en ;
  skos:prefLabel "Fish-finder echosounders"@en ;
.
sdev:ICEP
  rdf:type skos:Concept ;
  dcterm:date "2013-04-23 12:40:29.0" ;
  dcterm:identifier "SDN:L05::ICEP" ;
  dcterm:source <http://vocab.nerc.ac.uk/scheme/EDMED_DCAT_THEMES/current> ;
  dcterm:source <http://vocab.nerc.ac.uk/scheme/SDNDEV/current> ;
  pav:authoredOn "2013-04-23 12:40:29.0" ;
  pav:hasCurrentVersion <http://vocab.nerc.ac.uk/collection/L05/current/ICEP/1> ;
  owl:versionInfo "1" ;
  skos:broader sdnc:ICAT04 ;
  skos:definition "Instruments that measure the freeboard, draught or thickness of ice sheets or sea ice. These are not to be confused with tethered ice profilers that are platforms that sample the water column beneath sea ice."@en ;
  skos:inScheme <http://vocab.nerc.ac.uk/scheme/EDMED_DCAT_THEMES/current> ;
  skos:inScheme <http://vocab.nerc.ac.uk/scheme/SDNDEV/current> ;
  skos:narrower <http://vocab.nerc.ac.uk/collection/W01/current/003> ;
  skos:notation "SDN:L05::ICEP" ;
  skos:note "accepted"@en ;
  skos:prefLabel "ice thickness profilers"@en ;
.
sdev:LAB01
  rdf:type skos:Concept ;
  dcterm:date "2008-01-10 16:10:12.0" ;
  dcterm:identifier "SDN:L05::LAB01" ;
  dcterm:source <http://vocab.nerc.ac.uk/scheme/EDMED_DCAT_THEMES/current> ;
  dcterm:source <http://vocab.nerc.ac.uk/scheme/SDNDEV/current> ;
  pav:authoredOn "2008-01-10 16:10:12.0" ;
  pav:hasCurrentVersion <http://vocab.nerc.ac.uk/collection/L05/current/LAB01/1> ;
  owl:versionInfo "1" ;
  skos:broader sdnc:ICAT03 ;
  skos:definition "Instruments that quantify carbon, nitrogen and sometimes other elements by combusting the sample at very high temperature and assaying the resulting gaseous oxides. Usually used for samples including organic material."@en ;
  skos:inScheme <http://vocab.nerc.ac.uk/scheme/EDMED_DCAT_THEMES/current> ;
  skos:inScheme <http://vocab.nerc.ac.uk/scheme/SDNDEV/current> ;
  skos:narrower <http://onto.nerc.ac.uk/CAST/124> ;
  skos:narrower <http://onto.nerc.ac.uk/CAST/127> ;
  skos:narrower <http://onto.nerc.ac.uk/CAST/144> ;
  skos:narrower <http://vocab.nerc.ac.uk/collection/W01/current/003> ;
  skos:notation "SDN:L05::LAB01" ;
  skos:note "accepted"@en ;
  skos:prefLabel "elemental analysers"@en ;
.
sdev:LAB02
  rdf:type skos:Concept ;
  dcterm:date "2008-01-10 16:10:12.0" ;
  dcterm:identifier "SDN:L05::LAB02" ;
  dcterm:source <http://vocab.nerc.ac.uk/scheme/EDMED_DCAT_THEMES/current> ;
  dcterm:source <http://vocab.nerc.ac.uk/scheme/SDNDEV/current> ;
  pav:authoredOn "2008-01-10 16:10:12.0" ;
  pav:hasCurrentVersion <http://vocab.nerc.ac.uk/collection/L05/current/LAB02/1> ;
  owl:versionInfo "1" ;
  skos:broader sdnc:ICAT03 ;
  skos:definition "Instruments separating gases, volatile substances or substances dissolved in a volatile solvent by transporting an inert gas through a column packed with a sorbent to a detector for assay."@en ;
  skos:inScheme <http://vocab.nerc.ac.uk/scheme/EDMED_DCAT_THEMES/current> ;
  skos:inScheme <http://vocab.nerc.ac.uk/scheme/SDNDEV/current> ;
  skos:narrower <http://vocab.nerc.ac.uk/collection/W01/current/003> ;
  skos:notation "SDN:L05::LAB02" ;
  skos:note "accepted"@en ;
  skos:prefLabel "gas chromatographs"@en ;
.
sdev:LAB03
  rdf:type skos:Concept ;
  dcterm:date "2008-01-10 16:10:12.0" ;
  dcterm:identifier "SDN:L05::LAB03" ;
  dcterm:source <http://vocab.nerc.ac.uk/scheme/EDMED_DCAT_THEMES/current> ;
  dcterm:source <http://vocab.nerc.ac.uk/scheme/NETMAR_OCEAN/current> ;
  dcterm:source <http://vocab.nerc.ac.uk/scheme/NETOC_INSTRUMENT/current> ;
  dcterm:source <http://vocab.nerc.ac.uk/scheme/SDNDEV/current> ;
  pav:authoredOn "2008-01-10 16:10:12.0" ;
  pav:hasCurrentVersion <http://vocab.nerc.ac.uk/collection/L05/current/LAB03/1> ;
  owl:versionInfo "1" ;
  skos:broader sdnc:ICAT03 ;
  skos:definition "Instruments measuring the amount of light of a given wavelength absorbed by a sample of solution to determine the concentration of a specific coloured solute."@en ;
  skos:inScheme <http://vocab.nerc.ac.uk/scheme/EDMED_DCAT_THEMES/current> ;
  skos:inScheme <http://vocab.nerc.ac.uk/scheme/NETMAR_OCEAN/current> ;
  skos:inScheme <http://vocab.nerc.ac.uk/scheme/NETOC_INSTRUMENT/current> ;
  skos:inScheme <http://vocab.nerc.ac.uk/scheme/SDNDEV/current> ;
  skos:narrower <http://vocab.nerc.ac.uk/collection/W01/current/003> ;
  skos:notation "SDN:L05::LAB03" ;
  skos:note "accepted"@en ;
  skos:prefLabel "colorimeters"@en ;
  skos:related <http://vocab.nerc.ac.uk/collection/P25/current/NO2> ;
  skos:related <http://vocab.nerc.ac.uk/collection/P25/current/NO3> ;
  skos:related <http://vocab.nerc.ac.uk/collection/P25/current/NO3NO2> ;
  skos:related <http://vocab.nerc.ac.uk/collection/P25/current/PO4> ;
  skos:related <http://vocab.nerc.ac.uk/collection/P25/current/SLCA> ;
.
sdev:LAB04
  rdf:type skos:Concept ;
  dcterm:date "2008-01-10 16:10:12.0" ;
  dcterm:identifier "SDN:L05::LAB04" ;
  dcterm:source <http://vocab.nerc.ac.uk/scheme/EDMED_DCAT_THEMES/current> ;
  dcterm:source <http://vocab.nerc.ac.uk/scheme/NETMAR_OCEAN/current> ;
  dcterm:source <http://vocab.nerc.ac.uk/scheme/NETOC_INSTRUMENT/current> ;
  dcterm:source <http://vocab.nerc.ac.uk/scheme/SDNDEV/current> ;
  pav:authoredOn "2008-01-10 16:10:12.0" ;
  pav:hasCurrentVersion <http://vocab.nerc.ac.uk/collection/L05/current/LAB04/1> ;
  owl:versionInfo "1" ;
  skos:broader sdnc:ICAT03 ;
  skos:definition "Instruments that continuously draw samples through plumbing adding reagents whilst controlling the environment to produce a chemical reaction before passing the sample to a detector, e.g. the automated colorimetric determination of nutrients."@en ;
  skos:inScheme <http://vocab.nerc.ac.uk/scheme/EDMED_DCAT_THEMES/current> ;
  skos:inScheme <http://vocab.nerc.ac.uk/scheme/NETMAR_OCEAN/current> ;
  skos:inScheme <http://vocab.nerc.ac.uk/scheme/NETOC_INSTRUMENT/current> ;
  skos:inScheme <http://vocab.nerc.ac.uk/scheme/SDNDEV/current> ;
  skos:narrower <http://onto.nerc.ac.uk/CAST/117> ;
  skos:narrower <http://vocab.nerc.ac.uk/collection/W01/current/003> ;
  skos:notation "SDN:L05::LAB04" ;
  skos:note "accepted"@en ;
  skos:prefLabel "autoanalysers"@en ;
  skos:related <http://vocab.nerc.ac.uk/collection/P25/current/NO2> ;
  skos:related <http://vocab.nerc.ac.uk/collection/P25/current/NO3> ;
  skos:related <http://vocab.nerc.ac.uk/collection/P25/current/NO3NO2> ;
  skos:related <http://vocab.nerc.ac.uk/collection/P25/current/PO4> ;
  skos:related <http://vocab.nerc.ac.uk/collection/P25/current/SLCA> ;
  skos:scopeNote "subclasses: colorimetric, coulometer" ;
.
sdev:LAB05
  rdf:type skos:Concept ;
  dcterm:date "2008-01-10 16:10:12.0" ;
  dcterm:identifier "SDN:L05::LAB05" ;
  dcterm:source <http://vocab.nerc.ac.uk/scheme/EDMED_DCAT_THEMES/current> ;
  dcterm:source <http://vocab.nerc.ac.uk/scheme/NETMAR_OCEAN/current> ;
  dcterm:source <http://vocab.nerc.ac.uk/scheme/NETOC_INSTRUMENT/current> ;
  dcterm:source <http://vocab.nerc.ac.uk/scheme/SDNDEV/current> ;
  pav:authoredOn "2008-01-10 16:10:12.0" ;
  pav:hasCurrentVersion <http://vocab.nerc.ac.uk/collection/L05/current/LAB05/1> ;
  owl:versionInfo "1" ;
  skos:broader sdnc:ICAT03 ;
  skos:definition "Instruments that generate enlarged images of samples using the phenomena of reflection and absorption of visible light. Includes conventional and inverted instruments."@en ;
  skos:inScheme <http://vocab.nerc.ac.uk/scheme/EDMED_DCAT_THEMES/current> ;
  skos:inScheme <http://vocab.nerc.ac.uk/scheme/NETMAR_OCEAN/current> ;
  skos:inScheme <http://vocab.nerc.ac.uk/scheme/NETOC_INSTRUMENT/current> ;
  skos:inScheme <http://vocab.nerc.ac.uk/scheme/SDNDEV/current> ;
  skos:narrower inst:TOOL1034 ;
  skos:narrower <http://vocab.nerc.ac.uk/collection/W01/current/003> ;
  skos:notation "SDN:L05::LAB05" ;
  skos:note "accepted"@en ;
  skos:prefLabel "optical microscopes"@en ;
  skos:related <http://vocab.nerc.ac.uk/collection/P25/current/PHYTABUND> ;
.
sdev:LAB06
  rdf:type skos:Concept ;
  dcterm:date "2008-01-10 16:10:12.0" ;
  dcterm:identifier "SDN:L05::LAB06" ;
  dcterm:source <http://vocab.nerc.ac.uk/scheme/EDMED_DCAT_THEMES/current> ;
  dcterm:source <http://vocab.nerc.ac.uk/scheme/NETMAR_OCEAN/current> ;
  dcterm:source <http://vocab.nerc.ac.uk/scheme/NETOC_INSTRUMENT/current> ;
  dcterm:source <http://vocab.nerc.ac.uk/scheme/SDNDEV/current> ;
  pav:authoredOn "2008-01-10 16:10:12.0" ;
  pav:hasCurrentVersion <http://vocab.nerc.ac.uk/collection/L05/current/LAB06/1> ;
  owl:versionInfo "1" ;
  skos:broader sdnc:ICAT03 ;
  skos:definition "Instruments that generate enlarged images of samples using the phenomena of fluorescence and phosphorescence instead of, or in addition to, reflection and absorption of visible light. Includes conventional and inverted instruments."@en ;
  skos:inScheme <http://vocab.nerc.ac.uk/scheme/EDMED_DCAT_THEMES/current> ;
  skos:inScheme <http://vocab.nerc.ac.uk/scheme/NETMAR_OCEAN/current> ;
  skos:inScheme <http://vocab.nerc.ac.uk/scheme/NETOC_INSTRUMENT/current> ;
  skos:inScheme <http://vocab.nerc.ac.uk/scheme/SDNDEV/current> ;
  skos:narrower <http://vocab.nerc.ac.uk/collection/W01/current/003> ;
  skos:notation "SDN:L05::LAB06" ;
  skos:note "accepted"@en ;
  skos:prefLabel "fluorescence microscopes"@en ;
  skos:related <http://vocab.nerc.ac.uk/collection/P25/current/PHYTABUND> ;
.
sdev:LAB07
  rdf:type skos:Concept ;
  dcterm:date "2008-01-10 16:10:12.0" ;
  dcterm:identifier "SDN:L05::LAB07" ;
  dcterm:source <http://vocab.nerc.ac.uk/scheme/EDMED_DCAT_THEMES/current> ;
  dcterm:source <http://vocab.nerc.ac.uk/scheme/SDNDEV/current> ;
  pav:authoredOn "2008-01-10 16:10:12.0" ;
  pav:hasCurrentVersion <http://vocab.nerc.ac.uk/collection/L05/current/LAB07/1> ;
  owl:versionInfo "1" ;
  skos:broader sdnc:ICAT03 ;
  skos:definition "Instruments that generate enlarged images of samples using the phenomena of reflection and absorption of electrons behaving as waves."@en ;
  skos:inScheme <http://vocab.nerc.ac.uk/scheme/EDMED_DCAT_THEMES/current> ;
  skos:inScheme <http://vocab.nerc.ac.uk/scheme/SDNDEV/current> ;
  skos:narrower <http://vocab.nerc.ac.uk/collection/W01/current/003> ;
  skos:notation "SDN:L05::LAB07" ;
  skos:note "accepted"@en ;
  skos:prefLabel "electron microscopes"@en ;
.
sdev:LAB08
  rdf:type skos:Concept ;
  dcterm:date "2008-01-10 16:10:12.0" ;
  dcterm:identifier "SDN:L05::LAB08" ;
  dcterm:source <http://vocab.nerc.ac.uk/scheme/EDMED_DCAT_THEMES/current> ;
  dcterm:source <http://vocab.nerc.ac.uk/scheme/SDNDEV/current> ;
  pav:authoredOn "2008-01-10 16:10:12.0" ;
  pav:hasCurrentVersion <http://vocab.nerc.ac.uk/collection/L05/current/LAB08/1> ;
  owl:versionInfo "1" ;
  skos:broader sdnc:ICAT03 ;
  skos:definition "Instruments that chemically analyse a small area of a sample by bombarding it with electrons and spectroscopically assaying the resulting X-Ray emissions."@en ;
  skos:inScheme <http://vocab.nerc.ac.uk/scheme/EDMED_DCAT_THEMES/current> ;
  skos:inScheme <http://vocab.nerc.ac.uk/scheme/SDNDEV/current> ;
  skos:narrower <http://vocab.nerc.ac.uk/collection/W01/current/003> ;
  skos:notation "SDN:L05::LAB08" ;
  skos:note "accepted"@en ;
  skos:prefLabel "electron microprobes"@en ;
.
sdev:LAB09
  rdf:type skos:Concept ;
  dcterm:date "2008-01-10 16:10:12.0" ;
  dcterm:identifier "SDN:L05::LAB09" ;
  dcterm:source <http://vocab.nerc.ac.uk/scheme/EDMED_DCAT_THEMES/current> ;
  dcterm:source <http://vocab.nerc.ac.uk/scheme/SDNDEV/current> ;
  pav:authoredOn "2008-01-10 16:10:12.0" ;
  pav:hasCurrentVersion <http://vocab.nerc.ac.uk/collection/L05/current/LAB09/1> ;
  owl:versionInfo "1" ;
  skos:broader sdnc:ICAT03 ;
  skos:definition "Instruments that isotopically analyse a small area of sample by bombarding it with ions to form a plasma that is analysed in a mass spectrometer."@en ;
  skos:inScheme <http://vocab.nerc.ac.uk/scheme/EDMED_DCAT_THEMES/current> ;
  skos:inScheme <http://vocab.nerc.ac.uk/scheme/SDNDEV/current> ;
  skos:narrower <http://vocab.nerc.ac.uk/collection/W01/current/003> ;
  skos:notation "SDN:L05::LAB09" ;
  skos:note "accepted"@en ;
  skos:prefLabel "ion microprobes"@en ;
.
sdev:LAB10
  rdf:type skos:Concept ;
  dcterm:date "2008-01-10 16:10:12.0" ;
  dcterm:identifier "SDN:L05::LAB10" ;
  dcterm:source <http://vocab.nerc.ac.uk/scheme/EDMED_DCAT_THEMES/current> ;
  dcterm:source <http://vocab.nerc.ac.uk/scheme/SDNDEV/current> ;
  pav:authoredOn "2008-01-10 16:10:12.0" ;
  pav:hasCurrentVersion <http://vocab.nerc.ac.uk/collection/L05/current/LAB10/1> ;
  owl:sameAs <http://onto.nerc.ac.uk/CAST/115> ;
  owl:versionInfo "1" ;
  skos:broader sdnc:ICAT03 ;
  skos:definition "Instruments that volatilise the sample, illuminate the resultant vapour with light wavelengths matched to the analyte of interest and quantify the radiation absorbed, which is proportional to concentration."@en ;
  skos:inScheme <http://vocab.nerc.ac.uk/scheme/EDMED_DCAT_THEMES/current> ;
  skos:inScheme <http://vocab.nerc.ac.uk/scheme/SDNDEV/current> ;
  skos:narrower <http://vocab.nerc.ac.uk/collection/W01/current/003> ;
  skos:notation "SDN:L05::LAB10" ;
  skos:note "accepted"@en ;
  skos:prefLabel "atomic absorption spectrometers"@en ;
.
sdev:LAB11
  rdf:type skos:Concept ;
  dcterm:date "2008-01-10 16:10:12.0" ;
  dcterm:identifier "SDN:L05::LAB11" ;
  dcterm:source <http://vocab.nerc.ac.uk/scheme/EDMED_DCAT_THEMES/current> ;
  dcterm:source <http://vocab.nerc.ac.uk/scheme/NETMAR_OCEAN/current> ;
  dcterm:source <http://vocab.nerc.ac.uk/scheme/NETOC_INSTRUMENT/current> ;
  dcterm:source <http://vocab.nerc.ac.uk/scheme/SDNDEV/current> ;
  pav:authoredOn "2008-01-10 16:10:12.0" ;
  pav:hasCurrentVersion <http://vocab.nerc.ac.uk/collection/L05/current/LAB11/1> ;
  owl:versionInfo "1" ;
  skos:broader sdnc:ICAT03 ;
  skos:definition "Instruments that separate and analyse mixtures of substances by high pressure pumping the sample through a column packed with microspheres coated with the stationary phase."@en ;
  skos:inScheme <http://vocab.nerc.ac.uk/scheme/EDMED_DCAT_THEMES/current> ;
  skos:inScheme <http://vocab.nerc.ac.uk/scheme/NETMAR_OCEAN/current> ;
  skos:inScheme <http://vocab.nerc.ac.uk/scheme/NETOC_INSTRUMENT/current> ;
  skos:inScheme <http://vocab.nerc.ac.uk/scheme/SDNDEV/current> ;
  skos:narrower <http://vocab.nerc.ac.uk/collection/W01/current/003> ;
  skos:notation "SDN:L05::LAB11" ;
  skos:note "accepted"@en ;
  skos:prefLabel "high performance liquid chromatographs"@en ;
  skos:related <http://vocab.nerc.ac.uk/collection/P25/current/CHLA> ;
.
sdev:LAB12
  rdf:type skos:Concept ;
  dcterm:date "2008-01-10 16:10:12.0" ;
  dcterm:identifier "SDN:L05::LAB12" ;
  dcterm:source <http://vocab.nerc.ac.uk/scheme/EDMED_DCAT_THEMES/current> ;
  dcterm:source <http://vocab.nerc.ac.uk/scheme/SDNDEV/current> ;
  pav:authoredOn "2008-01-10 16:10:12.0" ;
  pav:hasCurrentVersion <http://vocab.nerc.ac.uk/collection/L05/current/LAB12/1> ;
  owl:sameAs <http://onto.nerc.ac.uk/CAST/122> ;
  owl:versionInfo "1" ;
  skos:broader sdnc:ICAT03 ;
  skos:definition "Instruments that incrementally add quantified aliquites of a reagent to a sample until the end-point of a chemical reaction is reached."@en ;
  skos:inScheme <http://vocab.nerc.ac.uk/scheme/EDMED_DCAT_THEMES/current> ;
  skos:inScheme <http://vocab.nerc.ac.uk/scheme/SDNDEV/current> ;
  skos:narrower <http://vocab.nerc.ac.uk/collection/W01/current/003> ;
  skos:notation "SDN:L05::LAB12" ;
  skos:note "accepted"@en ;
  skos:prefLabel "titrators"@en ;
  skos:scopeNote "subclasses: alkalinity titrator, oxygen titrator, potentiometric titrator, Winkler titration system" ;
.
sdev:LAB13
  rdf:type skos:Concept ;
  dcterm:date "2010-07-02 14:19:32.0" ;
  dcterm:identifier "SDN:L05::LAB13" ;
  dcterm:source <http://vocab.nerc.ac.uk/scheme/EDMED_DCAT_THEMES/current> ;
  dcterm:source <http://vocab.nerc.ac.uk/scheme/SDNDEV/current> ;
  pav:authoredOn "2010-07-02 14:19:32.0" ;
  pav:hasCurrentVersion <http://vocab.nerc.ac.uk/collection/L05/current/LAB13/2> ;
  pav:hasVersion <http://vocab.nerc.ac.uk/collection/L05/current/LAB13/1> ;
  owl:versionInfo "2" ;
  skos:broader sdnc:ICAT03 ;
  skos:definition "Devices that determine the mass or weight of a sample."@en ;
  skos:inScheme <http://vocab.nerc.ac.uk/scheme/EDMED_DCAT_THEMES/current> ;
  skos:inScheme <http://vocab.nerc.ac.uk/scheme/SDNDEV/current> ;
  skos:narrower <http://onto.nerc.ac.uk/CAST/151> ;
  skos:narrower <http://vocab.nerc.ac.uk/collection/W01/current/003> ;
  skos:notation "SDN:L05::LAB13" ;
  skos:note "accepted"@en ;
  skos:prefLabel "balances and scales"@en ;
.
sdev:LAB14
  rdf:type skos:Concept ;
  dcterm:date "2008-01-10 16:10:12.0" ;
  dcterm:identifier "SDN:L05::LAB14" ;
  dcterm:source <http://vocab.nerc.ac.uk/scheme/EDMED_DCAT_THEMES/current> ;
  dcterm:source <http://vocab.nerc.ac.uk/scheme/SDNDEV/current> ;
  pav:authoredOn "2008-01-10 16:10:12.0" ;
  pav:hasCurrentVersion <http://vocab.nerc.ac.uk/collection/L05/current/LAB14/1> ;
  owl:sameAs <http://onto.nerc.ac.uk/CAST/137> ;
  owl:versionInfo "1" ;
  skos:broader sdnc:ICAT03 ;
  skos:definition "Instruments that pass nebulised samples into an inductively-coupled gas plasma (8-10000 K) where they are atomised and excited. The de-excitation optical emissions at characteristic wavelengths are spectroscopically analysed."@en ;
  skos:inScheme <http://vocab.nerc.ac.uk/scheme/EDMED_DCAT_THEMES/current> ;
  skos:inScheme <http://vocab.nerc.ac.uk/scheme/SDNDEV/current> ;
  skos:narrower <http://vocab.nerc.ac.uk/collection/W01/current/003> ;
  skos:notation "SDN:L05::LAB14" ;
  skos:note "accepted"@en ;
  skos:prefLabel "inductively-coupled plasma atomic emission spectroscopes"@en ;
.
sdev:LAB15
  rdf:type skos:Concept ;
  dcterm:date "2008-01-10 16:10:12.0" ;
  dcterm:identifier "SDN:L05::LAB15" ;
  dcterm:source <http://vocab.nerc.ac.uk/scheme/EDMED_DCAT_THEMES/current> ;
  dcterm:source <http://vocab.nerc.ac.uk/scheme/SDNDEV/current> ;
  pav:authoredOn "2008-01-10 16:10:12.0" ;
  pav:hasCurrentVersion <http://vocab.nerc.ac.uk/collection/L05/current/LAB15/1> ;
  owl:sameAs <http://onto.nerc.ac.uk/CAST/134> ;
  owl:versionInfo "1" ;
  skos:broader sdev:LAB16 ;
  skos:definition "Instruments that pass nebulised samples into an inductively-coupled gas plasma (8-10000 K) where they are atomised and ionised. Ions of specific mass-to-charge ratios are quantified in a quadrupole mass spectrometer. [editor note-- not all ICPMS use quadrupole mass analyzers]"@en ;
  skos:inScheme <http://vocab.nerc.ac.uk/scheme/EDMED_DCAT_THEMES/current> ;
  skos:inScheme <http://vocab.nerc.ac.uk/scheme/SDNDEV/current> ;
  skos:narrower <http://vocab.nerc.ac.uk/collection/W01/current/003> ;
  skos:notation "SDN:L05::LAB15" ;
  skos:note "accepted"@en ;
  skos:prefLabel "inductively-coupled plasma mass spectrometers"@en ;
.
sdev:LAB16
  rdf:type skos:Concept ;
  dcterm:date "2008-01-10 16:10:12.0" ;
  dcterm:identifier "SDN:L05::LAB16" ;
  dcterm:source <http://vocab.nerc.ac.uk/scheme/EDMED_DCAT_THEMES/current> ;
  dcterm:source <http://vocab.nerc.ac.uk/scheme/SDNDEV/current> ;
  pav:authoredOn "2008-01-10 16:10:12.0" ;
  pav:hasCurrentVersion <http://vocab.nerc.ac.uk/collection/L05/current/LAB16/1> ;
  owl:versionInfo "1" ;
  skos:broader sdnc:ICAT03 ;
  skos:definition "Instruments used to measure the mass-to-charge ratio of ions most generally used to find the composition of a sample by generating a mass spectrum representing the masses of sample components."@en ;
  skos:inScheme <http://vocab.nerc.ac.uk/scheme/EDMED_DCAT_THEMES/current> ;
  skos:inScheme <http://vocab.nerc.ac.uk/scheme/SDNDEV/current> ;
  skos:narrower sdev:LAB15 ;
  skos:narrower sdev:LAB17 ;
  skos:narrower sdev:LAB19 ;
  skos:narrower sdev:LAB46 ;
  skos:narrower sdev:LAB47 ;
  skos:narrower sdev:LAB48 ;
  skos:narrower <http://vocab.nerc.ac.uk/collection/W01/current/003> ;
  skos:notation "SDN:L05::LAB16" ;
  skos:note "accepted"@en ;
  skos:prefLabel "mass spectrometers"@en ;
.
sdev:LAB17
  rdf:type skos:Concept ;
  dcterm:date "2008-01-10 16:10:12.0" ;
  dcterm:identifier "SDN:L05::LAB17" ;
  dcterm:source <http://vocab.nerc.ac.uk/scheme/EDMED_DCAT_THEMES/current> ;
  dcterm:source <http://vocab.nerc.ac.uk/scheme/SDNDEV/current> ;
  pav:authoredOn "2008-01-10 16:10:12.0" ;
  pav:hasCurrentVersion <http://vocab.nerc.ac.uk/collection/L05/current/LAB17/1> ;
  owl:versionInfo "1" ;
  skos:broader sdev:LAB16 ;
  skos:definition "Instruments measuring the mass-to-charge ratio of the products of sample molecule disassociation, atom ionisation and ion acceleration in a particle accelerator."@en ;
  skos:inScheme <http://vocab.nerc.ac.uk/scheme/EDMED_DCAT_THEMES/current> ;
  skos:inScheme <http://vocab.nerc.ac.uk/scheme/SDNDEV/current> ;
  skos:narrower <http://vocab.nerc.ac.uk/collection/W01/current/003> ;
  skos:notation "SDN:L05::LAB17" ;
  skos:note "accepted"@en ;
  skos:prefLabel "accelerator mass spectrometers"@en ;
.
sdev:LAB18
  rdf:type skos:Concept ;
  dcterm:date "2008-01-10 16:10:12.0" ;
  dcterm:identifier "SDN:L05::LAB18" ;
  dcterm:source <http://vocab.nerc.ac.uk/scheme/EDMED_DCAT_THEMES/current> ;
  dcterm:source <http://vocab.nerc.ac.uk/scheme/SDNDEV/current> ;
  pav:authoredOn "2008-01-10 16:10:12.0" ;
  pav:hasCurrentVersion <http://vocab.nerc.ac.uk/collection/L05/current/LAB18/1> ;
  owl:versionInfo "1" ;
  skos:broader sdnc:ICAT03 ;
  skos:definition "Instruments that identify and quantify magnetically active chemical entities by subjecting a sample to orthogonal magnetic and electrical fields."@en ;
  skos:inScheme <http://vocab.nerc.ac.uk/scheme/EDMED_DCAT_THEMES/current> ;
  skos:inScheme <http://vocab.nerc.ac.uk/scheme/SDNDEV/current> ;
  skos:narrower <http://vocab.nerc.ac.uk/collection/W01/current/003> ;
  skos:notation "SDN:L05::LAB18" ;
  skos:note "accepted"@en ;
  skos:prefLabel "nuclear magnetic resonance spectrometers"@en ;
.
sdev:LAB19
  rdf:type skos:Concept ;
  dcterm:date "2008-01-10 16:10:12.0" ;
  dcterm:identifier "SDN:L05::LAB19" ;
  dcterm:source <http://vocab.nerc.ac.uk/scheme/EDMED_DCAT_THEMES/current> ;
  dcterm:source <http://vocab.nerc.ac.uk/scheme/SDNDEV/current> ;
  pav:authoredOn "2008-01-10 16:10:12.0" ;
  pav:hasCurrentVersion <http://vocab.nerc.ac.uk/collection/L05/current/LAB19/1> ;
  owl:versionInfo "1" ;
  skos:broader sdev:LAB16 ;
  skos:definition "Instruments separating gases, volatile substances or substances dissolved in a volatile solvent by transporting an inert gas through a column packed with a sorbent to a detector for assay by a mass spectrometer."@en ;
  skos:inScheme <http://vocab.nerc.ac.uk/scheme/EDMED_DCAT_THEMES/current> ;
  skos:inScheme <http://vocab.nerc.ac.uk/scheme/SDNDEV/current> ;
  skos:narrower <http://vocab.nerc.ac.uk/collection/W01/current/003> ;
  skos:notation "SDN:L05::LAB19" ;
  skos:note "accepted"@en ;
  skos:prefLabel "gas chromatograph mass spectrometers"@en ;
.
sdev:LAB20
  rdf:type skos:Concept ;
  dcterm:date "2011-04-15 14:18:31.0" ;
  dcterm:identifier "SDN:L05::LAB20" ;
  dcterm:source <http://vocab.nerc.ac.uk/scheme/EDMED_DCAT_THEMES/current> ;
  dcterm:source <http://vocab.nerc.ac.uk/scheme/SDNDEV/current> ;
  pav:authoredOn "2011-04-15 14:18:31.0" ;
  pav:hasCurrentVersion <http://vocab.nerc.ac.uk/collection/L05/current/LAB20/2> ;
  pav:hasVersion <http://vocab.nerc.ac.uk/collection/L05/current/LAB20/1> ;
  owl:versionInfo "2" ;
  skos:broader sdnc:ICAT03 ;
  skos:definition "Instruments measuring the relative absorption of electromagnetic radiation of different wavelengths in the near infra-red, visible and ultraviolet wavebands by samples."@en ;
  skos:inScheme <http://vocab.nerc.ac.uk/scheme/EDMED_DCAT_THEMES/current> ;
  skos:inScheme <http://vocab.nerc.ac.uk/scheme/SDNDEV/current> ;
  skos:narrower inst:TOOL1885 ;
  skos:narrower <http://vocab.nerc.ac.uk/collection/W01/current/003> ;
  skos:notation "SDN:L05::LAB20" ;
  skos:note "accepted"@en ;
  skos:prefLabel "spectrophotometers"@en ;
.
sdev:LAB21
  rdf:type skos:Concept ;
  dcterm:date "2018-07-30 16:26:53.0" ;
  dcterm:identifier "SDN:L05::LAB21" ;
  dcterm:source <http://vocab.nerc.ac.uk/scheme/EDMED_DCAT_THEMES/current> ;
  dcterm:source <http://vocab.nerc.ac.uk/scheme/SDNDEV/current> ;
  pav:authoredOn "2018-07-30 16:26:53.0" ;
  pav:hasCurrentVersion <http://vocab.nerc.ac.uk/collection/L05/current/LAB21/2> ;
  pav:hasVersion <http://vocab.nerc.ac.uk/collection/L05/current/LAB21/1> ;
  owl:versionInfo "2" ;
  skos:broader sdnc:ICAT03 ;
  skos:definition "Instruments assaying alpha and beta radiation by quantitative detection of visible light produced by the passage of rays or particles through a suitable scintillant incorporated into the sample."@en ;
  skos:inScheme <http://vocab.nerc.ac.uk/scheme/EDMED_DCAT_THEMES/current> ;
  skos:inScheme <http://vocab.nerc.ac.uk/scheme/SDNDEV/current> ;
  skos:narrower <http://vocab.nerc.ac.uk/collection/W01/current/003> ;
  skos:notation "SDN:L05::LAB21" ;
  skos:note "accepted"@en ;
  skos:prefLabel "liquid scintillation counters"@en ;
.
sdev:LAB22
  rdf:type skos:Concept ;
  dcterm:date "2011-04-15 14:18:31.0" ;
  dcterm:identifier "SDN:L05::LAB22" ;
  dcterm:source <http://vocab.nerc.ac.uk/scheme/EDMED_DCAT_THEMES/current> ;
  dcterm:source <http://vocab.nerc.ac.uk/scheme/SDNDEV/current> ;
  pav:authoredOn "2011-04-15 14:18:31.0" ;
  pav:hasCurrentVersion <http://vocab.nerc.ac.uk/collection/L05/current/LAB22/2> ;
  pav:hasVersion <http://vocab.nerc.ac.uk/collection/L05/current/LAB22/1> ;
  owl:versionInfo "2" ;
  skos:broader sdnc:ICAT03 ;
  skos:definition "Instruments measuring the relative levels of electromagnetic radiation of different wavelengths in the gamma-ray waveband."@en ;
  skos:inScheme <http://vocab.nerc.ac.uk/scheme/EDMED_DCAT_THEMES/current> ;
  skos:inScheme <http://vocab.nerc.ac.uk/scheme/SDNDEV/current> ;
  skos:narrower <http://vocab.nerc.ac.uk/collection/W01/current/003> ;
  skos:notation "SDN:L05::LAB22" ;
  skos:note "accepted"@en ;
  skos:prefLabel "gamma-ray spectrometers"@en ;
.
sdev:LAB23
  rdf:type skos:Concept ;
  dcterm:date "2008-01-10 16:10:12.0" ;
  dcterm:identifier "SDN:L05::LAB23" ;
  dcterm:source <http://vocab.nerc.ac.uk/scheme/EDMED_DCAT_THEMES/current> ;
  dcterm:source <http://vocab.nerc.ac.uk/scheme/NETMAR_OCEAN/current> ;
  dcterm:source <http://vocab.nerc.ac.uk/scheme/NETOC_INSTRUMENT/current> ;
  dcterm:source <http://vocab.nerc.ac.uk/scheme/SDNDEV/current> ;
  pav:authoredOn "2008-01-10 16:10:12.0" ;
  pav:hasCurrentVersion <http://vocab.nerc.ac.uk/collection/L05/current/LAB23/1> ;
  owl:versionInfo "1" ;
  skos:broader sdnc:ICAT03 ;
  skos:definition "Instruments that determinesthe amount of chlorophyll in in-vitro samples by measuring the quantity of red light (around 685nm) emitted following excitation by pulses of blue light (around 460-470nm)."@en ;
  skos:inScheme <http://vocab.nerc.ac.uk/scheme/EDMED_DCAT_THEMES/current> ;
  skos:inScheme <http://vocab.nerc.ac.uk/scheme/NETMAR_OCEAN/current> ;
  skos:inScheme <http://vocab.nerc.ac.uk/scheme/NETOC_INSTRUMENT/current> ;
  skos:inScheme <http://vocab.nerc.ac.uk/scheme/SDNDEV/current> ;
  skos:narrower <http://vocab.nerc.ac.uk/collection/W01/current/003> ;
  skos:notation "SDN:L05::LAB23" ;
  skos:note "accepted"@en ;
  skos:prefLabel "bench fluorometers"@en ;
  skos:related <http://vocab.nerc.ac.uk/collection/P25/current/CHLA> ;
  skos:related <http://vocab.nerc.ac.uk/collection/P25/current/PHAEO> ;
.
sdev:LAB24
  rdf:type skos:Concept ;
  dcterm:date "2008-01-10 16:10:12.0" ;
  dcterm:identifier "SDN:L05::LAB24" ;
  dcterm:source <http://vocab.nerc.ac.uk/scheme/EDMED_DCAT_THEMES/current> ;
  dcterm:source <http://vocab.nerc.ac.uk/scheme/SDNDEV/current> ;
  pav:authoredOn "2008-01-10 16:10:12.0" ;
  pav:hasCurrentVersion <http://vocab.nerc.ac.uk/collection/L05/current/LAB24/1> ;
  owl:versionInfo "1" ;
  skos:broader sdnc:ICAT03 ;
  skos:definition "Instruments that separate components in aqueous or organic solution based on molecular size generally for molecular weight determination."@en ;
  skos:inScheme <http://vocab.nerc.ac.uk/scheme/EDMED_DCAT_THEMES/current> ;
  skos:inScheme <http://vocab.nerc.ac.uk/scheme/SDNDEV/current> ;
  skos:narrower <http://vocab.nerc.ac.uk/collection/W01/current/003> ;
  skos:notation "SDN:L05::LAB24" ;
  skos:note "accepted"@en ;
  skos:prefLabel "gel permeation chromatographs"@en ;
.
sdev:LAB25
  rdf:type skos:Concept ;
  dcterm:date "2008-01-10 16:10:12.0" ;
  dcterm:identifier "SDN:L05::LAB25" ;
  dcterm:source <http://vocab.nerc.ac.uk/scheme/EDMED_DCAT_THEMES/current> ;
  dcterm:source <http://vocab.nerc.ac.uk/scheme/SDNDEV/current> ;
  pav:authoredOn "2008-01-10 16:10:12.0" ;
  pav:hasCurrentVersion <http://vocab.nerc.ac.uk/collection/L05/current/LAB25/1> ;
  owl:versionInfo "1" ;
  skos:broader sdnc:ICAT03 ;
  skos:definition "Instruments that identify and quantify the elemental constituents of a sample from the spectrum of electromagnetic radiation emitted by the atoms in the sample when excited by X-ray radiation."@en ;
  skos:inScheme <http://vocab.nerc.ac.uk/scheme/EDMED_DCAT_THEMES/current> ;
  skos:inScheme <http://vocab.nerc.ac.uk/scheme/SDNDEV/current> ;
  skos:narrower <http://vocab.nerc.ac.uk/collection/W01/current/003> ;
  skos:notation "SDN:L05::LAB25" ;
  skos:note "accepted"@en ;
  skos:prefLabel "X-ray fluorescence analysers"@en ;
.
sdev:LAB26
  rdf:type skos:Concept ;
  dcterm:date "2008-01-10 16:10:12.0" ;
  dcterm:identifier "SDN:L05::LAB26" ;
  dcterm:source <http://vocab.nerc.ac.uk/scheme/EDMED_DCAT_THEMES/current> ;
  dcterm:source <http://vocab.nerc.ac.uk/scheme/SDNDEV/current> ;
  pav:authoredOn "2008-01-10 16:10:12.0" ;
  pav:hasCurrentVersion <http://vocab.nerc.ac.uk/collection/L05/current/LAB26/1> ;
  owl:versionInfo "1" ;
  skos:broader sdnc:ICAT03 ;
  skos:definition "Instruments that identify crystalline solids by measuring the characteristic spaces between layers of atoms or molecules in a crystal."@en ;
  skos:inScheme <http://vocab.nerc.ac.uk/scheme/EDMED_DCAT_THEMES/current> ;
  skos:inScheme <http://vocab.nerc.ac.uk/scheme/SDNDEV/current> ;
  skos:narrower <http://vocab.nerc.ac.uk/collection/W01/current/003> ;
  skos:notation "SDN:L05::LAB26" ;
  skos:note "accepted"@en ;
  skos:prefLabel "X-ray diffractometers"@en ;
.
sdev:LAB27
  rdf:type skos:Concept ;
  dcterm:date "2017-08-08 14:51:13.0" ;
  dcterm:identifier "SDN:L05::LAB27" ;
  dcterm:source <http://vocab.nerc.ac.uk/scheme/EDMED_DCAT_THEMES/current> ;
  dcterm:source <http://vocab.nerc.ac.uk/scheme/SDNDEV/current> ;
  pav:authoredOn "2017-08-08 14:51:13.0" ;
  pav:hasCurrentVersion <http://vocab.nerc.ac.uk/collection/L05/current/LAB27/2> ;
  pav:hasVersion <http://vocab.nerc.ac.uk/collection/L05/current/LAB27/1> ;
  owl:versionInfo "2" ;
  skos:broader sdnc:ICAT03 ;
  skos:definition "Instruments that measure the size spectrum of particles in a water or sediment sample."@en ;
  skos:inScheme <http://vocab.nerc.ac.uk/scheme/EDMED_DCAT_THEMES/current> ;
  skos:inScheme <http://vocab.nerc.ac.uk/scheme/SDNDEV/current> ;
  skos:narrower <http://vocab.nerc.ac.uk/collection/W01/current/003> ;
  skos:notation "SDN:L05::LAB27" ;
  skos:note "accepted"@en ;
  skos:prefLabel "bench particle sizers"@en ;
.
sdev:LAB28
  rdf:type skos:Concept ;
  dcterm:date "2010-02-19 11:52:56.0" ;
  dcterm:identifier "SDN:L05::LAB28" ;
  dcterm:source <http://vocab.nerc.ac.uk/scheme/SDNDEV/current> ;
  pav:authoredOn "2010-02-19 11:52:56.0" ;
  pav:hasCurrentVersion <http://vocab.nerc.ac.uk/collection/L05/current/LAB28/1> ;
  owl:versionInfo "1" ;
  skos:broader sdnc:ICAT03 ;
  skos:definition "Laboratory instruments that determine the thermal conductivity of rock or sediment samples (including unopened cores)."@en ;
  skos:inScheme <http://vocab.nerc.ac.uk/scheme/SDNDEV/current> ;
  skos:narrower <http://vocab.nerc.ac.uk/collection/W01/current/003> ;
  skos:notation "SDN:L05::LAB28" ;
  skos:note "accepted"@en ;
  skos:prefLabel "thermal conductivimeters"@en ;
.
sdev:LAB29
  rdf:type skos:Concept ;
  dcterm:date "2010-04-22 15:04:00.0" ;
  dcterm:identifier "SDN:L05::LAB29" ;
  dcterm:source <http://vocab.nerc.ac.uk/scheme/EDMED_DCAT_THEMES/current> ;
  dcterm:source <http://vocab.nerc.ac.uk/scheme/SDNDEV/current> ;
  pav:authoredOn "2010-04-22 15:04:00.0" ;
  pav:hasCurrentVersion <http://vocab.nerc.ac.uk/collection/L05/current/LAB29/1> ;
  owl:versionInfo "1" ;
  skos:broader sdnc:ICAT03 ;
  skos:definition "Devices that allow one or more physical dimensions of a sample or specimen to be determined by visible comparison against marked graduations in units of measurement of dimension length."@en ;
  skos:inScheme <http://vocab.nerc.ac.uk/scheme/EDMED_DCAT_THEMES/current> ;
  skos:inScheme <http://vocab.nerc.ac.uk/scheme/SDNDEV/current> ;
  skos:narrower <http://vocab.nerc.ac.uk/collection/W01/current/003> ;
  skos:notation "SDN:L05::LAB29" ;
  skos:note "accepted"@en ;
  skos:prefLabel "rulers"@en ;
.
sdev:LAB30
  rdf:type skos:Concept ;
  dcterm:date "2015-02-11 09:18:46.0" ;
  dcterm:identifier "SDN:L05::LAB30" ;
  dcterm:source <http://vocab.nerc.ac.uk/scheme/EDMED_DCAT_THEMES/current> ;
  dcterm:source <http://vocab.nerc.ac.uk/scheme/NETMAR_OCEAN/current> ;
  dcterm:source <http://vocab.nerc.ac.uk/scheme/NETOC_INSTRUMENT/current> ;
  dcterm:source <http://vocab.nerc.ac.uk/scheme/SDNDEV/current> ;
  pav:authoredOn "2015-02-11 09:18:46.0" ;
  pav:hasCurrentVersion <http://vocab.nerc.ac.uk/collection/L05/current/LAB30/2> ;
  pav:hasVersion <http://vocab.nerc.ac.uk/collection/L05/current/LAB30/1> ;
  owl:sameAs <https://www.nodc.noaa.gov/cgi-bin/OAS/prd/insttype/details/75> ;
  owl:versionInfo "2" ;
  skos:broader sdnc:ICAT03 ;
  skos:definition "Instruments that measure the salinity of a collected water sample based on its electrical conductivity or optical properties."@en ;
  skos:inScheme <http://vocab.nerc.ac.uk/scheme/EDMED_DCAT_THEMES/current> ;
  skos:inScheme <http://vocab.nerc.ac.uk/scheme/NETMAR_OCEAN/current> ;
  skos:inScheme <http://vocab.nerc.ac.uk/scheme/NETOC_INSTRUMENT/current> ;
  skos:inScheme <http://vocab.nerc.ac.uk/scheme/SDNDEV/current> ;
  skos:narrower <http://vocab.nerc.ac.uk/collection/W01/current/003> ;
  skos:notation "SDN:L05::LAB30" ;
  skos:note "accepted"@en ;
  skos:prefLabel "salinometers"@en ;
  skos:related <http://vocab.nerc.ac.uk/collection/P25/current/ICESSALIN> ;
  skos:related <http://vocab.nerc.ac.uk/collection/P25/current/SALIN> ;
.
sdev:LAB31
  rdf:type skos:Concept ;
  dcterm:date "2013-02-26 17:11:07.0" ;
  dcterm:identifier "SDN:L05::LAB31" ;
  dcterm:source <http://vocab.nerc.ac.uk/scheme/SDNDEV/current> ;
  pav:authoredOn "2013-02-26 17:11:07.0" ;
  pav:hasCurrentVersion <http://vocab.nerc.ac.uk/collection/L05/current/LAB31/2> ;
  pav:hasVersion <http://vocab.nerc.ac.uk/collection/L05/current/LAB31/1> ;
  owl:versionInfo "2" ;
  skos:broader sdnc:ICAT03 ;
  skos:definition "Sensors, probes and meters that measure the degree to which a sample or part thereof is influenced by a magnetic field."@en ;
  skos:inScheme <http://vocab.nerc.ac.uk/scheme/SDNDEV/current> ;
  skos:narrower <http://vocab.nerc.ac.uk/collection/W01/current/003> ;
  skos:notation "SDN:L05::LAB31" ;
  skos:note "accepted"@en ;
  skos:prefLabel "magnetic susceptibility systems"@en ;
.
sdev:LAB32
  rdf:type skos:Concept ;
  dcterm:date "2013-02-26 17:11:07.0" ;
  dcterm:identifier "SDN:L05::LAB32" ;
  dcterm:source <http://vocab.nerc.ac.uk/scheme/EDMED_DCAT_THEMES/current> ;
  dcterm:source <http://vocab.nerc.ac.uk/scheme/SDNDEV/current> ;
  pav:authoredOn "2013-02-26 17:11:07.0" ;
  pav:hasCurrentVersion <http://vocab.nerc.ac.uk/collection/L05/current/LAB32/2> ;
  pav:hasVersion <http://vocab.nerc.ac.uk/collection/L05/current/LAB32/1> ;
  owl:versionInfo "2" ;
  skos:broader sdnc:ICAT03 ;
  skos:definition "Instruments that measure the speed or velocity of sound, including P-waves, in samples of solids, liquids or gases."@en ;
  skos:inScheme <http://vocab.nerc.ac.uk/scheme/EDMED_DCAT_THEMES/current> ;
  skos:inScheme <http://vocab.nerc.ac.uk/scheme/SDNDEV/current> ;
  skos:narrower <http://vocab.nerc.ac.uk/collection/W01/current/003> ;
  skos:notation "SDN:L05::LAB32" ;
  skos:note "accepted"@en ;
  skos:prefLabel "acoustic velocity systems"@en ;
.
sdev:LAB33
  rdf:type skos:Concept ;
  dcterm:date "2012-03-01 16:00:54.0" ;
  dcterm:identifier "SDN:L05::LAB33" ;
  dcterm:source <http://vocab.nerc.ac.uk/scheme/EDMED_DCAT_THEMES/current> ;
  dcterm:source <http://vocab.nerc.ac.uk/scheme/SDNDEV/current> ;
  pav:authoredOn "2012-03-01 16:00:54.0" ;
  pav:hasCurrentVersion <http://vocab.nerc.ac.uk/collection/L05/current/LAB33/1> ;
  owl:versionInfo "1" ;
  skos:broader sdnc:ICAT03 ;
  skos:definition "Laboratory apparatus  that automatically introduces one or more samples with a predetermined volume or mass into an analytical instrument."@en ;
  skos:inScheme <http://vocab.nerc.ac.uk/scheme/EDMED_DCAT_THEMES/current> ;
  skos:inScheme <http://vocab.nerc.ac.uk/scheme/SDNDEV/current> ;
  skos:narrower <http://vocab.nerc.ac.uk/collection/W01/current/003> ;
  skos:notation "SDN:L05::LAB33" ;
  skos:note "accepted"@en ;
  skos:prefLabel "laboratory autosamplers"@en ;
.
sdev:LAB34
  rdf:type skos:Concept ;
  dcterm:date "2012-03-22 17:49:10.0" ;
  dcterm:identifier "SDN:L05::LAB34" ;
  dcterm:source <http://vocab.nerc.ac.uk/scheme/SDNDEV/current> ;
  pav:authoredOn "2012-03-22 17:49:10.0" ;
  pav:hasCurrentVersion <http://vocab.nerc.ac.uk/collection/L05/current/LAB34/1> ;
  owl:versionInfo "1" ;
  skos:broader sdnc:ICAT03 ;
  skos:definition "Laboratory apparatus that detemines the concentration of a chemical species by quantification of the electromagnetic radiation (usually visible light) produced by a chemical reaction."@en ;
  skos:inScheme <http://vocab.nerc.ac.uk/scheme/SDNDEV/current> ;
  skos:narrower <http://vocab.nerc.ac.uk/collection/W01/current/003> ;
  skos:notation "SDN:L05::LAB34" ;
  skos:note "accepted"@en ;
  skos:prefLabel "chemiluminescence analysers"@en ;
.
sdev:LAB35
  rdf:type skos:Concept ;
  dcterm:date "2012-08-02 14:41:42.0" ;
  dcterm:identifier "SDN:L05::LAB35" ;
  dcterm:source <http://vocab.nerc.ac.uk/scheme/SDNDEV/current> ;
  pav:authoredOn "2012-08-02 14:41:42.0" ;
  pav:hasCurrentVersion <http://vocab.nerc.ac.uk/collection/L05/current/LAB35/1> ;
  owl:versionInfo "1" ;
  skos:broader sdnc:ICAT03 ;
  skos:definition "Instruments that obtain information about an analyte by applying a potential and measuring the current produced in the analyte."@en ;
  skos:inScheme <http://vocab.nerc.ac.uk/scheme/SDNDEV/current> ;
  skos:narrower <http://vocab.nerc.ac.uk/collection/W01/current/003> ;
  skos:notation "SDN:L05::LAB35" ;
  skos:note "accepted"@en ;
  skos:prefLabel "voltammetry analysers"@en ;
.
sdev:LAB36
  rdf:type skos:Concept ;
  dcterm:date "2012-08-02 14:44:24.0" ;
  dcterm:identifier "SDN:L05::LAB36" ;
  dcterm:source <http://vocab.nerc.ac.uk/scheme/SDNDEV/current> ;
  pav:authoredOn "2012-08-02 14:44:24.0" ;
  pav:hasCurrentVersion <http://vocab.nerc.ac.uk/collection/L05/current/LAB36/1> ;
  owl:versionInfo "1" ;
  skos:broader sdnc:ICAT03 ;
  skos:definition "Instruments that inject a sample into a flowing carrier solution, adding reagents whilst controlling the environment to produce a chemical reaction before passing the sample to a detector."@en ;
  skos:inScheme <http://vocab.nerc.ac.uk/scheme/SDNDEV/current> ;
  skos:narrower <http://vocab.nerc.ac.uk/collection/W01/current/003> ;
  skos:notation "SDN:L05::LAB36" ;
  skos:note "accepted"@en ;
  skos:prefLabel "flow injection analysers"@en ;
.
sdev:LAB37
  rdf:type skos:Concept ;
  dcterm:date "2012-08-02 14:45:33.0" ;
  dcterm:identifier "SDN:L05::LAB37" ;
  dcterm:source <http://vocab.nerc.ac.uk/scheme/EDMED_DCAT_THEMES/current> ;
  dcterm:source <http://vocab.nerc.ac.uk/scheme/SDNDEV/current> ;
  pav:authoredOn "2012-08-02 14:45:33.0" ;
  pav:hasCurrentVersion <http://vocab.nerc.ac.uk/collection/L05/current/LAB37/1> ;
  owl:versionInfo "1" ;
  skos:broader sdnc:ICAT03 ;
  skos:definition "Instruments that suspend cells in a stream of fluid past detection sensors whilst illuminating them with laser light. Used for cell counting, sorting, biomarker detection and protein engineering."@en ;
  skos:inScheme <http://vocab.nerc.ac.uk/scheme/EDMED_DCAT_THEMES/current> ;
  skos:inScheme <http://vocab.nerc.ac.uk/scheme/SDNDEV/current> ;
  skos:narrower <http://vocab.nerc.ac.uk/collection/W01/current/003> ;
  skos:notation "SDN:L05::LAB37" ;
  skos:note "accepted"@en ;
  skos:prefLabel "flow cytometers"@en ;
.
sdev:LAB38
  rdf:type skos:Concept ;
  dcterm:date "2014-12-16 08:36:22.0" ;
  dcterm:identifier "SDN:L05::LAB38" ;
  dcterm:source <http://vocab.nerc.ac.uk/scheme/SDNDEV/current> ;
  pav:authoredOn "2014-12-16 08:36:22.0" ;
  pav:hasCurrentVersion <http://vocab.nerc.ac.uk/collection/L05/current/LAB38/2> ;
  pav:hasVersion <http://vocab.nerc.ac.uk/collection/L05/current/LAB38/1> ;
  owl:versionInfo "2" ;
  skos:altLabel "CEAS"@en ;
  skos:broader sdnc:ICAT03 ;
  skos:definition "Instruments that illuminate a sample inside an optical cavity, typically using laser light, and measure the concentration or amount of a species in gas phase by absorption spectroscopy. Techniques include cavity ring-down spectroscopy (CRDS) and integrated cavity output spectroscopy (ICOS)."@en ;
  skos:inScheme <http://vocab.nerc.ac.uk/scheme/SDNDEV/current> ;
  skos:narrower <http://vocab.nerc.ac.uk/collection/W01/current/003> ;
  skos:notation "SDN:L05::LAB38" ;
  skos:note "accepted"@en ;
  skos:prefLabel "cavity enhanced absorption spectrometers"@en ;
.
sdev:LAB39
  rdf:type skos:Concept ;
  dcterm:date "2012-08-30 14:13:49.0" ;
  dcterm:identifier "SDN:L05::LAB39" ;
  dcterm:source <http://vocab.nerc.ac.uk/scheme/SDNDEV/current> ;
  pav:authoredOn "2012-08-30 14:13:49.0" ;
  pav:hasCurrentVersion <http://vocab.nerc.ac.uk/collection/L05/current/LAB39/1> ;
  owl:versionInfo "1" ;
  skos:broader sdnc:ICAT03 ;
  skos:definition "Instruments that measure the amount of alpha, beta or gamma radiation through quantification of the ionization of a low-pressure gas contained in a tube. Sometimes referred to as Geiger-Mller counters."@en ;
  skos:inScheme <http://vocab.nerc.ac.uk/scheme/SDNDEV/current> ;
  skos:narrower <http://vocab.nerc.ac.uk/collection/W01/current/003> ;
  skos:notation "SDN:L05::LAB39" ;
  skos:note "accepted"@en ;
  skos:prefLabel "Geiger counters"@en ;
.
sdev:LAB40
  rdf:type skos:Concept ;
  dcterm:date "2012-11-29 15:53:17.0" ;
  dcterm:identifier "SDN:L05::LAB40" ;
  dcterm:source <http://vocab.nerc.ac.uk/scheme/EDMED_DCAT_THEMES/current> ;
  dcterm:source <http://vocab.nerc.ac.uk/scheme/SDNDEV/current> ;
  pav:authoredOn "2012-11-29 15:53:17.0" ;
  pav:hasCurrentVersion <http://vocab.nerc.ac.uk/collection/L05/current/LAB40/1> ;
  owl:versionInfo "1" ;
  skos:broader sdnc:ICAT03 ;
  skos:definition "Pieces of apparatus that determine the volume of a liquid sample or dispense measured volumes of liquid. Includes devices covering a wide range of sophistication from measuring cylinders, syringes and manual pipettes through to programmable electronic instruments."@en ;
  skos:editorialNote "actual instruments are all intended for dispensing carefully measured volumes as in titration, thus it seems that this is a workflow component [SMR 2023-03-09]" ;
  skos:inScheme <http://vocab.nerc.ac.uk/scheme/EDMED_DCAT_THEMES/current> ;
  skos:inScheme <http://vocab.nerc.ac.uk/scheme/SDNDEV/current> ;
  skos:narrower <http://vocab.nerc.ac.uk/collection/W01/current/003> ;
  skos:notation "SDN:L05::LAB40" ;
  skos:note "accepted"@en ;
  skos:prefLabel "Volume measures"@en ;
.
sdev:LAB42
  rdf:type skos:Concept ;
  dcterm:date "2013-12-19 09:08:24.0" ;
  dcterm:identifier "SDN:L05::LAB42" ;
  dcterm:source <http://vocab.nerc.ac.uk/scheme/SDNDEV/current> ;
  pav:authoredOn "2013-12-19 09:08:24.0" ;
  pav:hasCurrentVersion <http://vocab.nerc.ac.uk/collection/L05/current/LAB42/1> ;
  owl:versionInfo "1" ;
  skos:broader sdnc:ICAT03 ;
  skos:definition "Devices used to detect the distance between sensor and sample or presence/absence of an object based a light (often infrared and possibly laser) transmitter and a photoelectric receiver."@en ;
  skos:inScheme <http://vocab.nerc.ac.uk/scheme/SDNDEV/current> ;
  skos:narrower <http://vocab.nerc.ac.uk/collection/W01/current/003> ;
  skos:notation "SDN:L05::LAB42" ;
  skos:note "accepted"@en ;
  skos:prefLabel "laboratory optical rangefinders"@en ;
.
sdev:LAB43
  rdf:type skos:Concept ;
  dcterm:date "2015-02-03 10:32:36.0" ;
  dcterm:identifier "SDN:L05::LAB43" ;
  dcterm:source <http://vocab.nerc.ac.uk/scheme/SDNDEV/current> ;
  pav:authoredOn "2015-02-03 10:32:36.0" ;
  pav:hasCurrentVersion <http://vocab.nerc.ac.uk/collection/L05/current/LAB43/1> ;
  owl:versionInfo "1" ;
  skos:broader sdnc:ICAT03 ;
  skos:definition "Laboratory instruments detect biological, chemical or physical events in samples held in multiple (typically 6, 24, 96, 384 or 1536) wells arranged in a matrix in a flat plate. Samples in the plate wells are simultaneously assayed optically using techniques such as spectrophotometry or spectrofluorometry."@en ;
  skos:inScheme <http://vocab.nerc.ac.uk/scheme/SDNDEV/current> ;
  skos:notation "SDN:L05::LAB43" ;
  skos:note "accepted"@en ;
  skos:prefLabel "plate readers"@en ;
.
sdev:LAB44
  rdf:type skos:Concept ;
  dcterm:date "2015-02-11 09:21:48.0" ;
  dcterm:identifier "SDN:L05::LAB44" ;
  dcterm:source <http://vocab.nerc.ac.uk/scheme/SDNDEV/current> ;
  pav:authoredOn "2015-02-11 09:21:48.0" ;
  pav:hasCurrentVersion <http://vocab.nerc.ac.uk/collection/L05/current/LAB44/1> ;
  owl:versionInfo "1" ;
  skos:broader sdnc:ICAT03 ;
  skos:definition "Instruments that measure the refractive index of a sample."@en ;
  skos:inScheme <http://vocab.nerc.ac.uk/scheme/SDNDEV/current> ;
  skos:notation "SDN:L05::LAB44" ;
  skos:note "accepted"@en ;
  skos:prefLabel "refractometers"@en ;
.
sdev:LAB45
  rdf:type skos:Concept ;
  dcterm:date "2022-04-27 16:58:27.0" ;
  dcterm:identifier "SDN:L05::LAB45" ;
  dcterm:source <http://vocab.nerc.ac.uk/scheme/SDNDEV/current> ;
  pav:authoredOn "2022-04-27 16:58:27.0" ;
  pav:hasCurrentVersion <http://vocab.nerc.ac.uk/collection/L05/current/LAB45/2> ;
  pav:hasVersion <http://vocab.nerc.ac.uk/collection/L05/current/LAB45/1> ;
  owl:versionInfo "2" ;
  skos:broader sdnc:ICAT03 ;
  skos:definition "Instruments that use ion chromatography to separate ions and polar molecules based on their affinity to an ion exchanger resin. Sample solutions pass through a pressurized chromatographic column where ions are absorbed by the resin and subsequently eluted using an ion extraction liquid. The retention time of different species determines the ionic concentrations in the sample."@en ;
  skos:inScheme <http://vocab.nerc.ac.uk/scheme/SDNDEV/current> ;
  skos:notation "SDN:L05::LAB45" ;
  skos:note "accepted"@en ;
  skos:prefLabel "ion chromatography analysers"@en ;
.
sdev:LAB46
  rdf:type skos:Concept ;
  dcterm:date "2022-04-27 16:58:27.0" ;
  dcterm:identifier "SDN:L05::LAB46" ;
  dcterm:source <http://vocab.nerc.ac.uk/scheme/SDNDEV/current> ;
  pav:authoredOn "2022-04-27 16:58:27.0" ;
  pav:hasCurrentVersion <http://vocab.nerc.ac.uk/collection/L05/current/LAB46/2> ;
  pav:hasVersion <http://vocab.nerc.ac.uk/collection/L05/current/LAB46/1> ;
  owl:versionInfo "2" ;
  skos:broader sdev:LAB16 ;
  skos:definition "Instruments that ionise trace gas molecules by proton transfer from protonated water, H3O. Ions of specific mass-to-charge ratios are then quantified in a quadrupole or time-of-flight mass spectrometer."@en ;
  skos:inScheme <http://vocab.nerc.ac.uk/scheme/SDNDEV/current> ;
  skos:notation "SDN:L05::LAB46" ;
  skos:note "accepted"@en ;
  skos:prefLabel "proton transfer reaction mass spectrometers"@en ;
.
sdev:LAB47
  rdf:type skos:Concept ;
  dcterm:date "2022-04-27 16:58:27.0" ;
  dcterm:identifier "SDN:L05::LAB47" ;
  dcterm:source <http://vocab.nerc.ac.uk/scheme/SDNDEV/current> ;
  pav:authoredOn "2022-04-27 16:58:27.0" ;
  pav:hasCurrentVersion <http://vocab.nerc.ac.uk/collection/L05/current/LAB47/2> ;
  pav:hasVersion <http://vocab.nerc.ac.uk/collection/L05/current/LAB47/1> ;
  owl:versionInfo "2" ;
  skos:altLabel "TIMS"@en ;
  skos:broader sdev:LAB16 ;
  skos:definition "Instruments that measure isotopic ratios using thermal ionisation. Purified samples are heated to cause ionisation of atoms. Subsequently, ions are focused into a beam by an electromagnet and then separated into individual beams based on their mass/charge ratio."@en ;
  skos:inScheme <http://vocab.nerc.ac.uk/scheme/SDNDEV/current> ;
  skos:notation "SDN:L05::LAB47" ;
  skos:note "accepted"@en ;
  skos:prefLabel "thermal ionisation mass spectrometers"@en ;
.
sdev:LAB48
  rdf:type skos:Concept ;
  dcterm:date "2016-03-10 06:47:31.0" ;
  dcterm:identifier "SDN:L05::LAB48" ;
  dcterm:source <http://vocab.nerc.ac.uk/scheme/SDNDEV/current> ;
  pav:authoredOn "2016-03-10 06:47:31.0" ;
  pav:hasCurrentVersion <http://vocab.nerc.ac.uk/collection/L05/current/LAB48/1> ;
  owl:versionInfo "1" ;
  skos:altLabel "IRMS"@en ;
  skos:broader sdev:LAB16 ;
  skos:definition "Instruments that measure isotopic ratios using an electron ionisation source. Atoms in purified samples are ionised using a beam of electrons under vacuum. Subsequently, ions are focused into a beam by an electromagnet and then separated into individual beams based on their mass/charge ratio."@en ;
  skos:inScheme <http://vocab.nerc.ac.uk/scheme/SDNDEV/current> ;
  skos:notation "SDN:L05::LAB48" ;
  skos:note "accepted"@en ;
  skos:prefLabel "isotope ratio mass spectrometers"@en ;
.
sdev:LAB49
  rdf:type skos:Concept ;
  dcterm:date "2016-11-29 15:10:58.0" ;
  dcterm:identifier "SDN:L05::LAB49" ;
  dcterm:source <http://vocab.nerc.ac.uk/scheme/SDNDEV/current> ;
  pav:authoredOn "2016-11-29 15:10:58.0" ;
  pav:hasCurrentVersion <http://vocab.nerc.ac.uk/collection/L05/current/LAB49/1> ;
  owl:versionInfo "1" ;
  skos:altLabel "AFS"@en ;
  skos:broader sdnc:ICAT03 ;
  skos:definition "Instruments that illuminate the vapour from volatilised samples with light and quantify the intensity of light emitted, which is usually proportional to concentration."@en ;
  skos:inScheme <http://vocab.nerc.ac.uk/scheme/SDNDEV/current> ;
  skos:notation "SDN:L05::LAB49" ;
  skos:note "accepted"@en ;
  skos:prefLabel "Atomic fluorescence spectrometers"@en ;
.
sdev:LAB51
  rdf:type skos:Concept ;
  dcterm:date "2021-01-25 10:23:18.0" ;
  dcterm:identifier "SDN:L05::LAB51" ;
  dcterm:source <http://vocab.nerc.ac.uk/scheme/SDNDEV/current> ;
  pav:authoredOn "2021-01-25 10:23:18.0" ;
  pav:hasCurrentVersion <http://vocab.nerc.ac.uk/collection/L05/current/LAB51/1> ;
  owl:versionInfo "1" ;
  skos:broader sdnc:ICAT03 ;
  skos:definition "Instruments that generate enlarged images of samples using the phenomena of digital inline holography with numerical reconstruction instead of reflection and absorption of visible light."@en ;
  skos:inScheme <http://vocab.nerc.ac.uk/scheme/SDNDEV/current> ;
  skos:notation "SDN:L05::LAB51" ;
  skos:note "accepted"@en ;
  skos:prefLabel "holographic microscopes"@en ;
.
sdev:LVLST
  rdf:type skos:Concept ;
  dcterm:date "2017-09-06 11:47:02.0" ;
  dcterm:identifier "SDN:L05::LVLST" ;
  dcterm:source <http://vocab.nerc.ac.uk/scheme/SDNDEV/current> ;
  pav:authoredOn "2017-09-06 11:47:02.0" ;
  pav:hasCurrentVersion <http://vocab.nerc.ac.uk/collection/L05/current/LVLST/1> ;
  owl:versionInfo "1" ;
  skos:broader sdnc:ICAT04 ;
  skos:definition "Optical instruments and graduated poles used in surveying to determine the elevation of a location relative to a datum level."@en ;
  skos:inScheme <http://vocab.nerc.ac.uk/scheme/SDNDEV/current> ;
  skos:notation "SDN:L05::LVLST" ;
  skos:note "accepted"@en ;
  skos:prefLabel "Levels and staffs"@en ;
.
sdev:MMIS
  rdf:type skos:Concept ;
  dcterm:date "2013-02-18 08:17:53.0" ;
  dcterm:identifier "SDN:L05::MMIS" ;
  dcterm:source <http://vocab.nerc.ac.uk/scheme/EDMED_DCAT_THEMES/current> ;
  dcterm:source <http://vocab.nerc.ac.uk/scheme/SDNDEV/current> ;
  pav:authoredOn "2013-02-18 08:17:53.0" ;
  pav:hasCurrentVersion <http://vocab.nerc.ac.uk/collection/L05/current/MMIS/1> ;
  owl:versionInfo "1" ;
  skos:broader sdnc:ICAT04 ;
  skos:definition "High-frequency (>1 MHz), possibly multiple frequency, active sonar systems that provide images approaching the same quality as optical video cameras. They may be deployed in many ways including hand-held by divers, attached to profiling instruments, AUVs and ROVs, towed fish or moorings.  They have many scientific, commercial and military applications including observation and identification of fish, seabed characterisation, underwater vessel inspections and mine detection. Examples of this type of system are DIDSON (Dual-frequency IDentification SONar) and LIMIS (Limpet Mine Imaging Sonar).  Any instrument that may be considered the underwater acoustic equivalent of an optical video camera belongs in this category."@en ;
  skos:inScheme <http://vocab.nerc.ac.uk/scheme/EDMED_DCAT_THEMES/current> ;
  skos:inScheme <http://vocab.nerc.ac.uk/scheme/SDNDEV/current> ;
  skos:narrower <http://vocab.nerc.ac.uk/collection/W01/current/003> ;
  skos:notation "SDN:L05::MMIS" ;
  skos:note "accepted"@en ;
  skos:prefLabel "multi-frame imaging sonar"@en ;
.
sdev:MPIS
  rdf:type skos:Concept ;
  dcterm:date "2021-06-15 11:00:36.0" ;
  dcterm:identifier "SDN:L05::MPIS" ;
  dcterm:source <http://vocab.nerc.ac.uk/scheme/SDNDEV/current> ;
  pav:authoredOn "2021-06-15 11:00:36.0" ;
  pav:hasCurrentVersion <http://vocab.nerc.ac.uk/collection/L05/current/MPIS/1> ;
  owl:versionInfo "1" ;
  skos:broader sdnc:ICAT04 ;
  skos:definition "Active sonar systems that provide a cross-sectional profile of a target area. These instruments typically emit a series of acoustic pulses in a beam pattern like a spot or pencil beam and the peak echo return is recorded. They provide a digitised version of echo returns as opposed to multicoloured images by imaging sonars. They are generally deployed on survey vessels pointing the transducer down towards the target. Applications of profiling sonars include cross-sectional profiling in pipeline and trench survey, bottom profiles, and surveying of underwater cave systems or manmade structures like road and rail bridge foundations. Examples of this type of system are Tritech Super SeaKing DFP Profiler and Imagenex 881A Profiling Sonar Head."@en ;
  skos:inScheme <http://vocab.nerc.ac.uk/scheme/SDNDEV/current> ;
  skos:notation "SDN:L05::MPIS" ;
  skos:note "accepted"@en ;
  skos:prefLabel "profiling sonars"@en ;
.
sdev:PERMON
  rdf:type skos:Concept ;
  dcterm:date "2014-07-22 09:29:48.0" ;
  dcterm:identifier "SDN:L05::PERMON" ;
  dcterm:source <http://vocab.nerc.ac.uk/scheme/SDNDEV/current> ;
  pav:authoredOn "2014-07-22 09:29:48.0" ;
  pav:hasCurrentVersion <http://vocab.nerc.ac.uk/collection/L05/current/PERMON/1> ;
  owl:versionInfo "1" ;
  skos:broader sdnc:ICAT04 ;
  skos:definition "Sensors or instruments that monitor whether a platform or environmental sensors on the platform are functioning."@en ;
  skos:inScheme <http://vocab.nerc.ac.uk/scheme/SDNDEV/current> ;
  skos:narrower <http://vocab.nerc.ac.uk/collection/W01/current/003> ;
  skos:notation "SDN:L05::PERMON" ;
  skos:note "accepted"@en ;
  skos:prefLabel "Performance monitors"@en ;
  skos:scopeNote "subclasses: strain gauge" ;
.
sdev:TRTG
  rdf:type skos:Concept ;
  dcterm:date "2015-08-04 12:15:32.0" ;
  dcterm:identifier "SDN:L05::TRTG" ;
  dcterm:source <http://vocab.nerc.ac.uk/scheme/EDMED_DCAT_THEMES/current> ;
  dcterm:source <http://vocab.nerc.ac.uk/scheme/SDNDEV/current> ;
  pav:authoredOn "2015-08-04 12:15:32.0" ;
  pav:hasCurrentVersion <http://vocab.nerc.ac.uk/collection/L05/current/TRTG/2> ;
  pav:hasVersion <http://vocab.nerc.ac.uk/collection/L05/current/TRTG/1> ;
  owl:versionInfo "2" ;
  skos:broader sdnc:ICAT04 ;
  skos:definition "Devices attached to living organisms with the purpose of determining the location of those organisms as a function of time after tagging and release."@en ;
  skos:inScheme <http://vocab.nerc.ac.uk/scheme/EDMED_DCAT_THEMES/current> ;
  skos:inScheme <http://vocab.nerc.ac.uk/scheme/SDNDEV/current> ;
  skos:narrower <http://vocab.nerc.ac.uk/collection/W01/current/003> ;
  skos:notation "SDN:L05::TRTG" ;
  skos:note "accepted"@en ;
  skos:prefLabel "tracking tags"@en ;
.
sdev:WDRG
  rdf:type skos:Concept ;
  dcterm:date "2017-09-06 11:48:32.0" ;
  dcterm:identifier "SDN:L05::WDRG" ;
  dcterm:source <http://vocab.nerc.ac.uk/scheme/SDNDEV/current> ;
  pav:authoredOn "2017-09-06 11:48:32.0" ;
  pav:hasCurrentVersion <http://vocab.nerc.ac.uk/collection/L05/current/WDRG/1> ;
  owl:versionInfo "1" ;
  skos:broader sdnc:ICAT04 ;
  skos:definition "Wires, usually several thousand feet in length, maintained horizontally at any desired depth by means of attached weights, buoyed at intervals, towed by a power boat at each end, and used to locate submerged obstructions projecting above the depth at which it is set."@en ;
  skos:inScheme <http://vocab.nerc.ac.uk/scheme/SDNDEV/current> ;
  skos:notation "SDN:L05::WDRG" ;
  skos:note "accepted"@en ;
  skos:prefLabel "Wire drags"@en ;
.
sdev:WPS
  rdf:type skos:Concept ;
  dcterm:date "2015-02-11 09:24:01.0" ;
  dcterm:identifier "SDN:L05::WPS" ;
  dcterm:source <http://vocab.nerc.ac.uk/scheme/EDMED_DCAT_THEMES/current> ;
  dcterm:source <http://vocab.nerc.ac.uk/scheme/SDNDEV/current> ;
  pav:authoredOn "2015-02-11 09:24:01.0" ;
  pav:hasCurrentVersion <http://vocab.nerc.ac.uk/collection/L05/current/WPS/1> ;
  owl:versionInfo "1" ;
  skos:broader sdnc:ICAT04 ;
  skos:definition "Sensors measuring hydrostatic pressure that are capable of withstanding the physical demands made by in-situ measurements in water bodies. Depending upon the mode of deployment they may measure sea level, waves, mooring performance or the depth of a profiling instrument."@en ;
  skos:inScheme <http://vocab.nerc.ac.uk/scheme/EDMED_DCAT_THEMES/current> ;
  skos:inScheme <http://vocab.nerc.ac.uk/scheme/SDNDEV/current> ;
  skos:notation "SDN:L05::WPS" ;
  skos:note "accepted"@en ;
  skos:prefLabel "water pressure sensors"@en ;
.
sdnk:SDNKG01
  rdf:type skos:Concept ;
  dcterm:date "2015-03-12 10:48:49.0" ;
  dcterm:identifier "SDN:L19::SDNKG01" ;
  dcterm:source "<http://vocab.nerc.ac.uk/scheme/NETOC_INSTRUMENT/current/>" ;
  pav:hasCurrentVersion <http://vocab.nerc.ac.uk/collection/L19/current/SDNKG01/3> ;
  owl:versionInfo "3" ;
  skos:altLabel "instrument"@en ;
  skos:definition "Keyword describes or categorises sample collection or data production tools"@en ;
  skos:inScheme <http://w3id.org/ogeochem/def/instrument/measurement/conceptscheme> ;
  skos:notation "SDN:L19::SDNKG01" ;
  skos:note "accepted"@en ;
  skos:prefLabel "NERC measurement instrument"@en ;
  skos:topConceptOf <http://w3id.org/ogeochem/def/instrument/measurement/conceptscheme> ;
.
sdnk:SDNKG17
  rdf:type skos:Collection ;
  dcterm:date "2021-07-07 10:53:52.0" ;
  dcterm:identifier "SDN:L19::SDNKG17" ;
  pav:authoredOn "2021-07-07 10:53:52.0" ;
  pav:hasCurrentVersion <http://vocab.nerc.ac.uk/collection/L19/current/SDNKG17/1> ;
  pav:version "1" ;
  owl:versionInfo "1" ;
  skos:altLabel "sensor_model"@en ;
  skos:definition "Keyword identifies a sensor model"@en ;
  skos:member inst:NETT0001 ;
  skos:member inst:NETT0002 ;
  skos:member inst:NETT0003 ;
  skos:member inst:NETT0005 ;
  skos:member inst:NETT0006 ;
  skos:member inst:NETT0009 ;
  skos:member inst:NETT0010 ;
  skos:member inst:NETT0012 ;
  skos:member inst:NETT0016 ;
  skos:member inst:NETT0019 ;
  skos:member inst:NETT0020 ;
  skos:member inst:NETT0022 ;
  skos:member inst:NETT0023 ;
  skos:member inst:NETT0024 ;
  skos:member inst:NETT0026 ;
  skos:member inst:NETT0027 ;
  skos:member inst:NETT0030 ;
  skos:member inst:NETT0031 ;
  skos:member inst:NETT0032 ;
  skos:member inst:NETT0034 ;
  skos:member inst:NETT0035 ;
  skos:member inst:NETT0036 ;
  skos:member inst:NETT0039 ;
  skos:member inst:NETT0040 ;
  skos:member inst:NETT0041 ;
  skos:member inst:NETT0042 ;
  skos:member inst:NETT0043 ;
  skos:member inst:NETT0044 ;
  skos:member inst:NETT0045 ;
  skos:member inst:NETT0047 ;
  skos:member inst:NETT0052 ;
  skos:member inst:NETT0053 ;
  skos:member inst:NETT0054 ;
  skos:member inst:NETT0055 ;
  skos:member inst:NETT0056 ;
  skos:member inst:NETT0057 ;
  skos:member inst:NETT0058 ;
  skos:member inst:NETT0059 ;
  skos:member inst:NETT0060 ;
  skos:member inst:NETT0061 ;
  skos:member inst:NETT0062 ;
  skos:member inst:NETT0063 ;
  skos:member inst:NETT0065 ;
  skos:member inst:NETT0066 ;
  skos:member inst:NETT0067 ;
  skos:member inst:NETT0068 ;
  skos:member inst:NETT0071 ;
  skos:member inst:NETT0072 ;
  skos:member inst:NETT0073 ;
  skos:member inst:NETT0074 ;
  skos:member inst:NETT0075 ;
  skos:member inst:NETT0077 ;
  skos:member inst:NETT0078 ;
  skos:member inst:NETT0079 ;
  skos:member inst:NETT0080 ;
  skos:member inst:NETT0090 ;
  skos:member inst:NETT0091 ;
  skos:member inst:NETT0092 ;
  skos:member inst:NETT0095 ;
  skos:member inst:NETT0096 ;
  skos:member inst:NETT0098 ;
  skos:member inst:NETT0100 ;
  skos:member inst:NETT0102 ;
  skos:member inst:NETT0103 ;
  skos:member inst:NETT0104 ;
  skos:member inst:NETT0105 ;
  skos:member inst:NETT0106 ;
  skos:member inst:NETT0108 ;
  skos:member inst:NETT0109 ;
  skos:member inst:NETT0111 ;
  skos:member inst:NETT0112 ;
  skos:member inst:NETT0113 ;
  skos:member inst:NETT0114 ;
  skos:member inst:NETT0115 ;
  skos:member inst:NETT0116 ;
  skos:member inst:NETT0118 ;
  skos:member inst:NETT0122 ;
  skos:member inst:NETT0124 ;
  skos:member inst:NETT0125 ;
  skos:member inst:NETT0126 ;
  skos:member inst:NETT0127 ;
  skos:member inst:NETT0128 ;
  skos:member inst:NETT0129 ;
  skos:member inst:NETT0131 ;
  skos:member inst:NETT0132 ;
  skos:member inst:NETT0133 ;
  skos:member inst:NETT0134 ;
  skos:member inst:NETT0135 ;
  skos:member inst:NETT0136 ;
  skos:member inst:NETT0137 ;
  skos:member inst:NETT0138 ;
  skos:member inst:NETT0139 ;
  skos:member inst:NETT0140 ;
  skos:member inst:NETT0141 ;
  skos:member inst:NETT0142 ;
  skos:member inst:NETT0143 ;
  skos:member inst:NETT0144 ;
  skos:member inst:NETT0145 ;
  skos:member inst:NETT0147 ;
  skos:member inst:NETT0150 ;
  skos:member inst:NETT0151 ;
  skos:member inst:NETT0153 ;
  skos:member inst:NETT0154 ;
  skos:member inst:NETT0155 ;
  skos:member inst:NETT0161 ;
  skos:member inst:NETT0162 ;
  skos:member inst:NETT0163 ;
  skos:member inst:NETT0164 ;
  skos:member inst:NETT0165 ;
  skos:member inst:NETT0166 ;
  skos:member inst:NETT0167 ;
  skos:member inst:NETT0169 ;
  skos:member inst:NETT0171 ;
  skos:member inst:NETT0173 ;
  skos:member inst:NETT0174 ;
  skos:member inst:NETT0175 ;
  skos:member inst:NETT0176 ;
  skos:member inst:NETT0177 ;
  skos:member inst:NETT0178 ;
  skos:member inst:NETT0179 ;
  skos:member inst:NETT0180 ;
  skos:member inst:NETT0181 ;
  skos:member inst:NETT0182 ;
  skos:member inst:NETT0183 ;
  skos:member inst:NETT0184 ;
  skos:member inst:NETT0186 ;
  skos:member inst:NETT0188 ;
  skos:member inst:NETT0189 ;
  skos:member inst:NETT0190 ;
  skos:member inst:NETT0191 ;
  skos:member inst:NETT0192 ;
  skos:member inst:NETT0195 ;
  skos:member inst:NETT0196 ;
  skos:member inst:NETT0197 ;
  skos:member inst:NETT0198 ;
  skos:member inst:TOOL0001 ;
  skos:member inst:TOOL000X ;
  skos:member inst:TOOL0148 ;
  skos:member inst:TOOL0235 ;
  skos:member inst:TOOL0236 ;
  skos:member inst:TOOL0237 ;
  skos:member inst:TOOL0238 ;
  skos:member inst:TOOL0248 ;
  skos:member inst:TOOL0281 ;
  skos:member inst:TOOL0282 ;
  skos:member inst:TOOL0283 ;
  skos:member inst:TOOL0353 ;
  skos:member inst:TOOL0354 ;
  skos:member inst:TOOL0355 ;
  skos:member inst:TOOL0356 ;
  skos:member inst:TOOL0357 ;
  skos:member inst:TOOL0358 ;
  skos:member inst:TOOL0381 ;
  skos:member inst:TOOL0412 ;
  skos:member inst:TOOL0413 ;
  skos:member inst:TOOL0418 ;
  skos:member inst:TOOL0427 ;
  skos:member inst:TOOL0430 ;
  skos:member inst:TOOL0472 ;
  skos:member inst:TOOL0501 ;
  skos:member inst:TOOL0502 ;
  skos:member inst:TOOL0503 ;
  skos:member inst:TOOL0504 ;
  skos:member inst:TOOL0505 ;
  skos:member inst:TOOL0506 ;
  skos:member inst:TOOL0508 ;
  skos:member inst:TOOL0535 ;
  skos:member inst:TOOL0536 ;
  skos:member inst:TOOL0537 ;
  skos:member inst:TOOL0538 ;
  skos:member inst:TOOL0539 ;
  skos:member inst:TOOL0540 ;
  skos:member inst:TOOL0541 ;
  skos:member inst:TOOL0542 ;
  skos:member inst:TOOL0543 ;
  skos:member inst:TOOL0544 ;
  skos:member inst:TOOL0545 ;
  skos:member inst:TOOL0546 ;
  skos:member inst:TOOL0547 ;
  skos:member inst:TOOL0548 ;
  skos:member inst:TOOL0550 ;
  skos:member inst:TOOL0551 ;
  skos:member inst:TOOL0552 ;
  skos:member inst:TOOL0553 ;
  skos:member inst:TOOL0554 ;
  skos:member inst:TOOL0555 ;
  skos:member inst:TOOL0556 ;
  skos:member inst:TOOL0557 ;
  skos:member inst:TOOL0561 ;
  skos:member inst:TOOL0562 ;
  skos:member inst:TOOL0563 ;
  skos:member inst:TOOL0571 ;
  skos:member inst:TOOL0573 ;
  skos:member inst:TOOL0588 ;
  skos:member inst:TOOL0651 ;
  skos:member inst:TOOL0652 ;
  skos:member inst:TOOL0653 ;
  skos:member inst:TOOL0660 ;
  skos:member inst:TOOL0784 ;
  skos:member inst:TOOL0785 ;
  skos:member inst:TOOL0786 ;
  skos:member inst:TOOL0787 ;
  skos:member inst:TOOL0788 ;
  skos:member inst:TOOL0806 ;
  skos:member inst:TOOL0807 ;
  skos:member inst:TOOL0817 ;
  skos:member inst:TOOL0818 ;
  skos:member inst:TOOL0819 ;
  skos:member inst:TOOL0828 ;
  skos:member inst:TOOL0843 ;
  skos:member inst:TOOL0917 ;
  skos:member inst:TOOL0939 ;
  skos:member inst:TOOL0940 ;
  skos:member inst:TOOL0960 ;
  skos:member inst:TOOL0961 ;
  skos:member inst:TOOL0962 ;
  skos:member inst:TOOL0963 ;
  skos:member inst:TOOL0978 ;
  skos:member inst:TOOL0979 ;
  skos:member inst:TOOL0980 ;
  skos:member inst:TOOL0981 ;
  skos:member inst:TOOL0982 ;
  skos:member inst:TOOL0983 ;
  skos:member inst:TOOL0984 ;
  skos:member inst:TOOL0985 ;
  skos:member inst:TOOL0986 ;
  skos:member inst:TOOL0987 ;
  skos:member inst:TOOL0988 ;
  skos:member inst:TOOL0989 ;
  skos:member inst:TOOL0990 ;
  skos:member inst:TOOL0991 ;
  skos:member inst:TOOL0992 ;
  skos:member inst:TOOL0993 ;
  skos:member inst:TOOL0994 ;
  skos:member inst:TOOL0995 ;
  skos:member inst:TOOL0996 ;
  skos:member inst:TOOL0997 ;
  skos:member inst:TOOL1012 ;
  skos:member inst:TOOL1038 ;
  skos:member inst:TOOL1083 ;
  skos:member inst:TOOL1135 ;
  skos:member inst:TOOL1165 ;
  skos:member inst:TOOL1166 ;
  skos:member inst:TOOL1169 ;
  skos:member inst:TOOL1170 ;
  skos:member inst:TOOL1171 ;
  skos:member inst:TOOL1172 ;
  skos:member inst:TOOL1173 ;
  skos:member inst:TOOL1174 ;
  skos:member inst:TOOL1175 ;
  skos:member inst:TOOL1176 ;
  skos:member inst:TOOL1177 ;
  skos:member inst:TOOL1178 ;
  skos:member inst:TOOL1179 ;
  skos:member inst:TOOL1181 ;
  skos:member inst:TOOL1191 ;
  skos:member inst:TOOL1199 ;
  skos:member inst:TOOL1204 ;
  skos:member inst:TOOL1214 ;
  skos:member inst:TOOL1215 ;
  skos:member inst:TOOL1216 ;
  skos:member inst:TOOL1235 ;
  skos:member inst:TOOL1249 ;
  skos:member inst:TOOL1252 ;
  skos:member inst:TOOL1253 ;
  skos:member inst:TOOL1259 ;
  skos:member inst:TOOL1260 ;
  skos:member inst:TOOL1261 ;
  skos:member inst:TOOL1272 ;
  skos:member inst:TOOL1274 ;
  skos:member inst:TOOL1285 ;
  skos:member inst:TOOL1304 ;
  skos:member inst:TOOL1326 ;
  skos:member inst:TOOL1339 ;
  skos:member inst:TOOL1371 ;
  skos:member inst:TOOL1372 ;
  skos:member inst:TOOL1373 ;
  skos:member inst:TOOL1374 ;
  skos:member inst:TOOL1375 ;
  skos:member inst:TOOL1376 ;
  skos:member inst:TOOL1378 ;
  skos:member inst:TOOL1379 ;
  skos:member inst:TOOL1405 ;
  skos:member inst:TOOL1413 ;
  skos:member inst:TOOL1414 ;
  skos:member inst:TOOL1415 ;
  skos:member inst:TOOL1416 ;
  skos:member inst:TOOL1417 ;
  skos:member inst:TOOL1454 ;
  skos:member inst:TOOL1455 ;
  skos:member inst:TOOL1462 ;
  skos:member inst:TOOL1463 ;
  skos:member inst:TOOL1464 ;
  skos:member inst:TOOL1465 ;
  skos:member inst:TOOL1466 ;
  skos:member inst:TOOL1467 ;
  skos:member inst:TOOL1468 ;
  skos:member inst:TOOL1469 ;
  skos:member inst:TOOL1477 ;
  skos:member inst:TOOL1478 ;
  skos:member inst:TOOL1480 ;
  skos:member inst:TOOL1485 ;
  skos:member inst:TOOL1486 ;
  skos:member inst:TOOL1487 ;
  skos:member inst:TOOL1527 ;
  skos:member inst:TOOL1533 ;
  skos:member inst:TOOL1535 ;
  skos:member inst:TOOL1536 ;
  skos:member inst:TOOL1537 ;
  skos:member inst:TOOL1560 ;
  skos:member inst:TOOL1574 ;
  skos:member inst:TOOL1575 ;
  skos:member inst:TOOL1576 ;
  skos:member inst:TOOL1638 ;
  skos:member inst:TOOL1644 ;
  skos:member inst:TOOL1654 ;
  skos:member inst:TOOL1668 ;
  skos:member inst:TOOL1703 ;
  skos:member inst:TOOLZZZ ;
  skos:notation "SDN:L19::SDNKG17" ;
  skos:note "accepted"@en ;
  skos:prefLabel "sensor_model"@en ;
.
sdnc:ICAT03
  rdf:type skos:Concept ;
  dcterm:date "2008-01-10 13:02:59.0" ;
  dcterm:identifier "SDN:L21::ICAT03" ;
  dcterm:source <http://w3id.org/ogeochem/def/instrument/measurement/conceptscheme> ;
  pav:authoredOn "2008-01-10 13:02:59.0" ;
  pav:hasCurrentVersion <http://vocab.nerc.ac.uk/collection/L21/current/ICAT03/1> ;
  owl:versionInfo "1" ;
  skos:altLabel "SeaDataNet sample measurer categories"@en ;
  skos:altLabel "sample measurers"@en ;
  skos:broader sdnk:SDNKG01 ;
  skos:definition "Categories used in the SeaDataNet project to classify devices that measure properties of samples out of situ, generally in a laboratory environment."@en ;
  skos:editorialNote "move to subclass of instrument" ;
  skos:inScheme <http://w3id.org/ogeochem/def/instrument/measurement/conceptscheme> ;
  skos:narrower <http://vocab.nerc.ac.uk/collection/L05/current/311> ;
  skos:narrower <http://vocab.nerc.ac.uk/collection/L05/current/86> ;
  skos:narrower sdev:LAB01 ;
  skos:narrower sdev:LAB02 ;
  skos:narrower sdev:LAB03 ;
  skos:narrower sdev:LAB04 ;
  skos:narrower sdev:LAB05 ;
  skos:narrower sdev:LAB06 ;
  skos:narrower sdev:LAB07 ;
  skos:narrower sdev:LAB08 ;
  skos:narrower sdev:LAB09 ;
  skos:narrower sdev:LAB10 ;
  skos:narrower sdev:LAB11 ;
  skos:narrower sdev:LAB12 ;
  skos:narrower sdev:LAB13 ;
  skos:narrower sdev:LAB14 ;
  skos:narrower sdev:LAB15 ;
  skos:narrower sdev:LAB16 ;
  skos:narrower sdev:LAB17 ;
  skos:narrower sdev:LAB18 ;
  skos:narrower sdev:LAB19 ;
  skos:narrower sdev:LAB20 ;
  skos:narrower sdev:LAB21 ;
  skos:narrower sdev:LAB22 ;
  skos:narrower sdev:LAB23 ;
  skos:narrower sdev:LAB24 ;
  skos:narrower sdev:LAB25 ;
  skos:narrower sdev:LAB26 ;
  skos:narrower sdev:LAB27 ;
  skos:narrower sdev:LAB28 ;
  skos:narrower sdev:LAB29 ;
  skos:narrower sdev:LAB30 ;
  skos:narrower sdev:LAB31 ;
  skos:narrower sdev:LAB32 ;
  skos:narrower sdev:LAB33 ;
  skos:narrower sdev:LAB34 ;
  skos:narrower sdev:LAB35 ;
  skos:narrower sdev:LAB36 ;
  skos:narrower sdev:LAB37 ;
  skos:narrower sdev:LAB38 ;
  skos:narrower sdev:LAB39 ;
  skos:narrower sdev:LAB40 ;
  skos:narrower sdev:LAB42 ;
  skos:narrower sdev:LAB43 ;
  skos:narrower sdev:LAB44 ;
  skos:narrower sdev:LAB45 ;
  skos:narrower sdev:LAB46 ;
  skos:narrower sdev:LAB47 ;
  skos:narrower sdev:LAB48 ;
  skos:narrower sdev:LAB49 ;
  skos:narrower sdev:LAB51 ;
  skos:notation "SDN:L21::ICAT03" ;
  skos:note "accepted"@en ;
  skos:prefLabel "Lab-based instruments"@en ;
.
sdnc:ICAT04
  rdf:type skos:Concept ;
  dcterm:date "2008-01-10 13:02:59.0" ;
  dcterm:identifier "SDN:L21::ICAT04" ;
  dcterm:source <http://w3id.org/ogeochem/def/instrument/measurement/conceptscheme> ;
  pav:authoredOn "2008-01-10 13:02:59.0" ;
  pav:hasCurrentVersion <http://vocab.nerc.ac.uk/collection/L21/current/ICAT04/1> ;
  owl:versionInfo "1" ;
  skos:altLabel "SeaDataNet in-situ sensor and instrument package categories"@en ;
  skos:altLabel "in-situ sensors and packages"@en ;
  skos:broader sdnk:SDNKG01 ;
  skos:definition "Categories used in the SeaDataNet project to classify devices that make in-situ measurements of phenomena from fixed or mobile platforms."@en ;
  skos:editorialNote "make child of instrument" ;
  skos:inScheme <http://w3id.org/ogeochem/def/instrument/measurement/conceptscheme> ;
  skos:narrower <http://vocab.nerc.ac.uk/collection/L05/current/101> ;
  skos:narrower <http://vocab.nerc.ac.uk/collection/L05/current/102> ;
  skos:narrower <http://vocab.nerc.ac.uk/collection/L05/current/103> ;
  skos:narrower <http://vocab.nerc.ac.uk/collection/L05/current/110> ;
  skos:narrower <http://vocab.nerc.ac.uk/collection/L05/current/113> ;
  skos:narrower <http://vocab.nerc.ac.uk/collection/L05/current/114> ;
  skos:narrower <http://vocab.nerc.ac.uk/collection/L05/current/115> ;
  skos:narrower <http://vocab.nerc.ac.uk/collection/L05/current/122> ;
  skos:narrower <http://vocab.nerc.ac.uk/collection/L05/current/123> ;
  skos:narrower <http://vocab.nerc.ac.uk/collection/L05/current/124> ;
  skos:narrower <http://vocab.nerc.ac.uk/collection/L05/current/130> ;
  skos:narrower <http://vocab.nerc.ac.uk/collection/L05/current/131> ;
  skos:narrower <http://vocab.nerc.ac.uk/collection/L05/current/132> ;
  skos:narrower <http://vocab.nerc.ac.uk/collection/L05/current/133> ;
  skos:narrower <http://vocab.nerc.ac.uk/collection/L05/current/134> ;
  skos:narrower <http://vocab.nerc.ac.uk/collection/L05/current/135> ;
  skos:narrower <http://vocab.nerc.ac.uk/collection/L05/current/150> ;
  skos:narrower <http://vocab.nerc.ac.uk/collection/L05/current/152> ;
  skos:narrower <http://vocab.nerc.ac.uk/collection/L05/current/153> ;
  skos:narrower <http://vocab.nerc.ac.uk/collection/L05/current/154> ;
  skos:narrower <http://vocab.nerc.ac.uk/collection/L05/current/155> ;
  skos:narrower <http://vocab.nerc.ac.uk/collection/L05/current/156> ;
  skos:narrower <http://vocab.nerc.ac.uk/collection/L05/current/157> ;
  skos:narrower <http://vocab.nerc.ac.uk/collection/L05/current/158> ;
  skos:narrower <http://vocab.nerc.ac.uk/collection/L05/current/159> ;
  skos:narrower <http://vocab.nerc.ac.uk/collection/L05/current/180> ;
  skos:narrower <http://vocab.nerc.ac.uk/collection/L05/current/181> ;
  skos:narrower <http://vocab.nerc.ac.uk/collection/L05/current/183> ;
  skos:narrower <http://vocab.nerc.ac.uk/collection/L05/current/184> ;
  skos:narrower <http://vocab.nerc.ac.uk/collection/L05/current/185> ;
  skos:narrower <http://vocab.nerc.ac.uk/collection/L05/current/311> ;
  skos:narrower <http://vocab.nerc.ac.uk/collection/L05/current/350> ;
  skos:narrower <http://vocab.nerc.ac.uk/collection/L05/current/351> ;
  skos:narrower <http://vocab.nerc.ac.uk/collection/L05/current/352> ;
  skos:narrower <http://vocab.nerc.ac.uk/collection/L05/current/353> ;
  skos:narrower <http://vocab.nerc.ac.uk/collection/L05/current/355> ;
  skos:narrower <http://vocab.nerc.ac.uk/collection/L05/current/356> ;
  skos:narrower <http://vocab.nerc.ac.uk/collection/L05/current/358> ;
  skos:narrower <http://vocab.nerc.ac.uk/collection/L05/current/359> ;
  skos:narrower <http://vocab.nerc.ac.uk/collection/L05/current/360> ;
  skos:narrower <http://vocab.nerc.ac.uk/collection/L05/current/361> ;
  skos:narrower <http://vocab.nerc.ac.uk/collection/L05/current/362> ;
  skos:narrower <http://vocab.nerc.ac.uk/collection/L05/current/363> ;
  skos:narrower <http://vocab.nerc.ac.uk/collection/L05/current/364> ;
  skos:narrower <http://vocab.nerc.ac.uk/collection/L05/current/365> ;
  skos:narrower <http://vocab.nerc.ac.uk/collection/L05/current/366> ;
  skos:narrower <http://vocab.nerc.ac.uk/collection/L05/current/367> ;
  skos:narrower <http://vocab.nerc.ac.uk/collection/L05/current/368> ;
  skos:narrower <http://vocab.nerc.ac.uk/collection/L05/current/369> ;
  skos:narrower <http://vocab.nerc.ac.uk/collection/L05/current/370> ;
  skos:narrower <http://vocab.nerc.ac.uk/collection/L05/current/371> ;
  skos:narrower <http://vocab.nerc.ac.uk/collection/L05/current/372> ;
  skos:narrower <http://vocab.nerc.ac.uk/collection/L05/current/373> ;
  skos:narrower <http://vocab.nerc.ac.uk/collection/L05/current/374> ;
  skos:narrower <http://vocab.nerc.ac.uk/collection/L05/current/375> ;
  skos:narrower <http://vocab.nerc.ac.uk/collection/L05/current/376> ;
  skos:narrower <http://vocab.nerc.ac.uk/collection/L05/current/377> ;
  skos:narrower <http://vocab.nerc.ac.uk/collection/L05/current/379> ;
  skos:narrower <http://vocab.nerc.ac.uk/collection/L05/current/380> ;
  skos:narrower <http://vocab.nerc.ac.uk/collection/L05/current/381> ;
  skos:narrower <http://vocab.nerc.ac.uk/collection/L05/current/382> ;
  skos:narrower <http://vocab.nerc.ac.uk/collection/L05/current/383> ;
  skos:narrower <http://vocab.nerc.ac.uk/collection/L05/current/384> ;
  skos:narrower <http://vocab.nerc.ac.uk/collection/L05/current/385> ;
  skos:narrower <http://vocab.nerc.ac.uk/collection/L05/current/386> ;
  skos:narrower <http://vocab.nerc.ac.uk/collection/L05/current/387> ;
  skos:narrower <http://vocab.nerc.ac.uk/collection/L05/current/388> ;
  skos:narrower <http://vocab.nerc.ac.uk/collection/L05/current/389> ;
  skos:narrower <http://vocab.nerc.ac.uk/collection/L05/current/390> ;
  skos:narrower <http://vocab.nerc.ac.uk/collection/L05/current/393> ;
  skos:narrower <http://vocab.nerc.ac.uk/collection/L05/current/395> ;
  skos:narrower sdev:ATRANS ;
  skos:narrower sdev:BLUMS ;
  skos:narrower sdev:CCOV ;
  skos:narrower sdev:COLCMP ;
  skos:narrower sdev:DLOG ;
  skos:narrower sdev:EMSR ;
  skos:narrower sdev:FFES ;
  skos:narrower sdev:ICEP ;
  skos:narrower sdev:LVLST ;
  skos:narrower sdev:MMIS ;
  skos:narrower sdev:MPIS ;
  skos:narrower sdev:PERMON ;
  skos:narrower sdev:TRTG ;
  skos:narrower sdev:WDRG ;
  skos:narrower sdev:WPS ;
  skos:notation "SDN:L21::ICAT04" ;
  skos:note "accepted"@en ;
  skos:prefLabel "In-situ measurement device"@en ;
.
sdnc:ICAT05
  rdf:type skos:Concept ;
  dcterm:date "2008-01-10 13:02:59.0" ;
  dcterm:identifier "SDN:L21::ICAT05" ;
  dcterm:source <http://w3id.org/ogeochem/def/instrument/measurement/conceptscheme> ;
  pav:authoredOn "2008-01-10 13:02:59.0" ;
  pav:hasCurrentVersion <http://vocab.nerc.ac.uk/collection/L21/current/ICAT05/1> ;
  owl:versionInfo "1" ;
  skos:altLabel "SeaDataNet remote sensor categories"@en ;
  skos:altLabel "remote sensors"@en ;
  skos:broader sdnk:SDNKG01 ;
  skos:definition "Categories used in the SeaDataNet project to classify devices that make remote measurements of phenomena from satellites or aircraft. Also includes categories of shipborne instruments that strictly speaking sense remotely such as magnetometers."@en ;
  skos:inScheme <http://w3id.org/ogeochem/def/instrument/measurement/conceptscheme> ;
  skos:narrower <http://vocab.nerc.ac.uk/collection/L05/current/121> ;
  skos:narrower <http://vocab.nerc.ac.uk/collection/L05/current/186> ;
  skos:narrower <http://vocab.nerc.ac.uk/collection/L05/current/301> ;
  skos:narrower <http://vocab.nerc.ac.uk/collection/L05/current/302> ;
  skos:narrower <http://vocab.nerc.ac.uk/collection/L05/current/303> ;
  skos:narrower <http://vocab.nerc.ac.uk/collection/L05/current/304> ;
  skos:narrower <http://vocab.nerc.ac.uk/collection/L05/current/305> ;
  skos:narrower <http://vocab.nerc.ac.uk/collection/L05/current/306> ;
  skos:narrower <http://vocab.nerc.ac.uk/collection/L05/current/307> ;
  skos:narrower <http://vocab.nerc.ac.uk/collection/L05/current/308> ;
  skos:narrower <http://vocab.nerc.ac.uk/collection/L05/current/309> ;
  skos:narrower <http://vocab.nerc.ac.uk/collection/L05/current/310> ;
  skos:narrower <http://vocab.nerc.ac.uk/collection/L05/current/311> ;
  skos:narrower <http://vocab.nerc.ac.uk/collection/L05/current/312> ;
  skos:narrower <http://vocab.nerc.ac.uk/collection/L05/current/313> ;
  skos:narrower <http://vocab.nerc.ac.uk/collection/L05/current/314> ;
  skos:narrower <http://vocab.nerc.ac.uk/collection/L05/current/315> ;
  skos:narrower <http://vocab.nerc.ac.uk/collection/L05/current/91> ;
  skos:narrower <http://vocab.nerc.ac.uk/collection/L05/current/92> ;
  skos:narrower sdev:CSEM ;
  skos:notation "SDN:L21::ICAT05" ;
  skos:note "accepted"@en ;
  skos:prefLabel "Remote sensing instruments"@en ;
.
sdnc:collection
  rdf:type skos:Collection ;
  dcterm:alternative "Device category types" ;
  dcterm:creator "SeaDataNet" ;
  dcterm:date "2012-07-17 02:00:03.0" ;
  dcterm:description "High-level classification of devices based on function and mode of deployment." ;
  dcterm:license <https://creativecommons.org/licenses/by/4.0> ;
  dcterm:publisher "Natural Environment Research Council" ;
  dcterm:title "SeaDataNet device category types" ;
  grg:RE_RegisterManager "British Oceanographic Data Centre" ;
  grg:RE_RegisterOwner "SeaDataNet" ;
  rdfs:comment "Governance for vocabularies used in the EU SeaDataNet project implemented as consultation between BODC and the members of the SeaDataNet Technical Task Team" ;
  owl:versionInfo "5" ;
  skos:altLabel "Device category types" ;
  skos:member sdnc:ICAT03 ;
  skos:member sdnc:ICAT04 ;
  skos:member sdnc:ICAT05 ;
  skos:prefLabel "SeaDataNet device category types" ;
.
inst:TOOL0001
  rdf:type skos:Concept ;
  dcterm:date "2012-01-05 09:34:05.0" ;
  dcterm:identifier "SDN:L22::TOOL0001" ;
  dcterm:source <http://vocab.nerc.ac.uk/scheme/SDNDEV/current> ;
  pav:hasCurrentVersion <http://vocab.nerc.ac.uk/collection/L22/current/TOOL0001/1> ;
  owl:versionInfo "1" ;
  skos:altLabel "CTD"@en ;
  skos:broader <http://vocab.nerc.ac.uk/collection/L05/current/134> ;
  skos:broader <http://vocab.nerc.ac.uk/collection/L05/current/350> ;
  skos:definition "A generic term for a set of co-located conductivity, temperature and pressure (proxy for depth) sensors.  The pressure sensor is generally used to ascertain the instrument Z co-ordinate in the water body, whilst the other sensors determine water temperature and salinity. Deployed on a range of platforms such as vertically lowered metal frames, towed fish, AUVs or moorings."@en ;
  skos:inScheme <http://vocab.nerc.ac.uk/scheme/SDNDEV/current> ;
  skos:notation "SDN:L22::TOOL0001" ;
  skos:note "accepted"@en ;
  skos:prefLabel "Conductivity, temperature and depth package"@en ;
  skos:related <http://vocab.nerc.ac.uk/collection/B75/current/ORG00001> ;
  skos:related <http://vocab.nerc.ac.uk/collection/L05/current/130> ;
  skos:related <http://vocab.nerc.ac.uk/collection/P01/current/PRESPR01> ;
  skos:related <http://vocab.nerc.ac.uk/collection/P01/current/PSALPR01> ;
  skos:related <http://vocab.nerc.ac.uk/collection/P01/current/TEMPST01> ;
.
inst:TOOL0148
  rdf:type skos:Concept ;
  dcterm:date "2010-05-18 16:10:58.0" ;
  dcterm:identifier "SDN:L22::TOOL0148" ;
  dcterm:source <http://vocab.nerc.ac.uk/scheme/SDNDEV/current> ;
  pav:hasCurrentVersion <http://vocab.nerc.ac.uk/collection/L22/current/TOOL0148/1> ;
  owl:versionInfo "1" ;
  skos:altLabel "Unknown transmissometer"@en ;
  skos:broader <http://vocab.nerc.ac.uk/collection/L05/current/124> ;
  skos:definition "An in-situ instrument that transmits monochromatic light through a region of the surrounding water body and records how much is received by a sensor a fixed distance away."@en ;
  skos:inScheme <http://vocab.nerc.ac.uk/scheme/SDNDEV/current> ;
  skos:notation "SDN:L22::TOOL0148" ;
  skos:note "accepted"@en ;
  skos:prefLabel "Unknown transmissometer"@en ;
  skos:related <http://vocab.nerc.ac.uk/collection/B75/current/ORG00001> ;
  skos:related <http://vocab.nerc.ac.uk/collection/P01/current/ATTNZR01> ;
  skos:related <http://vocab.nerc.ac.uk/collection/P01/current/POATCV01> ;
.
inst:TOOL0237
  rdf:type skos:Concept ;
  dcterm:date "2010-05-18 16:10:58.0" ;
  dcterm:identifier "SDN:L22::TOOL0237" ;
  dcterm:source <http://vocab.nerc.ac.uk/scheme/SDNDEV/current> ;
  pav:hasCurrentVersion <http://vocab.nerc.ac.uk/collection/L22/current/TOOL0237/1> ;
  owl:versionInfo "1" ;
  skos:altLabel "Thermometer"@en ;
  skos:broader <http://vocab.nerc.ac.uk/collection/L05/current/134> ;
  skos:definition "A generic term for a temperature sensor capable of being immersed in water primarily intended to measure water body temperature but could also be used to determine temperature of other matrices."@en ;
  skos:inScheme <http://vocab.nerc.ac.uk/scheme/SDNDEV/current> ;
  skos:notation "SDN:L22::TOOL0237" ;
  skos:note "accepted"@en ;
  skos:prefLabel "Waterproof thermometer"@en ;
  skos:related <http://vocab.nerc.ac.uk/collection/B75/current/ORG00001> ;
.
inst:TOOL0238
  rdf:type skos:Concept ;
  dcterm:date "2010-05-18 16:10:58.0" ;
  dcterm:identifier "SDN:L22::TOOL0238" ;
  dcterm:source <http://vocab.nerc.ac.uk/scheme/SDNDEV/current> ;
  pav:hasCurrentVersion <http://vocab.nerc.ac.uk/collection/L22/current/TOOL0238/1> ;
  owl:versionInfo "1" ;
  skos:altLabel "Hg RTM"@en ;
  skos:broader <http://vocab.nerc.ac.uk/collection/L05/current/134> ;
  skos:definition "A generic term for a mercury-in-glass thermometer that freezes the temperature reading when turned upside-down."@en ;
  skos:inScheme <http://vocab.nerc.ac.uk/scheme/SDNDEV/current> ;
  skos:notation "SDN:L22::TOOL0238" ;
  skos:note "accepted"@en ;
  skos:prefLabel "Mercury reversing thermometer"@en ;
  skos:related <http://vocab.nerc.ac.uk/collection/B75/current/ORG00001> ;
.
inst:TOOL0281
  rdf:type skos:Concept ;
  dcterm:date "2010-05-18 16:10:58.0" ;
  dcterm:identifier "SDN:L22::TOOL0281" ;
  dcterm:source <http://vocab.nerc.ac.uk/scheme/SDNDEV/current> ;
  pav:hasCurrentVersion <http://vocab.nerc.ac.uk/collection/L22/current/TOOL0281/1> ;
  owl:versionInfo "1" ;
  skos:altLabel "Barometer"@en ;
  skos:broader <http://vocab.nerc.ac.uk/collection/L05/current/102> ;
  skos:definition "A generic term for a device that measures atmospheric pressure. The term is for use where details of the make, model number and measurement principle are not known."@en ;
  skos:inScheme <http://vocab.nerc.ac.uk/scheme/SDNDEV/current> ;
  skos:notation "SDN:L22::TOOL0281" ;
  skos:note "accepted"@en ;
  skos:prefLabel "Barometer"@en ;
  skos:related <http://vocab.nerc.ac.uk/collection/B75/current/ORG00001> ;
.
inst:TOOL0282
  rdf:type skos:Concept ;
  dcterm:date "2010-05-18 16:10:58.0" ;
  dcterm:identifier "SDN:L22::TOOL0282" ;
  dcterm:source <http://vocab.nerc.ac.uk/scheme/SDNDEV/current> ;
  pav:hasCurrentVersion <http://vocab.nerc.ac.uk/collection/L22/current/TOOL0282/1> ;
  owl:versionInfo "1" ;
  skos:altLabel "Hygrometer"@en ;
  skos:broader <http://vocab.nerc.ac.uk/collection/L05/current/102> ;
  skos:definition "A generic term for a device that measures atmospheric humidity. The term is for use where details of the make, model number and measurement principle are not known."@en ;
  skos:inScheme <http://vocab.nerc.ac.uk/scheme/SDNDEV/current> ;
  skos:notation "SDN:L22::TOOL0282" ;
  skos:note "accepted"@en ;
  skos:prefLabel "Hygrometer"@en ;
  skos:related <http://vocab.nerc.ac.uk/collection/B75/current/ORG00001> ;
.
inst:TOOL0283
  rdf:type skos:Concept ;
  dcterm:date "2010-05-18 16:10:58.0" ;
  dcterm:identifier "SDN:L22::TOOL0283" ;
  dcterm:source <http://vocab.nerc.ac.uk/scheme/SDNDEV/current> ;
  pav:hasCurrentVersion <http://vocab.nerc.ac.uk/collection/L22/current/TOOL0283/1> ;
  owl:versionInfo "1" ;
  skos:altLabel "Air thermometer"@en ;
  skos:broader <http://vocab.nerc.ac.uk/collection/L05/current/102> ;
  skos:definition "A generic term for a device that measures atmospheric temperature. The term is for use where details of the make, model number and measurement principle are not known."@en ;
  skos:inScheme <http://vocab.nerc.ac.uk/scheme/SDNDEV/current> ;
  skos:notation "SDN:L22::TOOL0283" ;
  skos:note "accepted"@en ;
  skos:prefLabel "Atmospheric thermometer"@en ;
  skos:related <http://vocab.nerc.ac.uk/collection/B75/current/ORG00001> ;
.
inst:TOOL0354
  rdf:type skos:Concept ;
  dcterm:date "2010-11-18 12:37:16.0" ;
  dcterm:identifier "SDN:L22::TOOL0354" ;
  dcterm:source <http://vocab.nerc.ac.uk/scheme/SDNDEV/current> ;
  pav:hasCurrentVersion <http://vocab.nerc.ac.uk/collection/L22/current/TOOL0354/1> ;
  owl:versionInfo "1" ;
  skos:altLabel "Hydrophone"@en ;
  skos:broader <http://vocab.nerc.ac.uk/collection/L05/current/369> ;
  skos:definition "A generic term for an acoustic intensity sensor (microphone) with an acoustic impedence matched to the density of water to optimise sonic detection under water."@en ;
  skos:inScheme <http://vocab.nerc.ac.uk/scheme/SDNDEV/current> ;
  skos:notation "SDN:L22::TOOL0354" ;
  skos:note "accepted"@en ;
  skos:prefLabel "Hydrophone"@en ;
  skos:related <http://vocab.nerc.ac.uk/collection/B75/current/ORG00001> ;
  skos:related <http://vocab.nerc.ac.uk/collection/L05/current/153> ;
  skos:related <http://vocab.nerc.ac.uk/collection/L05/current/154> ;
  skos:related <http://vocab.nerc.ac.uk/collection/L05/current/362> ;
  skos:related <http://vocab.nerc.ac.uk/collection/L05/current/363> ;
  skos:related <http://vocab.nerc.ac.uk/collection/L05/current/364> ;
  skos:related <http://vocab.nerc.ac.uk/collection/L05/current/365> ;
  skos:related <http://vocab.nerc.ac.uk/collection/L05/current/366> ;
  skos:related <http://vocab.nerc.ac.uk/collection/L05/current/371> ;
  skos:related <http://vocab.nerc.ac.uk/collection/L05/current/372> ;
  skos:related <http://vocab.nerc.ac.uk/collection/L05/current/373> ;
  skos:related <http://vocab.nerc.ac.uk/collection/L05/current/374> ;
  skos:related <http://vocab.nerc.ac.uk/collection/L05/current/375> ;
.
inst:TOOL0430
  rdf:type skos:Concept ;
  dcterm:date "2011-11-02 11:37:25.0" ;
  dcterm:identifier "SDN:L22::TOOL0430" ;
  dcterm:source <http://vocab.nerc.ac.uk/scheme/SDNDEV/current> ;
  pav:hasCurrentVersion <http://vocab.nerc.ac.uk/collection/L22/current/TOOL0430/1> ;
  owl:versionInfo "1" ;
  skos:altLabel "Secchi disk"@en ;
  skos:broader <http://vocab.nerc.ac.uk/collection/L05/current/124> ;
  skos:definition "A circular disk, typically 20cm in diameter, used to measure water transparency. For marine applications, the disk is usually entirely white, while for limnological studies it is common to use one with alternating black and white quadrants. The reasons for this may be historical rather thah theoretical. A black Secchi disk has recently been developed for use in shallow rivers and streams. The disk is lowered slowly into the water on a pole or line until it can no longer be seen by the observer. The depth of disappearance provides an estimate of the transparency of the water, although any reading is affected by the observer's eyesight and ambient light conditions."@en ;
  skos:inScheme <http://vocab.nerc.ac.uk/scheme/SDNDEV/current> ;
  skos:notation "SDN:L22::TOOL0430" ;
  skos:note "accepted"@en ;
  skos:prefLabel "Secchi disk"@en ;
  skos:related <http://vocab.nerc.ac.uk/collection/B75/current/ORG00001> ;
.
inst:TOOL0695
  rdf:type skos:Concept ;
  dcterm:date "2014-05-01 15:18:08.0" ;
  dcterm:identifier "SDN:L22::TOOL0695" ;
  dcterm:source <http://vocab.nerc.ac.uk/scheme/SDNDEV/current> ;
  pav:hasCurrentVersion <http://vocab.nerc.ac.uk/collection/L22/current/TOOL0695/1> ;
  owl:versionInfo "1" ;
  skos:altLabel "CAE HE20/K pyranometer"@en ;
  skos:broader <http://vocab.nerc.ac.uk/collection/L05/current/308> ;
  skos:definition "A HE20/K pyranometer measuring total incident solar radiation with temperature dependence of less than 2 percent, and nonlinearity of +/-1.5 percent from 0 to 1500 W/m2. Operating temperature range is -40 to 60 degC."@en ;
  skos:inScheme <http://vocab.nerc.ac.uk/scheme/SDNDEV/current> ;
  skos:notation "SDN:L22::TOOL0695" ;
  skos:note "accepted"@en ;
  skos:prefLabel "CAE HE20/K pyranometer"@en ;
  skos:related <http://vocab.nerc.ac.uk/collection/B75/current/ORG00757> ;
.
inst:TOOL0697
  rdf:type skos:Concept ;
  dcterm:date "2017-03-22 11:27:08.0" ;
  dcterm:identifier "SDN:L22::TOOL0697" ;
  dcterm:isReplacedBy inst:TOOL000X ;
  dcterm:source <http://vocab.nerc.ac.uk/scheme/SDNDEV/current> ;
  pav:hasCurrentVersion <http://vocab.nerc.ac.uk/collection/L22/current/TOOL0697/3> ;
  pav:hasVersion <http://vocab.nerc.ac.uk/collection/L22/current/TOOL0697/1> ;
  pav:hasVersion <http://vocab.nerc.ac.uk/collection/L22/current/TOOL0697/2> ;
  owl:deprecated "true" ;
  owl:versionInfo "3" ;
  skos:altLabel "MetOcean SVP-Iridium Drifter"@en ;
  skos:broader <http://vocab.nerc.ac.uk/collection/L05/current/121> ;
  skos:definition "Code deprecated because it refers to a platform and not an instrument. Original description was: a drifting surface buoy equipped with a bi-directional Iridium satellite system communications link, which also provides the primary position information.  More accurate position information is provided by a GPS module.  The drifter has an SST sensor and battery voltage sensor as standard, and can optionally be equipped with sensors for salinity, high resolution SST, and barometric pressure.  The drifter can either comprise a spherical surface unit with no drogue (the iSphere), or be attached to a holey-sock drogue by a tether (SVP).  The latter configuration has a strain gauge drogue presence system."@en ;
  skos:inScheme <http://vocab.nerc.ac.uk/scheme/SDNDEV/current> ;
  skos:notation "SDN:L22::TOOL0697" ;
  skos:note "deprecated"@en ;
  skos:prefLabel "MetOcean Surface Velocity Program (SVP)-Iridium Drifter"@en ;
  skos:related <http://vocab.nerc.ac.uk/collection/B75/current/ORG00802> ;
.
inst:TOOL0702
  rdf:type skos:Concept ;
  dcterm:date "2022-10-24 12:57:12.0" ;
  dcterm:identifier "SDN:L22::TOOL0702" ;
  dcterm:source <http://vocab.nerc.ac.uk/scheme/SDNDEV/current> ;
  pav:hasCurrentVersion <http://vocab.nerc.ac.uk/collection/L22/current/TOOL0702/2> ;
  pav:hasVersion <http://vocab.nerc.ac.uk/collection/L22/current/TOOL0702/1> ;
  owl:versionInfo "2" ;
  skos:altLabel "K&Z CNR4"@en ;
  skos:broader <http://vocab.nerc.ac.uk/collection/L05/current/308> ;
  skos:definition "The CNR4 is a net radiometer that measures the energy balance between incoming and shortwave IR radiation versus surface reflected shortwave and outgoing longwave IR radiation. The instrument comprises an upward-facing pyranometer/pyrgeometer pair, and a downward facing pair. There is an internal thermisor, an internal Pt-100 RTD, and a solar shield. There is an optional ventilation unit with heater to minimise condensation."@en ;
  skos:inScheme <http://vocab.nerc.ac.uk/scheme/SDNDEV/current> ;
  skos:notation "SDN:L22::TOOL0702" ;
  skos:note "accepted"@en ;
  skos:prefLabel "Kipp and Zonen CNR4 Net Radiometer"@en ;
  skos:related <http://vocab.nerc.ac.uk/collection/B75/current/ORG00324> ;
.
inst:TOOL0703
  rdf:type skos:Concept ;
  dcterm:date "2022-10-24 12:57:12.0" ;
  dcterm:identifier "SDN:L22::TOOL0703" ;
  dcterm:source <http://vocab.nerc.ac.uk/scheme/SDNDEV/current> ;
  pav:hasCurrentVersion <http://vocab.nerc.ac.uk/collection/L22/current/TOOL0703/2> ;
  pav:hasVersion <http://vocab.nerc.ac.uk/collection/L22/current/TOOL0703/1> ;
  owl:versionInfo "2" ;
  skos:altLabel "K&Z CNR1"@en ;
  skos:broader <http://vocab.nerc.ac.uk/collection/L05/current/308> ;
  skos:definition "The CNR4 is a net radiometer that measures the energy balance between incoming and shortwave IR radiation versus surface reflected shortwave and outgoing longwave IR radiation. The instrument comprises an upward-facing pyranometer/pyrgeometer pair, and a downward facing pair. There is an internal RTD, and a heater to prevent condensation."@en ;
  skos:inScheme <http://vocab.nerc.ac.uk/scheme/SDNDEV/current> ;
  skos:notation "SDN:L22::TOOL0703" ;
  skos:note "accepted"@en ;
  skos:prefLabel "Kipp and Zonen CNR1 Net Radiometer"@en ;
  skos:related <http://vocab.nerc.ac.uk/collection/B75/current/ORG00324> ;
.
inst:TOOL0722
  rdf:type skos:Concept ;
  dcterm:date "2014-07-09 16:23:06.0" ;
  dcterm:identifier "SDN:L22::TOOL0722" ;
  dcterm:source <http://vocab.nerc.ac.uk/scheme/SDNDEV/current> ;
  pav:hasCurrentVersion <http://vocab.nerc.ac.uk/collection/L22/current/TOOL0722/1> ;
  owl:versionInfo "1" ;
  skos:altLabel "Middleton EQ08"@en ;
  skos:broader <http://vocab.nerc.ac.uk/collection/L05/current/308> ;
  skos:definition "The Middleton EQ08 Solar Pyranometer is designed for the measurement of global solar irradiance on a plane surface. It has a response time (to 95%) of less than 11 seconds; zero offset at 200 W/m2 of less than 3 W/m2 and at 5K/h of less than 2W/m2; non-linearity of less than 0.5 percent; directional response with respect to 1000 W/m2 of less than 15 W/m2, Spectral selectivity (0.35 to 1.5 um) of less than 3 percent; temperature response (for 50K interval) of less than 2 percent; and tilt response (0-90 degrees) of less than 0.35 percent."@en ;
  skos:inScheme <http://vocab.nerc.ac.uk/scheme/SDNDEV/current> ;
  skos:notation "SDN:L22::TOOL0722" ;
  skos:note "accepted"@en ;
  skos:prefLabel "Middleton Solar EQ08 Pyranometer"@en ;
  skos:related <http://vocab.nerc.ac.uk/collection/B75/current/ORG00835> ;
.
inst:TOOL0723
  rdf:type skos:Concept ;
  dcterm:date "2014-07-09 16:23:06.0" ;
  dcterm:identifier "SDN:L22::TOOL0723" ;
  dcterm:source <http://vocab.nerc.ac.uk/scheme/SDNDEV/current> ;
  pav:hasCurrentVersion <http://vocab.nerc.ac.uk/collection/L22/current/TOOL0723/1> ;
  owl:versionInfo "1" ;
  skos:altLabel "Middleton SK01-DP2"@en ;
  skos:broader <http://vocab.nerc.ac.uk/collection/L05/current/308> ;
  skos:definition "The Middleton SK01-DP2 PAR Sensor (or Quantum Sensor) is for measuring electromagnetic radiation  at Photosynthetically Active wavelengths. It uses a silicon photodiode detector, shielded by a cosine-corrected diffuser and an interference reflector, to measure PAR on a horizontal surface. The detector is boosted by a low noise amplifier that is drift stabilised. The SK01-DP2 features: viewing angle 2*pi steradians; spectral range of 400-700nm; irradiance of 0-3000 umol/s/m2; sensitivity of 0.5 mV/umol/s/m2; response time (to 95 percent) of 30 ms; operating temperature of -35 to 60 degreesC; non-linearity of less than 1 percent; spectral response of +/- 5 percent."@en ;
  skos:inScheme <http://vocab.nerc.ac.uk/scheme/SDNDEV/current> ;
  skos:notation "SDN:L22::TOOL0723" ;
  skos:note "accepted"@en ;
  skos:prefLabel "Middleton Solar SK01-DP2 Pyranometer"@en ;
  skos:related <http://vocab.nerc.ac.uk/collection/B75/current/ORG00835> ;
.
inst:TOOL0844
  rdf:type skos:Concept ;
  dcterm:date "2015-04-28 12:36:02.0" ;
  dcterm:identifier "SDN:L22::TOOL0844" ;
  dcterm:source <http://vocab.nerc.ac.uk/scheme/SDNDEV/current> ;
  pav:hasCurrentVersion <http://vocab.nerc.ac.uk/collection/L22/current/TOOL0844/1> ;
  owl:versionInfo "1" ;
  skos:altLabel "Pico-Technology PT-100"@en ;
  skos:broader <http://vocab.nerc.ac.uk/collection/L05/current/302> ;
  skos:definition "The platinum resistance thermometer offers a temperature range from -50 deg C to 250 deg C an accuracy of +/- 0.03 deg C at 0 deg C"@en ;
  skos:inScheme <http://vocab.nerc.ac.uk/scheme/SDNDEV/current> ;
  skos:notation "SDN:L22::TOOL0844" ;
  skos:note "accepted"@en ;
  skos:prefLabel "Pico-Technology PT-100 Temperature Sensor Model SE012"@en ;
  skos:related <http://vocab.nerc.ac.uk/collection/B75/current/ORG00837> ;
.
inst:TOOL0867
  rdf:type skos:Concept ;
  dcterm:date "2016-04-11 16:29:35.0" ;
  dcterm:identifier "SDN:L22::TOOL0867" ;
  dcterm:source <http://vocab.nerc.ac.uk/scheme/SDNDEV/current> ;
  pav:hasCurrentVersion <http://vocab.nerc.ac.uk/collection/L22/current/TOOL0867/2> ;
  pav:hasVersion <http://vocab.nerc.ac.uk/collection/L22/current/TOOL0867/1> ;
  owl:versionInfo "2" ;
  skos:altLabel "SeaWiFS"@en ;
  skos:broader <http://vocab.nerc.ac.uk/collection/L05/current/304> ;
  skos:definition "The Sea-viewing Wide Field-of-view Sensor (SeaWiFS) is an optical scanner designed to provide quantitative ocean colour data for derivation of global ocean bio-optical properties. Incoming radiation is collected by a folded telescope and reflected onto a rotating half-angle mirror. The collected radiation is relayed through dichroic beam splitters to separate it into four wavelength intervals, each of which is directed through two spectral bandpass filters to further separate it into the eight SeaWiFS spectral bands, imaged onto one of four detectors and amplified for processing. The scanning telescope rotates at a rate of six revolutions per second, and a scanner tilt mechanism enables the instrument to tilt from -20 degrees to +20 degrees to avoid sun glint from the sea surface. The SeaWiFS instrument has a spatial resolution of 1.6 mrads, and measures radiation in eight optical bands: 402-422nm; 433-453nm; 480-500nm; 500-520nm; 545-565nm; 660-680nm; 745-785nm; 845-885nm. For more information visit http://oceancolor.gsfc.nasa.gov/SeaWiFS/SEASTAR/SPACECRAFT.html."@en ;
  skos:inScheme <http://vocab.nerc.ac.uk/scheme/SDNDEV/current> ;
  skos:notation "SDN:L22::TOOL0867" ;
  skos:note "accepted"@en ;
  skos:prefLabel "Sea-viewing Wide Field-of-view Sensor - SeaWiFS"@en ;
  skos:related <http://vocab.nerc.ac.uk/collection/B75/current/ORG00959> ;
.
inst:TOOL0912
  rdf:type skos:Concept ;
  dcterm:date "2015-07-15 10:34:42.0" ;
  dcterm:identifier "SDN:L22::TOOL0912" ;
  dcterm:source <http://vocab.nerc.ac.uk/scheme/SDNDEV/current> ;
  pav:hasCurrentVersion <http://vocab.nerc.ac.uk/collection/L22/current/TOOL0912/1> ;
  owl:versionInfo "1" ;
  skos:altLabel "RMR PRP model 1 solar radiation"@en ;
  skos:broader <http://vocab.nerc.ac.uk/collection/L05/current/308> ;
  skos:definition "An integrated system for making measurements of atmospheric downwelling radiation on moving platforms. The system consists of an Eppley Precision Solar Pyranometer (PSP) which measures total broadband (0.285 to 2.8 um) downwelling shortwave (solar) irradiance, an Eppley Precision Infrared Pyrgeometer (PIR) which measures the broadband (4-50 um) downwelling longwave irradiance, and a Brookhaven National Laboratory Fast-Rotating Shadowband Radiometer which decomposes incoming shortwave irradiance into direct-beam and diffuse (sky) irradiance and these are used to compute the aerosol optical depth (AOD) in six 10 nm wide bands (415, 500, 615, 680, 870, 940 nm). A seventh band is a broad open Si cell. The PRP also includes a pitch-roll-FG compass sensor to compensate for measurements on moving platforms."@en ;
  skos:inScheme <http://vocab.nerc.ac.uk/scheme/SDNDEV/current> ;
  skos:notation "SDN:L22::TOOL0912" ;
  skos:note "accepted"@en ;
  skos:prefLabel "Remote Measurement and Research Co. Portable Radiation Package model 1"@en ;
  skos:related <http://vocab.nerc.ac.uk/collection/B75/current/ORG00977> ;
.
inst:TOOL0930
  rdf:type skos:Concept ;
  dcterm:date "2015-08-04 13:54:57.0" ;
  dcterm:identifier "SDN:L22::TOOL0930" ;
  dcterm:source <http://vocab.nerc.ac.uk/scheme/SDNDEV/current> ;
  pav:hasCurrentVersion <http://vocab.nerc.ac.uk/collection/L22/current/TOOL0930/1> ;
  owl:versionInfo "1" ;
  skos:altLabel "Sea-Therm 4000L TS"@en ;
  skos:broader <http://vocab.nerc.ac.uk/collection/L05/current/302> ;
  skos:definition "A rugged temperature sensor designed to measure water surface temperature in harsh environments such as oil platforms. It is a non-contact system that measures infra-red radiation with a second senor - the Sky Spy - that provides input for sky radiation correction. It measures temperatures in the range -10-70C with an accuracy of 0.3C below 30C and 0.5C above 30C. The standard field of view is 10 degrees with 5 and 2 degrees available as options. The sensor is encased in a solid block of plastic hermetically sealed into a titanium case to provide waterproofing and resistance to salt spray."@en ;
  skos:inScheme <http://vocab.nerc.ac.uk/scheme/SDNDEV/current> ;
  skos:notation "SDN:L22::TOOL0930" ;
  skos:note "accepted"@en ;
  skos:prefLabel "Everest Interscience Sea-Therm 4000L temperature sensor"@en ;
  skos:related <http://vocab.nerc.ac.uk/collection/B75/current/ORG00985> ;
.
inst:TOOL1016
  rdf:type skos:Concept ;
  dcterm:date "2017-08-10 12:25:40.0" ;
  dcterm:identifier "SDN:L22::TOOL1016" ;
  dcterm:source <http://vocab.nerc.ac.uk/scheme/SDNDEV/current> ;
  pav:hasCurrentVersion <http://vocab.nerc.ac.uk/collection/L22/current/TOOL1016/2> ;
  pav:hasVersion <http://vocab.nerc.ac.uk/collection/L22/current/TOOL1016/1> ;
  owl:versionInfo "2" ;
  skos:altLabel "UOS ISAR SST"@en ;
  skos:broader <http://vocab.nerc.ac.uk/collection/L05/current/302> ;
  skos:definition "An autonomous radiometer developed by the University of Southampton (UK) and Brookhaven National Laboratories (US) for satellite Sea Surface Temperature (SST) validation and other scientific programs. It detects infrared temperature using a single channel with a spectral bandpass of 9.6-11.5 um. It is compact (570 mm  220 mm cylinder) and employs two reference blackbody cavities to maintain the radiance calibration of a special Heitronics KT15.85D radiometer to an accuracy of +/-0.1K. It has a temperature range of 173-373 K. It can be deployed continuously on voluntary observing ships (VOS) without any service requirement or operator intervention for periods of up to 3 months. http://dx.doi.org/10.1175/2007JTECHO505.1"@en ;
  skos:inScheme <http://vocab.nerc.ac.uk/scheme/SDNDEV/current> ;
  skos:notation "SDN:L22::TOOL1016" ;
  skos:note "accepted"@en ;
  skos:prefLabel """University of Southampton ISAR SST radiometer
"""@en ;
  skos:related <http://vocab.nerc.ac.uk/collection/B75/current/ORG00016> ;
.
inst:TOOL1034
  rdf:type skos:Concept ;
  dcterm:date "2016-11-10 12:55:24.0" ;
  dcterm:identifier "SDN:L22::TOOL1034" ;
  dcterm:source <http://vocab.nerc.ac.uk/scheme/SDNDEV/current> ;
  pav:hasCurrentVersion <http://vocab.nerc.ac.uk/collection/L22/current/TOOL1034/1> ;
  owl:versionInfo "1" ;
  skos:altLabel "Unknown microscope"@en ;
  skos:broader sdev:LAB05 ;
  skos:definition "A generic term for an inverted (the light source illuminates the specimen from above) optical microscope."@en ;
  skos:inScheme <http://vocab.nerc.ac.uk/scheme/SDNDEV/current> ;
  skos:notation "SDN:L22::TOOL1034" ;
  skos:note "accepted"@en ;
  skos:prefLabel "Inverted Microscope (generic)"@en ;
  skos:related <http://vocab.nerc.ac.uk/collection/B75/current/UNSPEC> ;
.
inst:TOOL1035
  rdf:type skos:Concept ;
  dcterm:date "2016-11-15 14:35:44.0" ;
  dcterm:identifier "SDN:L22::TOOL1035" ;
  dcterm:source <http://vocab.nerc.ac.uk/scheme/SDNDEV/current> ;
  pav:hasCurrentVersion <http://vocab.nerc.ac.uk/collection/L22/current/TOOL1035/3> ;
  pav:hasVersion <http://vocab.nerc.ac.uk/collection/L22/current/TOOL1035/1> ;
  pav:hasVersion <http://vocab.nerc.ac.uk/collection/L22/current/TOOL1035/2> ;
  owl:versionInfo "3" ;
  skos:altLabel "MODIS"@en ;
  skos:broader <http://vocab.nerc.ac.uk/collection/L05/current/304> ;
  skos:broader <http://vocab.nerc.ac.uk/collection/L05/current/308> ;
  skos:definition "The Moderate Resolution Imaging Spectroradiometer (MODIS) is an optical spectroradiometer that acquires photo-radometric data of terrestrial, oceanic and lower atmospheric environments for the study of global dynamics. Incoming radiation is directed by a continuously rotating double-sided scan mirror, scanning from -50 to +50 degrees. It directs radiation into a two-mirror off-axis afocal telescope. A dichroic beam splitter then splits the radiation into four optical objective and focal plane assemblies. There are separate assemblies for both near infrared (short and long-wave) and visible spectral bands. These are further split into 36 spectral bands ranging in wavelength from 0.4 to 14.4 micrometres. Bands 1-2 are imaged at a nominal spatial resolution of 250 m at nadir, with bands 3-7 at 500 m and the remaining bands (8-36) at 1 km.  The MODIS instrument has a cross track scan rate of 20.3 rpm, and measures radiation in 36 optical bands (bands 1-19 are in nanometres and bands 20-36 are in micrometres): 620-670 nm; 841-876 nm; 459-479 nm; 545-565 nm; 1230-1250 nm; 1628-1652 nm; 2105-2155 nm; 405-420 nm; 438-448 nm; 483-493 nm; 526-536 nm; 546-556 nm; 662-672 nm; 673-683 nm; 743-753 nm; 862-877 nm; 890-920 nm; 931-941 nm; 915-965 nm; 3.660-3.840 micrometres; 3.929-3.989 micrometres; 3.929-3.989 micrometres; 4.020-4.080 micrometres; 4.433-4.498 micrometres; 4.482-4.549 micrometres; 1.360-1.390 micrometres; 6.535-6.895 micrometres; 7.175-7.475 micrometres; 8.400-8.700 micrometres; 9.580-9.880 micrometres; 10.780-11.280 micrometres; 13.185-13.485 micrometres; 13.485-13.785 micrometres; 13.785-14.085 micrometres; 14.085-14.385 micrometres. Flown on Terra, Aqua. http://modis.gsfc.nasa.gov/about/"@en ;
  skos:inScheme <http://vocab.nerc.ac.uk/scheme/SDNDEV/current> ;
  skos:notation "SDN:L22::TOOL1035" ;
  skos:note "accepted"@en ;
  skos:prefLabel "Moderate Resolution Imaging Spectroradiometer"@en ;
.
inst:TOOL1036
  rdf:type skos:Concept ;
  dcterm:date "2016-11-15 14:35:44.0" ;
  dcterm:identifier "SDN:L22::TOOL1036" ;
  dcterm:source <http://vocab.nerc.ac.uk/scheme/SDNDEV/current> ;
  pav:hasCurrentVersion <http://vocab.nerc.ac.uk/collection/L22/current/TOOL1036/2> ;
  pav:hasVersion <http://vocab.nerc.ac.uk/collection/L22/current/TOOL1036/1> ;
  owl:versionInfo "2" ;
  skos:altLabel "MSS"@en ;
  skos:broader <http://vocab.nerc.ac.uk/collection/L05/current/309> ;
  skos:definition "The Multispectral Scanner System (MSS) is a high resolution optical imager designed to measure Earth's surface reflectance in four optical bands in the visible and near-infrared spectrums, for use in monitoring the global land surface and vegetation cover.  Earth-reflected sunlight is detected by an oscillating cross-track scan mirror, which scans six lines simultaneously in four spectral bands per mirror sweep. Two of these bands are in the visible spectrum, with the remaining two in the near-infrared spectrum. The four spectral bands have a spatial resolution of 79m. Their wavelengths are 0.5-0.6 micrometres, 0.6-0.7 micrometeres, 0.7-0.8 micrometres, and 0.8-1.1 micrometres. MSS has a swath width of 185 km and an 80 m instantaneous field of view (IFOV). Flown on Landsat. http://www.wmo-sat.info/oscar/instruments/view/316"@en ;
  skos:inScheme <http://vocab.nerc.ac.uk/scheme/SDNDEV/current> ;
  skos:notation "SDN:L22::TOOL1036" ;
  skos:note "accepted"@en ;
  skos:prefLabel "Multispectral Scanner System"@en ;
.
inst:TOOL1037
  rdf:type skos:Concept ;
  dcterm:date "2016-11-15 14:35:44.0" ;
  dcterm:identifier "SDN:L22::TOOL1037" ;
  dcterm:source <http://vocab.nerc.ac.uk/scheme/SDNDEV/current> ;
  pav:hasCurrentVersion <http://vocab.nerc.ac.uk/collection/L22/current/TOOL1037/2> ;
  pav:hasVersion <http://vocab.nerc.ac.uk/collection/L22/current/TOOL1037/1> ;
  owl:versionInfo "2" ;
  skos:altLabel "MWRI"@en ;
  skos:broader <http://vocab.nerc.ac.uk/collection/L05/current/308> ;
  skos:broader <http://vocab.nerc.ac.uk/collection/L05/current/309> ;
  skos:definition "The Microwave Radiation Imager (MWRI) is a conical-scanning microwave imaging radiometer designed to measure precipitation, soil moisture, vegetation, cloud liquid water and sea surface parameters such as wind. The MWRI gathers light through a ground-pointing telescope, whose scan mirror oscillates (1 cycle every 33 milliseconds) over an angular displacement of plus-or-minus 2.89 degrees that is perpendicular to the orbital track. Light reflected from the surface and atmosphere as gathered by this scan passes through an optical lens train, during which the beam is divided to pass through 4 bandpass filters that produce images in 4 spectral bands. The light from each filter then reaches a set of six electronic detectors (24 in total, 6 per spectral band) that subdivides the across-track scan into 6 parallel lines, each equivalent to a ground width of 79 m.  The MWRI features 10 channels with five frequencies in the range 10.65-89 GHz. The nadir spatial resolution range varies from 15-85 km depending on frequency. The wavelengths of the four spectral bands are 0.5-0.6 micrometres, 0.6-0.7 micrometres, 0.7-0.8 micrometres and 0.8-1.1 micrometres. The instrument has a swath width of 1400 km and a scan rate of 35.3 scan/min, or 11.2 km/scan. Flown on FY-3. http://www.wmo-sat.info/oscar/instruments/view/350"@en ;
  skos:inScheme <http://vocab.nerc.ac.uk/scheme/SDNDEV/current> ;
  skos:notation "SDN:L22::TOOL1037" ;
  skos:note "accepted"@en ;
  skos:prefLabel "Micro-Wave Radiation Imager"@en ;
.
inst:TOOL1038
  rdf:type skos:Concept ;
  dcterm:date "2017-08-10 12:25:40.0" ;
  dcterm:identifier "SDN:L22::TOOL1038" ;
  dcterm:source <http://vocab.nerc.ac.uk/scheme/SDNDEV/current> ;
  pav:hasCurrentVersion <http://vocab.nerc.ac.uk/collection/L22/current/TOOL1038/3> ;
  pav:hasVersion <http://vocab.nerc.ac.uk/collection/L22/current/TOOL1038/1> ;
  pav:hasVersion <http://vocab.nerc.ac.uk/collection/L22/current/TOOL1038/2> ;
  owl:versionInfo "3" ;
  skos:altLabel "OLI"@en ;
  skos:broader <http://vocab.nerc.ac.uk/collection/L05/current/309> ;
  skos:broader <http://vocab.nerc.ac.uk/collection/L05/current/311> ;
  skos:definition "The Operational Land Imager (OLI) is a high resolution optical imager designed for land and vegetation observation. It measures in the visible, near-infrared, and short-wave infrared spectrums over nine spectral bands.  The OLI uses long detector arrays (of over 7000 detectors per spectral band) aligned across its focal plane to view across the swath. A four-mirror anastigmatic telescope focuses incident radiation onto the focal plane while providing a 15 degree field of view (FOV). Periodic sampling of the cross-track detectors as the observatory progresses along a ground track forms the multispectral digital images. The detectors are divided into 14 modules arranged in an alternating pattern along the centreline of the focal plane. The spectral differentiation is achieved by interference filters arranged in a butcher-block pattern over the detector arrays in each module. Silicon PIN (SiPIN) detectors collect the data for the visible and near-infrared spectral bands (bands 1 to 4 and 8) while Mercury-Cadmium-Telluride (MgCdTe) detectors are used for the shortwave infrared bands (bands 6, 7, and 9). The OLI has a swath width of 185 km and produces images with a 30 m multi-spectral spatial resolution. The wavelengths of the nine spectral bands are 0.433-0.453 micrometres, 0.450-0.515 micrometres, 0.525-0.600 micrometres, 0.630-0.680 micrometres, 0.845-0.885 micrometres, 1.560-1.660 micrometres,  2.100-2.300 micrometres,  0.500-0.680 micrometres and 1.360-1.390 micrometres. The OLI produced data calibrated to an uncertainty of less than 5 percent in terms of absolute, at-aperture spectral radiance and to an uncertainty of less than 3 percent in terms of top-of-atmosphere spectral reflectance for each of the spectral bands. Flown on Landsat. http://www.wmo-sat.info/oscar/instruments/view/375"@en ;
  skos:inScheme <http://vocab.nerc.ac.uk/scheme/SDNDEV/current> ;
  skos:notation "SDN:L22::TOOL1038" ;
  skos:note "accepted"@en ;
  skos:prefLabel "Operational Land Image"@en ;
.
inst:TOOL1039
  rdf:type skos:Concept ;
  dcterm:date "2016-11-15 14:35:44.0" ;
  dcterm:identifier "SDN:L22::TOOL1039" ;
  dcterm:source <http://vocab.nerc.ac.uk/scheme/SDNDEV/current> ;
  pav:hasCurrentVersion <http://vocab.nerc.ac.uk/collection/L22/current/TOOL1039/2> ;
  pav:hasVersion <http://vocab.nerc.ac.uk/collection/L22/current/TOOL1039/1> ;
  owl:versionInfo "2" ;
  skos:altLabel "OMI"@en ;
  skos:broader <http://vocab.nerc.ac.uk/collection/L05/current/314> ;
  skos:definition "The Ozone Monitoring Instrument (OMI) is a cross-nadir scanning sounder which follows on from NASA's Total Ozone Mapping Spectrometer (TOMS). OMI is designed to monitor recovery of the ozone layer by measuring different aerosols (smoke, dust, sulfates) and other criteria pollutants such as O3 (ozone), NO2 (nitrogen dioxide), BrO (bromine) and chlorine dioxide (OCLO). The OMI observes Earth's solar backscattered radiation in the visible and ultraviolet spectrums with a wide-field telescope, using hyperspectral imaging in a push-broom mode. This feeds two imaging grating spectrometers, each of which employs a charged coupled device (CCD) detector. Onboard calibration includes a white light source, LEDs, and a multi-surface solar-calibration diffuser. A depolariser removes the polarisation from the backscattered radiation. The OMI has a 13 x 24 km spatial resolution which can be zoomed to 13 x 13 km for detecting and tracking urban-scale pollution sources. The OMI employs three spectral bands, with wavelengths detected in the visible spectrum from 350 - 500 nm (band 1) and wavelengths detected in the ultraviolet spectrum from 270 - 314 nm (band 2) and  306 - 380 nm (band 3). In total there are 1560 channels across the tree bands. The overall spectral resolution of the OMI is from 0.45 -1.0 nm for full width at half maximum (FWHM). Flown on Aura. http://www.wmo-sat.info/oscar/instruments/view/377"@en ;
  skos:inScheme <http://vocab.nerc.ac.uk/scheme/SDNDEV/current> ;
  skos:notation "SDN:L22::TOOL1039" ;
  skos:note "accepted"@en ;
  skos:prefLabel "Ozone Monitoring Instrument"@en ;
.
inst:TOOL1040
  rdf:type skos:Concept ;
  dcterm:date "2016-11-15 14:35:44.0" ;
  dcterm:identifier "SDN:L22::TOOL1040" ;
  dcterm:source <http://vocab.nerc.ac.uk/scheme/SDNDEV/current> ;
  pav:hasCurrentVersion <http://vocab.nerc.ac.uk/collection/L22/current/TOOL1040/2> ;
  pav:hasVersion <http://vocab.nerc.ac.uk/collection/L22/current/TOOL1040/1> ;
  owl:versionInfo "2" ;
  skos:altLabel "OSIRIS"@en ;
  skos:broader <http://vocab.nerc.ac.uk/collection/L05/current/314> ;
  skos:definition "The OpticalSpectrograph and infraredImagerSystem (OSIRIS) is a limb-scanning spectrometer. It measures vertical profiles of spectrally dispersed, limb-scattered sunlight from the upper troposphere into the lower mesosphere to produce height profiles of O3 (ozone), NO2 (nitrogen dioxide) and stratospheric aerosols. It operates in the visible, near-infrared and near-ultraviolet spectrums.  The OSIRIS instrument is essentially two optical subsystems, suggested by its name: an optical spectrograph (OS) module and an infrared imager (IRI) module. The OS is a grating spectrometer with a CCD (charged coupled device) detector. Vertical profiles of the limb radiance are obtained by taking OS exposures while performing a repetitive vertical scan of the single line-of-sight through selected tangent altitude ranges (10 - 100 km). The IRI is composed of three vertical near infrared co-aligned linear array imagers that capture one-dimensional images of the limb radiance with a tangent altitude resolution of approximately 1 km. The imagers have parallel bore-sights; each one consists of an identical baffling system, lens, narrow-band interference filter, and a one-dimensional linear array of 128 thermo-electrically cooled photodetectors placed in the focal plane of the lens. Approximately 30 photodetector elements at one end of each array are covered with a mask in order to provide a continuous measure of the dark signal in the array. Therefore there are approximately 100 lines of sight from each imager channel that measure simultaneously over 100 vertical kilometres in tangent altitude. OSIRIS (OS) has a spectral range of 280 - 800 nm and a spectral resolution of 1 nm when at an altitude range of 5 -100 km. Each scan takes 40 - 70 seconds. The OS also has a minimum sensitivty of 12 kR per Angstrom per pixel. The IRI captures images of the limb radiance at at 1260, 1270, and 1530 nm and has a sensitivity of 50 kR per band per pixel. Flown on Odin. http://www.wmo-sat.info/oscar/instruments/view/383"@en ;
  skos:inScheme <http://vocab.nerc.ac.uk/scheme/SDNDEV/current> ;
  skos:notation "SDN:L22::TOOL1040" ;
  skos:note "accepted"@en ;
  skos:prefLabel "OpticalSpectrograph and infraredImagerSystem"@en ;
.
inst:TOOL1041
  rdf:type skos:Concept ;
  dcterm:date "2022-03-18 14:33:52.0" ;
  dcterm:identifier "SDN:L22::TOOL1041" ;
  dcterm:source <http://vocab.nerc.ac.uk/scheme/SDNDEV/current> ;
  pav:hasCurrentVersion <http://vocab.nerc.ac.uk/collection/L22/current/TOOL1041/3> ;
  pav:hasVersion <http://vocab.nerc.ac.uk/collection/L22/current/TOOL1041/1> ;
  pav:hasVersion <http://vocab.nerc.ac.uk/collection/L22/current/TOOL1041/2> ;
  owl:versionInfo "3" ;
  skos:altLabel "PALSAR"@en ;
  skos:broader <http://vocab.nerc.ac.uk/collection/L05/current/309> ;
  skos:definition "The Phased Array type L-band Synthetic Aperture Radar (PALSAR) is an active microwave sensor using L-band frequency to achieve high resolution cloud-free, day-and-night land observation, all-weather soil moisture observation and ocean surface features observation. PALSAR can observe in three different modes; fine-resolution mode, a secondary ScanSAR (burst mode SAR) observation mode for monitoring sea-ice and rainforest extent, and Polarimetric mode for receiving simultaneous horizontal and vertical polarisation (multi-polarimetry). PALSAR transmits successive pulses of radio waves to illuminate the target scene, and the echo of each pulse is received and recorded via an array of side-viewing beam-forming antennas. All elements of these arrays receive echos simultaneously in real time so the signals passing through them are individually subjected to controlled shifts of the phases of those signals. Signal processing of the successive recorded radar echoes allows the combining of the recordings from these multiple antenna positions to produce a high-resolution image. PALSAR has a centre frequency of 1270 MHz (L-band). In fine resolution mode, the swath width ranges from 40-70 km and a resolution of 7 - 44 m.  In ScanSAR mode, the swath width ranges from 250 350 km with a 100 m multi-look resolution. In polarimetric mode, the swath width ranges from 20 - 65 km with a spatial resolution of 24 - 89 m. Radiometric accuracy of the scene is 1 dB. Flown on ALOS. https://earth.esa.int/web/guest/missions/3rd-party-missions/historical-missions/alos/instruments/palsar"@en ;
  skos:inScheme <http://vocab.nerc.ac.uk/scheme/SDNDEV/current> ;
  skos:notation "SDN:L22::TOOL1041" ;
  skos:note "accepted"@en ;
  skos:prefLabel "Phased Array type L-band Synthetic Aperture Radar"@en ;
.
inst:TOOL1042
  rdf:type skos:Concept ;
  dcterm:date "2016-11-15 14:35:44.0" ;
  dcterm:identifier "SDN:L22::TOOL1042" ;
  dcterm:source <http://vocab.nerc.ac.uk/scheme/SDNDEV/current> ;
  pav:hasCurrentVersion <http://vocab.nerc.ac.uk/collection/L22/current/TOOL1042/2> ;
  pav:hasVersion <http://vocab.nerc.ac.uk/collection/L22/current/TOOL1042/1> ;
  owl:versionInfo "2" ;
  skos:altLabel "POLDER"@en ;
  skos:broader <http://vocab.nerc.ac.uk/collection/L05/current/308> ;
  skos:definition "POLDER (Polarisation and Directionality of the Earth's Reflectances) is a passive optical imaging radiometer and polarimeter designed to observe solar radiation reflected by Earth's atmosphere, including studies of tropospheric aerosols, sea surface reflectance, bidirectional reflectance distribution function of land surfaces, and the Earth Radiation Budget. It measures surface reflectance in the visible and near-infrared bands. POLDER consists consists of a digital staring camera composed of a 274 x 242 pixel CCD (charged coupled device) detection array, wide field-of-view telecentric optics (plus-or-minus 51 degrees cross-track and plus-or-minus 43 degrees along-track) and of a rotating wheel carrying spectral and polarised filters of an optical subsystem and electronics subsystem. The optical subsystem consists of a telecentric lens, a filter wheel and a CCD array as a detector. The light is almost vertically incident on the filter wheel after the telecentric lens makes the optical correction. The CCD array (244 x 274 elements) can collect two-dimensionnal images. The filter wheel has 16 filters and is rotated so that 16-channel images are acquired per one rotation. The main functions of electronics subsystem are to process imagery (eg. A/D conversion), to handle telemetry/command for operation of the processed image and POLDER and to control the filter wheel, the electric power and the heat. POLDER measures radiation in nine spectral bands with wavelengths centred at 443.5 nanometres (nm), 490.9 nm, 563.8 nm, 669.9 nm, 762.9 nm, 762.7 nm, 863.7 nm, 907.1 nm and 1019.6 nm. It has a total of 15 channels and 3 polarisations at 3 wavelengths. Flown on ADEOS, ADEOS-2, PARASOL. http://www.wmo-sat.info/oscar/instruments/view/405"@en ;
  skos:inScheme <http://vocab.nerc.ac.uk/scheme/SDNDEV/current> ;
  skos:notation "SDN:L22::TOOL1042" ;
  skos:note "accepted"@en ;
  skos:prefLabel "Polarisation andDirectionality of theEarth'sReflectances"@en ;
.
inst:TOOL1043
  rdf:type skos:Concept ;
  dcterm:date "2016-11-15 14:35:44.0" ;
  dcterm:identifier "SDN:L22::TOOL1043" ;
  dcterm:source <http://vocab.nerc.ac.uk/scheme/SDNDEV/current> ;
  pav:hasCurrentVersion <http://vocab.nerc.ac.uk/collection/L22/current/TOOL1043/2> ;
  pav:hasVersion <http://vocab.nerc.ac.uk/collection/L22/current/TOOL1043/1> ;
  owl:versionInfo "2" ;
  skos:altLabel "SSALT"@en ;
  skos:broader <http://vocab.nerc.ac.uk/collection/L05/current/186> ;
  skos:definition "SSALT (Single-frequency Solid-state Altimeter), alternatively referred to as Poseidon-1, is a radar altimeter designed to measure ocean topography, significant wave height and wind speed on sea surface. It was a low-power, low-mass test-bed for future space-borne altimeters. SSALT consists of two packages: the processing and control unit (PCU), and the radio frequency unit (RFU). SSALT sends a pulse generated by a surface acoustic wave generator with a 300 MHz bandwidth and 900 MHz frequency to the sea surface. The pulses are amplified before transmission, and frequency converted to 13.65 GHz after generation. The received pulses are also amplified and an FFT (fast fourier transform) analyser computes the power spectrum of the signal. The signal is sent through a microprocessor which performs the waveform computations to produce the output data.  SSALT operates at a single frequency of 13.65 GHz (Ku band), with a measurement accuracy within 10 cm (typically 2.5 cm).  Flown on TOPEX/Poseidon. https://directory.eoportal.org/web/eoportal/satellite-missions/t/topex-poseidon"@en ;
  skos:inScheme <http://vocab.nerc.ac.uk/scheme/SDNDEV/current> ;
  skos:notation "SDN:L22::TOOL1043" ;
  skos:note "accepted"@en ;
  skos:prefLabel "Single-frequency Solid-state Altimeter"@en ;
.
inst:TOOL1044
  rdf:type skos:Concept ;
  dcterm:date "2016-11-15 14:35:44.0" ;
  dcterm:identifier "SDN:L22::TOOL1044" ;
  dcterm:source <http://vocab.nerc.ac.uk/scheme/SDNDEV/current> ;
  pav:hasCurrentVersion <http://vocab.nerc.ac.uk/collection/L22/current/TOOL1044/2> ;
  pav:hasVersion <http://vocab.nerc.ac.uk/collection/L22/current/TOOL1044/1> ;
  owl:versionInfo "2" ;
  skos:altLabel "Poseidon-2"@en ;
  skos:broader <http://vocab.nerc.ac.uk/collection/L05/current/186> ;
  skos:definition "Poseidon-2 is a radar altimeter designed to measure ocean topography, significant wave height and surface wind speed. It is also able to measure the amount of rain in the atmosphere. The Poseidon-2 altimeter emits a radar beam that is reflected back to the antenna from the Earth's surface. Poseidon-2 operates at two frequencies (in the Ku and C bands) to determine atmospheric electron content, which affects the radar signal path delay. These two frequencies also serve to measure the amount of rain in the atmosphere. Poseidon-2 operates at 13.6 GHz in the Ku band and 5.3 GHz in the C band. It has a pulse duration of 105 microseconds and a bandwidth of 320 MHz. The altimeter is nadir-only viewing, sampling at 30 km intervals along-track. Flown on JASON-1. http://www.aviso.altimetry.fr/en/missions/past-missions/jason-1/instruments/poseidon-2.html"@en ;
  skos:inScheme <http://vocab.nerc.ac.uk/scheme/SDNDEV/current> ;
  skos:notation "SDN:L22::TOOL1044" ;
  skos:note "accepted"@en ;
  skos:prefLabel "Poseidon-2"@en ;
.
inst:TOOL1045
  rdf:type skos:Concept ;
  dcterm:date "2016-11-15 14:35:44.0" ;
  dcterm:identifier "SDN:L22::TOOL1045" ;
  dcterm:source <http://vocab.nerc.ac.uk/scheme/SDNDEV/current> ;
  pav:hasCurrentVersion <http://vocab.nerc.ac.uk/collection/L22/current/TOOL1045/2> ;
  pav:hasVersion <http://vocab.nerc.ac.uk/collection/L22/current/TOOL1045/1> ;
  owl:versionInfo "2" ;
  skos:altLabel "Poseidon-3"@en ;
  skos:broader <http://vocab.nerc.ac.uk/collection/L05/current/186> ;
  skos:definition "The Poseidon-3 radar altimeter is the main instrument on the Jason-2 mission. Derived from the Poseidon-1 altimeter on TOPEX/Poseidon and the Poseidon-2 on Jason-1, it measures sea level, wave heights and wind speed. The Poseidon-3 altimeter emits pulses at two frequencies  to measure the distance from the satellite to the surface (range). Free electrons in the atmosphere can delay the signal's return, affecting the measurement accuracy. The delay is directly related to the radar frequency, so the difference between the two measurements can be used to determine atmospheric electron content. Poseidon-3 is coupled with Doris/Diode, to improve measurements over coastal areas, inland waters and ice. Poseidon-3 emits pulses at 13.6 and 5.3 GHz in the C band, with pulse duration at 105 microseconds. Flown on JASON-2. http://sealevel.jpl.nasa.gov/technology/technologyinstrumentdescription/instrumentdescriptaltimeter/"@en ;
  skos:inScheme <http://vocab.nerc.ac.uk/scheme/SDNDEV/current> ;
  skos:notation "SDN:L22::TOOL1045" ;
  skos:note "accepted"@en ;
  skos:prefLabel "Poseidon-3"@en ;
.
inst:TOOL1046
  rdf:type skos:Concept ;
  dcterm:date "2016-11-15 14:35:44.0" ;
  dcterm:identifier "SDN:L22::TOOL1046" ;
  dcterm:source <http://vocab.nerc.ac.uk/scheme/SDNDEV/current> ;
  pav:hasCurrentVersion <http://vocab.nerc.ac.uk/collection/L22/current/TOOL1046/2> ;
  pav:hasVersion <http://vocab.nerc.ac.uk/collection/L22/current/TOOL1046/1> ;
  owl:versionInfo "2" ;
  skos:altLabel "RA"@en ;
  skos:broader <http://vocab.nerc.ac.uk/collection/L05/current/186> ;
  skos:definition "The Radar Altimeter (RA) is a nadir-pointing active microwave sensor designed to measure the time return echoes from ocean and ice surfaces. Functioning in one of two operational modes (ocean or ice), the Radar Altimeter provides information on significant wave height, surface wind speed, sea surface elevation which relates to ocean currents, the surface geoid and tides, plus various parameters over sea ice and ice sheets. RA operates by timing the two-way delay for a short duration radio frequency pulse, transmitted vertically downwards. The required level of accuracy in range measurement calls for a pulse compression (chirp) technique. In ocean mode a chirped pulse of 20 microsecond duration is generated with a band width of 330 MHz. For tracking in ice mode an increased dynamic range is used, obtained by reducing the chirp bandwidth by a factor of four to 82.5 MHz, though resulting in a coarser resolution. RA operates in the Ku-band at 13.8 GHz, with an accuracy in range better than 10cm. Flown on ERS-1, ERS-2. https://earth.esa.int/web/guest/missions/esa-operational-eo-missions/ers/instruments/ra"@en ;
  skos:inScheme <http://vocab.nerc.ac.uk/scheme/SDNDEV/current> ;
  skos:notation "SDN:L22::TOOL1046" ;
  skos:note "accepted"@en ;
  skos:prefLabel "Radar Altimeter"@en ;
.
inst:TOOL1047
  rdf:type skos:Concept ;
  dcterm:date "2016-11-15 14:35:44.0" ;
  dcterm:identifier "SDN:L22::TOOL1047" ;
  dcterm:source <http://vocab.nerc.ac.uk/scheme/SDNDEV/current> ;
  pav:hasCurrentVersion <http://vocab.nerc.ac.uk/collection/L22/current/TOOL1047/2> ;
  pav:hasVersion <http://vocab.nerc.ac.uk/collection/L22/current/TOOL1047/1> ;
  owl:versionInfo "2" ;
  skos:altLabel "RA-2"@en ;
  skos:broader <http://vocab.nerc.ac.uk/collection/L05/current/186> ;
  skos:definition "Radar Altimeter 2 (RA-2) is a dual-frequency, nadir-pointing, pulse-limited active microwave sensor designed to measure the two-way delay of the radar echo from the Earth's surface. RA-2 also measures the power and the shape of the reflected radar pulses.  It's design is based on the heritage of ERS-1 Radar Altimeter (RA). RA-2  transmits frequency modulated pulses (chirp) pulses. This frequency modulation is a coding of the signal which spreads the energy of a short pulse over a longer time interval, thus allowing reduced peak power in the pulse. The transmit pulses, which are generated in the chirp generator (by means of SAW  RAC) are amplified by either Ku-band or S-Band amplifiers, depending on the selected transmit frequency. The Ku-band HPA uses a traveling wave tube whilst the S-band transmitter applies the solid state technology. The Ku-band front end electronics (KFEE) or the S-band front end electronics (SFEE) feed the signals to be transmitted to the antenna which is designed as a dual-frequency parabolic antenna.  RA-2  operates at 13.575 GHz (Ku-band) and 3.2 GHz (S-Band) and at high precision at less than a nanosecond. It measures the power level and time delay of 128 samples of echoes from ocean, ice, and land surfaces. It is optimised to maintain the leading edge of this echo in the range window. Flown on Envisat. https://earth.esa.int/web/guest/missions/esa-operational-eo-missions/envisat/instruments/ra-2"@en ;
  skos:inScheme <http://vocab.nerc.ac.uk/scheme/SDNDEV/current> ;
  skos:notation "SDN:L22::TOOL1047" ;
  skos:note "accepted"@en ;
  skos:prefLabel "Radar Altimeter 2"@en ;
.
inst:TOOL1048
  rdf:type skos:Concept ;
  dcterm:date "2016-11-15 14:35:44.0" ;
  dcterm:identifier "SDN:L22::TOOL1048" ;
  dcterm:source <http://vocab.nerc.ac.uk/scheme/SDNDEV/current> ;
  pav:hasCurrentVersion <http://vocab.nerc.ac.uk/collection/L22/current/TOOL1048/2> ;
  pav:hasVersion <http://vocab.nerc.ac.uk/collection/L22/current/TOOL1048/1> ;
  owl:versionInfo "2" ;
  skos:altLabel "SCIAMACHY"@en ;
  skos:broader <http://vocab.nerc.ac.uk/collection/L05/current/314> ;
  skos:definition "The Scanning Imaging Absorption spectrometer for Atmospheric Chartography (SCIAMACHY) is an imaging spectrometer designed for the global measurement of trace gases, aerosols and clouds in the troposphere and stratosphere via observation of transmitted, back scattered and reflected radiation from the atmosphere. The instrument consists of a nadir and limb scanning component. Measurements are performed by observing the atmosphere under different viewing angles. In Nadir Mode, global distribution (total column values) of the atmospheric trace gases, clouds and aerosols are observed. In this mode, the instrument is scanning across-track. To obtain the altitude distribution of trace gases, SCIAMACHY performs observations in limb over an altitude range of 100 km, with a vertical resolution of 3 km. Light from the atmosphere is fed by the scanner unit consisting of an azimuth and an elevation scanner into the telescope which directs it onto the entrance slit of the spectrometer. The spectrometer contains a pre-disperser which separates the light into three spectral bands followed by a series of dichroic mirrors which further divide the light into a total of eight channels. A grating is located in each channel to diffract the light into a high resolution spectrum which is then focused onto eight detectors. The pre-disperser also serves as a Brewster window to separate polarised light, a part of which is sensed by the Polarisation Measurement Device (PMD). The output of the PMD is later used to correct for the polarisation effects. SCIAMACHY has a resolution ranging from 0.2 to 0.5 nm, and operates in wavelengths over the range 240 to 1700 nm, and 2000 to 2400 nm. Flown on Envisat. https://earth.esa.int/web/guest/missions/esa-operational-eo-missions/envisat/instruments/sciamachy"@en ;
  skos:inScheme <http://vocab.nerc.ac.uk/scheme/SDNDEV/current> ;
  skos:notation "SDN:L22::TOOL1048" ;
  skos:note "accepted"@en ;
  skos:prefLabel "SCanningImagingAbsorption spectroMeter forAtmospheric CHartographY"@en ;
.
inst:TOOL1049
  rdf:type skos:Concept ;
  dcterm:date "2017-08-10 12:37:04.0" ;
  dcterm:identifier "SDN:L22::TOOL1049" ;
  dcterm:source <http://vocab.nerc.ac.uk/scheme/SDNDEV/current> ;
  pav:hasCurrentVersion <http://vocab.nerc.ac.uk/collection/L22/current/TOOL1049/3> ;
  pav:hasVersion <http://vocab.nerc.ac.uk/collection/L22/current/TOOL1049/1> ;
  pav:hasVersion <http://vocab.nerc.ac.uk/collection/L22/current/TOOL1049/2> ;
  owl:versionInfo "3" ;
  skos:altLabel "SEVIRI"@en ;
  skos:broader <http://vocab.nerc.ac.uk/collection/L05/current/308> ;
  skos:definition "The Spinning Enhanced Visible and Infrared Imager (SEVIRI) is an optical imaging radiometer designed for cloud imaging and tracking, fog detection, measurement of the Earth-surface and cloud-top temperatures, and the tracking of ozone patterns. This enables analysis of the characteristics of atmospheric air masses to reconstruct a three-dimensional view of the atmosphere. The SEVIRI instrument is composed of a Telescope and Scan Assembly (TSA), a Focal Plane and Cooler Assembly (FPCA), and an Electronic Unit Assembly (EUA). SEVIRI  has 12 channels; 8 in the infrared, 1 in the high resolution visible, 2 in the visible, and 1 in the near-infrared spectrums. The scanning mirror is used to move the instrument line-of-sight (LOS) in the south-north direction. The target radiance is collected by the telescope and focused onto the detectors. Channel separation is performed at telescope focal-plane level, by means of folding mirrors. A flip-flop type mechanism is periodically actuated to place the IR calibration reference source in the instrument's field of view. The image data are directly transferred from the Main Detection Unit (MDU) to the onboard data-handling subsystem. The Functional Control Unit (FCU) controls the SEVIRI functions and provides the telemetry and telecommand interfaces with the satellite. SEVIRI has a spin rate of 100 rpm and a spectral range of 0.4-1.6 micrometres (visible and near-infrared) and 3.9-13.4 micrometres (infrared). The instrument has a spatial resolution of 1 km for the high-resolution visible channel, and 3 km for all other channels. Flown on Meteosat. http://www.esa.int/esapub/bulletin/bullet111/chapter4_bul111.pdf"@en ;
  skos:inScheme <http://vocab.nerc.ac.uk/scheme/SDNDEV/current> ;
  skos:notation "SDN:L22::TOOL1049" ;
  skos:note "accepted"@en ;
  skos:prefLabel "Spinning Enhanced Visible and Infrared Imager"@en ;
.
inst:TOOL1050
  rdf:type skos:Concept ;
  dcterm:date "2016-11-15 14:35:44.0" ;
  dcterm:identifier "SDN:L22::TOOL1050" ;
  dcterm:source <http://vocab.nerc.ac.uk/scheme/SDNDEV/current> ;
  pav:hasCurrentVersion <http://vocab.nerc.ac.uk/collection/L22/current/TOOL1050/2> ;
  pav:hasVersion <http://vocab.nerc.ac.uk/collection/L22/current/TOOL1050/1> ;
  owl:versionInfo "2" ;
  skos:altLabel "SMMR"@en ;
  skos:broader <http://vocab.nerc.ac.uk/collection/L05/current/302> ;
  skos:broader <http://vocab.nerc.ac.uk/collection/L05/current/308> ;
  skos:definition "The Scanning Multichannel Microwave Radiometer (SMMR) is a 5-frequency, 10-channel microwave radiometer designed for the creation of areal sea-ice climatologies for the Arctic and Antarctic. This involves measurements of sea surface temperatures, low altitude winds, water vapour and cloud liquid water content, sea ice extent, sea ice concentration, snow cover, snow moisture, rainfall rates, and differentiation of ice types. Six conventional Dicke-type radiometers are used. Those operating at the four longest wavelengths measure alternate polarisations during successive scans of the antenna; the others, at the shortest wavelength, operate continuously for each polarisation. A two-point reference signal system is used, consisting of an ambient RF termination and a horn antenna viewing deep space. A switching network of latching ferrite circulators selects the appropriate polarisation or calibration input for each radiometer. The SMMR also contains an antenna subsystem in which a 42 degree offset parabolic reflector focuses the received power into a single feedhorn covering the entire range of operating wavelengths, and provides coaxial antenna beams for all channels. The SMMR delivers orthogonally polarised antenna temperature data at five microwave wavelengths: 0.81, 1.36, 1.66, 2.8 and 4.54 cm, at frequencies of 6.63, 10.69, 18.0, 21.0, and 37.0 GHz. Flown on Seasat, Nimbus 7. https://nsidc.org/data/docs/daac/smmr_instrument.gd.html"@en ;
  skos:inScheme <http://vocab.nerc.ac.uk/scheme/SDNDEV/current> ;
  skos:notation "SDN:L22::TOOL1050" ;
  skos:note "accepted"@en ;
  skos:prefLabel "Scanning Multichannel Microwave Radiometer"@en ;
.
inst:TOOL1051
  rdf:type skos:Concept ;
  dcterm:date "2017-08-10 12:37:04.0" ;
  dcterm:identifier "SDN:L22::TOOL1051" ;
  dcterm:source <http://vocab.nerc.ac.uk/scheme/SDNDEV/current> ;
  pav:hasCurrentVersion <http://vocab.nerc.ac.uk/collection/L22/current/TOOL1051/3> ;
  pav:hasVersion <http://vocab.nerc.ac.uk/collection/L22/current/TOOL1051/1> ;
  pav:hasVersion <http://vocab.nerc.ac.uk/collection/L22/current/TOOL1051/2> ;
  owl:versionInfo "3" ;
  skos:altLabel "SMR"@en ;
  skos:broader <http://vocab.nerc.ac.uk/collection/L05/current/314> ;
  skos:definition "The Sub-Millimetre Radiometer (SMR) is a passive microwave limb sounder designed to detect molecular chemical species in the high atmosphere for astronomical and atmospheric research such as  depletion of the ozone layer and the effects of global warming. SMR observes thermal emissions radiating from Earth's limb using a 1.1 m telescope. The instrument employs four tunable single-sideband Schottky diode heterodyne receivers, as well as two high resolution auto-correlator spectrometers. The main target species tracked by SMR are O3, ClO, N2O, HNO3, H2O, CO, and isotopes of H2O and O3. A typical stratospheric mode scan covers the altitude range from 7 to 70 km. Measurements cover the latitude range 82.5 degrees South to 82.5 degrees North. Profile information is retrieved from the calibrated spectral measurements of a limb scan by inverting the radiative transfer equation for a non-scattering atmosphere. Optimized retrieval schemes based on the Optimal Estimation Method (OEM) have been developed and implemented for level 2 processing. SMR has a receiver at a wavelength of 3 mm and an additional four bands within the submillimeter range (0.5 - 1.0 mm), corresponding to a frequency range of 486 - 580 GHz. SMR has a scan rate of approximately 90 seconds. Flown on ODIN. http://earth.esa.int/workshops/atmos2006/participants/68/paper_frascati2006.pdf"@en ;
  skos:inScheme <http://vocab.nerc.ac.uk/scheme/SDNDEV/current> ;
  skos:notation "SDN:L22::TOOL1051" ;
  skos:note "accepted"@en ;
  skos:prefLabel "Sub-Millimetre Radiometer"@en ;
.
inst:TOOL1052
  rdf:type skos:Concept ;
  dcterm:date "2016-11-15 14:35:44.0" ;
  dcterm:identifier "SDN:L22::TOOL1052" ;
  dcterm:source <http://vocab.nerc.ac.uk/scheme/SDNDEV/current> ;
  pav:hasCurrentVersion <http://vocab.nerc.ac.uk/collection/L22/current/TOOL1052/2> ;
  pav:hasVersion <http://vocab.nerc.ac.uk/collection/L22/current/TOOL1052/1> ;
  owl:versionInfo "2" ;
  skos:altLabel "SSM/I"@en ;
  skos:broader <http://vocab.nerc.ac.uk/collection/L05/current/308> ;
  skos:definition "The Special Sensor Microwave Imager (SSM/I) is a passive microwave radiometer that measures atmospheric, oceanic and terrestrial microwave brightness temperatures at 19.35, 22.2, 37.0, and 85.5 GHz, from which ocean surface wind speed, atmospheric water vapour, cloud liquid water and rain rate can be derived. The SSM/I consists of an offset parabolic reflector of dimensions 24 x 26 inches, fed by a corrugated, broad-band, seven-port horn antenna. The reflector and feed are mounted on a drum that contains the radiometers, digital data subsystem, mechanical scanning subsystem, and power subsystem. The reflector-feed-drum assembly is rotated about the axis of the drum by a coaxially mounted bearing and power transfer assembly (BAPTA). All data, commands, timing and telemetry signals, and power pass through the BAPTA on slip ring connectors to the rotating assembly. The absolute brightness temperature of the scene incident upon the antenna is received and spatially filtered by the antenna to produce an effective input signal or antenna temperature at the input of the feed horn antenna. The SSM/I has seven channels, four frequencies, and is orthogonally polarised. It rotates continuously about an axis parallel to the local spacecraft at 31.6 rpm and measures the upwelling scene brightness temperature over an angular range of 102.4 degrees at nadir. The active scene measurements lie +51.2 to -51.2 degrees about the forward (F10, F11) or aft (F8) direction. This results in a swath width of approximately 1400 kilometres. During each 1.9 second scan, 128 discrete uniformly spaced radiometric samples are taken at the two 85 GHz channels and, on alternate scans, 64 discrete samples are taken at the remaining lower frequency channels. The antenna beam intersects the Earth's surface at an incidence angle of 53.1 degrees. Flown on F08, F10, F11, F13, F14, F15, F16, F17, F18 F19. https://nsidc.org/data/docs/daac/ssmi_instrument.gd.html"@en ;
  skos:inScheme <http://vocab.nerc.ac.uk/scheme/SDNDEV/current> ;
  skos:notation "SDN:L22::TOOL1052" ;
  skos:note "accepted"@en ;
  skos:prefLabel "Special Sensor Microwave Imager"@en ;
.
inst:TOOL1053
  rdf:type skos:Concept ;
  dcterm:date "2017-08-10 12:25:40.0" ;
  dcterm:identifier "SDN:L22::TOOL1053" ;
  dcterm:source <http://vocab.nerc.ac.uk/scheme/SDNDEV/current> ;
  pav:hasCurrentVersion <http://vocab.nerc.ac.uk/collection/L22/current/TOOL1053/3> ;
  pav:hasVersion <http://vocab.nerc.ac.uk/collection/L22/current/TOOL1053/1> ;
  pav:hasVersion <http://vocab.nerc.ac.uk/collection/L22/current/TOOL1053/2> ;
  owl:versionInfo "3" ;
  skos:altLabel "SSMI/S"@en ;
  skos:broader <http://vocab.nerc.ac.uk/collection/L05/current/308> ;
  skos:definition "The Special Sensor Microwave Imager Sounder (SSMI/S) is a passive microwave radiometer that is an enhanced version of the The Special Sensor Microwave Imager (SSM/I). It measures atmospheric, oceanic and terrestrial microwave brightness temperatures from  19 to 183 GHz, from which ocean surface wind speed, atmospheric water vapour, cloud liquid water and rain rate can be derived. The SSMI/S is an enhanced version of the SSM/I. It consists of an offset 24-inch parabolic reflector fed by a corrugated, broad-band, seven-port horn antenna. The reflector and feed are mounted on a drum that contains the radiometers, digital data subsystem, mechanical scanning subsystem, and power subsystem. The reflector-feed-drum assembly is rotated about the axis of the drum by a coaxially mounted bearing and power transfer assembly (BAPTA). All data, commands, timing and telemetry signals, and power pass through the BAPTA on slip ring connectors to the rotating assembly.The absolute brightness temperature of the scene incident upon the antenna is received and spatially filtered by the antenna to produce an effective input signal or antenna temperature at the input of the feed horn antenna. The feedhorn data are input to the receiver subsystem where frequency multiplexing occurs to produce 24 channels of data. The receiver outputs are converted to the video spectrum, digitized and formatted. The SSMI/S has 24 channels and eight frequencies. It measures the same frequencies and polarisations as the SSM/I, with the exception of the 85.5 GHz channel which has been replaced by a 91.655 GHz channel. A 183 GHz channel has also been added. The instrument rotates continuously about an axis parallel to the local spacecraft at 31.6 rpm and measures the upwelling scene brightness temperature over an angular range of 143.2 degrees at nadir. It has a swath width of approximately 1700 kilometres. Frequency multiplexing occurs as the main reflector is illuminated by six broadband corrugated feedhorns, grouping Channels 1-5; Channels 6, 7, 19-24; Channels 12-14; Channels 15-16; Channels 8-11; and Channels 17-18. Flown on F16, F17, F18, F19. https://nsidc.org/data/docs/daac/ssmis_instrument/"@en ;
  skos:inScheme <http://vocab.nerc.ac.uk/scheme/SDNDEV/current> ;
  skos:notation "SDN:L22::TOOL1053" ;
  skos:note "accepted"@en ;
  skos:prefLabel "Special Sensor Microwave Imager Sounder"@en ;
.
inst:TOOL1054
  rdf:type skos:Concept ;
  dcterm:date "2016-11-15 14:35:44.0" ;
  dcterm:identifier "SDN:L22::TOOL1054" ;
  dcterm:source <http://vocab.nerc.ac.uk/scheme/SDNDEV/current> ;
  pav:hasCurrentVersion <http://vocab.nerc.ac.uk/collection/L22/current/TOOL1054/2> ;
  pav:hasVersion <http://vocab.nerc.ac.uk/collection/L22/current/TOOL1054/1> ;
  owl:versionInfo "2" ;
  skos:altLabel "TANSO-CAI"@en ;
  skos:broader <http://vocab.nerc.ac.uk/collection/L05/current/308> ;
  skos:definition "The Thermal And Near-infrared Sensor for Carbon Observation -Cloud and Aerosol Imager (TANSO-CAI) is one of two instruments that the Thermal And Near-infrared Sensor for Carbon Observation (TANSO) is composed of. It is a radiometer designed to measure aerosol spatial distribution and cloud coverage in the visible, ultraviolet and shortwave infrared spectrums. This information is primarily used to correct the effects of clouds and aerosols on the spectra obtained from the primary TANSO instrument, Thermal And Near-infrared Sensor for Carbon Observation - Fourier Transform Spectrometer (TANSO-FTS). TANSO-CAI has a continuous spatial coverage, wider field of view, and higher spatial resolution than TANSO-FTS in order to detect aerosol spatial distribution and cloud coverage. Using the multispectral bands, the spectral characteristics of the aerosol scattering can be retrieved together with optical thickness. In addition, the UV-band range observations provide the aerosol data over land. With the FTS spectra, imager data, and the retrieval algorithm to remove cloud and aerosol contamination, the column density of the gases can be retrieved with an accuracy of 1%. The TANSO-CAI instrument operates within four sepctral bands in the following wavelength ranges: 0.370-0.390 micrometres (band1); 0.664-0.684 micrometres (band 2); 0.860-0.880 micrometres (band 3); 1.56-1.65 micrometres (band 4). The instrument has a spatial resolution of 0.5 km at nadir for bands 1-3, and 1.5 km at band 4. Flown on GOSAT. https://earth.esa.int/web/guest/data-access/latest-data-products/-/article/gosat-cai-l1-l2-l3-full-archive-and-new-products"@en ;
  skos:inScheme <http://vocab.nerc.ac.uk/scheme/SDNDEV/current> ;
  skos:notation "SDN:L22::TOOL1054" ;
  skos:note "accepted"@en ;
  skos:prefLabel "Thermal And Near-infrared Sensor for Carbon Observation -Cloud and Aerosol Imager"@en ;
.
inst:TOOL1055
  rdf:type skos:Concept ;
  dcterm:date "2016-11-15 14:35:44.0" ;
  dcterm:identifier "SDN:L22::TOOL1055" ;
  dcterm:source <http://vocab.nerc.ac.uk/scheme/SDNDEV/current> ;
  pav:hasCurrentVersion <http://vocab.nerc.ac.uk/collection/L22/current/TOOL1055/2> ;
  pav:hasVersion <http://vocab.nerc.ac.uk/collection/L22/current/TOOL1055/1> ;
  owl:versionInfo "2" ;
  skos:altLabel "TANSO-FTS"@en ;
  skos:broader <http://vocab.nerc.ac.uk/collection/L05/current/314> ;
  skos:definition "The Thermal And Near-infrared Sensor for Carbon Observation -Fourier Transform Spectrometer (TANSO-FTS) is one of two instruments that the Thermal And Near-infrared Sensor for Carbon Observation (TANSO) is composed of. It is a four-band interferometer designed to measure infrared light reflected and emitted from the earth's surface and atmosphere. Column abundances of carbon dioxide and methane are calculated from the observational data.  Incoming light is split into two beams which propagate in separate optical paths to create an optical path difference. The beams then recombine to cause interference. FTS measures the intensity of interference by continuously changing the optical path length difference. A spectrum is obtained by performing a Fourier transform on the measured data. Light reflected from the earth's surface is observed in the spectral bands 1 through 3 of FTS during daytime, and the light emitted from the atmosphere is captured in band 4 during both day and night time. Prior to reaching the detectors of the instrument, the light in the bands 1 through 3 is split into two orthogonally-polarised components (P and S components) and measured independently. The light in the band 4, however, is not split. The instrument thereby observes the incoming light in seven different channels. The TANSO-FTS instrument operates within four spectral bands in the following wavelength ranges: 0.758-0.775 micrometres (band 1); 1.56-1.72 (band 2); 1.92-2.08 (band 3); 5.56-14.3 (band 4). The intstrument has a spectral resolution of 0.2 cm-1. The angle of instantaneous field of view is 15.8 mrad. Flown on GOSAT. http://www.gosat.nies.go.jp/eng/gosat/page2.htm"@en ;
  skos:inScheme <http://vocab.nerc.ac.uk/scheme/SDNDEV/current> ;
  skos:notation "SDN:L22::TOOL1055" ;
  skos:note "accepted"@en ;
  skos:prefLabel "Thermal And Near-infrared Sensor for Carbon Observation - Fourier Transform Spectrometer"@en ;
.
inst:TOOL1056
  rdf:type skos:Concept ;
  dcterm:date "2017-08-10 12:37:04.0" ;
  dcterm:identifier "SDN:L22::TOOL1056" ;
  dcterm:source <http://vocab.nerc.ac.uk/scheme/SDNDEV/current> ;
  pav:hasCurrentVersion <http://vocab.nerc.ac.uk/collection/L22/current/TOOL1056/3> ;
  pav:hasVersion <http://vocab.nerc.ac.uk/collection/L22/current/TOOL1056/1> ;
  pav:hasVersion <http://vocab.nerc.ac.uk/collection/L22/current/TOOL1056/2> ;
  owl:versionInfo "3" ;
  skos:altLabel "TIRS"@en ;
  skos:broader <http://vocab.nerc.ac.uk/collection/L05/current/309> ;
  skos:definition "The Thermal Infrared Sensor (TIRS) is a push-boom sensor designed to measure land surface temperature in two thermal bands for high-resolution land and vegetation observation. A four-element refractive telescope focuses an f/1.64 beam of thermal radiation onto a cryogenically cooled focal plane, which holds three modules with quantum-well-infrared-photodetector (QWIP) arrays arranged in an alternating pattern along the focal plane centerline. The QWIPs detect long wavelengths of light emitted by the Earth whose intensity depends on surface temperature. The QWIPs TIRS uses are sensitive to two thermal infrared wavelength bands, helping it separate the temperature of the Earth's surface from that of the atmosphere. Their design operates on the complex principles of quantum mechanics. Gallium arsenide semiconductor chips trap electrons in an energy state 'well' until the electrons are elevated to a higher state by thermal infrared light of a certain wavelength. The elevated electrons create an electrical signal that can be read out and recorded to create a digital image. Each QWIP array is 640 detectors long cross-track allowing for overlap between the arrays to produce an effective linear array of 1850 pixels, spanning the 185 km ground swath with a 100 m spatial resolution. The spectral bands have wavelengths centred on 10.8 micrometres (band 1) and 12 micrometres (band 2). Flown on Landsat-8. http://landsat.gsfc.nasa.gov/?p=5474"@en ;
  skos:inScheme <http://vocab.nerc.ac.uk/scheme/SDNDEV/current> ;
  skos:notation "SDN:L22::TOOL1056" ;
  skos:note "accepted"@en ;
  skos:prefLabel "Thermal Infrared Sensor"@en ;
.
inst:TOOL1057
  rdf:type skos:Concept ;
  dcterm:date "2016-11-15 14:35:44.0" ;
  dcterm:identifier "SDN:L22::TOOL1057" ;
  dcterm:source <http://vocab.nerc.ac.uk/scheme/SDNDEV/current> ;
  pav:hasCurrentVersion <http://vocab.nerc.ac.uk/collection/L22/current/TOOL1057/2> ;
  pav:hasVersion <http://vocab.nerc.ac.uk/collection/L22/current/TOOL1057/1> ;
  owl:versionInfo "2" ;
  skos:altLabel "TM"@en ;
  skos:broader <http://vocab.nerc.ac.uk/collection/L05/current/309> ;
  skos:definition "The TM (Thematic Mapper) is a whick broom passive optical imager designed to measure Earth's surface reflectance in seven spectral bands for high-resolution land and vegetation observation. It is a follow-on instrument to the MSS (Multispectral Scanner System). TM provides information on the Earth's surface in the visible, near, middle and thermal infrared regions of the electromagnetic spectrum. IT does this using a mirror which scans across the satellite's ground track, reflecting light into a single detector which collects data one pixel at a time.  The seven spectral bands range in wavelength from 0.45-0.52 micrometres (band1); 0.53-0.61 micrometres (band 2); 0.63-0.69 micrometres (band 3); 0.78-0.90 micrometres (band 4); 1.55-1.75 micrometres (band 5); 10.4-12.5 micrometres (band 6); 2.09-2.35 micrometres (band 7). All bands have a 30 m resolution except band 6 which has a 120 m resolution. Flown on Landsat-4, Landsat-5. http://wiki.landscapetoolbox.org/doku.php/remote_sensor_types:landsat_tm_5#description"@en ;
  skos:inScheme <http://vocab.nerc.ac.uk/scheme/SDNDEV/current> ;
  skos:notation "SDN:L22::TOOL1057" ;
  skos:note "accepted"@en ;
  skos:prefLabel "Thematic Mapper"@en ;
.
inst:TOOL1058
  rdf:type skos:Concept ;
  dcterm:date "2016-11-15 14:35:44.0" ;
  dcterm:identifier "SDN:L22::TOOL1058" ;
  dcterm:source <http://vocab.nerc.ac.uk/scheme/SDNDEV/current> ;
  pav:hasCurrentVersion <http://vocab.nerc.ac.uk/collection/L22/current/TOOL1058/2> ;
  pav:hasVersion <http://vocab.nerc.ac.uk/collection/L22/current/TOOL1058/1> ;
  owl:versionInfo "2" ;
  skos:altLabel "TMI"@en ;
  skos:broader <http://vocab.nerc.ac.uk/collection/L05/current/308> ;
  skos:definition "The Tropical Rainfall Measuring Mission's (TRMM) Microwave Imager (TMI) is a conical-scanning passive microwave radiometer designed to provide quantitative rainfall information over a wide swath width. It measures microwave energy emitted by the Earth and atmosphere to quantify the water vapour, cloud water, rainfall intensity and rainfall rates in the atmosphere. The TMI design is based on the SSM/I, detecting microwave energy in the form of of brightness temperatures from Earth's surface and atmosphere. It measures this at five separate frequencies. TMI consists of nine separate total-power radiometers, each simultaneously measuring the microwave emission coming from the Earth's surface with the intervening atmosphere. TMI employs an offset parabolic reflector (antenna aperture size of 61 cm) to collect the microwave radiation. The reflector focuses the radiation into two feedhorn. The reflector and feedhorns spin as a unit about an axis parallel to the S/X nadir direction. A cold-space mirror and a warm reference load are attached to the spin axis and do not rotate. The rotating feedhorns observe the fixed cold mirror and warm load once each scan for calibration purposes. The TMI measures radiation intensity at 10.7, 19.4, 21.3, 37 and 85.5 GHz. It has a resolution ranging from 7 km x 5 km to 63 km x 37 km depending on the frequency used, and a feedhorn-reflector rotation period of 1.9 s. Flown on TRMM. https://directory.eoportal.org/web/eoportal/satellite-missions/t/trmm#sensors"@en ;
  skos:inScheme <http://vocab.nerc.ac.uk/scheme/SDNDEV/current> ;
  skos:notation "SDN:L22::TOOL1058" ;
  skos:note "accepted"@en ;
  skos:prefLabel "Tropical Rainfall Measuring Mission (TRMM) Microwave Imager"@en ;
.
inst:TOOL1059
  rdf:type skos:Concept ;
  dcterm:date "2016-11-15 14:35:44.0" ;
  dcterm:identifier "SDN:L22::TOOL1059" ;
  dcterm:source <http://vocab.nerc.ac.uk/scheme/SDNDEV/current> ;
  pav:hasCurrentVersion <http://vocab.nerc.ac.uk/collection/L22/current/TOOL1059/2> ;
  pav:hasVersion <http://vocab.nerc.ac.uk/collection/L22/current/TOOL1059/1> ;
  owl:versionInfo "2" ;
  skos:altLabel "VEGETATION"@en ;
  skos:broader <http://vocab.nerc.ac.uk/collection/L05/current/309> ;
  skos:definition "VEGETATION is a 4-channel optical imager operating in the visible, near-infrared and shortwave-infrared spectral bands. It measures the spectral signature of chlorophyll, and also detects soil moisture and vegetation for the characterization and correction of atmospheric effects on reflectance. This information is used for measurements of vegetation canopies, either for scientific studies involving both regional and global scale experiments (for example development of models of biosphere dynamics interacting with climate models), or for monitoring crops, pastures and forests. The instrument collects radiation reflected by the earth's surface to convert it into usable electrical signals. Silicon linear arrays are used for spectral band B0 (Blue), B2 (Red) and B3 (Near-Infrared), while InGaAs linear array is used for the Short Wave Infrared spectral band. Each array features 1728 individual CCD detectors. The output voltage signals are fed to a multiplexer (beforehand SWIR voltages are adjusted for dark current values), then to a single analogue to digital converter (ADC). All sensors are processed by a single high precision 11 bit ADC, thus completely by-passing the problem of electronic interband calibration. VEGETATION operates in the following spectrums: blue (0.43-0.47 micrometres), red (0.61-0.68 micrometres), near-infrared (0.78-0.89 micrometres) and shortwave-infrared (1.58-1.75 micrometres). It has aground swath of 2200 km and a spatial resolution of 1.15 to 1.7 km. Flown on Spot-4, Spot-5. https://vegetation.cnes.fr/en/VEGETATION/index.htm"@en ;
  skos:inScheme <http://vocab.nerc.ac.uk/scheme/SDNDEV/current> ;
  skos:notation "SDN:L22::TOOL1059" ;
  skos:note "accepted"@en ;
  skos:prefLabel "VEGETATION"@en ;
.
inst:TOOL1060
  rdf:type skos:Concept ;
  dcterm:date "2016-11-15 14:35:44.0" ;
  dcterm:identifier "SDN:L22::TOOL1060" ;
  dcterm:source <http://vocab.nerc.ac.uk/scheme/SDNDEV/current> ;
  pav:hasCurrentVersion <http://vocab.nerc.ac.uk/collection/L22/current/TOOL1060/2> ;
  pav:hasVersion <http://vocab.nerc.ac.uk/collection/L22/current/TOOL1060/1> ;
  owl:versionInfo "2" ;
  skos:altLabel "WindSat"@en ;
  skos:broader <http://vocab.nerc.ac.uk/collection/L05/current/302> ;
  skos:broader <http://vocab.nerc.ac.uk/collection/L05/current/308> ;
  skos:definition "The WindStat Polarimetric Microwave Radiometer is a 22-channel microwave radiometer designed to measure the ocean surface wind vector from space, in addition to sea surface temperature, total precipitable water, integrated cloud liquid water, and rain rate over the ocean. WindSat is also used to measure soil moisture, sea ice and tropical cyclone structure. WindSat uses a 1.8 m offset reflector antenna fed by 11 dual-polarised feed horns. The antenna beams view the Earth at incidence angles ranging from 50 to 55 degrees. The feedhorns of each frequency channel trace out different arcs along the scan, therefore the Earth Incidence Angles (EIA) are different for each frequency band. The WindSat sensor takes observations during both the forward and aft looking scans. The 10.7, 18.7 and 37.0 GHz bands are fully polarimetric. Six principal polarisations are measured directly using three dual polarisation feeds at each of the polarimetric frequencies. The 6.8 and 23.8 GHz channels are dual-polarised as data at these frequencies are used for secondary parameters such as sea surface temperature and water vapour, which support the wind vector retrievals. WindSat operates in discrete bands at frequencies of 6.8, 10.7, 18.7, 23.8, and 37.0 GHz. The antenna rotates at 30 rpm. Measurements are made over a forward swath of 1400 km and an aft swath of 750 km. Flown on Coriolis. https://www.nrl.navy.mil/WindSat/Description.php"@en ;
  skos:inScheme <http://vocab.nerc.ac.uk/scheme/SDNDEV/current> ;
  skos:notation "SDN:L22::TOOL1060" ;
  skos:note "accepted"@en ;
  skos:prefLabel "WindSat Polarimetric Microwave Radiometer"@en ;
.
inst:TOOL1061
  rdf:type skos:Concept ;
  dcterm:date "2016-11-15 15:28:05.0" ;
  dcterm:identifier "SDN:L22::TOOL1061" ;
  dcterm:source <http://vocab.nerc.ac.uk/scheme/SDNDEV/current> ;
  pav:hasCurrentVersion <http://vocab.nerc.ac.uk/collection/L22/current/TOOL1061/1> ;
  owl:versionInfo "1" ;
  skos:altLabel "AATSR"@en ;
  skos:broader <http://vocab.nerc.ac.uk/collection/L05/current/302> ;
  skos:broader <http://vocab.nerc.ac.uk/collection/L05/current/308> ;
  skos:broader <http://vocab.nerc.ac.uk/collection/L05/current/309> ;
  skos:definition "A passive optical imager with dual view composed of a 7-channel infra-red radiometer, designed to measure sea surface temperature, cloud attributes, as well as vegetation and sea-ice cover. The infra-red radiometer uses an along-track scanning telescope to focus incoming radiation from two views at different angles: one at nadir and one fore-looking at approximately 47 degrees. The same point on the Earth's surface is thus observed twice through differing atmospheric thickness, allowing for direct estimation of the atmospheric absorption and scattering, which can be used for atmospheric correction of the surface dataset. The instrument carries an on-board visible calibration system. The AATSR is functionally identical to ATSR-2, but its structure is adapted to the Envisat platform. Moreover, AATSR has a larger telemetry bandwidth compared to ATSR-2, allowing it to collect and telemeter a greater amount of visible data. The instrument's bandwidths are: (0.53 - 0.57)um, (0.64 - 0.68)um, (0.85 - 0.89)um, (1.31 - 1.91)um, (3.55 - 3.85)um, (10.35 - 11.35)um, (11.50 - 12.50)um. The instrument's resolution is 1 km at the instantaneous field of view (IFOV). The swath is 500 km. The accuracy of sea surface temperature measurements is approximately 0.1 degC. Flown on Envisat. http://www.wmo-sat.info/oscar/instruments/view/2"@en ;
  skos:inScheme <http://vocab.nerc.ac.uk/scheme/SDNDEV/current> ;
  skos:notation "SDN:L22::TOOL1061" ;
  skos:note "accepted"@en ;
  skos:prefLabel "Advanced Along-Track Scanning Radiometer"@en ;
.
inst:TOOL1062
  rdf:type skos:Concept ;
  dcterm:date "2016-11-15 15:28:05.0" ;
  dcterm:identifier "SDN:L22::TOOL1062" ;
  dcterm:source <http://vocab.nerc.ac.uk/scheme/SDNDEV/current> ;
  pav:hasCurrentVersion <http://vocab.nerc.ac.uk/collection/L22/current/TOOL1062/1> ;
  owl:versionInfo "1" ;
  skos:altLabel "ACE-FTS"@en ;
  skos:broader <http://vocab.nerc.ac.uk/collection/L05/current/314> ;
  skos:definition "An infrared Fourier Transform Spectrometer, designed to perform solar occultation measurements to infer the chemical composition of the atmosphere at high latitudes and high altitudes. The spectrometer is composed of a Michelson interferometer with two cube corners and a visible/near infrared imager with two filtered channels. A pointing mirror tracks the Sun's centre as a movable mirror inside the instrument generates an interferogram from the incoming radiation, which is then converted to a spectrum through Fourier transform. The instrument operates using the solar occultation technique, thus carrying out measurements of the Sun-emitted radiation during the short time span at which it travels tangent to the Earth's surface through the atmosphere at sunrise and sunset. The instrument on SCISAT-1 captures approximately 30 occultations per day, as determined by the satellite's polar orbit. The spatial resolution is 1-2 km (vertical), and 500 km (horizontal). The spectral range is (2.2 - 13.3) um, equivalent to (750 - 4400) cm^-1; the spectral resolution is 0.02 cm^-1. The FTS has a circular field of view is 1.25 mrad. The imager within the instrument has two filtered channels at 0.525 um and 1.02 um respectively, and a total field of view of 30 mrad.Flown on SCISAT-1. http://www.wmo-sat.info/oscar/instruments/view/6"@en ;
  skos:inScheme <http://vocab.nerc.ac.uk/scheme/SDNDEV/current> ;
  skos:notation "SDN:L22::TOOL1062" ;
  skos:note "accepted"@en ;
  skos:prefLabel "Atmospheric Chemistry Experiment - Fourier Transform Spectrometer"@en ;
.
inst:TOOL1063
  rdf:type skos:Concept ;
  dcterm:date "2016-11-15 15:28:05.0" ;
  dcterm:identifier "SDN:L22::TOOL1063" ;
  dcterm:source <http://vocab.nerc.ac.uk/scheme/SDNDEV/current> ;
  pav:hasCurrentVersion <http://vocab.nerc.ac.uk/collection/L22/current/TOOL1063/1> ;
  owl:versionInfo "1" ;
  skos:altLabel "AIRS"@en ;
  skos:broader <http://vocab.nerc.ac.uk/collection/L05/current/308> ;
  skos:definition "A space-based cross-track scanning instrument designed to measure the amount of infrared energy emitted from the atmosphere, with the purpose of creating three-dimensional maps of air and surface temperature, water vapour and cloud properties, as well as determining the amount of trace greenhouse gases (e.g. ozone, carbon monoxide, carbon dioxide and methane). A mirror rotating around an axis along the line of flight of the spacecraft scans the Earth on either side of the ground track and directs the infrared energy into the instrument. A total of 2378 detectors measure within the thermal infrared range of (3.7 - 15.4) micrometres, and 4 detectors measure within the visible range of (0.4 - 1.0) micrometres. The accuracy level is 1 degC in layers 1 kilometre thick for atmospheric temperature measurements, and 20 percent in layers 2 kilometres thick for humidity measurements in the troposphere. The swath centred on the nadir is approximately 49.5 degrees, and is scanned every 2 seconds. Each scan line contains 90 infrared footprints, with a resolution of 13.5 kilometres at nadir, and (41 x 21.4) kilometres at the scan extremes from a nominal orbit of 705.3 kilometres. The visible/near infrared spatial resolution is approximately 2.3 kilometres at nadir. Flown on Aqua (NASA). http://www.wmo-sat.info/oscar/instruments/view/16"@en ;
  skos:inScheme <http://vocab.nerc.ac.uk/scheme/SDNDEV/current> ;
  skos:notation "SDN:L22::TOOL1063" ;
  skos:note "accepted"@en ;
  skos:prefLabel "Atmospheric Infrared Sounder"@en ;
.
inst:TOOL1064
  rdf:type skos:Concept ;
  dcterm:date "2022-03-18 14:36:09.0" ;
  dcterm:identifier "SDN:L22::TOOL1064" ;
  dcterm:source <http://vocab.nerc.ac.uk/scheme/SDNDEV/current> ;
  pav:hasCurrentVersion <http://vocab.nerc.ac.uk/collection/L22/current/TOOL1064/2> ;
  pav:hasVersion <http://vocab.nerc.ac.uk/collection/L22/current/TOOL1064/1> ;
  owl:versionInfo "2" ;
  skos:altLabel "AMI"@en ;
  skos:broader <http://vocab.nerc.ac.uk/collection/L05/current/305> ;
  skos:broader <http://vocab.nerc.ac.uk/collection/L05/current/306> ;
  skos:definition "An active microwave instrument consisting of a synthetic aperture radar (SAR) and a wind scatterometer (SCAT), the former designed to capture imagery of ocean, land and ice at high resolution and independently of weather conditions, and the latter utilised to measure horizontal wind speed and wind vector over the surface, as well as soil moisture and sea-ice type. The SAR radar operates by obtaining strips of imagery in two modes: the imaging mode, and the wave mode. In imaging mode, SAR provides two-dimensional images between (6 - 30)m along-track at a spatial resolution of 26m. In wave mode, imagettes of 5 km by 5 km in size are captured at regular intervals of 200 km along track; the imagettes are then processed within the swath to obtain the wave spectra, as changes in radar reflectivity on the sea surface are proxies for length and direction of surface waves. SCAT is composed by three sideways-looking antennas which generate radar beams at 45, 90 and 135 degrees azimuth across a swath 500 km wide situated 200 km to the right of the sub-satellite track. The radar backscatter is then measured for overlapping cells of 50 km resolution, using a grid spacing of 25 km. This technique permits three different viewing directions almost simultaneously, facilitating the determination of surface wind vectors. SAR and SCAT can be operated together, unless SAR is in imaging mode. The wave direction detected range is (0 - 180) degrees, at an accuracy of +/- 20 degrees; the detected wavelength range is (100 - 1000) m, with an accuracy of +/- 25%. AMI-SAR operates at the C-band frequency of 5.3 GHz with a bandwidth of 15.5 MHz, using vertically polarised antennas. The spatial resolution achieved is 30 m over a 100 km swath, located 250 km to the right of the sub-satellite track; the look angle is 23 degrees. Wind direction detected range is (0 - 360) degrees, at an accuracy of +/- 20 degrees; wind speed detected range is (4 - 24) m/s, at an accuracy of 2 m/s and spatial resolution of 50 km. AMI-SCAT operates at the C-band frequency of 5.3 GHz +/- 200 kHz. Flown on ERS-1, ERS-2. http://www.wmo-sat.info/oscar/instruments/view/23; https://www.wmo-sat.info/oscar/instruments/view/24"@en ;
  skos:inScheme <http://vocab.nerc.ac.uk/scheme/SDNDEV/current> ;
  skos:notation "SDN:L22::TOOL1064" ;
  skos:note "accepted"@en ;
  skos:prefLabel "Active Microwave Instrument"@en ;
.
inst:TOOL1065
  rdf:type skos:Concept ;
  dcterm:date "2016-11-15 15:28:05.0" ;
  dcterm:identifier "SDN:L22::TOOL1065" ;
  dcterm:source <http://vocab.nerc.ac.uk/scheme/SDNDEV/current> ;
  pav:hasCurrentVersion <http://vocab.nerc.ac.uk/collection/L22/current/TOOL1065/1> ;
  owl:versionInfo "1" ;
  skos:altLabel "AMSR-2"@en ;
  skos:broader <http://vocab.nerc.ac.uk/collection/L05/current/302> ;
  skos:broader <http://vocab.nerc.ac.uk/collection/L05/current/308> ;
  skos:broader <http://vocab.nerc.ac.uk/collection/L05/current/309> ;
  skos:definition "A conical scanning, passive microwave radiometer designed for multiple purposes, including the determination of precipitation intensity at the surface, sea surface temperature, sea-ice cover, horizontal wind speed over the surface, and surface biomass. The antenna is at 55 degrees zenith angle, and operates by a conical scan mechanism, thus enabling the acquisition of both daytime and night-time data; its swath is 1450 kilometres, and it completes 40 scans per minute (10 kilometres per scan). The instrument's antenna is 2 metres in diameter, and receives 7 frequency bands over 14 channels in the range of 6.9 to 89 gigahertz (window channels only). The resolution changes with the frequency, and is consistent with the antenna's dimensions. Flown on GCOM-W1, GCOM-W2, GCOM-W3. http://www.wmo-sat.info/oscar/instruments/view/28"@en ;
  skos:inScheme <http://vocab.nerc.ac.uk/scheme/SDNDEV/current> ;
  skos:notation "SDN:L22::TOOL1065" ;
  skos:note "accepted"@en ;
  skos:prefLabel "Advanced Microwave Scanning Radiometer-2"@en ;
.
inst:TOOL1066
  rdf:type skos:Concept ;
  dcterm:date "2016-11-15 15:28:05.0" ;
  dcterm:identifier "SDN:L22::TOOL1066" ;
  dcterm:source <http://vocab.nerc.ac.uk/scheme/SDNDEV/current> ;
  pav:hasCurrentVersion <http://vocab.nerc.ac.uk/collection/L22/current/TOOL1066/1> ;
  owl:versionInfo "1" ;
  skos:altLabel "AMSR-E"@en ;
  skos:broader <http://vocab.nerc.ac.uk/collection/L05/current/302> ;
  skos:broader <http://vocab.nerc.ac.uk/collection/L05/current/308> ;
  skos:broader <http://vocab.nerc.ac.uk/collection/L05/current/309> ;
  skos:definition "A conical scanning, passive microwave radiometer designed for multiple purposes, including the determination of precipitation intensity at the surface, sea surface temperature, sea-ice cover, horizontal wind speed over the surface, and surface biomass. The antenna is at 55 degrees zenith angle, and operates by a conical scan mechanism, thus enabling the acquisition of both daytime and night-time data; its swath is 1450 kilometres, and it completes 40 scans per minute (10 kilometres per scan). The instrument's antenna is 1.6 metres in diameter, and receives 6 frequency bands over 12 channels in the range of 6.9 to 89 gigahertz (window channels only). The resolution changes with the frequency, and is consistent with the antenna's dimensions. Flown on Aqua (NASA). http://www.wmo-sat.info/oscar/instruments/view/29"@en ;
  skos:inScheme <http://vocab.nerc.ac.uk/scheme/SDNDEV/current> ;
  skos:notation "SDN:L22::TOOL1066" ;
  skos:note "accepted"@en ;
  skos:prefLabel "Advanced Microwave Scanning Radiometer for Earth Observation from Space (AMSR-E)"@en ;
.
inst:TOOL1067
  rdf:type skos:Concept ;
  dcterm:date "2016-11-15 15:28:05.0" ;
  dcterm:identifier "SDN:L22::TOOL1067" ;
  dcterm:source <http://vocab.nerc.ac.uk/scheme/SDNDEV/current> ;
  pav:hasCurrentVersion <http://vocab.nerc.ac.uk/collection/L22/current/TOOL1067/1> ;
  owl:versionInfo "1" ;
  skos:altLabel "AMSU-A"@en ;
  skos:broader <http://vocab.nerc.ac.uk/collection/L05/current/308> ;
  skos:definition "A multi-channel microwave radiometer designed to measure global atmospheric temperature profiles in nearly all weather conditions. AMSU-A samples thirty consecutive scene radiances in a stepped-scan fashion every eight seconds, and measures the atmospheric temperature profile by examining fifteen bands of microwave radiation ranging between (23 - 90) GHz. The instrument consists of two independent modules with their own spacecraft interface: AMSU-A1 and AMSU-A2. AMSU-A2 identifies precipitation and corrects for surface emissivity, atmospheric liquid water and water vapour effects by processing the first two microwave radiation channels using one antenna. In AMSU-A1, two antenna-radiometer systems provide the other thirteen channels to retrieve atmospheric temperature profiles up to 42 km from the Earth's surface. The swath is 1690 km wide, and the spatial resolution is 40 km (horizontal) at nadir. The field of view is +/- 49.5 degrees cross-track, and the instantaneous field of view is 3.3 degrees circular. The thermal operating range is (0 - 20) degC. AMSU-A2 central channel frequencies are: (23.800, 31.400) GHz; AMSU-A1 central channel frequencies are: (50.300, 52.800, 53.596 +/- 0.115, 54.400, 54.940, 55.500, f0 = 57.290344, f0 +/- 0.217, f0 +/- 0.3222 +/- 0.048, f0 +/- 0.3222 +/- 0.022, f0 +/- 0.3222 +/- 0.010, f0 +/- 0.3222 +/- 0.0045, 89.0) GHz. Flown on Aqua, Metop-A, Metop-B, Metop-C, NOAA-15, NOAA-16, NOAA-17, NOAA-18, NOAA-19 . http://www.wmo-sat.info/oscar/instruments/view/30"@en ;
  skos:inScheme <http://vocab.nerc.ac.uk/scheme/SDNDEV/current> ;
  skos:notation "SDN:L22::TOOL1067" ;
  skos:note "accepted"@en ;
  skos:prefLabel "Advanced Microwave Sounding Unit - A"@en ;
.
inst:TOOL1068
  rdf:type skos:Concept ;
  dcterm:date "2016-11-15 15:28:05.0" ;
  dcterm:identifier "SDN:L22::TOOL1068" ;
  dcterm:source <http://vocab.nerc.ac.uk/scheme/SDNDEV/current> ;
  pav:hasCurrentVersion <http://vocab.nerc.ac.uk/collection/L22/current/TOOL1068/1> ;
  owl:versionInfo "1" ;
  skos:altLabel "AMSU-B"@en ;
  skos:broader <http://vocab.nerc.ac.uk/collection/L05/current/308> ;
  skos:definition "A five-channel microwave radiometer designed for humidity and precipitation sounding in nearly all weather conditions. AMSU-B is a cross-track, line scanned instrument which samples ninety consecutive scene radiances in a continuous fashion, and measures atmospheric humidity profiles by examining five bands of microwave radiation ranging between (89.0 - 193.31)GHz. The instrument consists of a scanning parabolic reflector antenna which rotates and focuses incoming radiation from the atmosphere into a quasi-optic system. The frequencies of interest are then separated into three discreet feed horns of the receiver assembly. AMSU-B works in conjunction with AMSU-A to provide a twenty-channel microwave radiometer. The swath is 2250 km wide, and the spatial resolution is 16 km (horizontal) at nadir. The scan period is 8/3 seconds. The instrument covers +/- 49.5 degrees cross-track from the sub-satellite point, and the instantaneous field of view is 1.1 degrees circular. AMSU-B central frequencies are: (89.0, 150.0, 183.31 +/- 7.0, 183.31 +/- 3.0, 183.31 +/- 1.0) GHz. Flown on NOAA-15, NOAA-16, NOAA-17. http://www.wmo-sat.info/oscar/instruments/view/33"@en ;
  skos:inScheme <http://vocab.nerc.ac.uk/scheme/SDNDEV/current> ;
  skos:notation "SDN:L22::TOOL1068" ;
  skos:note "accepted"@en ;
  skos:prefLabel "Advanced Microwave Sounding Unit - B"@en ;
.
inst:TOOL1069
  rdf:type skos:Concept ;
  dcterm:date "2016-11-15 15:28:05.0" ;
  dcterm:identifier "SDN:L22::TOOL1069" ;
  dcterm:source <http://vocab.nerc.ac.uk/scheme/SDNDEV/current> ;
  pav:hasCurrentVersion <http://vocab.nerc.ac.uk/collection/L22/current/TOOL1069/1> ;
  owl:versionInfo "1" ;
  skos:altLabel "ASAR"@en ;
  skos:broader <http://vocab.nerc.ac.uk/collection/L05/current/306> ;
  skos:definition "A radio-occultation imaging radar designed to capture imagery of ocean, land and ice at high resolution and independently of weather conditions. The instrument operates as an active remote sensing device, emitting microwave pulses in the C-band frequency range (2 GHz - 4 GHz) and recording the response reflected by the Earth's surface targeted. The time it takes for each emitted pulse to return to the instrument holds information on the distance of the target object, whilst the amount of the signal returned is used to extract information on surface properties. ASAR operates in five mutually exclusive modes, which output images of different sizes and spatial resolution. The instrument is able to create orthogonal polarised waves, the return signal of which can be used to extract information on the type of surface targeted. The user can select an operating mode out of five mutually exclusive options: the Image mode (IM), generating products at a spatial resolution of 30 m over one of seven selectable swath widths determined by incidence angles between 15 degrees to 45 degrees, at horizontal transmit and receive polarisation (HH) or vertical transmit and receive polarisation (VV); the Alternating Polarisation mode (AP), generating products at a spatial resolution of 30 m over one of seven selectable swath widths determined by incidence angles between 15 degrees to 45 degrees, at different dual polarisation combinations (HH/VV or HH/HV or VV/VH); the Wide Swath mode (WS), which uses the ScanSAR technique, thus providing images at 150 m resolution over five combined sub-swaths covering a total of 405 km, in HH or VV polarisation; the Global Monitoring mode (GM), outputting 1 km resolution images over a 405 km swath, in HH or VV polarisation; and the Wave mode (WV), which generates backscatter vignettes of 5 km by 5 km size, spaced 100 km along track in HH or VV polarisation. Flown on Envisat. http://www.wmo-sat.info/oscar/instruments/view/44"@en ;
  skos:inScheme <http://vocab.nerc.ac.uk/scheme/SDNDEV/current> ;
  skos:notation "SDN:L22::TOOL1069" ;
  skos:note "accepted"@en ;
  skos:prefLabel "Advanced Synthetic Aperture Radar"@en ;
.
inst:TOOL1070
  rdf:type skos:Concept ;
  dcterm:date "2016-11-15 15:28:05.0" ;
  dcterm:identifier "SDN:L22::TOOL1070" ;
  dcterm:source <http://vocab.nerc.ac.uk/scheme/SDNDEV/current> ;
  pav:hasCurrentVersion <http://vocab.nerc.ac.uk/collection/L22/current/TOOL1070/1> ;
  owl:versionInfo "1" ;
  skos:altLabel "ASCAT"@en ;
  skos:broader <http://vocab.nerc.ac.uk/collection/L05/current/305> ;
  skos:definition "A C-band scatterometer designed to detect wind speed and vector over the sea surface, as well as large-scale soil moisture. Three sideways-looking antennas located on both sides of the instrument transmit microwave pulses toward the sea surface and measure the ground echoes returned back to the instrument. The backscattering properties of the signal detected are related to wind-generated sea-surface roughness, and can thus be used to infer wind speed and direction. The three antennas on each side are oriented at 45, 90 and 135 degrees azimuth respectively, and scan two 500 km swaths separated by a 700 km gap along-track. ASCAT operates at the C-band frequency of 5.233 GHz. The spatial resolution is 50 km (nominal) or 25 km (experimental). Flown on Metop-A, Metop-B, Metop-C. http://www.wmo-sat.info/oscar/instruments/view/47"@en ;
  skos:inScheme <http://vocab.nerc.ac.uk/scheme/SDNDEV/current> ;
  skos:notation "SDN:L22::TOOL1070" ;
  skos:note "accepted"@en ;
  skos:prefLabel "Advanced SCATterometer"@en ;
.
inst:TOOL1071
  rdf:type skos:Concept ;
  dcterm:date "2016-11-15 15:28:05.0" ;
  dcterm:identifier "SDN:L22::TOOL1071" ;
  dcterm:source <http://vocab.nerc.ac.uk/scheme/SDNDEV/current> ;
  pav:hasCurrentVersion <http://vocab.nerc.ac.uk/collection/L22/current/TOOL1071/1> ;
  owl:versionInfo "1" ;
  skos:altLabel "ASTER"@en ;
  skos:broader <http://vocab.nerc.ac.uk/collection/L05/current/309> ;
  skos:definition "An optical imager detecting 14 spectral bands ranging from visible to thermal infrared light, designed to produce stereoscopic images and detailed terrain height models for high resolution land and vegetation observation. ASTER uses three sub-systems to detect radiation in the visible near-infrared (VNIR), short-wave infrared (SWIR), and thermal infrared (TIR), each with the ability to change the viewing angle in the cross-track direction. The VNIR radiometer has along-track stereo coverage in its third band (0.76 um - 0.86 um), with nadir and backward views. The swath width is 60 km. Bands of radiation wavelengths and their resolution at sub satellite point are: (0.52 - 0.60) um, (0.63 - 0.69) um, (0.76 - 0.86) um, which constitute the VNIR bands and have a resolution of 15 m; (1.60 - 1.70) um,  (2.145 - 2.185) um, (2.185 - 2.225) um, (2.235 - 2.285) um, (2.295 - 2.365) um, (2.360 - 2.430) um, which constitute the SWIR bands and have a resolution of 30 m; (8.125 - 8.475) um, (8.475 - 8.825) um, (8.925 - 9.275) um, (10.25 - 10.95) um, (10.95 - 11.65), which constitute the TIR bands and have a resolution of 90 m. Flown on Terra. http://www.wmo-sat.info/oscar/instruments/view/50"@en ;
  skos:inScheme <http://vocab.nerc.ac.uk/scheme/SDNDEV/current> ;
  skos:notation "SDN:L22::TOOL1071" ;
  skos:note "accepted"@en ;
  skos:prefLabel "Advanced Spaceborne Thermal Emission and Reflection Radiometer"@en ;
.
inst:TOOL1072
  rdf:type skos:Concept ;
  dcterm:date "2016-11-15 15:28:05.0" ;
  dcterm:identifier "SDN:L22::TOOL1072" ;
  dcterm:source <http://vocab.nerc.ac.uk/scheme/SDNDEV/current> ;
  pav:hasCurrentVersion <http://vocab.nerc.ac.uk/collection/L22/current/TOOL1072/1> ;
  owl:versionInfo "1" ;
  skos:altLabel "ATSR-1"@en ;
  skos:broader <http://vocab.nerc.ac.uk/collection/L05/current/302> ;
  skos:broader <http://vocab.nerc.ac.uk/collection/L05/current/308> ;
  skos:definition "A passive optical imager with dual view composed of a 4-channel infra-red radiometer and a 2-channel nadir-viewing microwave sounder, designed to measure sea surface temperature and cloud parameters. The infra-red radiometer uses an along-track scanning telescope to focus incoming radiation from two views at different angles: one at nadir and one fore-looking at approximately 47 degrees. The same point on the Earth's surface is thus observed twice through differing atmospheric thickness, allowing for direct estimation of the atmospheric effect as well as atmospheric correction for the surface dataset. The radiometer's bandwidths are (1.46 - 1.76)um, (3.55 - 3.85) um, (10.35 - 11.35) um, and (11.50 - 12.50)um; the microwave sounder's central frequencies are 23.8 GHz and 36.5 GHz, and have a bandwidth of 400 MHz. The instrument's resolutions at sub-satellite point are 1 km (infra-red radiometer) and 20 km (microwave sounder). The swath is 500 km. The accuracy of sea surface temperature measurements is approximately 0.3 degC. Flown on ERS-1. http://www.wmo-sat.info/oscar/instruments/view/55"@en ;
  skos:inScheme <http://vocab.nerc.ac.uk/scheme/SDNDEV/current> ;
  skos:notation "SDN:L22::TOOL1072" ;
  skos:note "accepted"@en ;
  skos:prefLabel "Along Track Scanning Radiometer - 1"@en ;
.
inst:TOOL1073
  rdf:type skos:Concept ;
  dcterm:date "2016-11-15 15:28:05.0" ;
  dcterm:identifier "SDN:L22::TOOL1073" ;
  dcterm:source <http://vocab.nerc.ac.uk/scheme/SDNDEV/current> ;
  pav:hasCurrentVersion <http://vocab.nerc.ac.uk/collection/L22/current/TOOL1073/1> ;
  owl:versionInfo "1" ;
  skos:altLabel "ATSR-2"@en ;
  skos:broader <http://vocab.nerc.ac.uk/collection/L05/current/302> ;
  skos:broader <http://vocab.nerc.ac.uk/collection/L05/current/308> ;
  skos:broader <http://vocab.nerc.ac.uk/collection/L05/current/309> ;
  skos:definition "A passive optical imager with dual view composed of a 7-channel infra-red radiometer, designed to measure sea surface temperature, cloud attributes, as well as vegetation and sea-ice cover. The infra-red radiometer uses an along-track scanning telescope to focus incoming radiation from two views at different angles: one at nadir and one fore-looking at approximately 47 degrees. The same point on the Earth's surface is thus observed twice through differing atmospheric thickness, allowing for direct estimation of the atmospheric absorption and scattering, which can be used for atmospheric correction of the surface dataset. The instrument carries an on-board visible calibration system. The ATSR-2 is functionally identical to AATSR, but its structure is adapted to the ERS-2 platform. Moreover, ATSR-2 has a narrower telemetry bandwidth compared to AATSR, allowing it to collect and telemeter a smaller amount of visible data. The instrument's bandwidths are: (0.53 - 0.57)um, (0.64 - 0.68)um, (0.85 - 0.89)um, (1.31 - 1.91)um, (3.55 - 3.85)um, (10.35 - 11.35)um and (11.50 - 12.50)um. The instrument's resolution is 1 km at the instantaneous field of view (IFOV). The swath is 500 km. The accuracy of sea surface temperature measurements is approximately 0.1 degC. Flown on ERS-2. http://www.wmo-sat.info/oscar/instruments/view/56"@en ;
  skos:inScheme <http://vocab.nerc.ac.uk/scheme/SDNDEV/current> ;
  skos:notation "SDN:L22::TOOL1073" ;
  skos:note "accepted"@en ;
  skos:prefLabel "Along Track Scanning Radiometer - 2"@en ;
.
inst:TOOL1074
  rdf:type skos:Concept ;
  dcterm:date "2016-11-15 15:28:05.0" ;
  dcterm:identifier "SDN:L22::TOOL1074" ;
  dcterm:source <http://vocab.nerc.ac.uk/scheme/SDNDEV/current> ;
  pav:hasCurrentVersion <http://vocab.nerc.ac.uk/collection/L22/current/TOOL1074/1> ;
  owl:versionInfo "1" ;
  skos:altLabel "AVHRR/1"@en ;
  skos:broader <http://vocab.nerc.ac.uk/collection/L05/current/302> ;
  skos:broader <http://vocab.nerc.ac.uk/collection/L05/current/308> ;
  skos:broader <http://vocab.nerc.ac.uk/collection/L05/current/309> ;
  skos:definition "A radiation-detection imager with four spectral bands, designed to provide global data collection from the visible, near-infrared and thermal infrared portions of the electromagnetic spectrum at a high temporal resolution. Derived parameters include Sea Surface Temperatures (SST), Normalised Difference Vegetation Index (NDVI), atmospheric aerosols and volcanic ash, snow and ice distribution, cloud patterns and land-water boundaries. A flat scanning mirror undergoes a continuous 360 degrees rotation at six scans per second around an axis parallel to the Earth's surface, thus scanning a field of view perpendicular to the satellite orbit track and at such speed that adjacent scan lines are contiguous at nadir position. The AVHRR instrument has an angular resolution of 1.3 mrad and a spatial resolution of 1.1 km at nadir. The swath width is 2900 km and the scan angle is 55.4 degrees from nadir. The scanning radiometer uses four detectors to collect different bands of radiation wavelengths: (0.55 - 0.68) um, (0.725 - 1.10) um, (3.55 - 3.93) um and (10.50 - 11.50) um. The instrument does not carry an on-board calibration system. AVHRR/1 was first deployed in 1978. AVHRR/2 is an improved version comprising five channels, and was first deployed in 1981. AVHRR/3 is the latest version advanced to six channels, and first deployed in 1998. Flown on NOAA-8, NOAA-10, TIROS-N, NOAA-6. http://www.wmo-sat.info/oscar/instruments/view/60"@en ;
  skos:inScheme <http://vocab.nerc.ac.uk/scheme/SDNDEV/current> ;
  skos:notation "SDN:L22::TOOL1074" ;
  skos:note "accepted"@en ;
  skos:prefLabel "Advanced Very High Resolution Radiometer - 1"@en ;
.
inst:TOOL1075
  rdf:type skos:Concept ;
  dcterm:date "2016-11-15 15:28:05.0" ;
  dcterm:identifier "SDN:L22::TOOL1075" ;
  dcterm:source <http://vocab.nerc.ac.uk/scheme/SDNDEV/current> ;
  pav:hasCurrentVersion <http://vocab.nerc.ac.uk/collection/L22/current/TOOL1075/1> ;
  owl:versionInfo "1" ;
  skos:altLabel "AVHRR/2"@en ;
  skos:broader <http://vocab.nerc.ac.uk/collection/L05/current/302> ;
  skos:broader <http://vocab.nerc.ac.uk/collection/L05/current/308> ;
  skos:broader <http://vocab.nerc.ac.uk/collection/L05/current/309> ;
  skos:definition "A radiation-detection imager with five spectral bands, designed to provide global data collection from the visible, near-infrared and thermal infrared portions of the electromagnetic spectrum at a high temporal resolution. Derived parameters include Sea Surface Temperatures (SST), Normalised Difference Vegetation Index (NDVI), atmospheric aerosols and volcanic ash, snow and ice distribution, cloud patterns and land-water boundaries. A flat scanning mirror undergoes a continuous 360 degrees rotation at six scans per second around an axis parallel to the Earth's surface, thus scanning a field of view perpendicular to the satellite orbit track and at such speed that adjacent scan lines are contiguous at nadir position. The AVHRR instrument has an angular resolution of 1.3 mrad and a spatial resolution of 1.1 km at nadir. The swath width is 2900 km and the scan angle is 55.4 degrees from nadir. The scanning radiometer uses five detectors to collect different bands of radiation wavelengths: (0.55 - 0.68) um, (0.725 - 1.10) um, (3.55 - 3.93) um, (10.30 - 11.30) um, (11.50 - 12.50) um. The instrument does not carry an on-board calibration system. AVHRR/1 was first deployed in 1978, and only had four channels. AVHRR/2 is an improved version comprising five channels, and was first deployed in 1981. AVHRR/3 is the latest version advanced to six channels, and was first deployed in 1998. Flown on NOAA-9, NOAA-11, NOAA-12, NOAA-13, NOAA-14, NOAA-7. http://www.wmo-sat.info/oscar/instruments/view/61"@en ;
  skos:inScheme <http://vocab.nerc.ac.uk/scheme/SDNDEV/current> ;
  skos:notation "SDN:L22::TOOL1075" ;
  skos:note "accepted"@en ;
  skos:prefLabel "Advanced Very High Resolution Radiometer - 2"@en ;
.
inst:TOOL1076
  rdf:type skos:Concept ;
  dcterm:date "2016-11-15 15:28:05.0" ;
  dcterm:identifier "SDN:L22::TOOL1076" ;
  dcterm:source <http://vocab.nerc.ac.uk/scheme/SDNDEV/current> ;
  pav:hasCurrentVersion <http://vocab.nerc.ac.uk/collection/L22/current/TOOL1076/1> ;
  owl:versionInfo "1" ;
  skos:altLabel "AVHRR/3"@en ;
  skos:broader <http://vocab.nerc.ac.uk/collection/L05/current/302> ;
  skos:broader <http://vocab.nerc.ac.uk/collection/L05/current/308> ;
  skos:broader <http://vocab.nerc.ac.uk/collection/L05/current/309> ;
  skos:definition "A radiation-detection imager with six spectral bands, designed to provide global data collection from the visible, near-infrared and thermal infrared portions of the electromagnetic spectrum at a high temporal resolution. Derived parameters include Sea Surface Temperatures (SST), Normalised Difference Vegetation Index (NDVI), atmospheric aerosols and volcanic ash, snow and ice distribution, cloud patterns and land-water boundaries. A flat scanning mirror undergoes a continuous 360 degrees rotation at six scans per second around an axis parallel to the Earth's surface, thus scanning a field of view perpendicular to the satellite orbit track and at such speed that adjacent scan lines are contiguous at nadir position. The AVHRR instrument has an angular resolution of 1.3 mrad and a spatial resolution of 1.1 km at nadir. The swath width is 2900 km and the scan angle is 55.4 degrees from nadir. The scanning radiometer uses six detectors to collect different bands of radiation wavelengths: (0.58 - 0.68) um, (0.725 - 1.00) um, (1.58 - 1.64) um, (3.55 - 3.93) um, (10.30 - 11.30) um, (11.50 - 12.50) um. The instrument does not carry an on-board calibration system. The first AVHRR was deployed in 1978, and only had four channels. AVHRR/2 was an improved version comprising five channels, and first deployed in 1981. AVHRR/3 is the latest version advanced to six channels, and first deployed in 1998. Flown on Metop-A, Metop-B, Metop-C, NOAA-15, NOAA-16, NOAA-17, NOAA-18, NOAA-19. http://www.wmo-sat.info/oscar/instruments/view/62"@en ;
  skos:inScheme <http://vocab.nerc.ac.uk/scheme/SDNDEV/current> ;
  skos:notation "SDN:L22::TOOL1076" ;
  skos:note "accepted"@en ;
  skos:prefLabel "Advanced Very High Resolution Radiometer - 3"@en ;
.
inst:TOOL1077
  rdf:type skos:Concept ;
  dcterm:date "2016-11-15 15:28:05.0" ;
  dcterm:identifier "SDN:L22::TOOL1077" ;
  dcterm:source <http://vocab.nerc.ac.uk/scheme/SDNDEV/current> ;
  pav:hasCurrentVersion <http://vocab.nerc.ac.uk/collection/L22/current/TOOL1077/1> ;
  owl:versionInfo "1" ;
  skos:altLabel "ETM+"@en ;
  skos:broader <http://vocab.nerc.ac.uk/collection/L05/current/309> ;
  skos:definition "An eight-band whiskbroom scanning radiometer designed for land and vegetation observation. The instrument consists of a primary mirror sweeping across-track to produce image scans, and a scan line corrector (SLC) mirror assembly sweeping forward-to-back along-track, to compensate for the forward motion of the satellite during integration time. A panchromatic channel covers the wavelength range (0.50 - 0.90) um, at a spatial resolution of 15 m and 12000 pixel per line;  six-narrow band channels in the visible/near-infrared/short-wave infrared (VIS/NIR/SWIR) span wavelength ranges (0.45 - 0.52) um, (0.53 - 0.61), (0.63 - 0.69) um, (0.78 - 0.90) um, (1.55 - 1.75) um, (2.09 - 2.35) um,  at a spatial resolution of 30m and 6000 pixel per line; a thermal infrared (TIR) channel covers the band (10.4 - 12.5) um, at a spatial resolution of 60 m and 3000 pixel per line. The swath width is 185 km. Flown on Landsat-7. http://www.wmo-sat.info/oscar/instruments/view/136"@en ;
  skos:inScheme <http://vocab.nerc.ac.uk/scheme/SDNDEV/current> ;
  skos:notation "SDN:L22::TOOL1077" ;
  skos:note "accepted"@en ;
  skos:prefLabel "Enhanced Thematic Mapper Plus"@en ;
.
inst:TOOL1078
  rdf:type skos:Concept ;
  dcterm:date "2016-11-15 15:28:05.0" ;
  dcterm:identifier "SDN:L22::TOOL1078" ;
  dcterm:source <http://vocab.nerc.ac.uk/scheme/SDNDEV/current> ;
  pav:hasCurrentVersion <http://vocab.nerc.ac.uk/collection/L22/current/TOOL1078/1> ;
  owl:versionInfo "1" ;
  skos:altLabel "GFO-RA"@en ;
  skos:broader <http://vocab.nerc.ac.uk/collection/L05/current/186> ;
  skos:definition "A radio-occultation radar altimeter designed for ocean topography, significant wave height, and sea surface wind speed observations. A digital chirp generator produces a pulse, which is up-converted in a frequency multiplier, amplified by a power amplifier and routed to the antenna by a T/R switch; the same switch directs the return signal to the receiver, which transforms range separation into frequency separation to allow sampling using Fourier Transform techniques. The receiver carries out automatic gain control (AGC) and down-converts the return signal. GFO-RA performs continuous sampling along the sub-track (nadir-only viewing), and it is supported by a microwave radiometer (MWR) for atmospheric correction. Radar cross section and height are calibrated on board. The instrument only detects at Ku-band frequency centred at 13.5 GHz. The resolution is 25 km at sub-satellite point. The pulse-limited footprint is 2 km along the sub-track. Flown on GFO. http://www.wmo-sat.info/oscar/instruments/view/154"@en ;
  skos:inScheme <http://vocab.nerc.ac.uk/scheme/SDNDEV/current> ;
  skos:notation "SDN:L22::TOOL1078" ;
  skos:note "accepted"@en ;
  skos:prefLabel "GEOSat Follow-On Radar Altimeter"@en ;
.
inst:TOOL1079
  rdf:type skos:Concept ;
  dcterm:date "2016-11-15 15:28:05.0" ;
  dcterm:identifier "SDN:L22::TOOL1079" ;
  dcterm:source <http://vocab.nerc.ac.uk/scheme/SDNDEV/current> ;
  pav:hasCurrentVersion <http://vocab.nerc.ac.uk/collection/L22/current/TOOL1079/1> ;
  owl:versionInfo "1" ;
  skos:altLabel "GLAS"@en ;
  skos:broader <http://vocab.nerc.ac.uk/collection/L05/current/310> ;
  skos:broader <http://vocab.nerc.ac.uk/collection/L05/current/92> ;
  skos:definition "A laser-ranging (lidar) instrument designed to perform continuous global observations of clouds, atmospheric properties and ice-sheet topography, used for short-term climate and weather prediction. The instrument includes a laser system, a telescope, a Global Positioning System (GPS) and Stellar Reference System (SRS), the latter composed of a star tracker and a Laser Reference System (LRS).  The laser transmits two pulses at 40 Hz of visible green light (1064 nm) and infrared light (532 nm) towards the Earth's surface, the return signals of which are detected by the telescope and recorded along the laser pointing vector. The time interval taken by the laser pulse to make a round trip from the instrument to the Earth's surface and back, can be converted into distance; this series of altimeter measurements, together with positional measurements and calibrations carried out by the various instrument components, can be assembled to determine surface topography as well as temporal changes in surface topography. The instruments samples along-track (nadir only view) at intervals of 170m within an instantaneous field of view (IFOV) of 66m. The vertical resolution is 10cm at the surface, and 200m at cloud top. Flown on ICESat. http://www.wmo-sat.info/oscar/instruments/view/155"@en ;
  skos:inScheme <http://vocab.nerc.ac.uk/scheme/SDNDEV/current> ;
  skos:notation "SDN:L22::TOOL1079" ;
  skos:note "accepted"@en ;
  skos:prefLabel "Geoscience Laser Altimeter System"@en ;
.
inst:TOOL1080
  rdf:type skos:Concept ;
  dcterm:date "2016-11-15 15:28:05.0" ;
  dcterm:identifier "SDN:L22::TOOL1080" ;
  dcterm:source <http://vocab.nerc.ac.uk/scheme/SDNDEV/current> ;
  pav:hasCurrentVersion <http://vocab.nerc.ac.uk/collection/L22/current/TOOL1080/1> ;
  owl:versionInfo "1" ;
  skos:altLabel "GOME"@en ;
  skos:broader <http://vocab.nerc.ac.uk/collection/L05/current/314> ;
  skos:definition "An optical across-scanning, shortwave grating spectrometer, designed to measure trace gases (e.g. ozone, nitrogen dioxide) as well as aerosol distribution in the atmosphere. The instrument detects reflected sunlight from the Earth's surface and atmosphere within the ultraviolet and visible (UV/VIS) spectral range at nadir. The detected radiation is split into different wavelengths, and quantitative information on ozone (O3) and several other trace-gas species is obtained from the absorption properties of the observed spectrum. GOME has four optical channels with 1024 spectral elements each, contiguously covering a total range of (0.24 - 0.79) um at spectral resolution ranging from (0.0002 - 0.0004) um. The instrument also carries three polarisation monitoring devices (PMD), with one channel each, measuring within (0.29 - 0.79) um at a spectra resolution range of (0.11 - 0.19) um. The swath width is 960 km wide and the scan angle is 32 degrees from nadir. The pixel size is 40 x 320 km^2. Flown on ERS-2. http://www.wmo-sat.info/oscar/instruments/view/166"@en ;
  skos:inScheme <http://vocab.nerc.ac.uk/scheme/SDNDEV/current> ;
  skos:notation "SDN:L22::TOOL1080" ;
  skos:note "accepted"@en ;
  skos:prefLabel "Global Monitoring of Atmospheric Ozone"@en ;
.
inst:TOOL1081
  rdf:type skos:Concept ;
  dcterm:date "2016-11-15 15:28:05.0" ;
  dcterm:identifier "SDN:L22::TOOL1081" ;
  dcterm:source <http://vocab.nerc.ac.uk/scheme/SDNDEV/current> ;
  pav:hasCurrentVersion <http://vocab.nerc.ac.uk/collection/L22/current/TOOL1081/1> ;
  owl:versionInfo "1" ;
  skos:altLabel "GOME-2"@en ;
  skos:broader <http://vocab.nerc.ac.uk/collection/L05/current/314> ;
  skos:definition "An optical across-scanning, shortwave grating spectrometer, designed to measure trace gases (e.g. ozone, nitrogen dioxide) as well as aerosol distribution in the atmosphere. The instrument detects reflected sunlight from the Earth's surface and atmosphere within the ultraviolet, visible and near-infrared (UV/VIS/NIR) spectral range at nadir. The detected radiation is split into different wavelengths , and quantitative information on ozone (O3) and several other trace-gas species is obtained from the absorption properties of the observed spectrum. Sideways viewing for polar coverage and instrument characterisation measurements using the Moon are also carried out. GOME-2 has four optical channels with 1024 spectral elements each, contiguously covering a total range of (0.24 - 0.79) um at spectral resolution ranging from (0.0002 - 0.0005) um. The instrument also carries a polarisation monitoring device (PMD) with 200 channels, measuring within (0.31 - 0.79) um at a spectral resolution range of (0.0028 - 0.04) um. The swath width is 1920 km wide and the scan angle is 55 degrees from nadir. The pixel size is 40 x 80 km^2. Flown on Metop-A, Metop-B, Metop-C. http://www.wmo-sat.info/oscar/instruments/view/167"@en ;
  skos:inScheme <http://vocab.nerc.ac.uk/scheme/SDNDEV/current> ;
  skos:notation "SDN:L22::TOOL1081" ;
  skos:note "accepted"@en ;
  skos:prefLabel "Global Monitoring of Atmospheric Ozone - 2"@en ;
.
inst:TOOL1082
  rdf:type skos:Concept ;
  dcterm:date "2016-11-15 15:28:05.0" ;
  dcterm:identifier "SDN:L22::TOOL1082" ;
  dcterm:source <http://vocab.nerc.ac.uk/scheme/SDNDEV/current> ;
  pav:hasCurrentVersion <http://vocab.nerc.ac.uk/collection/L22/current/TOOL1082/1> ;
  owl:versionInfo "1" ;
  skos:altLabel "GOMOS"@en ;
  skos:broader <http://vocab.nerc.ac.uk/collection/L05/current/314> ;
  skos:definition "A grating spectrometer designed to perform stellar occultation measurements in the ultraviolet, visible and near-infrared spectral range to monitor the levels of ozone and other gas species in the atmosphere. The instrument operates using the technique of stellar occultation, which involves tracking a pre-selected star and making measurements of its emitted radiation through the Earth's atmosphere until it disappears behind the horizon. The spectrometer uses a grating to disperse the detected radiation into its spectrum, which holds information on the atmospheric concentration of different gases. The instrument also carries two fast photometers to detect the scintillation of the input signal, which carries information on turbulence. The spectrometer operates in approximately 1000 channels spread across three spectral bands ranging between (0.25 - 0.67) um, (0.75 - 0.77) um and (0.93 - 0.95) um, at a spectral resolution of (0.0002 - 0.0012) um. The photometers operate within the (0.47 - 0.52) um and (0.62 - 0.70) um spectral bands respectively, at a spectral resolution of 0.05 um. The instrument measures approximately 500 star occultations per day, or 25-40 occultations per orbit.  The instrument's vertical resolution is 1.7 km, whilst the horizontal effective resolution is approximately 300 km. GOMOS measures within the altitude range of (20 - 100) km. Flown on Envisat. http://www.wmo-sat.info/oscar/instruments/view/168"@en ;
  skos:inScheme <http://vocab.nerc.ac.uk/scheme/SDNDEV/current> ;
  skos:notation "SDN:L22::TOOL1082" ;
  skos:note "accepted"@en ;
  skos:prefLabel "Global Ozone Monitoring by Occultation of Stars"@en ;
.
inst:TOOL1083
  rdf:type skos:Concept ;
  dcterm:date "2016-11-15 15:28:05.0" ;
  dcterm:identifier "SDN:L22::TOOL1083" ;
  dcterm:source <http://vocab.nerc.ac.uk/scheme/SDNDEV/current> ;
  pav:hasCurrentVersion <http://vocab.nerc.ac.uk/collection/L22/current/TOOL1083/1> ;
  owl:versionInfo "1" ;
  skos:altLabel "HRS"@en ;
  skos:broader <http://vocab.nerc.ac.uk/collection/L05/current/311> ;
  skos:definition "An optical imager designed for high-resolution land observation, in particular fire fractional cover, as well as glacier, sea-ice, snow and cloud cover. The instrument carries out along-track stereoscopic measurements using two telescopes with a 20 degree fore and aft view respectively. Stereo images are thus acquired in pairs and within a 90 second interval, covering an area 120 km wide (swath), by up to 600 km long. The instrument has a panchromatic single-channel detector in the visible (VIS) spectrum within the (0.51 - 0.73) um range. The signal-to-noise ratio is 120 at 50% albedo, and the resolution at sub-satellite point is 10 m (cross-track), and 5 m (along-track). Flown on SPOT-5. http://www.wmo-sat.info/oscar/instruments/view/193"@en ;
  skos:inScheme <http://vocab.nerc.ac.uk/scheme/SDNDEV/current> ;
  skos:notation "SDN:L22::TOOL1083" ;
  skos:note "accepted"@en ;
  skos:prefLabel "High-Resolution Stereoscopic instrument"@en ;
.
inst:TOOL1084
  rdf:type skos:Concept ;
  dcterm:date "2016-11-15 15:28:05.0" ;
  dcterm:identifier "SDN:L22::TOOL1084" ;
  dcterm:source <http://vocab.nerc.ac.uk/scheme/SDNDEV/current> ;
  pav:hasCurrentVersion <http://vocab.nerc.ac.uk/collection/L22/current/TOOL1084/1> ;
  owl:versionInfo "1" ;
  skos:altLabel "IASI"@en ;
  skos:broader <http://vocab.nerc.ac.uk/collection/L05/current/308> ;
  skos:definition "A cross-nadir, hyperspectral infrared sounder, designed to measure temperature, humidity, ozone profile and total-column reactive trace gases and greenhouse gases in the troposphere and lower stratosphere. The observations retrieved by the IASI instrument are primarily used to support numerical weather prediction. Measurements are carried out by an infrared imager and a calibrated Fourier Transform Spectrometer for passive infrared remote-sensing. A Michelson interferometer with 8461 channels is used for the optical configuration of the sounder. The spectrometer operates in the (3.6 - 15.5) um spectral range, equivalent to (645 - 2760) cm^-1; the spectral resolution is 0.25 cm^-1. The imager operates in the (10.3 - 12.5) um spectral range. The swath width is approximately 2130 km. Cross-track scans consist of 30 steps of 48 km at sub-satellite point, whilst along-track scans cover one line of 48 km every 8 seconds. The horizontal resolution is 4 by 12 km near the centre of a (48 by 48) km^2 cell, whilst the vertical resolution in the lower troposphere is 1 km. Flown on Metop-A, Metop-B, Metop-C. http://www.wmo-sat.info/oscar/instruments/view/207"@en ;
  skos:inScheme <http://vocab.nerc.ac.uk/scheme/SDNDEV/current> ;
  skos:notation "SDN:L22::TOOL1084" ;
  skos:note "accepted"@en ;
  skos:prefLabel "Infrared Atmospheric Sounding Interferometer"@en ;
.
inst:TOOL1085
  rdf:type skos:Concept ;
  dcterm:date "2016-11-15 15:28:05.0" ;
  dcterm:identifier "SDN:L22::TOOL1085" ;
  dcterm:source <http://vocab.nerc.ac.uk/scheme/SDNDEV/current> ;
  pav:hasCurrentVersion <http://vocab.nerc.ac.uk/collection/L22/current/TOOL1085/1> ;
  owl:versionInfo "1" ;
  skos:altLabel "JAMI"@en ;
  skos:broader <http://vocab.nerc.ac.uk/collection/L05/current/308> ;
  skos:definition "A five-channel moderate resolution optical imager designed to carry out meteorological observations for Japan, East Asia, Australia and adjacent areas, by tracking clouds and water vapour features. The imager detects radiation from the visible and infrared spectrum using an off-axis focal telescope with two focal planes and infrared bands integrated into a single sensor assembly. The incident spectrum is then separated into visible and infrared channels by a beam splitter, and the infrared channels are further split into four bands by infrared optical filters. On-board calibration is provided for all bands. JAMI exploits the Nyquist spatial sampling technique. The imager uses the Nyquist spatial sampling technique, and detects radiation within five spectral bands of ranges (0.55 - 0.90) um, (3.50 - 4.00) um, (6.50 - 7.00) um, (10.3 - 11.3) um and (11.5 - 12.5) um. The ground resolution is 1 km for solar reflective band (VNIR) measurements, and 4 km for infrared (IR) measurements. The image frame is 21.4 degrees in longitude, and 23.6 degrees in latitude. The field of view is 0.269 degrees per swath. Flown on Himawari-6 (MTSAT-1R). http://www.wmo-sat.info/oscar/instruments/view/236"@en ;
  skos:inScheme <http://vocab.nerc.ac.uk/scheme/SDNDEV/current> ;
  skos:notation "SDN:L22::TOOL1085" ;
  skos:note "accepted"@en ;
  skos:prefLabel "Japanese Advanced Meteorological Imager"@en ;
.
inst:TOOL1086
  rdf:type skos:Concept ;
  dcterm:date "2016-11-15 15:28:05.0" ;
  dcterm:identifier "SDN:L22::TOOL1086" ;
  dcterm:source <http://vocab.nerc.ac.uk/scheme/SDNDEV/current> ;
  pav:hasCurrentVersion <http://vocab.nerc.ac.uk/collection/L22/current/TOOL1086/1> ;
  owl:versionInfo "1" ;
  skos:altLabel "MERIS"@en ;
  skos:broader <http://vocab.nerc.ac.uk/collection/L05/current/304> ;
  skos:definition "A programmable, medium-spectral resolution, imaging spectrometer which operates in the solar reflective spectral range. It was designed to observe the colour of the open surface ocean and coastal zones, in order to estimate chlorophyll concentration and water turbidity. The instrument is composed of five identical optical modules arranged side by side, each equipped with a \"push-broom\" spectrometer. Each spectrometer uses linear charge-coupled devices (CCDs) to carry out simultaneous across-track sampling as the satellite moves in the along-track direction. The MERIS instrument covers a swath width of 1150 km, and has a total field of view around nadir of 68.5 degrees. The frequency of complete earth scans is three days at the equator. Flown on Envisat. http://www.wmo-sat.info/oscar/instruments/view/277"@en ;
  skos:inScheme <http://vocab.nerc.ac.uk/scheme/SDNDEV/current> ;
  skos:notation "SDN:L22::TOOL1086" ;
  skos:note "accepted"@en ;
  skos:prefLabel "Medium-Spectral Resolution, Imaging Spectrometer"@en ;
.
inst:TOOL1087
  rdf:type skos:Concept ;
  dcterm:date "2016-11-15 15:28:05.0" ;
  dcterm:identifier "SDN:L22::TOOL1087" ;
  dcterm:source <http://vocab.nerc.ac.uk/scheme/SDNDEV/current> ;
  pav:hasCurrentVersion <http://vocab.nerc.ac.uk/collection/L22/current/TOOL1087/1> ;
  owl:versionInfo "1" ;
  skos:altLabel "MIPAS"@en ;
  skos:broader <http://vocab.nerc.ac.uk/collection/L05/current/314> ;
  skos:definition "A Fourier Transform Spectrometer, designed to perform natural occultation limb measurements to infer the chemical composition of the middle and upper atmosphere. Using a fore and side limb scanning technique, the instrument detects limb emission spectra, which is generated by sunrays that had been scattered in the atmosphere within an altitude of 5-150 km before reaching the instrument. From these measurements, the atmospheric concentration of approximately twenty chemical species can be spectroscopically identified. The space segment of MIPAS comprises front-end optics, a Michelson interferometer, a focal plane subsystem and a signal processing subsystem. On-board calibration is carried out using deep space and a blackbody inside the instrument as references. The ground segment of MIPAS calibrates the interferogram produced by the space segment and calculates the concentration profiles of the various chemical species. The spectral range is (4.15 - 14.6) um, equivalent to (685 - 2410) cm^-1. The spatial resolution is 3 km (vertical), and the field of view is 3 km by 30 km; the unapodised spectral resolution is 0.035 cm^-1. The radiometric precision is 1% within the (685-970) cm^-1 spectral range, and 3% at 2410 cm^-1. Flown on Envisat. http://www.wmo-sat.info/oscar/instruments/view/286"@en ;
  skos:inScheme <http://vocab.nerc.ac.uk/scheme/SDNDEV/current> ;
  skos:notation "SDN:L22::TOOL1087" ;
  skos:note "accepted"@en ;
  skos:prefLabel "Michelson Interferometer for Passive Atmospheric Sounding"@en ;
.
inst:TOOL1088
  rdf:type skos:Concept ;
  dcterm:date "2016-11-15 15:28:05.0" ;
  dcterm:identifier "SDN:L22::TOOL1088" ;
  dcterm:source <http://vocab.nerc.ac.uk/scheme/SDNDEV/current> ;
  pav:hasCurrentVersion <http://vocab.nerc.ac.uk/collection/L22/current/TOOL1088/1> ;
  owl:versionInfo "1" ;
  skos:altLabel "SAR-X"@en ;
  skos:broader <http://vocab.nerc.ac.uk/collection/L05/current/306> ;
  skos:definition "SAR is an active system that transmits a beam of radiation in the microwave region of the electromagnetic spectrum in order to create images of a targeted object. Its application in remote sensing allows the mapping of the Earth's surface. An antenna sends successive pulses of radio waves to a target scene, and receives and records the echo of each pulse. AS the satellites moves along track, the antenna records successive target scenes thus forming the 'synthetic antenna aperture'. Signal processing of the recorded scenes allows the creation of higher resolution images. Data collection is independent of light and heat, and is therefore possible day and night, under any weather condition. TerraSAR-X operates in three alternate operating modes: SpotLight, giving 1 m resolution for a surface area of 5 km by 10 km; StripMap, giving 3 m resolution for a surface area of 30 km by 50 km; and ScanSAR giving 16 m resolution for a surface area of 100 km by 150 km. X-Band SAR has a phased array antenna of 31 mm wavelength and 9.6 GHz frequency; this antenna allows single, dual or full polarimetric data takes. Flown on TerraSAR-X. http://www.wmo-sat.info/oscar/instruments/view/459"@en ;
  skos:inScheme <http://vocab.nerc.ac.uk/scheme/SDNDEV/current> ;
  skos:notation "SDN:L22::TOOL1088" ;
  skos:note "accepted"@en ;
  skos:prefLabel "Synthetic Aperture Radar X-band"@en ;
.
inst:TOOL1090
  rdf:type skos:Concept ;
  dcterm:date "2017-08-10 12:37:04.0" ;
  dcterm:identifier "SDN:L22::TOOL1090" ;
  dcterm:source <http://vocab.nerc.ac.uk/scheme/SDNDEV/current> ;
  pav:hasCurrentVersion <http://vocab.nerc.ac.uk/collection/L22/current/TOOL1090/2> ;
  pav:hasVersion <http://vocab.nerc.ac.uk/collection/L22/current/TOOL1090/1> ;
  owl:versionInfo "2" ;
  skos:altLabel "GOES IMAGER (8-11)"@en ;
  skos:broader <http://vocab.nerc.ac.uk/collection/L05/current/308> ;
  skos:definition "A five-channel imaging radiometer designed to measure radiant and solar reflected energy from sampled areas of the earth, with the primary mission of determining cloud cover and characteristics, as well as water vapour features and horizontal wind. The Imager's optical system collects scene radiance, which is then separated into spectral channels by beam splitters. One of the bands captures the Earth's reflected radiation in the visible part of the electro-magnetic spectrum; the other four bands sense the Earth's emitted or infrared energy. The spectral energy is then directed to different visible and infrared sets of detectors, and converted into an electrical signal by each detector. The signal goes through amplification, filtration and digitalization before being sent to a ground station through a sensor data transmitter. The Imager uses a Cassegrain telescope in conjunction with a servo-driven, two-axis gimbaled mirror scan system to simultaneously sweep an 8 km north-to south swath along an east-to-west/west-to-east path at a rate of 20 degrees per second. The Imager collects at five bands of radiation wavelengths: (0.55 - 0.75) um, which is the visible band and has a spatial resolution of 1 km; (3.80 - 4.00) um, (6.50 - 7.00) um, (10.2 - 11.2) um and (11.5 - 12.4) um, which are the infrared bands, and have a spatial resolution of 4 km. Flown on GOES-8, GOES-9, GOES-10, GOES-11, GOES-9 (GMS backup), GOES-10 (S-America). https://www.wmo-sat.info/oscar/instruments/view/217"@en ;
  skos:inScheme <http://vocab.nerc.ac.uk/scheme/SDNDEV/current> ;
  skos:notation "SDN:L22::TOOL1090" ;
  skos:note "accepted"@en ;
  skos:prefLabel "Geostationary Operational Environmental Satellite Imager (8-11)"@en ;
.
inst:TOOL1091
  rdf:type skos:Concept ;
  dcterm:date "2017-08-10 12:37:04.0" ;
  dcterm:identifier "SDN:L22::TOOL1091" ;
  dcterm:source <http://vocab.nerc.ac.uk/scheme/SDNDEV/current> ;
  pav:hasCurrentVersion <http://vocab.nerc.ac.uk/collection/L22/current/TOOL1091/2> ;
  pav:hasVersion <http://vocab.nerc.ac.uk/collection/L22/current/TOOL1091/1> ;
  owl:versionInfo "2" ;
  skos:altLabel "GOES IMAGER (12-15)"@en ;
  skos:broader <http://vocab.nerc.ac.uk/collection/L05/current/308> ;
  skos:definition "A five-channel imaging radiometer designed to measure radiant and solar reflected energy from sampled areas of the earth, with the primary mission of determining cloud cover and characteristics, as well as water vapour features and horizontal wind. The Imager's optical system collects scene radiance, which is then separated into spectral channels by beam splitters. One of the bands captures the Earth's reflected radiation in the visible part of the electro-magnetic spectrum; the other four bands sense the Earth's emitted or infrared energy. The spectral energy is then directed to different visible and infrared sets of detectors, and converted into an electrical signal by each detector. The signal goes through amplification, filtration and digitalization before being sent to a ground station through a sensor data transmitter. The Imager uses a Cassegrain telescope in conjunction with a servo-driven, two-axis gimbaled mirror scan system to simultaneously sweep an 8 km north-to south swath along an east-to-west/west-to-east path at a rate of 20 degrees per second. The Imager collects at five bands of radiation wavelengths: (0.55 - 0.75) um, which is the visible band and has a spatial resolution of 1 km; (3.80 - 4.00) um, (5.80 - 7.30) um, (10.2 - 11.2) um and (13.0 - 13.7) um, which are the infrared bands, and have a spatial resolution of 4 km. Flown on GOES-12, GOES-13, GOES-14, GOES-15, GOES-12 (S-America). https://www.wmo-sat.info/oscar/instruments/view/879"@en ;
  skos:inScheme <http://vocab.nerc.ac.uk/scheme/SDNDEV/current> ;
  skos:notation "SDN:L22::TOOL1091" ;
  skos:note "accepted"@en ;
  skos:prefLabel "Geostationary Operational Environmental Satellite Imager (12-15)"@en ;
.
inst:TOOL1120
  rdf:type skos:Concept ;
  dcterm:date "2017-04-04 10:06:11.0" ;
  dcterm:identifier "SDN:L22::TOOL1120" ;
  dcterm:source <http://vocab.nerc.ac.uk/scheme/SDNDEV/current> ;
  pav:hasCurrentVersion <http://vocab.nerc.ac.uk/collection/L22/current/TOOL1120/1> ;
  owl:versionInfo "1" ;
  skos:altLabel "AERONET SeaPRISM"@en ;
  skos:broader <http://vocab.nerc.ac.uk/collection/L05/current/304> ;
  skos:broader <http://vocab.nerc.ac.uk/collection/L05/current/308> ;
  skos:definition "A CIMEL CE 318 Sun Photometer that has been modified to validate satellite ocean colour measurements in the AERONET-OC network. It autonomously performs sky and sea radiance observations at programmable viewing and azimuth angles at centre wavelengths in the 412-1020 nanometre spectral range."@en ;
  skos:inScheme <http://vocab.nerc.ac.uk/scheme/SDNDEV/current> ;
  skos:notation "SDN:L22::TOOL1120" ;
  skos:note "accepted"@en ;
  skos:prefLabel "AERONET SeaWIFS SeaPRISM radiometer"@en ;
  skos:related <http://vocab.nerc.ac.uk/collection/B75/current/ORG00116> ;
.
inst:TOOL1261
  rdf:type skos:Concept ;
  dcterm:date "2018-08-02 15:26:57.0" ;
  dcterm:identifier "SDN:L22::TOOL1261" ;
  dcterm:source <http://vocab.nerc.ac.uk/scheme/SDNDEV/current> ;
  pav:hasCurrentVersion <http://vocab.nerc.ac.uk/collection/L22/current/TOOL1261/1> ;
  owl:versionInfo "1" ;
  skos:altLabel "UnSpec sonobuoy"@en ;
  skos:broader <http://vocab.nerc.ac.uk/collection/L05/current/369> ;
  skos:definition "An expendable underwater listening device designed to be dropped from an aircraft or a ship and deploy upon water impact. Sonobuoys include hydrophone sensors which descend underwater and send detected signals to a radio transmitter mounted on an inflatable float which stays at the surface. The transmitter subsequently sends the signals to a monitoring unit for processing, analysis and classification."@en ;
  skos:inScheme <http://vocab.nerc.ac.uk/scheme/SDNDEV/current> ;
  skos:notation "SDN:L22::TOOL1261" ;
  skos:note "accepted"@en ;
  skos:prefLabel "Unspecified sonobuoy"@en ;
.
inst:TOOL1272
  rdf:type skos:Concept ;
  dcterm:date "2018-08-02 15:26:57.0" ;
  dcterm:identifier "SDN:L22::TOOL1272" ;
  dcterm:source <http://vocab.nerc.ac.uk/scheme/SDNDEV/current> ;
  pav:hasCurrentVersion <http://vocab.nerc.ac.uk/collection/L22/current/TOOL1272/1> ;
  owl:versionInfo "1" ;
  skos:altLabel "UnSpec conductivity sensor"@en ;
  skos:broader <http://vocab.nerc.ac.uk/collection/L05/current/350> ;
  skos:definition "Instrument that measures the electrical conductivity of the water body."@en ;
  skos:inScheme <http://vocab.nerc.ac.uk/scheme/SDNDEV/current> ;
  skos:notation "SDN:L22::TOOL1272" ;
  skos:note "accepted"@en ;
  skos:prefLabel "Unspecified conductivity sensor"@en ;
.
inst:TOOL1334
  rdf:type skos:Concept ;
  dcterm:date "2019-06-13 09:51:58.0" ;
  dcterm:identifier "SDN:L22::TOOL1334" ;
  dcterm:source <http://vocab.nerc.ac.uk/scheme/SDNDEV/current> ;
  pav:hasCurrentVersion <http://vocab.nerc.ac.uk/collection/L22/current/TOOL1334/1> ;
  owl:versionInfo "1" ;
  skos:altLabel "HyperSAS radiometer"@en ;
  skos:broader <http://vocab.nerc.ac.uk/collection/L05/current/304> ;
  skos:definition "An above-water optical sensing system designed to provide continuous ocean colour measurements over the spectral range 350-800 nm. The HyperSAS can be mounted on ships and fixed platforms, or on aircrafts for remote sensing surveys. The standard configuration of the system includes one irradiance sensor to measure downwelling irradiance, and two hyperspectral radiance sensors to capture the sea surface signal. The irradiance sensor response is proportional to the cosine of the angle of incidence of the incoming radiation, while each radiance sensor has a 3 deg field of view (FOV). The orientation precision, geo-referencing and time-stamp accuracy may be improved by mounting an optional GPS unit with Satlantic tilt and heading sensor. Moreover, a radiation pyrometer may also be added to measure land or sea surface temperature."@en ;
  skos:inScheme <http://vocab.nerc.ac.uk/scheme/SDNDEV/current> ;
  skos:notation "SDN:L22::TOOL1334" ;
  skos:note "accepted"@en ;
  skos:prefLabel "Satlantic Hyperspectral Surface Acquisition System (HyperSAS) radiometer"@en ;
  skos:related <http://vocab.nerc.ac.uk/collection/B75/current/ORG00226> ;
  skos:related <http://vocab.nerc.ac.uk/collection/L35/current/MAN0027> ;
.
inst:TOOL1349
  rdf:type skos:Concept ;
  dcterm:date "2019-08-09 15:59:15.0" ;
  dcterm:identifier "SDN:L22::TOOL1349" ;
  dcterm:source <http://vocab.nerc.ac.uk/scheme/SDNDEV/current> ;
  pav:hasCurrentVersion <http://vocab.nerc.ac.uk/collection/L22/current/TOOL1349/2> ;
  pav:hasVersion <http://vocab.nerc.ac.uk/collection/L22/current/TOOL1349/1> ;
  owl:versionInfo "2" ;
  skos:altLabel "Nanometrics Titan Accelerometer"@en ;
  skos:broader <http://vocab.nerc.ac.uk/collection/L05/current/307> ;
  skos:definition "A force balance triaxial accelerometer for use in free-field strong-motion ground monitoring, or state-of-health monitoring of large structures. Simultaneous measurements are made in three orthogonal directions, and it incorporates digitally selectable full scale range and offset zeroing capabilities. The Titans features are ideal for remote deployments. It has an operational frequency bandwidth from DC to 430 Hz, with 166 dB dynamic range. It has a full-scale range of +/- 0.25 g to +/- 4 g with independent horizontal and vertical range selection."@en ;
  skos:inScheme <http://vocab.nerc.ac.uk/scheme/SDNDEV/current> ;
  skos:notation "SDN:L22::TOOL1349" ;
  skos:note "accepted"@en ;
  skos:prefLabel "Nanometrics Titan Accelerometer"@en ;
  skos:related <http://vocab.nerc.ac.uk/collection/B75/current/ORG01193> ;
  skos:related <http://vocab.nerc.ac.uk/collection/L35/current/MAN0048> ;
.
inst:TOOL1351
  rdf:type skos:Concept ;
  dcterm:date "2019-08-09 15:57:21.0" ;
  dcterm:identifier "SDN:L22::TOOL1351" ;
  dcterm:source <http://vocab.nerc.ac.uk/scheme/SDNDEV/current> ;
  pav:hasCurrentVersion <http://vocab.nerc.ac.uk/collection/L22/current/TOOL1351/2> ;
  pav:hasVersion <http://vocab.nerc.ac.uk/collection/L22/current/TOOL1351/1> ;
  owl:versionInfo "2" ;
  skos:altLabel "Nanometrics Titan EA"@en ;
  skos:broader <http://vocab.nerc.ac.uk/collection/L05/current/307> ;
  skos:definition "A strong motion ethernet accelerograph designed for high precision observational and structural engineering applications, such as monitoring the response of a structure to ground acceleration (e.g. earthquakes). It features the same triaxial sensor and digitiser/recorder technology as the Titan Strong Motion Accelerometer (SMA) but features power-over-ethernet and Network Timing capabilities specifically designed for networked deployments on civil structures such as hydro-electric dams and bridges. A single CAT5 ethernet cable is required for all functions: power, precision, timing, data and management. The Titan EA Master is also available which incorporates a GNSS receiver to get accurate satellite timings. It has an operational frequency bandwidth from DC to 430 Hz, with 166 dB dynamic range. It has a full-scale range of +/- 0.25 g to +/- 4 g with independent horizontal and vertical range selection."@en ;
  skos:inScheme <http://vocab.nerc.ac.uk/scheme/SDNDEV/current> ;
  skos:notation "SDN:L22::TOOL1351" ;
  skos:note "accepted"@en ;
  skos:prefLabel "Nanometrics Titan Ethernet Accelerograph"@en ;
  skos:related <http://vocab.nerc.ac.uk/collection/B75/current/ORG01193> ;
  skos:related <http://vocab.nerc.ac.uk/collection/L35/current/MAN0048> ;
.
inst:TOOL1352
  rdf:type skos:Concept ;
  dcterm:date "2019-08-09 15:57:45.0" ;
  dcterm:identifier "SDN:L22::TOOL1352" ;
  dcterm:source <http://vocab.nerc.ac.uk/scheme/SDNDEV/current> ;
  pav:hasCurrentVersion <http://vocab.nerc.ac.uk/collection/L22/current/TOOL1352/2> ;
  pav:hasVersion <http://vocab.nerc.ac.uk/collection/L22/current/TOOL1352/1> ;
  owl:versionInfo "2" ;
  skos:altLabel "Nanometrics Titan SMA"@en ;
  skos:broader <http://vocab.nerc.ac.uk/collection/L05/current/307> ;
  skos:definition "A strong motion accelerograph designed for high precision observational and structural engineering applications, such as monitoring the response of a structure to ground acceleration (e.g. earthquakes). It features the same triaxial sensor as the Titan Accelerometer, but features an integrated digitiser and recorder to facilitate both standalone networked and free-field monitoring deployments. It offers GNSS, PTP or NTP timing, HTTP data communications, and data retrieval via SD card or local ethernet in MiniSEED or ASCII formats. It can detect P-wave events and broadcast warnings. It has a latency of 0.25 seconds, an operational frequency bandwidth from DC to 430 Hz, with 166 dB dynamic range. It has a full-scale range of +/- 0.25 g to +/- 4 g with independent horizontal and vertical range selection."@en ;
  skos:inScheme <http://vocab.nerc.ac.uk/scheme/SDNDEV/current> ;
  skos:notation "SDN:L22::TOOL1352" ;
  skos:note "accepted"@en ;
  skos:prefLabel "Nanometrics Titan Strong Motion Accelerograph"@en ;
  skos:related <http://vocab.nerc.ac.uk/collection/B75/current/ORG01193> ;
  skos:related <http://vocab.nerc.ac.uk/collection/L35/current/MAN0048> ;
.
inst:TOOL1477
  rdf:type skos:Concept ;
  dcterm:date "2020-06-04 16:56:25.0" ;
  dcterm:identifier "SDN:L22::TOOL1477" ;
  dcterm:source <http://vocab.nerc.ac.uk/scheme/SDNDEV/current> ;
  pav:hasCurrentVersion <http://vocab.nerc.ac.uk/collection/L22/current/TOOL1477/1> ;
  owl:versionInfo "1" ;
  skos:altLabel "Unspecified telescope"@en ;
  skos:broader <http://vocab.nerc.ac.uk/collection/L05/current/393> ;
  skos:definition "An optical device that renders distant objects more distinct by enlarging their images on a single retina of the observer. Consisting of various types such as spotting scopes, fieldscopes and monoculars, they are used for observation of distant objects on the Earth's surface. Reflected visible light is converged via an objective lens to magnify the view, which is initially inverted. An erect (non-inverted) image is achieved either by an erecting lens (long instrument) or a prism (compact instrument). Very small instruments may be of the Galilean type, which yields an erect image using a positive objective lens and a negative eyepiece lens. Terrestrial telescopes typically use objective lenses 50 to 100 mm in diameter with 20x or 30x eyepiece magnification but, this can vary."@en ;
  skos:inScheme <http://vocab.nerc.ac.uk/scheme/SDNDEV/current> ;
  skos:notation "SDN:L22::TOOL1477" ;
  skos:note "accepted"@en ;
  skos:prefLabel "Unspecified telescope"@en ;
  skos:related <http://vocab.nerc.ac.uk/collection/B75/current/UNSPEC> ;
  skos:related <http://vocab.nerc.ac.uk/collection/L35/current/MAN0001> ;
.
inst:TOOL1478
  rdf:type skos:Concept ;
  dcterm:date "2020-06-04 16:56:25.0" ;
  dcterm:identifier "SDN:L22::TOOL1478" ;
  dcterm:source <http://vocab.nerc.ac.uk/scheme/SDNDEV/current> ;
  pav:hasCurrentVersion <http://vocab.nerc.ac.uk/collection/L22/current/TOOL1478/1> ;
  owl:versionInfo "1" ;
  skos:altLabel "Unspecified binoculars"@en ;
  skos:broader <http://vocab.nerc.ac.uk/collection/L05/current/393> ;
  skos:definition "An optical device that renders distant objects more distinct by enlarging their images on both retinas of the observer. They are used for observation of distant objects on the Earth's surface. Unlike telescopes, binoculars present two images from slightly different viewpoints, producing a merged view with an impression of depth for the observer. Reflected visible light is converged via two objective lenses to magnify the view, which is initially inverted. An erect (non-inverted) image is achieved either by an erecting lens or a prism. Porro prism binoculars use a pair of porro prisms in a Z configuration to erect the image, offering a bright image and good depth sensation. Roof prism binoculars are more compact as the objectives lenses are in line with the eyepieces, but produce images with reduced brightness. Very small instruments may be of the Galilean type, which yields an erect image using a positive objective lens and a negative eyepiece lens. Hand-held binoculars typically use objective lenses 25 to 50 mm in diameter with 7x to 10x eyepiece magnification, but this can vary."@en ;
  skos:inScheme <http://vocab.nerc.ac.uk/scheme/SDNDEV/current> ;
  skos:notation "SDN:L22::TOOL1478" ;
  skos:note "accepted"@en ;
  skos:prefLabel "Unspecified binoculars"@en ;
  skos:related <http://vocab.nerc.ac.uk/collection/B75/current/UNSPEC> ;
  skos:related <http://vocab.nerc.ac.uk/collection/L35/current/MAN0001> ;
.
inst:TOOL1591
  rdf:type skos:Concept ;
  dcterm:date "2021-01-18 12:15:06.0" ;
  dcterm:identifier "SDN:L22::TOOL1591" ;
  dcterm:source <http://vocab.nerc.ac.uk/scheme/SDNDEV/current> ;
  pav:hasCurrentVersion <http://vocab.nerc.ac.uk/collection/L22/current/TOOL1591/1> ;
  owl:versionInfo "1" ;
  skos:altLabel "Kistler 8395A accelerometer"@en ;
  skos:broader <http://vocab.nerc.ac.uk/collection/L05/current/307> ;
  skos:definition "A triaxial capacitive MEMS accelerometer designed to measure low frequency vibration and acceleration for a variety of applications, such as civil engineering, aerospace, structural analysis, and more. It features a quartz element which is sensitive to either compressive or shear loads. The sensor is connected to an electronic device for converting the charge signal into a voltage signal proportional to the mechanical force. The conversion is made either by means of a separate charge amplifier or an impedance converter with coupler, typically integrated into the sensor The 8395A also features built-in low-pass filters. It has a measurement range of 2-250 g, a frequency response of 0-1000 hz (+/- 5 %) and an operating temperature range from -54 to +121 deg C."@en ;
  skos:inScheme <http://vocab.nerc.ac.uk/scheme/SDNDEV/current> ;
  skos:notation "SDN:L22::TOOL1591" ;
  skos:note "accepted"@en ;
  skos:prefLabel "Kistler K-Beam 8395A capacitive MEMS triaxial accelerometer series"@en ;
  skos:related <http://vocab.nerc.ac.uk/collection/B75/current/ORG01766> ;
  skos:related <http://vocab.nerc.ac.uk/collection/L35/current/MAN0142> ;
.
inst:TOOL1624
  rdf:type skos:Concept ;
  dcterm:date "2021-02-10 18:43:00.0" ;
  dcterm:identifier "SDN:L22::TOOL1624" ;
  dcterm:source <http://vocab.nerc.ac.uk/scheme/SDNDEV/current> ;
  pav:hasCurrentVersion <http://vocab.nerc.ac.uk/collection/L22/current/TOOL1624/1> ;
  owl:versionInfo "1" ;
  skos:altLabel "Thales DG16 DGPS"@en ;
  skos:broader <http://vocab.nerc.ac.uk/collection/L05/current/301> ;
  skos:definition "A 16 channel Differential Global Positioning System (DGPS) receiver with 12 GPS L1 code and carrier channels. The receiver incorporates signals from 2 Satellite Based Augmentation System (SBAS) channels and 2 300 KHz DGPS beacon channels, to provide up to 20 Hz sub-metre three-dimensional differential positioning. The receiver uses a Receiver Autonomous Integrated Monitoring (RAIM) algorithm to exclude satellite signals with consistent bias errors, further improving accuracy and reliability. In differential mode, the receiver has an accuracy of 40 cm, with a velocity accuracy of 0.1 knots."@en ;
  skos:inScheme <http://vocab.nerc.ac.uk/scheme/SDNDEV/current> ;
  skos:notation "SDN:L22::TOOL1624" ;
  skos:note "accepted"@en ;
  skos:prefLabel "Thales DG16 Differential Global Positioning System receiver"@en ;
  skos:related <http://vocab.nerc.ac.uk/collection/B75/current/ORG01756> ;
  skos:related <http://vocab.nerc.ac.uk/collection/L35/current/MAN0125> ;
.
inst:TOOL1625
  rdf:type skos:Concept ;
  dcterm:date "2021-02-10 18:43:00.0" ;
  dcterm:identifier "SDN:L22::TOOL1625" ;
  dcterm:source <http://vocab.nerc.ac.uk/scheme/SDNDEV/current> ;
  pav:hasCurrentVersion <http://vocab.nerc.ac.uk/collection/L22/current/TOOL1625/1> ;
  owl:versionInfo "1" ;
  skos:altLabel "Forsberg DNAV-212 DGPS"@en ;
  skos:broader <http://vocab.nerc.ac.uk/collection/L05/current/301> ;
  skos:definition "A 12 channel Differential Global Positioning System (DGPS) receiver with an automatic 2 channel beacon receiver. The receiver yields real-time positioning, ground speed, course, and time measurement data at an output rate of 10 Hz. The instrument has applications in GIS data collection, agriculture and hydrographic surveys, providing continuous sub-metre positional accuracy with a latency of 15-40 ms. The Starlink DNAV-212 is waterproof, and designed for rugged professional use. It features multiple interface ports, enabling it to interface easily with software packages or systems capable of accepting standard GPS data input."@en ;
  skos:inScheme <http://vocab.nerc.ac.uk/scheme/SDNDEV/current> ;
  skos:notation "SDN:L22::TOOL1625" ;
  skos:note "accepted"@en ;
  skos:prefLabel "Forsberg Starlink DNAV-212 Differential Global Positioning System receiver"@en ;
  skos:related <http://vocab.nerc.ac.uk/collection/B75/current/ORG01753> ;
  skos:related <http://vocab.nerc.ac.uk/collection/L35/current/MAN0126> ;
.
inst:TOOL1626
  rdf:type skos:Concept ;
  dcterm:date "2021-02-10 18:43:00.0" ;
  dcterm:identifier "SDN:L22::TOOL1626" ;
  dcterm:source <http://vocab.nerc.ac.uk/scheme/SDNDEV/current> ;
  pav:hasCurrentVersion <http://vocab.nerc.ac.uk/collection/L22/current/TOOL1626/1> ;
  owl:versionInfo "1" ;
  skos:altLabel "Kongsberg Seatex DPS 112"@en ;
  skos:broader <http://vocab.nerc.ac.uk/collection/L05/current/301> ;
  skos:definition "A combined Differential Global Positioning System (DGPS) L1/L2, GLONASS L1/L2 and Satellite Based Augmentation System (SBAS) receiver. Features a built-in display for system configuration and status monitoring. Positional accuracy is <1 m, 95% CEP (DGPS/DGLONASS and SBAS), with the possibility improved (10 cm) accuracy when utilising the Fugro Seastar G2 service of reference stations. Output rate of 1 Hz."@en ;
  skos:inScheme <http://vocab.nerc.ac.uk/scheme/SDNDEV/current> ;
  skos:notation "SDN:L22::TOOL1626" ;
  skos:note "accepted"@en ;
  skos:prefLabel "Kongsberg Seatex Differential Positioning Sensor 112"@en ;
  skos:related <http://vocab.nerc.ac.uk/collection/B75/current/ORG00360> ;
  skos:related <http://vocab.nerc.ac.uk/collection/L35/current/MAN0015> ;
.
inst:TOOL1627
  rdf:type skos:Concept ;
  dcterm:date "2021-02-10 18:43:00.0" ;
  dcterm:identifier "SDN:L22::TOOL1627" ;
  dcterm:source <http://vocab.nerc.ac.uk/scheme/SDNDEV/current> ;
  pav:hasCurrentVersion <http://vocab.nerc.ac.uk/collection/L22/current/TOOL1627/1> ;
  owl:versionInfo "1" ;
  skos:altLabel "Trimble DSM 232 GPS"@en ;
  skos:broader <http://vocab.nerc.ac.uk/collection/L05/current/301> ;
  skos:definition "The Trimble DSM 232 GPS is modular GPS receiver, with a separate antenna and receiver unit. The modularity enables different antenna options, in order to accept GPS corrections from a variety of sources, allowing sub-metre, decimetre, or centimetre accuracy depending on the user application. Compatible with Satellite Based Augmentation Systems (SBAS) such as WAAS and EGNOS for centimetre accuracy. The DSM 232 receiver outputs positional data at rates up to 10 Hz."@en ;
  skos:inScheme <http://vocab.nerc.ac.uk/scheme/SDNDEV/current> ;
  skos:notation "SDN:L22::TOOL1627" ;
  skos:note "accepted"@en ;
  skos:prefLabel "Trimble DSM 232 Global Positioning System receiver"@en ;
  skos:related <http://vocab.nerc.ac.uk/collection/B75/current/ORG00357> ;
  skos:related <http://vocab.nerc.ac.uk/collection/L35/current/MAN0077> ;
.
inst:TOOL1633
  rdf:type skos:Concept ;
  dcterm:date "2021-02-10 18:43:00.0" ;
  dcterm:identifier "SDN:L22::TOOL1633" ;
  dcterm:source <http://vocab.nerc.ac.uk/scheme/SDNDEV/current> ;
  pav:hasCurrentVersion <http://vocab.nerc.ac.uk/collection/L22/current/TOOL1633/1> ;
  owl:versionInfo "1" ;
  skos:altLabel "Furuno GP170"@en ;
  skos:broader <http://vocab.nerc.ac.uk/collection/L05/current/301> ;
  skos:definition "A 12-channel Global Positioning System (GPS) receiver. The GP170 outputs positional information, in addition to speed over ground and course over ground, and features a visual plotter. Optional dual-channel Satellite Based Augmentation System (SBAS) beacon receiver in the frequency range of 283.5 to 325 kHz and Differential GPS (DGPS) radio beacon receiver (requiring GPA-021S antenna unit). Designed for application on large yachts, ferries, and commercial vessels. Accuracies of <10 m (GPS), <5 m (DGPS), <3 m (WAAS), and <7 m (MSAS). Outputs positional data at a rate of 10 Hz."@en ;
  skos:inScheme <http://vocab.nerc.ac.uk/scheme/SDNDEV/current> ;
  skos:notation "SDN:L22::TOOL1633" ;
  skos:note "accepted"@en ;
  skos:prefLabel "Furuno Navigator GP170 Global Positioning System receiver"@en ;
  skos:related <http://vocab.nerc.ac.uk/collection/B75/current/ORG00571> ;
  skos:related <http://vocab.nerc.ac.uk/collection/L35/current/MAN0115> ;
.
inst:TOOL1638
  rdf:type skos:Concept ;
  dcterm:date "2021-02-11 16:32:18.0" ;
  dcterm:identifier "SDN:L22::TOOL1638" ;
  dcterm:source <http://vocab.nerc.ac.uk/scheme/SDNDEV/current> ;
  pav:hasCurrentVersion <http://vocab.nerc.ac.uk/collection/L22/current/TOOL1638/1> ;
  owl:versionInfo "1" ;
  skos:altLabel "Smartfin temperature sensor"@en ;
  skos:broader <http://vocab.nerc.ac.uk/collection/L05/current/134> ;
  skos:definition "Smartfin is a surfboard fin with integrated research grade ocean health sensors. Integrated sensors currently include temperature, motion, and GPS sensors (pH, oxygen, algae, and water clarity sensors could be added in future). It has applications in large scale citizen science and funded research projects. The external sensor is on the tip of the fin. There is also an internal sensor on the motherboard in the centre of the fin. The external sensor is more accurate and has a quicker response than the internal sensor."@en ;
  skos:inScheme <http://vocab.nerc.ac.uk/scheme/SDNDEV/current> ;
  skos:notation "SDN:L22::TOOL1638" ;
  skos:note "accepted"@en ;
  skos:prefLabel "Smartfin temperature sensor"@en ;
  skos:related <http://vocab.nerc.ac.uk/collection/B75/current/ORG01215> ;
  skos:related <http://vocab.nerc.ac.uk/collection/L35/current/MAN0159> ;
.
inst:TOOL1675
  rdf:type skos:Concept ;
  dcterm:date "2021-04-20 15:56:20.0" ;
  dcterm:identifier "SDN:L22::TOOL1675" ;
  dcterm:source <http://vocab.nerc.ac.uk/scheme/SDNDEV/current> ;
  pav:hasCurrentVersion <http://vocab.nerc.ac.uk/collection/L22/current/TOOL1675/1> ;
  owl:versionInfo "1" ;
  skos:altLabel "Vaisala FD70 series"@en ;
  skos:broader <http://vocab.nerc.ac.uk/collection/L05/current/305> ;
  skos:definition "A series of forward scatter sensors designed for precipitation type identification, plus intensity and accumulation quantification. They also measure droplet size distributions and reflectivity. The series includes the FD70, FD71 Visibility sensor and the FD71P Visibility and Present Weather sensor. The FD71P incorporates a Vaisala HMP155 HUMICAP probe, which measures the humidity and temperature of ambient air. A near infra-red light source is transmitted and optically transformed into a thin light sheet. The receiver measures the forward scattered light at an angle of 42 degrees and evaluates every precipitation particle with respect to signal strength and time to determine particle size, shape, and fall speed. The look-down geometry and hood heating protect the sensor windows against external disturbances. The FD70 series complies with ICAO, FAA, and WMO requirements and uses WMO and NWS weather codes in reporting. It has a visibility up to 100 k and an optimal forward scattering angle of 42 degrees. It has a 5 MHz sampling frequency and 5 s measuring cycle."@en ;
  skos:inScheme <http://vocab.nerc.ac.uk/scheme/SDNDEV/current> ;
  skos:notation "SDN:L22::TOOL1675" ;
  skos:note "accepted"@en ;
  skos:prefLabel "Vaisala FD70 Forward Scatter Sensor series"@en ;
  skos:related <http://vocab.nerc.ac.uk/collection/B75/current/ORG00323> ;
  skos:related <http://vocab.nerc.ac.uk/collection/L35/current/MAN0025> ;
.
inst:TOOL1734
  rdf:type skos:Concept ;
  dcterm:date "2022-10-24 12:57:12.0" ;
  dcterm:identifier "SDN:L22::TOOL1734" ;
  dcterm:source <http://vocab.nerc.ac.uk/scheme/SDNDEV/current> ;
  pav:hasCurrentVersion <http://vocab.nerc.ac.uk/collection/L22/current/TOOL1734/2> ;
  pav:hasVersion <http://vocab.nerc.ac.uk/collection/L22/current/TOOL1734/1> ;
  owl:versionInfo "2" ;
  skos:altLabel "K&Z SGR-V"@en ;
  skos:broader <http://vocab.nerc.ac.uk/collection/L05/current/308> ;
  skos:definition "The SGR3 is a pyrgeometer, designed for meteorological measurements of downward atmospheric long wave radiation. It uses a specially designed silicon window, and, on the inside, a solar-blind filter blocks solar radiation. The SGR3 data represents the radiation exchange within the whole hemisphere. This is because the reference SGR3 is calibrated outdoors with respect to a reference CGR4, which has a 180 degrees field of view. The instrument's spectral range (overall) is 4.4 to 50 micro meters (4400 to 50000 nm), it's response time (95%) is < 18 s, and its operational temperature range is -40 to +80 degrees Celsius."@en ;
  skos:inScheme <http://vocab.nerc.ac.uk/scheme/SDNDEV/current> ;
  skos:notation "SDN:L22::TOOL1734" ;
  skos:note "accepted"@en ;
  skos:prefLabel "Kipp and Zonen SGR3 V pyrgeometer"@en ;
  skos:related <http://vocab.nerc.ac.uk/collection/B75/current/ORG00324> ;
  skos:related <http://vocab.nerc.ac.uk/collection/L35/current/MAN0041> ;
.
inst:TOOL1873
  rdf:type skos:Concept ;
  dcterm:date "2022-11-01 14:23:59.0" ;
  dcterm:identifier "SDN:L22::TOOL1873" ;
  dcterm:source <http://vocab.nerc.ac.uk/scheme/SDNDEV/current> ;
  pav:hasCurrentVersion <http://vocab.nerc.ac.uk/collection/L22/current/TOOL1873/1> ;
  owl:versionInfo "1" ;
  skos:altLabel "K&Z CMP6 pyranometer"@en ;
  skos:broader <http://vocab.nerc.ac.uk/collection/L05/current/308> ;
  skos:definition "A first class pyranometer that monitors solar radiation for the full solar spectrum range, which is fully compliant with all ISO 9060 spectrally flat Class B instrument performance criteria. It uses a blackened thermopile composed of a 64-thermocouple junction sensing element, is protected by two glass domes and features increased thermal mass to improve performance. Designed for use in environmental monitoring, solar resource assessment and solar power performance applications. The instrument sensitivity is 5 - 20 microV/W m-2, impedance is 20 - 200 ohms, maximum irradiance is 2000 W/m2, spectral range is 285 - 2800 nm, and expected daily uncertainty is < 5%."@en ;
  skos:inScheme <http://vocab.nerc.ac.uk/scheme/SDNDEV/current> ;
  skos:notation "SDN:L22::TOOL1873" ;
  skos:note "accepted"@en ;
  skos:prefLabel "Kipp and Zonen CMP6 pyranometer"@en ;
  skos:related <http://vocab.nerc.ac.uk/collection/B75/current/ORG00324> ;
  skos:related <http://vocab.nerc.ac.uk/collection/L35/current/MAN0041> ;
.
inst:TOOL1885
  rdf:type skos:Concept ;
  dcterm:date "2022-12-21 16:50:36.0" ;
  dcterm:identifier "SDN:L22::TOOL1885" ;
  dcterm:source <http://vocab.nerc.ac.uk/scheme/SDNDEV/current> ;
  pav:hasCurrentVersion <http://vocab.nerc.ac.uk/collection/L22/current/TOOL1885/1> ;
  owl:versionInfo "1" ;
  skos:altLabel "Unspecified quanta meter"@en ;
  skos:broader sdev:LAB20 ;
  skos:definition "A quanta and energy meter with applications in primary production studies. The instrument is used to measure the amount of light available for photosynthesis. As this is a photoelectric process, light is described in terms of quanta per second per surface unit for unit wavelength for the specific wavelength range 350 - 700 nm. This provides a complete spectral analysis of the energy available for photosynthesis."@en ;
  skos:inScheme <http://vocab.nerc.ac.uk/scheme/SDNDEV/current> ;
  skos:notation "SDN:L22::TOOL1885" ;
  skos:note "accepted"@en ;
  skos:prefLabel "Unspecified quanta spectrophotometer"@en ;
  skos:related <http://vocab.nerc.ac.uk/collection/B75/current/UNSPEC> ;
  skos:related <http://vocab.nerc.ac.uk/collection/L35/current/MAN0001> ;
.
inst:seavoxdevicecatalog
  rdf:type skos:Collection ;
  dcterm:alternative "SeaVoX Device Catalogue" ;
  dcterm:creator "SeaDataNet and MarineXML Vocabulary Content Governance Group" ;
  dcterm:date "2023-03-07 02:00:03.0" ;
  dcterm:description "Terms for distinct sampling or measuring devices that may be identified in the real world in terms of manufacturer and model number." ;
  dcterm:license <https://creativecommons.org/licenses/by/4.0> ;
  dcterm:publisher "Natural Environment Research Council" ;
  dcterm:title "SeaVoX Device Catalogue" ;
  grg:RE_RegisterManager "British Oceanographic Data Centre" ;
  grg:RE_RegisterOwner "SeaDataNet and MarineXML Vocabulary Content Governance Group" ;
  rdfs:comment "Group set up under the joint auspices of the SeaDataNet project and the Intergovernmental Oceanographic Commission MarineXML Steering Group for controlled vocabulary governance in the marine domain" ;
  rdfs:seeAlso <https://github.com/nvs-vocabs/L22> ;
  owl:versionInfo "613" ;
  skos:altLabel "SeaVoX Device Catalogue" ;
  skos:member inst:NETT0001 ;
  skos:member inst:NETT0002 ;
  skos:member inst:NETT0003 ;
  skos:member inst:NETT0005 ;
  skos:member inst:NETT0006 ;
  skos:member inst:NETT0009 ;
  skos:member inst:NETT0010 ;
  skos:member inst:NETT0012 ;
  skos:member inst:NETT0016 ;
  skos:member inst:NETT0019 ;
  skos:member inst:NETT0020 ;
  skos:member inst:NETT0022 ;
  skos:member inst:NETT0023 ;
  skos:member inst:NETT0024 ;
  skos:member inst:NETT0026 ;
  skos:member inst:NETT0027 ;
  skos:member inst:NETT0030 ;
  skos:member inst:NETT0031 ;
  skos:member inst:NETT0032 ;
  skos:member inst:NETT0034 ;
  skos:member inst:NETT0035 ;
  skos:member inst:NETT0036 ;
  skos:member inst:NETT0039 ;
  skos:member inst:NETT0040 ;
  skos:member inst:NETT0041 ;
  skos:member inst:NETT0042 ;
  skos:member inst:NETT0043 ;
  skos:member inst:NETT0044 ;
  skos:member inst:NETT0045 ;
  skos:member inst:NETT0047 ;
  skos:member inst:NETT0052 ;
  skos:member inst:NETT0053 ;
  skos:member inst:NETT0054 ;
  skos:member inst:NETT0055 ;
  skos:member inst:NETT0056 ;
  skos:member inst:NETT0057 ;
  skos:member inst:NETT0058 ;
  skos:member inst:NETT0059 ;
  skos:member inst:NETT0060 ;
  skos:member inst:NETT0061 ;
  skos:member inst:NETT0062 ;
  skos:member inst:NETT0063 ;
  skos:member inst:NETT0065 ;
  skos:member inst:NETT0066 ;
  skos:member inst:NETT0067 ;
  skos:member inst:NETT0068 ;
  skos:member inst:NETT0071 ;
  skos:member inst:NETT0072 ;
  skos:member inst:NETT0073 ;
  skos:member inst:NETT0074 ;
  skos:member inst:NETT0075 ;
  skos:member inst:NETT0077 ;
  skos:member inst:NETT0078 ;
  skos:member inst:NETT0079 ;
  skos:member inst:NETT0080 ;
  skos:member inst:NETT0090 ;
  skos:member inst:NETT0091 ;
  skos:member inst:NETT0092 ;
  skos:member inst:NETT0095 ;
  skos:member inst:NETT0096 ;
  skos:member inst:NETT0098 ;
  skos:member inst:NETT0100 ;
  skos:member inst:NETT0102 ;
  skos:member inst:NETT0103 ;
  skos:member inst:NETT0104 ;
  skos:member inst:NETT0105 ;
  skos:member inst:NETT0106 ;
  skos:member inst:NETT0108 ;
  skos:member inst:NETT0109 ;
  skos:member inst:NETT0111 ;
  skos:member inst:NETT0112 ;
  skos:member inst:NETT0113 ;
  skos:member inst:NETT0114 ;
  skos:member inst:NETT0115 ;
  skos:member inst:NETT0116 ;
  skos:member inst:NETT0118 ;
  skos:member inst:NETT0122 ;
  skos:member inst:NETT0124 ;
  skos:member inst:NETT0125 ;
  skos:member inst:NETT0126 ;
  skos:member inst:NETT0127 ;
  skos:member inst:NETT0128 ;
  skos:member inst:NETT0129 ;
  skos:member inst:NETT0131 ;
  skos:member inst:NETT0132 ;
  skos:member inst:NETT0133 ;
  skos:member inst:NETT0134 ;
  skos:member inst:NETT0135 ;
  skos:member inst:NETT0136 ;
  skos:member inst:NETT0137 ;
  skos:member inst:NETT0138 ;
  skos:member inst:NETT0139 ;
  skos:member inst:NETT0140 ;
  skos:member inst:NETT0141 ;
  skos:member inst:NETT0142 ;
  skos:member inst:NETT0143 ;
  skos:member inst:NETT0144 ;
  skos:member inst:NETT0145 ;
  skos:member inst:NETT0147 ;
  skos:member inst:NETT0150 ;
  skos:member inst:NETT0151 ;
  skos:member inst:NETT0153 ;
  skos:member inst:NETT0154 ;
  skos:member inst:NETT0155 ;
  skos:member inst:NETT0161 ;
  skos:member inst:NETT0162 ;
  skos:member inst:NETT0163 ;
  skos:member inst:NETT0164 ;
  skos:member inst:NETT0165 ;
  skos:member inst:NETT0166 ;
  skos:member inst:NETT0167 ;
  skos:member inst:NETT0169 ;
  skos:member inst:NETT0171 ;
  skos:member inst:NETT0173 ;
  skos:member inst:NETT0174 ;
  skos:member inst:NETT0175 ;
  skos:member inst:NETT0176 ;
  skos:member inst:NETT0177 ;
  skos:member inst:NETT0178 ;
  skos:member inst:NETT0179 ;
  skos:member inst:NETT0180 ;
  skos:member inst:NETT0181 ;
  skos:member inst:NETT0182 ;
  skos:member inst:NETT0183 ;
  skos:member inst:NETT0184 ;
  skos:member inst:NETT0186 ;
  skos:member inst:NETT0188 ;
  skos:member inst:NETT0189 ;
  skos:member inst:NETT0190 ;
  skos:member inst:NETT0191 ;
  skos:member inst:NETT0192 ;
  skos:member inst:NETT0195 ;
  skos:member inst:NETT0196 ;
  skos:member inst:NETT0197 ;
  skos:member inst:NETT0198 ;
  skos:member inst:NETT0199 ;
  skos:member inst:NETT0200 ;
  skos:member inst:NETT0201 ;
  skos:member inst:NETT0202 ;
  skos:member inst:TOOL0001 ;
  skos:member inst:TOOL000X ;
  skos:member inst:TOOL0078 ;
  skos:member inst:TOOL0148 ;
  skos:member inst:TOOL0199 ;
  skos:member inst:TOOL0235 ;
  skos:member inst:TOOL0236 ;
  skos:member inst:TOOL0237 ;
  skos:member inst:TOOL0238 ;
  skos:member inst:TOOL0248 ;
  skos:member inst:TOOL0281 ;
  skos:member inst:TOOL0282 ;
  skos:member inst:TOOL0283 ;
  skos:member inst:TOOL0304 ;
  skos:member inst:TOOL0313 ;
  skos:member inst:TOOL0337 ;
  skos:member inst:TOOL0348 ;
  skos:member inst:TOOL0349 ;
  skos:member inst:TOOL0353 ;
  skos:member inst:TOOL0354 ;
  skos:member inst:TOOL0355 ;
  skos:member inst:TOOL0356 ;
  skos:member inst:TOOL0357 ;
  skos:member inst:TOOL0358 ;
  skos:member inst:TOOL0359 ;
  skos:member inst:TOOL0381 ;
  skos:member inst:TOOL0388 ;
  skos:member inst:TOOL0389 ;
  skos:member inst:TOOL0390 ;
  skos:member inst:TOOL0391 ;
  skos:member inst:TOOL0412 ;
  skos:member inst:TOOL0413 ;
  skos:member inst:TOOL0418 ;
  skos:member inst:TOOL0420 ;
  skos:member inst:TOOL0427 ;
  skos:member inst:TOOL0430 ;
  skos:member inst:TOOL0457 ;
  skos:member inst:TOOL0469 ;
  skos:member inst:TOOL0472 ;
  skos:member inst:TOOL0482 ;
  skos:member inst:TOOL0491 ;
  skos:member inst:TOOL0500 ;
  skos:member inst:TOOL0501 ;
  skos:member inst:TOOL0502 ;
  skos:member inst:TOOL0503 ;
  skos:member inst:TOOL0504 ;
  skos:member inst:TOOL0505 ;
  skos:member inst:TOOL0506 ;
  skos:member inst:TOOL0507 ;
  skos:member inst:TOOL0508 ;
  skos:member inst:TOOL0524 ;
  skos:member inst:TOOL0535 ;
  skos:member inst:TOOL0536 ;
  skos:member inst:TOOL0537 ;
  skos:member inst:TOOL0538 ;
  skos:member inst:TOOL0539 ;
  skos:member inst:TOOL0540 ;
  skos:member inst:TOOL0541 ;
  skos:member inst:TOOL0542 ;
  skos:member inst:TOOL0543 ;
  skos:member inst:TOOL0544 ;
  skos:member inst:TOOL0545 ;
  skos:member inst:TOOL0546 ;
  skos:member inst:TOOL0547 ;
  skos:member inst:TOOL0548 ;
  skos:member inst:TOOL0550 ;
  skos:member inst:TOOL0551 ;
  skos:member inst:TOOL0552 ;
  skos:member inst:TOOL0553 ;
  skos:member inst:TOOL0554 ;
  skos:member inst:TOOL0555 ;
  skos:member inst:TOOL0556 ;
  skos:member inst:TOOL0557 ;
  skos:member inst:TOOL0561 ;
  skos:member inst:TOOL0562 ;
  skos:member inst:TOOL0563 ;
  skos:member inst:TOOL0567 ;
  skos:member inst:TOOL0571 ;
  skos:member inst:TOOL0573 ;
  skos:member inst:TOOL0588 ;
  skos:member inst:TOOL0601 ;
  skos:member inst:TOOL0623 ;
  skos:member inst:TOOL0651 ;
  skos:member inst:TOOL0652 ;
  skos:member inst:TOOL0653 ;
  skos:member inst:TOOL0660 ;
  skos:member inst:TOOL0695 ;
  skos:member inst:TOOL0697 ;
  skos:member inst:TOOL0698 ;
  skos:member inst:TOOL0702 ;
  skos:member inst:TOOL0703 ;
  skos:member inst:TOOL0722 ;
  skos:member inst:TOOL0723 ;
  skos:member inst:TOOL0735 ;
  skos:member inst:TOOL0742 ;
  skos:member inst:TOOL0743 ;
  skos:member inst:TOOL0751 ;
  skos:member inst:TOOL0753 ;
  skos:member inst:TOOL0758 ;
  skos:member inst:TOOL0759 ;
  skos:member inst:TOOL0760 ;
  skos:member inst:TOOL0761 ;
  skos:member inst:TOOL0762 ;
  skos:member inst:TOOL0763 ;
  skos:member inst:TOOL0764 ;
  skos:member inst:TOOL0765 ;
  skos:member inst:TOOL0766 ;
  skos:member inst:TOOL0767 ;
  skos:member inst:TOOL0768 ;
  skos:member inst:TOOL0769 ;
  skos:member inst:TOOL0784 ;
  skos:member inst:TOOL0785 ;
  skos:member inst:TOOL0786 ;
  skos:member inst:TOOL0787 ;
  skos:member inst:TOOL0788 ;
  skos:member inst:TOOL0792 ;
  skos:member inst:TOOL0798 ;
  skos:member inst:TOOL0799 ;
  skos:member inst:TOOL0800 ;
  skos:member inst:TOOL0801 ;
  skos:member inst:TOOL0802 ;
  skos:member inst:TOOL0803 ;
  skos:member inst:TOOL0806 ;
  skos:member inst:TOOL0807 ;
  skos:member inst:TOOL0817 ;
  skos:member inst:TOOL0818 ;
  skos:member inst:TOOL0819 ;
  skos:member inst:TOOL0828 ;
  skos:member inst:TOOL0833 ;
  skos:member inst:TOOL0843 ;
  skos:member inst:TOOL0844 ;
  skos:member inst:TOOL0862 ;
  skos:member inst:TOOL0867 ;
  skos:member inst:TOOL0882 ;
  skos:member inst:TOOL0885 ;
  skos:member inst:TOOL0899 ;
  skos:member inst:TOOL0900 ;
  skos:member inst:TOOL0912 ;
  skos:member inst:TOOL0917 ;
  skos:member inst:TOOL0926 ;
  skos:member inst:TOOL0930 ;
  skos:member inst:TOOL0933 ;
  skos:member inst:TOOL0934 ;
  skos:member inst:TOOL0935 ;
  skos:member inst:TOOL0936 ;
  skos:member inst:TOOL0939 ;
  skos:member inst:TOOL0940 ;
  skos:member inst:TOOL0960 ;
  skos:member inst:TOOL0961 ;
  skos:member inst:TOOL0962 ;
  skos:member inst:TOOL0963 ;
  skos:member inst:TOOL0978 ;
  skos:member inst:TOOL0979 ;
  skos:member inst:TOOL0980 ;
  skos:member inst:TOOL0981 ;
  skos:member inst:TOOL0982 ;
  skos:member inst:TOOL0983 ;
  skos:member inst:TOOL0984 ;
  skos:member inst:TOOL0985 ;
  skos:member inst:TOOL0986 ;
  skos:member inst:TOOL0987 ;
  skos:member inst:TOOL0988 ;
  skos:member inst:TOOL0989 ;
  skos:member inst:TOOL0990 ;
  skos:member inst:TOOL0991 ;
  skos:member inst:TOOL0992 ;
  skos:member inst:TOOL0993 ;
  skos:member inst:TOOL0994 ;
  skos:member inst:TOOL0995 ;
  skos:member inst:TOOL0996 ;
  skos:member inst:TOOL0997 ;
  skos:member inst:TOOL1012 ;
  skos:member inst:TOOL1016 ;
  skos:member inst:TOOL1034 ;
  skos:member inst:TOOL1035 ;
  skos:member inst:TOOL1036 ;
  skos:member inst:TOOL1037 ;
  skos:member inst:TOOL1038 ;
  skos:member inst:TOOL1039 ;
  skos:member inst:TOOL1040 ;
  skos:member inst:TOOL1041 ;
  skos:member inst:TOOL1042 ;
  skos:member inst:TOOL1043 ;
  skos:member inst:TOOL1044 ;
  skos:member inst:TOOL1045 ;
  skos:member inst:TOOL1046 ;
  skos:member inst:TOOL1047 ;
  skos:member inst:TOOL1048 ;
  skos:member inst:TOOL1049 ;
  skos:member inst:TOOL1050 ;
  skos:member inst:TOOL1051 ;
  skos:member inst:TOOL1052 ;
  skos:member inst:TOOL1053 ;
  skos:member inst:TOOL1054 ;
  skos:member inst:TOOL1055 ;
  skos:member inst:TOOL1056 ;
  skos:member inst:TOOL1057 ;
  skos:member inst:TOOL1058 ;
  skos:member inst:TOOL1059 ;
  skos:member inst:TOOL1060 ;
  skos:member inst:TOOL1061 ;
  skos:member inst:TOOL1062 ;
  skos:member inst:TOOL1063 ;
  skos:member inst:TOOL1064 ;
  skos:member inst:TOOL1065 ;
  skos:member inst:TOOL1066 ;
  skos:member inst:TOOL1067 ;
  skos:member inst:TOOL1068 ;
  skos:member inst:TOOL1069 ;
  skos:member inst:TOOL1070 ;
  skos:member inst:TOOL1071 ;
  skos:member inst:TOOL1072 ;
  skos:member inst:TOOL1073 ;
  skos:member inst:TOOL1074 ;
  skos:member inst:TOOL1075 ;
  skos:member inst:TOOL1076 ;
  skos:member inst:TOOL1077 ;
  skos:member inst:TOOL1078 ;
  skos:member inst:TOOL1079 ;
  skos:member inst:TOOL1080 ;
  skos:member inst:TOOL1081 ;
  skos:member inst:TOOL1082 ;
  skos:member inst:TOOL1083 ;
  skos:member inst:TOOL1084 ;
  skos:member inst:TOOL1085 ;
  skos:member inst:TOOL1086 ;
  skos:member inst:TOOL1087 ;
  skos:member inst:TOOL1088 ;
  skos:member inst:TOOL1090 ;
  skos:member inst:TOOL1091 ;
  skos:member inst:TOOL1111 ;
  skos:member inst:TOOL1120 ;
  skos:member inst:TOOL1135 ;
  skos:member inst:TOOL1165 ;
  skos:member inst:TOOL1166 ;
  skos:member inst:TOOL1169 ;
  skos:member inst:TOOL1170 ;
  skos:member inst:TOOL1171 ;
  skos:member inst:TOOL1172 ;
  skos:member inst:TOOL1173 ;
  skos:member inst:TOOL1174 ;
  skos:member inst:TOOL1175 ;
  skos:member inst:TOOL1176 ;
  skos:member inst:TOOL1177 ;
  skos:member inst:TOOL1178 ;
  skos:member inst:TOOL1179 ;
  skos:member inst:TOOL1181 ;
  skos:member inst:TOOL1191 ;
  skos:member inst:TOOL1199 ;
  skos:member inst:TOOL1204 ;
  skos:member inst:TOOL1214 ;
  skos:member inst:TOOL1215 ;
  skos:member inst:TOOL1216 ;
  skos:member inst:TOOL1227 ;
  skos:member inst:TOOL1228 ;
  skos:member inst:TOOL1235 ;
  skos:member inst:TOOL1249 ;
  skos:member inst:TOOL1252 ;
  skos:member inst:TOOL1253 ;
  skos:member inst:TOOL1259 ;
  skos:member inst:TOOL1260 ;
  skos:member inst:TOOL1261 ;
  skos:member inst:TOOL1272 ;
  skos:member inst:TOOL1274 ;
  skos:member inst:TOOL1280 ;
  skos:member inst:TOOL1285 ;
  skos:member inst:TOOL1299 ;
  skos:member inst:TOOL1304 ;
  skos:member inst:TOOL1326 ;
  skos:member inst:TOOL1334 ;
  skos:member inst:TOOL1339 ;
  skos:member inst:TOOL1348 ;
  skos:member inst:TOOL1349 ;
  skos:member inst:TOOL1351 ;
  skos:member inst:TOOL1352 ;
  skos:member inst:TOOL1371 ;
  skos:member inst:TOOL1372 ;
  skos:member inst:TOOL1373 ;
  skos:member inst:TOOL1374 ;
  skos:member inst:TOOL1375 ;
  skos:member inst:TOOL1376 ;
  skos:member inst:TOOL1378 ;
  skos:member inst:TOOL1379 ;
  skos:member inst:TOOL1405 ;
  skos:member inst:TOOL1413 ;
  skos:member inst:TOOL1414 ;
  skos:member inst:TOOL1415 ;
  skos:member inst:TOOL1416 ;
  skos:member inst:TOOL1417 ;
  skos:member inst:TOOL1433 ;
  skos:member inst:TOOL1434 ;
  skos:member inst:TOOL1435 ;
  skos:member inst:TOOL1446 ;
  skos:member inst:TOOL1454 ;
  skos:member inst:TOOL1455 ;
  skos:member inst:TOOL1462 ;
  skos:member inst:TOOL1463 ;
  skos:member inst:TOOL1464 ;
  skos:member inst:TOOL1465 ;
  skos:member inst:TOOL1466 ;
  skos:member inst:TOOL1467 ;
  skos:member inst:TOOL1468 ;
  skos:member inst:TOOL1469 ;
  skos:member inst:TOOL1477 ;
  skos:member inst:TOOL1478 ;
  skos:member inst:TOOL1480 ;
  skos:member inst:TOOL1485 ;
  skos:member inst:TOOL1486 ;
  skos:member inst:TOOL1487 ;
  skos:member inst:TOOL1521 ;
  skos:member inst:TOOL1524 ;
  skos:member inst:TOOL1527 ;
  skos:member inst:TOOL1533 ;
  skos:member inst:TOOL1535 ;
  skos:member inst:TOOL1536 ;
  skos:member inst:TOOL1537 ;
  skos:member inst:TOOL1547 ;
  skos:member inst:TOOL1553 ;
  skos:member inst:TOOL1554 ;
  skos:member inst:TOOL1560 ;
  skos:member inst:TOOL1574 ;
  skos:member inst:TOOL1575 ;
  skos:member inst:TOOL1576 ;
  skos:member inst:TOOL1591 ;
  skos:member inst:TOOL1606 ;
  skos:member inst:TOOL1621 ;
  skos:member inst:TOOL1623 ;
  skos:member inst:TOOL1624 ;
  skos:member inst:TOOL1625 ;
  skos:member inst:TOOL1626 ;
  skos:member inst:TOOL1627 ;
  skos:member inst:TOOL1633 ;
  skos:member inst:TOOL1636 ;
  skos:member inst:TOOL1637 ;
  skos:member inst:TOOL1638 ;
  skos:member inst:TOOL1644 ;
  skos:member inst:TOOL1654 ;
  skos:member inst:TOOL1668 ;
  skos:member inst:TOOL1675 ;
  skos:member inst:TOOL1684 ;
  skos:member inst:TOOL1697 ;
  skos:member inst:TOOL1698 ;
  skos:member inst:TOOL1699 ;
  skos:member inst:TOOL1703 ;
  skos:member inst:TOOL1709 ;
  skos:member inst:TOOL1727 ;
  skos:member inst:TOOL1734 ;
  skos:member inst:TOOL1741 ;
  skos:member inst:TOOL1755 ;
  skos:member inst:TOOL1756 ;
  skos:member inst:TOOL1757 ;
  skos:member inst:TOOL1790 ;
  skos:member inst:TOOL1791 ;
  skos:member inst:TOOL1815 ;
  skos:member inst:TOOL1820 ;
  skos:member inst:TOOL1823 ;
  skos:member inst:TOOL1848 ;
  skos:member inst:TOOL1853 ;
  skos:member inst:TOOL1854 ;
  skos:member inst:TOOL1857 ;
  skos:member inst:TOOL1858 ;
  skos:member inst:TOOL1859 ;
  skos:member inst:TOOL1860 ;
  skos:member inst:TOOL1861 ;
  skos:member inst:TOOL1873 ;
  skos:member inst:TOOL1879 ;
  skos:member inst:TOOL1885 ;
  skos:member inst:TOOL1899 ;
  skos:member inst:TOOLZZZ ;
  skos:prefLabel "SeaVoX Device Catalogue" ;
.
<http://vocab.nerc.ac.uk/scheme/EDMED_DCAT_THEMES/current>
  rdf:type skos:ConceptScheme ;
  dcterm:creator "SeaDataNet" ;
  dcterm:date "2023-01-04 02:00:08.0" ;
  dcterm:description "A SKOS concept scheme to allow the representation of the SeaDataNet EDMED catalogue as Linked Data following the W3C DCAT profile." ;
  dcterm:publisher "Natural Environment Research Council" ;
  dcterm:title "W3C DCAT Themes for the SeaDataNet EDMED Catalogue" ;
  owl:versionInfo "24" ;
  skos:altLabel "EDMED DCAT themes" ;
  skos:hasTopConcept <http://vocab.nerc.ac.uk/collection/D01/current/D0100001> ;
  skos:hasTopConcept <http://vocab.nerc.ac.uk/collection/D01/current/D0100002> ;
  skos:hasTopConcept <http://vocab.nerc.ac.uk/collection/D01/current/D0100003> ;
  skos:hasTopConcept <http://vocab.nerc.ac.uk/collection/D01/current/D0100004> ;
  skos:hasTopConcept <http://vocab.nerc.ac.uk/collection/D01/current/D0100005> ;
  skos:prefLabel "W3C DCAT Themes for the SeaDataNet EDMED Catalogue" ;
.
<http://vocab.nerc.ac.uk/scheme/NETMAR_OCEAN/current>
  rdf:type skos:ConceptScheme ;
  dcterm:creator "NETMAR Ontology Governance Group" ;
  dcterm:date "2023-02-04 02:00:09.0" ;
  dcterm:description "Thesaurus centred on parameter descriptions from the BODC PUV and CF Standard Names mapping to parameter discovery, units, instrument, platform, project and coverage concepts.  Underpins discovery and semantic service chain validation for the NETMAR sea ice and oceanography pilots." ;
  dcterm:publisher "Natural Environment Research Council" ;
  dcterm:title "NETMAR Oceanography Thesaurus" ;
  owl:versionInfo "91" ;
  skos:altLabel "NETMAR Oceans" ;
  skos:hasTopConcept sdnk:SDNKG01 ;
  skos:hasTopConcept sdnk:SDNKG02 ;
  skos:hasTopConcept sdnk:SDNKG04 ;
  skos:hasTopConcept sdnk:SDNKG05 ;
  skos:hasTopConcept sdnk:SDNKG16 ;
  skos:prefLabel "NETMAR Oceanography Thesaurus" ;
.
<http://vocab.nerc.ac.uk/scheme/NETOC_INSTRUMENT/current>
  rdf:type skos:ConceptScheme ;
  dcterm:creator "NETMAR Ontology Governance Group" ;
  dcterm:date "2020-09-18 15:00:10.0" ;
  dcterm:description "Instrument facet of a thesaurus centred on parameter descriptions from the BODC PUV and CF Standard Names mapping to parameter discovery, units, instrument, platform, project and coverage concepts.  Underpins discovery and semantic service chain validation for the NETMAR sea ice and oceanography pilots." ;
  dcterm:publisher "Natural Environment Research Council" ;
  dcterm:title "NETMAR Oceanography Thesaurus Instrument Facet" ;
  owl:versionInfo "10" ;
  skos:altLabel "NETMAR Oceans Instrument" ;
  skos:hasTopConcept sdnk:SDNKG01 ;
  skos:prefLabel "NETMAR Oceanography Thesaurus Instrument Facet" ;
.
<http://vocab.nerc.ac.uk/scheme/NETOC_ORTHO/current>
  rdf:type skos:ConceptScheme ;
  dcterm:creator "NETMAR Ontology Governance Group" ;
  dcterm:date "2022-12-03 02:00:06.0" ;
  dcterm:description "Linking concepts and concepts external to the NVS of a thesaurus centred on parameter descriptions from the BODC PUV and CF Standard Names mapping to parameter discovery, units, instrument, platform, project and coverage concepts.  Underpins discovery and semantic service chain validation for the NETMAR sea ice and oceanography pilots." ;
  dcterm:publisher "Natural Environment Research Council" ;
  dcterm:title "NETMAR Oceanography Thesaurus Facet linkages and external concepts" ;
  owl:versionInfo "15" ;
  skos:altLabel "NETMAR Oceans Orthogonal" ;
  skos:prefLabel "NETMAR Oceanography Thesaurus Facet linkages and external concepts" ;
.
<http://vocab.nerc.ac.uk/scheme/NETOC_PARAM/current>
  rdf:type skos:ConceptScheme ;
  dcterm:creator "NETMAR Ontology Governance Group" ;
  dcterm:date "2023-02-04 02:00:09.0" ;
  dcterm:description "Parameter facet of a thesaurus centred on parameter descriptions from the BODC PUV and CF Standard Names mapping to parameter discovery, units, instrument, platform, project and coverage concepts.  Underpins discovery and semantic service chain validation for the NETMAR sea ice and oceanography pilots." ;
  dcterm:publisher "Natural Environment Research Council" ;
  dcterm:title "NETMAR Oceanography Thesaurus Parameter Facet" ;
  owl:versionInfo "70" ;
  skos:altLabel "NETMAR Oceans Parameter" ;
  skos:prefLabel "NETMAR Oceanography Thesaurus Parameter Facet" ;
.
<http://vocab.nerc.ac.uk/scheme/SDNDEV/current>
  rdf:type skos:ConceptScheme ;
  dcterm:creator "SeaDataNet" ;
  dcterm:date "2023-03-09 02:00:06.0" ;
  dcterm:description "A thesarus comprising categorisations of devices (sensors, instrument packages and sample collectors) developed by SeaDataNet mapped to a catalogue of specific devices maintained by SeaVoX." ;
  dcterm:publisher "Natural Environment Research Council" ;
  dcterm:title "SeaDataNet Device Thesaurus" ;
  owl:versionInfo "541" ;
  skos:altLabel "Devices" ;
  skos:hasTopConcept sdnc:ICAT03 ;
  skos:hasTopConcept sdnc:ICAT04 ;
  skos:hasTopConcept sdnc:ICAT05 ;
  skos:prefLabel "SeaDataNet Device Thesaurus" ;
.
<http://w3id.org/def/nerc/discipline-P08/collection>
  rdf:type owl:Ontology ;
  rdf:type skos:Collection ;
  dcterm:alternative "SeaDataNet Disciplines" ;
  dcterm:creator "SeaDataNet" ;
  dcterm:date "2017-02-03 02:00:03.0" ;
  dcterm:description "Terms used to classify SeaDataNet Agreed Parameter Groups to provide topic/theme level terms in a hierarchical parameter discovery interface." ;
  dcterm:license <https://creativecommons.org/licenses/by/4.0> ;
  dcterm:publisher "Natural Environment Research Council" ;
  dcterm:title "SeaDataNet Parameter Disciplines" ;
  grg:RE_RegisterManager "British Oceanographic Data Centre" ;
  grg:RE_RegisterOwner "SeaDataNet" ;
  rdfs:comment "Governance for vocabularies used in the EU SeaDataNet project implemented as consultation between BODC and the members of the SeaDataNet Technical Task Team" ;
  owl:imports <http://www.w3.org/2004/02/skos/core> ;
  owl:versionInfo "5" ;
  skos:altLabel "SeaDataNet Disciplines" ;
  skos:member dspl:DS06 ;
  skos:member dspl:DS07 ;
  skos:member dspl:DS08 ;
  skos:member dspl:DS12 ;
  skos:prefLabel "SeaDataNet Parameter Disciplines" ;
.
<http://w3id.org/def/nerc/instrument-L05/collection>
  rdf:type owl:Ontology ;
  rdf:type skos:Collection ;
  <http://purl.org/dc/terms/:alternative> "SDN devices" ;
  <http://purl.org/dc/terms/:creator> "SeaDataNet" ;
  <http://purl.org/dc/terms/:description> "Terms used to classify groups of sensors, instruments, sources of algorithmically computed data (numerical models) or samplers (collectors of water, SPM, sediment, rock, air or biota samples)." ;
  <http://purl.org/dc/terms/:license> <https://creativecommons.org/licenses/by/4.0/> ;
  <http://purl.org/dc/terms/:publisher> "Natural Environment Research Council" ;
  <http://purl.org/dc/terms/:title> "SeaDataNet device categories" ;
  dcterm:date "2023-02-17 02:00:01.0" ;
  grg:RE_RegisterManager "British Oceanographic Data Centre" ;
  grg:RE_RegisterOwner "SeaDataNet" ;
  rdfs:comment "Governance for vocabularies used in the EU SeaDataNet project implemented as consultation between BODC and the members of the SeaDataNet Technical Task Team" ;
  rdfs:seeAlso <https://github.com/nvs-vocabs/L05> ;
  owl:imports <http://w3id.org/def/nerc/sdncategories-L21/conceptscheme> ;
  owl:imports <http://w3id.org/def/nerc/seadatanetdatacat/collection> ;
  owl:imports <http://www.w3.org/2004/02/skos/core> ;
  owl:versionInfo "86" ;
  skos:altLabel "SDN devices" ;
  skos:historyNote "original URI http://vocab.nerc.ac.uk/collection/L05/current/, SMR change to put instrument vocabs together"@en ;
  skos:member <http://vocab.nerc.ac.uk/collection/L05/current/101> ;
  skos:member <http://vocab.nerc.ac.uk/collection/L05/current/102> ;
  skos:member <http://vocab.nerc.ac.uk/collection/L05/current/103> ;
  skos:member <http://vocab.nerc.ac.uk/collection/L05/current/110> ;
  skos:member <http://vocab.nerc.ac.uk/collection/L05/current/113> ;
  skos:member <http://vocab.nerc.ac.uk/collection/L05/current/114> ;
  skos:member <http://vocab.nerc.ac.uk/collection/L05/current/115> ;
  skos:member <http://vocab.nerc.ac.uk/collection/L05/current/121> ;
  skos:member <http://vocab.nerc.ac.uk/collection/L05/current/122> ;
  skos:member <http://vocab.nerc.ac.uk/collection/L05/current/123> ;
  skos:member <http://vocab.nerc.ac.uk/collection/L05/current/124> ;
  skos:member <http://vocab.nerc.ac.uk/collection/L05/current/130> ;
  skos:member <http://vocab.nerc.ac.uk/collection/L05/current/131> ;
  skos:member <http://vocab.nerc.ac.uk/collection/L05/current/132> ;
  skos:member <http://vocab.nerc.ac.uk/collection/L05/current/133> ;
  skos:member <http://vocab.nerc.ac.uk/collection/L05/current/134> ;
  skos:member <http://vocab.nerc.ac.uk/collection/L05/current/135> ;
  skos:member <http://vocab.nerc.ac.uk/collection/L05/current/150> ;
  skos:member <http://vocab.nerc.ac.uk/collection/L05/current/152> ;
  skos:member <http://vocab.nerc.ac.uk/collection/L05/current/153> ;
  skos:member <http://vocab.nerc.ac.uk/collection/L05/current/154> ;
  skos:member <http://vocab.nerc.ac.uk/collection/L05/current/155> ;
  skos:member <http://vocab.nerc.ac.uk/collection/L05/current/156> ;
  skos:member <http://vocab.nerc.ac.uk/collection/L05/current/157> ;
  skos:member <http://vocab.nerc.ac.uk/collection/L05/current/158> ;
  skos:member <http://vocab.nerc.ac.uk/collection/L05/current/159> ;
  skos:member <http://vocab.nerc.ac.uk/collection/L05/current/180> ;
  skos:member <http://vocab.nerc.ac.uk/collection/L05/current/181> ;
  skos:member <http://vocab.nerc.ac.uk/collection/L05/current/183> ;
  skos:member <http://vocab.nerc.ac.uk/collection/L05/current/184> ;
  skos:member <http://vocab.nerc.ac.uk/collection/L05/current/185> ;
  skos:member <http://vocab.nerc.ac.uk/collection/L05/current/186> ;
  skos:member <http://vocab.nerc.ac.uk/collection/L05/current/301> ;
  skos:member <http://vocab.nerc.ac.uk/collection/L05/current/302> ;
  skos:member <http://vocab.nerc.ac.uk/collection/L05/current/303> ;
  skos:member <http://vocab.nerc.ac.uk/collection/L05/current/304> ;
  skos:member <http://vocab.nerc.ac.uk/collection/L05/current/305> ;
  skos:member <http://vocab.nerc.ac.uk/collection/L05/current/306> ;
  skos:member <http://vocab.nerc.ac.uk/collection/L05/current/307> ;
  skos:member <http://vocab.nerc.ac.uk/collection/L05/current/308> ;
  skos:member <http://vocab.nerc.ac.uk/collection/L05/current/309> ;
  skos:member <http://vocab.nerc.ac.uk/collection/L05/current/310> ;
  skos:member <http://vocab.nerc.ac.uk/collection/L05/current/311> ;
  skos:member <http://vocab.nerc.ac.uk/collection/L05/current/312> ;
  skos:member <http://vocab.nerc.ac.uk/collection/L05/current/313> ;
  skos:member <http://vocab.nerc.ac.uk/collection/L05/current/314> ;
  skos:member <http://vocab.nerc.ac.uk/collection/L05/current/315> ;
  skos:member <http://vocab.nerc.ac.uk/collection/L05/current/350> ;
  skos:member <http://vocab.nerc.ac.uk/collection/L05/current/351> ;
  skos:member <http://vocab.nerc.ac.uk/collection/L05/current/352> ;
  skos:member <http://vocab.nerc.ac.uk/collection/L05/current/353> ;
  skos:member <http://vocab.nerc.ac.uk/collection/L05/current/355> ;
  skos:member <http://vocab.nerc.ac.uk/collection/L05/current/356> ;
  skos:member <http://vocab.nerc.ac.uk/collection/L05/current/358> ;
  skos:member <http://vocab.nerc.ac.uk/collection/L05/current/359> ;
  skos:member <http://vocab.nerc.ac.uk/collection/L05/current/360> ;
  skos:member <http://vocab.nerc.ac.uk/collection/L05/current/361> ;
  skos:member <http://vocab.nerc.ac.uk/collection/L05/current/362> ;
  skos:member <http://vocab.nerc.ac.uk/collection/L05/current/363> ;
  skos:member <http://vocab.nerc.ac.uk/collection/L05/current/364> ;
  skos:member <http://vocab.nerc.ac.uk/collection/L05/current/365> ;
  skos:member <http://vocab.nerc.ac.uk/collection/L05/current/366> ;
  skos:member <http://vocab.nerc.ac.uk/collection/L05/current/367> ;
  skos:member <http://vocab.nerc.ac.uk/collection/L05/current/368> ;
  skos:member <http://vocab.nerc.ac.uk/collection/L05/current/369> ;
  skos:member <http://vocab.nerc.ac.uk/collection/L05/current/370> ;
  skos:member <http://vocab.nerc.ac.uk/collection/L05/current/371> ;
  skos:member <http://vocab.nerc.ac.uk/collection/L05/current/372> ;
  skos:member <http://vocab.nerc.ac.uk/collection/L05/current/373> ;
  skos:member <http://vocab.nerc.ac.uk/collection/L05/current/374> ;
  skos:member <http://vocab.nerc.ac.uk/collection/L05/current/375> ;
  skos:member <http://vocab.nerc.ac.uk/collection/L05/current/376> ;
  skos:member <http://vocab.nerc.ac.uk/collection/L05/current/377> ;
  skos:member <http://vocab.nerc.ac.uk/collection/L05/current/378> ;
  skos:member <http://vocab.nerc.ac.uk/collection/L05/current/379> ;
  skos:member <http://vocab.nerc.ac.uk/collection/L05/current/380> ;
  skos:member <http://vocab.nerc.ac.uk/collection/L05/current/381> ;
  skos:member <http://vocab.nerc.ac.uk/collection/L05/current/382> ;
  skos:member <http://vocab.nerc.ac.uk/collection/L05/current/383> ;
  skos:member <http://vocab.nerc.ac.uk/collection/L05/current/384> ;
  skos:member <http://vocab.nerc.ac.uk/collection/L05/current/385> ;
  skos:member <http://vocab.nerc.ac.uk/collection/L05/current/386> ;
  skos:member <http://vocab.nerc.ac.uk/collection/L05/current/387> ;
  skos:member <http://vocab.nerc.ac.uk/collection/L05/current/388> ;
  skos:member <http://vocab.nerc.ac.uk/collection/L05/current/389> ;
  skos:member <http://vocab.nerc.ac.uk/collection/L05/current/390> ;
  skos:member <http://vocab.nerc.ac.uk/collection/L05/current/393> ;
  skos:member <http://vocab.nerc.ac.uk/collection/L05/current/395> ;
  skos:member <http://vocab.nerc.ac.uk/collection/L05/current/86> ;
  skos:member <http://vocab.nerc.ac.uk/collection/L05/current/91> ;
  skos:member <http://vocab.nerc.ac.uk/collection/L05/current/92> ;
  skos:member sdev:ATRANS ;
  skos:member sdev:BLUMS ;
  skos:member sdev:CCOV ;
  skos:member sdev:COLCMP ;
  skos:member sdev:CSEM ;
  skos:member sdev:DLOG ;
  skos:member sdev:EMSR ;
  skos:member sdev:FFES ;
  skos:member sdev:ICEP ;
  skos:member sdev:LAB01 ;
  skos:member sdev:LAB02 ;
  skos:member sdev:LAB03 ;
  skos:member sdev:LAB04 ;
  skos:member sdev:LAB05 ;
  skos:member sdev:LAB06 ;
  skos:member sdev:LAB07 ;
  skos:member sdev:LAB08 ;
  skos:member sdev:LAB09 ;
  skos:member sdev:LAB10 ;
  skos:member sdev:LAB11 ;
  skos:member sdev:LAB12 ;
  skos:member sdev:LAB13 ;
  skos:member sdev:LAB14 ;
  skos:member sdev:LAB15 ;
  skos:member sdev:LAB16 ;
  skos:member sdev:LAB17 ;
  skos:member sdev:LAB18 ;
  skos:member sdev:LAB19 ;
  skos:member sdev:LAB20 ;
  skos:member sdev:LAB21 ;
  skos:member sdev:LAB22 ;
  skos:member sdev:LAB23 ;
  skos:member sdev:LAB24 ;
  skos:member sdev:LAB25 ;
  skos:member sdev:LAB26 ;
  skos:member sdev:LAB27 ;
  skos:member sdev:LAB28 ;
  skos:member sdev:LAB29 ;
  skos:member sdev:LAB30 ;
  skos:member sdev:LAB31 ;
  skos:member sdev:LAB32 ;
  skos:member sdev:LAB33 ;
  skos:member sdev:LAB34 ;
  skos:member sdev:LAB35 ;
  skos:member sdev:LAB36 ;
  skos:member sdev:LAB37 ;
  skos:member sdev:LAB38 ;
  skos:member sdev:LAB39 ;
  skos:member sdev:LAB40 ;
  skos:member sdev:LAB42 ;
  skos:member sdev:LAB43 ;
  skos:member sdev:LAB44 ;
  skos:member sdev:LAB45 ;
  skos:member sdev:LAB46 ;
  skos:member sdev:LAB47 ;
  skos:member sdev:LAB48 ;
  skos:member sdev:LAB49 ;
  skos:member sdev:LAB51 ;
  skos:member sdev:LVLST ;
  skos:member sdev:MMIS ;
  skos:member sdev:MPIS ;
  skos:member sdev:PERMON ;
  skos:member sdev:TRTG ;
  skos:member sdev:WDRG ;
  skos:member sdev:WPS ;
  skos:prefLabel "SeaDataNet device categories" ;
.
<http://w3id.org/def/nerc/instrumenttype/ontology>
  rdf:type owl:Ontology ;
  rdf:type skos:ConceptScheme ;
  rdfs:label "nerc collection W06"@en ;
  owl:imports <http://www.w3.org/2004/02/skos/core> ;
  skos:prefLabel "nerc collection W06"@en ;
.
<http://w3id.org/def/nerc/keyword-L19/collection>
  rdf:type owl:Ontology ;
  rdf:type skos:Collection ;
  dcterm:alternative "SDN keyword types" ;
  dcterm:creator "SeaDataNet" ;
  dcterm:date "2021-07-07 15:21:48.0" ;
  dcterm:description "Terms used in SeaDataNet metadata to describe the purpose of a keyword.  An extension of the ISO19115 KeywordTypeCode codelist." ;
  dcterm:license <https://creativecommons.org/licenses/by/4.0> ;
  dcterm:publisher "Natural Environment Research Council" ;
  dcterm:title "SeaDataNet keyword types" ;
  grg:RE_RegisterManager "British Oceanographic Data Centre" ;
  grg:RE_RegisterOwner "SeaDataNet" ;
  rdfs:comment "Governance for vocabularies used in the EU SeaDataNet project implemented as consultation between BODC and the members of the SeaDataNet Technical Task Team" ;
  owl:imports <http://www.w3.org/2004/02/skos/core> ;
  owl:versionInfo "4" ;
  skos:altLabel "SDN keyword types" ;
  skos:historyNote "original URI was http://vocab.nerc.ac.uk/collection/L19/current/"@en ;
  skos:member <http://vocab.nerc.ac.uk/collection/L19/current/002> ;
  skos:member <http://vocab.nerc.ac.uk/collection/L19/current/003> ;
  skos:member <http://vocab.nerc.ac.uk/collection/L19/current/004> ;
  skos:member sdnk:SDNKG01 ;
  skos:member sdnk:SDNKG02 ;
  skos:member sdnk:SDNKG04 ;
  skos:member sdnk:SDNKG05 ;
  skos:member sdnk:SDNKG06 ;
  skos:member sdnk:SDNKG07 ;
  skos:member sdnk:SDNKG08 ;
  skos:member sdnk:SDNKG09 ;
  skos:member sdnk:SDNKG10 ;
  skos:member sdnk:SDNKG11 ;
  skos:member sdnk:SDNKG12 ;
  skos:member sdnk:SDNKG13 ;
  skos:member sdnk:SDNKG14 ;
  skos:member sdnk:SDNKG15 ;
  skos:member sdnk:SDNKG16 ;
  skos:member sdnk:SDNKG17 ;
  skos:prefLabel "SeaDataNet keyword types" ;
.
<http://w3id.org/def/nerc/sdncategories-L21/conceptscheme>
  rdf:type owl:Ontology ;
  rdf:type skos:ConceptScheme ;
  rdfs:label "categories for SeaDataNet resources"@en ;
  owl:imports <http://www.w3.org/2004/02/skos/core> ;
.
<http://w3id.org/def/nerc/seadatanetdatacat/collection>
  rdf:type owl:Ontology ;
  rdf:type skos:Collection ;
  dcterm:alternative "SeaDataNet CSR data categories" ;
  dcterm:creator "SeaDataNet" ;
  dcterm:date "2022-09-27 03:00:02.0" ;
  dcterm:description "Terms used to describe shipboard activities (sometimes inaccurately described as parameters) by SeaDataNet in Cruise Summary Report (formerly known as ROSCOP) metadata." ;
  dcterm:license <https://creativecommons.org/licenses/by/4.0> ;
  dcterm:publisher "Natural Environment Research Council" ;
  dcterm:title "SeaDataNet Cruise Summary Report data categories" ;
  grg:RE_RegisterManager "British Oceanographic Data Centre" ;
  grg:RE_RegisterOwner "SeaDataNet" ;
  rdfs:comment "Governance for vocabularies used in the EU SeaDataNet project implemented as consultation between BODC and the members of the SeaDataNet Technical Task Team" ;
  owl:imports <http://w3id.org/def/nerc/discipline-P08/collection> ;
  owl:imports <http://w3id.org/def/nerc/instrument-L05/collection> ;
  owl:imports <http://w3id.org/def/nerc/keyword-L19/collection> ;
  owl:imports <http://www.w3.org/2004/02/skos/core> ;
  skos:altLabel "SeaDataNet CSR data categories" ;
  skos:historyNote "original URI was http://vocab.nerc.ac.uk/collection/C77/current/"@en ;
  skos:member sdnd:R01 ;
  skos:member sdnd:R02 ;
  skos:member sdnd:R03 ;
  skos:member sdnd:R04 ;
  skos:prefLabel "SeaDataNet Cruise Summary Report data categories" ;
.
<http://w3id.org/def/numericalmodel/conceptscheme>
  rdf:type skos:ConceptScheme ;
  rdfs:label "Numeric Model" ;
  skos:definition " " ;
  skos:prefLabel "Numeric Model" ;
.
<http://w3id.org/def/positioningsystem/conceptscheme>
  rdf:type skos:ConceptScheme ;
  rdfs:label "Positioning system "@en ;
  skos:definition " " ;
  skos:prefLabel "Positioning system "@en ;
.
<http://w3id.org/def/samplecollectioninstrument/conceptscheme>
  rdf:type skos:ConceptScheme ;
  rdfs:label "Sample collection instrument "@en ;
  skos:definition " " ;
  skos:prefLabel "Sample collection instrument "@en ;
.
<http://w3id.org/def/sampleprepreationinstrument/conceptscheme>
  rdf:type skos:ConceptScheme ;
  rdfs:label "Sample preparation instrument "@en ;
  skos:definition " " ;
  skos:prefLabel "Sample preparation instrument "@en ;
.
<http://w3id.org/def/seismicsource/conceptscheme>
  rdf:type skos:ConceptScheme ;
  rdfs:label "Seismic source instrument "@en ;
  skos:definition " " ;
  skos:prefLabel "Seismic source instrument "@en ;
.
<http://w3id.org/ogeochem/def/instrument/measurement/conceptscheme>
  rdf:type skos:ConceptScheme ;
  rdfs:label "Measurement instruments" ;
  skos:definition " " ;
  skos:prefLabel "Measurement instruments" ;
.
<http://w3id.org/ogeochem/def/instrument/ontology>
  rdf:type owl:Ontology ;
  dcterm:created "2023-02-09"^^xsd:date ;
  dcterm:creator "SMR" ;
  dcterm:modified "2023-03-09"^^xsd:date ;
  dcterm:publisher "TBD" ;
  dcterm:source "Compiled NERC vocabularies related to measurement instyruments" ;
  rdfs:label "Measurement instruments for geochemistry"@en ;
  owl:imports <http://purl.org/dc/elements/1.1/> ;
  owl:imports <http://www.w3.org/2000/01/rdf-schema> ;
  owl:imports <http://www.w3.org/2004/02/skos/core> ;
  skos:definition "TBD"@en ;
  skos:prefLabel "Measurement instruments for geochemistry"@en ;
.
<http://w3id.org/ogeochem/def/instrument/parameters/conceptscheme>
  rdf:type skos:ConceptScheme ;
  rdfs:label "Measurement type" ;
  skos:definition " " ;
  skos:prefLabel "Measurement type" ;
.
grg:RE_RegisterManager
  rdf:type owl:AnnotationProperty ;
.
grg:RE_RegisterOwner
  rdf:type owl:AnnotationProperty ;
.
skos:Collection
  rdf:type owl:Class ;
.
skos:Concept
  rdf:type owl:Class ;
.
skos:altLabel
  rdf:type owl:AnnotationProperty ;
.
skos:definition
  rdf:type owl:AnnotationProperty ;
.
skos:narrower
  rdf:type owl:AnnotationProperty ;
.
skos:notation
  rdf:type owl:AnnotationProperty ;
.
skos:note
  rdf:type owl:AnnotationProperty ;
.
skos:prefLabel
  rdf:type owl:AnnotationProperty ;
.
